<?xml version="1.0"?>


<!DOCTYPE rdf:RDF [
    <!ENTITY dcterms "http://purl.org/dc/terms/" >
    <!ENTITY foaf "http://xmlns.com/foaf/0.1/" >
    <!ENTITY vann "http://purl.org/vocab/vann/" >
    <!ENTITY cc "http://creativecommons.org/ns#" >
    <!ENTITY owl "http://www.w3.org/2002/07/owl#" >
    <!ENTITY dc "http://purl.org/dc/elements/1.1/" >
    <!ENTITY xsd "http://www.w3.org/2001/XMLSchema#" >
    <!ENTITY rdfs "http://www.w3.org/2000/01/rdf-schema#" >
    <!ENTITY maso "http://securitytoolbox.appspot.com/MASO#" >
    <!ENTITY stac "http://securitytoolbox.appspot.com/stac#" >
    <!ENTITY rdf "http://www.w3.org/1999/02/22-rdf-syntax-ns#" >
    <!ENTITY vs "http://www.w3.org/2003/06/sw-vocab-status/ns#" >
    <!ENTITY kim "http://securitytoolbox.appspot.com/securityMain#" >
    <!ENTITY kimalgorithms "http://securitytoolbox.appspot.com/securityAlgorithms#" >
    <!ENTITY securitysw "http://semanticweb.org/images/5/53/OntologySecurity.owl" >
    <!ENTITY iotsec "http://www-usr.inf.ufsm.br/~brunomozza/iotsec/iotsec.owl#" >
    <!ENTITY denker "http://www.daml.org/services/owl-s/security/security.owl#" >
    <!ENTITY herzog "http://www.ida.liu.se/~iislab/projects/secont/Security.owl" >
    <!ENTITY ct "http://www.tele.pw.edu.pl/~sims-onto/ConnectivityType.owl#" >
    <!ENTITY secberlin "http://preciosa.informatik.hu-berlin.de/ontology/security.owl" >
    <!ENTITY serviceContext "http://ontology.ist-spice.org/mobile-ontology/1/0/service_context/0/service_context.owl#" >
]>


<rdf:RDF xmlns="http://www-usr.inf.ufsm.br/~brunomozza/iotsec#"
     xml:base="http://www-usr.inf.ufsm.br/~brunomozza/iotsec"
     xmlns:serviceContext="http://ontology.ist-spice.org/mobile-ontology/1/0/service_context/0/service_context.owl#"
     xmlns:dc="http://purl.org/dc/elements/1.1/"
     xmlns:foaf="http://xmlns.com/foaf/0.1/"
     xmlns:kim="http://securitytoolbox.appspot.com/securityMain#"
     xmlns:iotsec="http://www-usr.inf.ufsm.br/~brunomozza/iotsec/iotsec.owl#"
     xmlns:vann="http://purl.org/vocab/vann/"
     xmlns:vs="http://www.w3.org/2003/06/sw-vocab-status/ns#"
     xmlns:denker="http://www.daml.org/services/owl-s/security/security.owl#"
     xmlns:securitysw="http://semanticweb.org/images/5/53/OntologySecurity.owl"
     xmlns:ct="http://www.tele.pw.edu.pl/~sims-onto/ConnectivityType.owl#"
     xmlns:dcterms="http://purl.org/dc/terms/"
     xmlns:rdfs="http://www.w3.org/2000/01/rdf-schema#"
     xmlns:herzog="http://www.ida.liu.se/~iislab/projects/secont/Security.owl"
     xmlns:maso="http://securitytoolbox.appspot.com/MASO#"
     xmlns:owl="http://www.w3.org/2002/07/owl#"
     xmlns:xsd="http://www.w3.org/2001/XMLSchema#"
     xmlns:stac="http://securitytoolbox.appspot.com/stac#"
     xmlns:rdf="http://www.w3.org/1999/02/22-rdf-syntax-ns#"
     xmlns:kimalgorithms="http://securitytoolbox.appspot.com/securityAlgorithms#"
     xmlns:secberlin="http://preciosa.informatik.hu-berlin.de/ontology/security.owl"
     xmlns:cc="http://creativecommons.org/ns#">
    <owl:Ontology rdf:about="http://www-usr.inf.ufsm.br/~brunomozza/iotsec/iotsec.owl#">
        <owl:versionInfo rdf:datatype="&xsd;decimal">0.1</owl:versionInfo>
        <dcterms:issued rdf:datatype="&xsd;date">2015-03-10</dcterms:issued>
        <dcterms:modified rdf:datatype="&xsd;date">2015-06-26</dcterms:modified>
        <dc:creator rdf:datatype="&xsd;string">Bruno A. Mozzaquatro</dc:creator>
        <rdfs:seeAlso rdf:datatype="&xsd;string">This work has been inspired for an ontology of attacks and countermeasures for M2M communications by &quot;The iotsec Ontology (Security Toolbox : Attacks and Countermeasures); [Gyrard 2014]</rdfs:seeAlso>
        <rdfs:seeAlso rdf:datatype="&xsd;string">This work has been inspired for the cryptographic concepts and security properties by &quot;An ontology of Information Security&quot; [Herzog et al. 2007]</rdfs:seeAlso>
        <rdfs:seeAlso rdf:datatype="&xsd;string">This work has been inspired for the cryptographic concepts and security properties by &quot;Construction d&apos;une ontologie pour le domaine de la securite&quot; [Lekhchine et al. 2009]</rdfs:seeAlso>
        <rdfs:seeAlso rdf:datatype="&xsd;string">This work has been inspired for the cryptographic concepts and security properties by &quot;Security Ontology for Annotating resources&quot; [Kim et al. 2005]</rdfs:seeAlso>
        <rdfs:seeAlso rdf:datatype="&xsd;string">This work has been inspired for the cryptographic concepts and security properties by &quot;Security in the Semantic Web using OWL&quot; [Denker et al. 2005]</rdfs:seeAlso>
        <rdfs:comment xml:lang="en"></rdfs:comment>
        <rdfs:comment xml:lang="en">A reference ontology to describe the IoT&apos;s security domain involving the main threats, assets, security mechanisms, OSI model, security protocols/tools and vulnerabilities.</rdfs:comment>
        <vann:preferredNamespacePrefix>iotsec</vann:preferredNamespacePrefix>
        <dc:title xml:lang="en">The Internet of Things (IoT) Security Ontology</dc:title>
        <vs:term_status>Work in progress</vs:term_status>
        <vann:preferredNamespaceUri>http://www-usr.inf.ufsm.br/~brunomozza/iotsec/iotsec.owl</vann:preferredNamespaceUri>
        <cc:license rdf:resource="http://creativecommons.org/licenses/by/3.0/"/>
    </owl:Ontology>
    


    <!-- 
    ///////////////////////////////////////////////////////////////////////////////////////
    //
    // Annotation properties
    //
    ///////////////////////////////////////////////////////////////////////////////////////
     -->

    


    <!-- http://purl.org/dc/terms/hasPart -->

    <owl:AnnotationProperty rdf:about="&dcterms;hasPart"/>
    


    <!-- http://www-usr.inf.ufsm.br/~brunomozza/iotsec/iotsec.owl#affects -->

    <owl:AnnotationProperty rdf:about="&iotsec;affects">
        <rdfs:label xml:lang="en">affects</rdfs:label>
        <rdfs:comment xml:lang="en">A threat affects one or more security properties. For instance, an eavesdropping threat affects the security property Authentication. </rdfs:comment>
    </owl:AnnotationProperty>
    


    <!-- http://www-usr.inf.ufsm.br/~brunomozza/iotsec/iotsec.owl#generates -->

    <owl:AnnotationProperty rdf:about="&iotsec;generates">
        <rdfs:label xml:lang="en">generates</rdfs:label>
        <rdfs:comment xml:lang="en">A vulnerability generates a risk for an organization because it can exposes sensitive information for malicious actions of intruders.</rdfs:comment>
    </owl:AnnotationProperty>
    


    <!-- http://www-usr.inf.ufsm.br/~brunomozza/iotsec/iotsec.owl#hasFeature -->

    <owl:AnnotationProperty rdf:about="&iotsec;hasFeature">
        <rdfs:label xml:lang="en">hasFeature</rdfs:label>
        <rdfs:comment xml:lang="en">A security mechanism has specific features that can incapacitate the use with a determined situation. For example, an asymmetric algorithm has high energy consuming and it can to harm the consume of battery of an active RFID.</rdfs:comment>
    </owl:AnnotationProperty>
    


    <!-- http://www-usr.inf.ufsm.br/~brunomozza/iotsec/iotsec.owl#hasModeOperation -->

    <owl:AnnotationProperty rdf:about="&iotsec;hasModeOperation">
        <rdfs:label xml:lang="en">hasModeOperation</rdfs:label>
        <rdfs:comment xml:lang="en"></rdfs:comment>
    </owl:AnnotationProperty>
    


    <!-- http://www-usr.inf.ufsm.br/~brunomozza/iotsec/iotsec.owl#hasPart -->

    <owl:AnnotationProperty rdf:about="&iotsec;hasPart">
        <rdfs:label xml:lang="en">hasPart</rdfs:label>
        <rdfs:comment xml:lang="en">A security mechanism can use or be used as part of other mechanism to mitigate an vulnerability or to protect an asset.</rdfs:comment>
    </owl:AnnotationProperty>
    


    <!-- http://www-usr.inf.ufsm.br/~brunomozza/iotsec/iotsec.owl#hasSecurityMechanism -->

    <owl:AnnotationProperty rdf:about="&iotsec;hasSecurityMechanism">
        <rdfs:label xml:lang="en">hasModeOperation</rdfs:label>
        <rdfs:comment xml:lang="en"></rdfs:comment>
    </owl:AnnotationProperty>
    


    <!-- http://www-usr.inf.ufsm.br/~brunomozza/iotsec/iotsec.owl#hasSeverity -->

    <owl:AnnotationProperty rdf:about="&iotsec;hasSeverity">
        <rdfs:label xml:lang="en">hasSeverity</rdfs:label>
        <rdfs:comment xml:lang="en">A vulnerability can be classified according to level of severity. For instance, high, medium and low level.</rdfs:comment>
    </owl:AnnotationProperty>
    


    <!-- http://www-usr.inf.ufsm.br/~brunomozza/iotsec/iotsec.owl#hasType -->

    <owl:AnnotationProperty rdf:about="&iotsec;hasType">
        <rdfs:label xml:lang="en">hasType</rdfs:label>
        <rdfs:comment xml:lang="en">A security mechanism implements a security tool to protect assets and to mitigate vulnerabilities using distinct type of defense such as: detection, prevention, recovery or corretion.</rdfs:comment>
    </owl:AnnotationProperty>
    


    <!-- http://www-usr.inf.ufsm.br/~brunomozza/iotsec/iotsec.owl#hasVulnerability -->

    <owl:AnnotationProperty rdf:about="&iotsec;hasVulnerability">
        <rdfs:label xml:lang="en">hasVulnerability</rdfs:label>
        <rdfs:comment xml:lang="en">An organization has flaws in your assets that can be physical, technical or administrative weakness which it makes vulnerable to attackers.</rdfs:comment>
    </owl:AnnotationProperty>
    


    <!-- http://www-usr.inf.ufsm.br/~brunomozza/iotsec/iotsec.owl#hashasModeOperation -->

    <owl:AnnotationProperty rdf:about="&iotsec;hashasModeOperation"/>
    


    <!-- http://www-usr.inf.ufsm.br/~brunomozza/iotsec/iotsec.owl#initiates -->

    <owl:AnnotationProperty rdf:about="&iotsec;initiates">
        <rdfs:label xml:lang="en">initiates</rdfs:label>
        <rdfs:comment xml:lang="en">An threat has a origin that can be accidental or intentional source.</rdfs:comment>
    </owl:AnnotationProperty>
    


    <!-- http://www-usr.inf.ufsm.br/~brunomozza/iotsec/iotsec.owl#isReplacedBy -->

    <owl:AnnotationProperty rdf:about="&iotsec;isReplacedBy">
        <rdfs:label xml:lang="en">isReplacedBy</rdfs:label>
        <rdfs:comment xml:lang="en"></rdfs:comment>
    </owl:AnnotationProperty>
    


    <!-- http://www-usr.inf.ufsm.br/~brunomozza/iotsec/iotsec.owl#isSecurityMechanismOf -->

    <owl:AnnotationProperty rdf:about="&iotsec;isSecurityMechanismOf">
        <rdfs:label xml:lang="en">isSecurityMechanismOf</rdfs:label>
        <rdfs:comment xml:lang="en">Security mechanisms are developed to mitigates flaws and protect assets. Normally, security mechanisms are defined as countermeasures to block, detect or prevent threats with specific behavior characterized. For instance, normally, firewall mechanism are used to block malicious traffic in network or web application.</rdfs:comment>
    </owl:AnnotationProperty>
    


    <!-- http://www-usr.inf.ufsm.br/~brunomozza/iotsec/iotsec.owl#isVulnerabilityOf -->

    <owl:AnnotationProperty rdf:about="&iotsec;isVulnerabilityOf">
        <rdfs:label xml:lang="en">isVulnerabilityOf</rdfs:label>
        <rdfs:comment xml:lang="en"></rdfs:comment>
    </owl:AnnotationProperty>
    


    <!-- http://www-usr.inf.ufsm.br/~brunomozza/iotsec/iotsec.owl#mitigates -->

    <owl:AnnotationProperty rdf:about="&iotsec;mitigates">
        <rdfs:label xml:lang="en">mitigates</rdfs:label>
        <rdfs:comment xml:lang="en">Security mechanism are projected to mitigate the asset&apos;s vulnerabilities which can be physical, technical or administrative weakness.</rdfs:comment>
    </owl:AnnotationProperty>
    


    <!-- http://www-usr.inf.ufsm.br/~brunomozza/iotsec/iotsec.owl#occursInLayer -->

    <owl:AnnotationProperty rdf:about="&iotsec;occursInLayer">
        <rdfs:label xml:lang="en">occursIn</rdfs:label>
        <rdfs:label xml:lang="en">occursInLayer</rdfs:label>
        <rdfs:comment xml:lang="en">A threat occurs in a specific layer of OSI Model. For instance, an eavesdropping attack explores the physical layer.</rdfs:comment>
    </owl:AnnotationProperty>
    


    <!-- http://www-usr.inf.ufsm.br/~brunomozza/iotsec/iotsec.owl#owner -->

    <owl:AnnotationProperty rdf:about="&iotsec;owner">
        <rdfs:label xml:lang="en">owner</rdfs:label>
        <rdfs:comment xml:lang="en"></rdfs:comment>
    </owl:AnnotationProperty>
    


    <!-- http://www-usr.inf.ufsm.br/~brunomozza/iotsec/iotsec.owl#protects -->

    <owl:AnnotationProperty rdf:about="&iotsec;protects">
        <rdfs:label xml:lang="en">protects</rdfs:label>
        <rdfs:comment xml:lang="en">The security mechanism allows to protect an organization&apos;s asset against malicious actions of the intruders. For instance, the security mechanism called Virtual Private Network (VPN) is used to protect an user when it is using an Wifi &quot;untrusted&quot; network.</rdfs:comment>
    </owl:AnnotationProperty>
    


    <!-- http://www-usr.inf.ufsm.br/~brunomozza/iotsec/iotsec.owl#protectsInLayer -->

    <owl:AnnotationProperty rdf:about="&iotsec;protectsInLayer">
        <rdfs:label xml:lang="en">protectsInLayer</rdfs:label>
        <rdfs:comment xml:lang="en"></rdfs:comment>
    </owl:AnnotationProperty>
    


    <!-- http://www-usr.inf.ufsm.br/~brunomozza/iotsec/iotsec.owl#satisfies -->

    <owl:AnnotationProperty rdf:about="&iotsec;satisfies">
        <rdfs:label xml:lang="en">satisfies</rdfs:label>
        <rdfs:comment xml:lang="en">Security mechanisms are designed to protect assets and to mitigate vulnerabilities, but in some situations they can not ensure security properties. In this context, the composition of several security mechanisms are used to cover them. In several situations, different security mechanisms are used to protect an organization&apos; asset. For instances, the TinySec is first fully-implemented link-layer security protocol to wireless sensor network (WSN) which have limited power resources, battery life and communication capabilities to guarantee authenticity, integrity and confidentiality. This protocol protects against resource consumption attacks, physical tamper resistance and node capture attacks. By another side, the TinySec protocol does not protect against replay attacks because it does not have the resources for this. So, the solution is add another higher level security protocol to solve this problem.</rdfs:comment>
    </owl:AnnotationProperty>
    


    <!-- http://www-usr.inf.ufsm.br/~brunomozza/iotsec/iotsec.owl#securityRecommendation -->

    <owl:AnnotationProperty rdf:about="&iotsec;securityRecommendation">
        <rdfs:label xml:lang="en">Security Recommendation</rdfs:label>
        <rdfs:comment xml:lang="en"></rdfs:comment>
    </owl:AnnotationProperty>
    


    <!-- http://www-usr.inf.ufsm.br/~brunomozza/iotsec/iotsec.owl#securityRequirement -->

    <owl:AnnotationProperty rdf:about="&iotsec;securityRequirement">
        <rdfs:label xml:lang="en">Security Requirement</rdfs:label>
        <rdfs:comment xml:lang="en"></rdfs:comment>
    </owl:AnnotationProperty>
    


    <!-- http://www-usr.inf.ufsm.br/~brunomozza/iotsec/iotsec.owl#threatens -->

    <owl:AnnotationProperty rdf:about="&iotsec;threatens">
        <rdfs:label xml:lang="en">threatens</rdfs:label>
        <rdfs:comment xml:lang="en">Threats are created to explores the physical, technical and administrative weakness. Many of them are used in one vulnerability already not explored and, it normally explores a flaw recently discovered (zero-day vulnerability) by a hacker. This threat will be efficiently until a security mechanism is designed to block it or the flaw is corrected.</rdfs:comment>
    </owl:AnnotationProperty>
    


    <!-- http://www-usr.inf.ufsm.br/~brunomozza/iotsec/iotsec.owl#uses -->

    <owl:AnnotationProperty rdf:about="&iotsec;uses">
        <rdfs:label xml:lang="en">uses</rdfs:label>
        <rdfs:comment xml:lang="en"></rdfs:comment>
    </owl:AnnotationProperty>
    


    <!-- 
    ///////////////////////////////////////////////////////////////////////////////////////
    //
    // Object Properties
    //
    ///////////////////////////////////////////////////////////////////////////////////////
     -->

    


    <!-- http://www-usr.inf.ufsm.br/~brunomozza/iotsec/iotsec.owl#affects -->

    <owl:ObjectProperty rdf:about="&iotsec;affects">
        <rdfs:label xml:lang="en">affects</rdfs:label>
        <rdfs:comment xml:lang="en">A threat affects one or more security properties. For instance, an eavesdropping threat affects the security property Authentication. </rdfs:comment>
        <rdfs:range rdf:resource="&iotsec;SecurityProperty"/>
        <rdfs:domain rdf:resource="&iotsec;Threat"/>
    </owl:ObjectProperty>
    


    <!-- http://www-usr.inf.ufsm.br/~brunomozza/iotsec/iotsec.owl#generates -->

    <owl:ObjectProperty rdf:about="&iotsec;generates">
        <rdfs:label xml:lang="en">generates</rdfs:label>
        <rdfs:comment xml:lang="en">A vulnerability generates a risk for an organization because it can exposes sensitive information for malicious actions of intruders.</rdfs:comment>
        <rdfs:range rdf:resource="&iotsec;Risk"/>
        <rdfs:domain rdf:resource="&iotsec;Vulnerability"/>
    </owl:ObjectProperty>
    


    <!-- http://www-usr.inf.ufsm.br/~brunomozza/iotsec/iotsec.owl#hasFeature -->

    <owl:ObjectProperty rdf:about="&iotsec;hasFeature">
        <rdfs:label xml:lang="en">hasFeature</rdfs:label>
        <rdfs:comment xml:lang="en">A security mechanism has specific features that can incapacitate the use with a determined situation. For example, an asymmetric algorithm has high energy consuming and it can to harm the consume of battery of an active RFID.</rdfs:comment>
        <rdfs:range rdf:resource="&iotsec;Feature"/>
        <rdfs:domain rdf:resource="&iotsec;SecurityMechanism"/>
    </owl:ObjectProperty>
    


    <!-- http://www-usr.inf.ufsm.br/~brunomozza/iotsec/iotsec.owl#hasPart -->

    <owl:ObjectProperty rdf:about="&iotsec;hasPart">
        <rdf:type rdf:resource="&owl;ReflexiveProperty"/>
        <rdfs:label xml:lang="en">hasPart</rdfs:label>
        <rdfs:comment xml:lang="en">A security mechanism can use or be used as part of other mechanism to mitigate an vulnerability or to protect an asset.</rdfs:comment>
        <rdfs:domain rdf:resource="&iotsec;SecurityMechanism"/>
    </owl:ObjectProperty>
    


    <!-- http://www-usr.inf.ufsm.br/~brunomozza/iotsec/iotsec.owl#hasSeverity -->

    <owl:ObjectProperty rdf:about="&iotsec;hasSeverity">
        <rdfs:label xml:lang="en">hasSeverity</rdfs:label>
        <rdfs:comment xml:lang="en">A vulnerability can be classified according to level of severity. For instance, high, medium and low level.</rdfs:comment>
        <rdfs:range rdf:resource="&iotsec;SeverityScale"/>
        <rdfs:domain rdf:resource="&iotsec;Vulnerability"/>
    </owl:ObjectProperty>
    


    <!-- http://www-usr.inf.ufsm.br/~brunomozza/iotsec/iotsec.owl#hasType -->

    <owl:ObjectProperty rdf:about="&iotsec;hasType">
        <rdfs:label xml:lang="en">hasType</rdfs:label>
        <rdfs:comment xml:lang="en">A security mechanism implements a security tool to protect assets and to mitigate vulnerabilities using distinct type of defense such as: detection, prevention, recovery or corretion.</rdfs:comment>
        <rdfs:domain rdf:resource="&iotsec;SecurityMechanism"/>
        <rdfs:range rdf:resource="&iotsec;TypeofDefense"/>
        <owl:inverseOf rdf:resource="&iotsec;isTypeOf"/>
    </owl:ObjectProperty>
    


    <!-- http://www-usr.inf.ufsm.br/~brunomozza/iotsec/iotsec.owl#hasVulnerability -->

    <owl:ObjectProperty rdf:about="&iotsec;hasVulnerability">
        <rdfs:label xml:lang="en">hasVulnerability</rdfs:label>
        <rdfs:comment xml:lang="en">An organization has flaws in your assets that can be physical, technical or administrative weakness which it makes vulnerable to attackers.</rdfs:comment>
        <rdfs:domain rdf:resource="&iotsec;Asset"/>
        <rdfs:range rdf:resource="&iotsec;Vulnerability"/>
        <owl:inverseOf rdf:resource="&iotsec;isVulnerabilityOf"/>
    </owl:ObjectProperty>
    


    <!-- http://www-usr.inf.ufsm.br/~brunomozza/iotsec/iotsec.owl#initiates -->

    <owl:ObjectProperty rdf:about="&iotsec;initiates">
        <rdfs:label xml:lang="en">initiates</rdfs:label>
        <rdfs:comment xml:lang="en">An threat has a origin that can be accidental or intentional source.</rdfs:comment>
        <rdfs:range rdf:resource="&iotsec;Threat"/>
    </owl:ObjectProperty>
    


    <!-- http://www-usr.inf.ufsm.br/~brunomozza/iotsec/iotsec.owl#isMitigateBy -->

    <owl:ObjectProperty rdf:about="&iotsec;isMitigateBy">
        <rdfs:label xml:lang="en">isMitigateBy</rdfs:label>
        <rdfs:comment xml:lang="en"></rdfs:comment>
        <owl:inverseOf rdf:resource="&iotsec;mitigates"/>
    </owl:ObjectProperty>
    


    <!-- http://www-usr.inf.ufsm.br/~brunomozza/iotsec/iotsec.owl#isSecurityMechanismOf -->

    <owl:ObjectProperty rdf:about="&iotsec;isSecurityMechanismOf">
        <rdfs:label xml:lang="en">isSecurityMechanismOf</rdfs:label>
        <rdfs:comment xml:lang="en">Security mechanisms are developed to mitigates flaws and protect assets. Normally, security mechanisms are defined as countermeasures to block, detect or prevent threats with specific behavior characterized. For instance, normally, firewall mechanism are used to block malicious traffic in network or web application.</rdfs:comment>
        <rdfs:domain rdf:resource="&iotsec;SecurityMechanism"/>
        <rdfs:range rdf:resource="&iotsec;Threat"/>
    </owl:ObjectProperty>
    


    <!-- http://www-usr.inf.ufsm.br/~brunomozza/iotsec/iotsec.owl#isTypeOf -->

    <owl:ObjectProperty rdf:about="&iotsec;isTypeOf">
        <rdfs:label xml:lang="en">isTypeOf</rdfs:label>
        <rdfs:comment xml:lang="en"></rdfs:comment>
    </owl:ObjectProperty>
    


    <!-- http://www-usr.inf.ufsm.br/~brunomozza/iotsec/iotsec.owl#isVulnerabilityOf -->

    <owl:ObjectProperty rdf:about="&iotsec;isVulnerabilityOf">
        <rdfs:label xml:lang="en">isVulnerabilityOf</rdfs:label>
        <rdfs:comment xml:lang="en"></rdfs:comment>
    </owl:ObjectProperty>
    


    <!-- http://www-usr.inf.ufsm.br/~brunomozza/iotsec/iotsec.owl#mitigates -->

    <owl:ObjectProperty rdf:about="&iotsec;mitigates">
        <rdfs:label xml:lang="en">mitigates</rdfs:label>
        <rdfs:comment xml:lang="en">Security mechanism are projected to mitigate the asset&apos;s vulnerabilities which can be physical, technical or administrative weakness.</rdfs:comment>
        <rdfs:domain rdf:resource="&iotsec;SecurityMechanism"/>
        <rdfs:range rdf:resource="&iotsec;Vulnerability"/>
    </owl:ObjectProperty>
    


    <!-- http://www-usr.inf.ufsm.br/~brunomozza/iotsec/iotsec.owl#occursInLayer -->

    <owl:ObjectProperty rdf:about="&iotsec;occursInLayer">
        <rdfs:label xml:lang="en">occursIn</rdfs:label>
        <rdfs:label xml:lang="en">occursInLayer</rdfs:label>
        <rdfs:comment xml:lang="en">A threat occurs in a specific layer of OSI Model. For instance, an eavesdropping attack explores the physical layer.</rdfs:comment>
        <rdfs:range rdf:resource="&iotsec;OSIModelLayer"/>
        <rdfs:domain rdf:resource="&iotsec;Threat"/>
    </owl:ObjectProperty>
    


    <!-- http://www-usr.inf.ufsm.br/~brunomozza/iotsec/iotsec.owl#protects -->

    <owl:ObjectProperty rdf:about="&iotsec;protects">
        <rdfs:label xml:lang="en">protects</rdfs:label>
        <rdfs:comment xml:lang="en">The security mechanism allows to protect an organization&apos;s asset against malicious actions of the intruders. For instance, the security mechanism called Virtual Private Network (VPN) is used to protect an user when it is using an Wifi &quot;untrusted&quot; network.</rdfs:comment>
        <rdfs:range rdf:resource="&iotsec;Asset"/>
        <rdfs:domain rdf:resource="&iotsec;SecurityMechanism"/>
    </owl:ObjectProperty>
    


    <!-- http://www-usr.inf.ufsm.br/~brunomozza/iotsec/iotsec.owl#requires -->

    <owl:ObjectProperty rdf:about="&iotsec;requires">
        <rdfs:label xml:lang="en">requires</rdfs:label>
        <rdfs:comment xml:lang="en">Organizations&apos; assets have requirements to work normally, involving the main security  properties. For instance, a web server need maintain the service available to users in all the time. For that, this security property is required by web server. In case of one threat attacks the web server, this security property will be affected.</rdfs:comment>
        <rdfs:domain rdf:resource="&iotsec;Asset"/>
        <rdfs:range rdf:resource="&iotsec;SecurityProperty"/>
    </owl:ObjectProperty>
    


    <!-- http://www-usr.inf.ufsm.br/~brunomozza/iotsec/iotsec.owl#satisfies -->

    <owl:ObjectProperty rdf:about="&iotsec;satisfies">
        <rdfs:label xml:lang="en">satisfies</rdfs:label>
        <rdfs:comment xml:lang="en">Security mechanisms are designed to protect assets and to mitigate vulnerabilities, but in some situations they can not ensure security properties. In this context, the composition of several security mechanisms are used to cover them. In several situations, different security mechanisms are used to protect an organization&apos; asset. For instances, the TinySec is first fully-implemented link-layer security protocol to wireless sensor network (WSN) which have limited power resources, battery life and communication capabilities to guarantee authenticity, integrity and confidentiality. This protocol protects against resource consumption attacks, physical tamper resistance and node capture attacks. By another side, the TinySec protocol does not protect against replay attacks because it does not have the resources for this. So, the solution is add another higher level security protocol to solve this problem.</rdfs:comment>
        <rdfs:domain rdf:resource="&iotsec;SecurityMechanism"/>
        <rdfs:range rdf:resource="&iotsec;SecurityProperty"/>
    </owl:ObjectProperty>
    


    <!-- http://www-usr.inf.ufsm.br/~brunomozza/iotsec/iotsec.owl#threatens -->

    <owl:ObjectProperty rdf:about="&iotsec;threatens">
        <rdfs:label xml:lang="en">threatens</rdfs:label>
        <rdfs:comment xml:lang="en">Threats are created to explores the physical, technical and administrative weakness. Many of them are used in one vulnerability already not explored and, it normally explores a flaw recently discovered (zero-day vulnerability) by a hacker. This threat will be efficiently until a security mechanism is designed to block it or the flaw is corrected.</rdfs:comment>
        <rdfs:domain rdf:resource="&iotsec;Threat"/>
        <rdfs:range rdf:resource="&iotsec;Vulnerability"/>
    </owl:ObjectProperty>
    


    <!-- 
    ///////////////////////////////////////////////////////////////////////////////////////
    //
    // Classes
    //
    ///////////////////////////////////////////////////////////////////////////////////////
     -->

    


    <!-- http://securitytoolbox.appspot.com/stac#Architecture -->

    <owl:Class rdf:about="&stac;Architecture">
        <rdfs:label xml:lang="en">Architecture</rdfs:label>
        <rdfs:subClassOf rdf:resource="&iotsec;Asset"/>
        <rdfs:comment xml:lang="en"></rdfs:comment>
    </owl:Class>
    


    <!-- http://securitytoolbox.appspot.com/stac#ExchangeKeyEasy -->

    <owl:Class rdf:about="&stac;ExchangeKeyEasy">
        <rdfs:label xml:lang="en">Exchange Key Easy</rdfs:label>
        <rdfs:subClassOf rdf:resource="&iotsec;PositiveFeature"/>
        <rdfs:comment xml:lang="en"></rdfs:comment>
    </owl:Class>
    


    <!-- http://securitytoolbox.appspot.com/stac#Flexible -->

    <owl:Class rdf:about="&stac;Flexible">
        <rdfs:label xml:lang="en">Flexible</rdfs:label>
        <rdfs:subClassOf rdf:resource="&iotsec;PositiveFeature"/>
        <rdfs:comment xml:lang="en"></rdfs:comment>
    </owl:Class>
    


    <!-- http://securitytoolbox.appspot.com/stac#GPRSArchitecture -->

    <owl:Class rdf:about="&stac;GPRSArchitecture">
        <rdfs:label xml:lang="en">GPRS Architecture</rdfs:label>
        <rdfs:subClassOf rdf:resource="&stac;Architecture"/>
        <rdfs:comment xml:lang="en">The GPRS system are a much more expesed to intruders, because of its IP based backbone.</rdfs:comment>
    </owl:Class>
    


    <!-- http://securitytoolbox.appspot.com/stac#GPRSArchitectureComponent -->

    <owl:Class rdf:about="&stac;GPRSArchitectureComponent">
        <rdfs:label xml:lang="en">GPRS Architecture component</rdfs:label>
        <rdfs:subClassOf rdf:resource="&stac;GPRSArchitecture"/>
        <rdfs:comment xml:lang="en"></rdfs:comment>
    </owl:Class>
    


    <!-- http://securitytoolbox.appspot.com/stac#GSMArchitecture -->

    <owl:Class rdf:about="&stac;GSMArchitecture">
        <rdfs:label xml:lang="en">GSM Architecture</rdfs:label>
        <rdfs:subClassOf rdf:resource="&stac;Architecture"/>
        <rdfs:comment xml:lang="en"></rdfs:comment>
    </owl:Class>
    


    <!-- http://securitytoolbox.appspot.com/stac#GSMArchitectureComponent -->

    <owl:Class rdf:about="&stac;GSMArchitectureComponent">
        <rdfs:label xml:lang="en">GSM Architecture component</rdfs:label>
        <rdfs:subClassOf rdf:resource="&stac;GSMArchitecture"/>
        <rdfs:comment xml:lang="en"></rdfs:comment>
    </owl:Class>
    


    <!-- http://securitytoolbox.appspot.com/stac#HighEnergyConsuming -->

    <owl:Class rdf:about="&stac;HighEnergyConsuming">
        <rdfs:label xml:lang="en">High Energy Consuming</rdfs:label>
        <rdfs:subClassOf rdf:resource="&iotsec;NegativeFeature"/>
        <rdfs:comment xml:lang="en"></rdfs:comment>
    </owl:Class>
    


    <!-- http://securitytoolbox.appspot.com/stac#LowCostDeployment -->

    <owl:Class rdf:about="&stac;LowCostDeployment">
        <rdfs:label xml:lang="en">Low Cost Deployment</rdfs:label>
        <rdfs:subClassOf rdf:resource="&iotsec;PositiveFeature"/>
        <rdfs:comment xml:lang="en"></rdfs:comment>
    </owl:Class>
    


    <!-- http://securitytoolbox.appspot.com/stac#Scalable -->

    <owl:Class rdf:about="&stac;Scalable">
        <rdfs:label xml:lang="en">Scalable</rdfs:label>
        <rdfs:subClassOf rdf:resource="&iotsec;PositiveFeature"/>
        <rdfs:comment xml:lang="en">Can scale to form large-scale networks with arbitrary coverage and complexity.</rdfs:comment>
    </owl:Class>
    


    <!-- http://www-usr.inf.ufsm.br/~brunomozza/iotsec/iotsec.owl#AccessControlMethod -->

    <owl:Class rdf:about="&iotsec;AccessControlMethod">
        <rdfs:label xml:lang="en">Access Control Method</rdfs:label>
        <rdfs:subClassOf rdf:resource="&iotsec;SecurityPropertyMethod"/>
        <rdfs:comment xml:lang="en">Access Control is the mechanism that allows owners of resources to define, manage and enforce access conditions applicable to each resource [Gyrard 2014].</rdfs:comment>
    </owl:Class>
    


    <!-- http://www-usr.inf.ufsm.br/~brunomozza/iotsec/iotsec.owl#ActiveAttack -->

    <owl:Class rdf:about="&iotsec;ActiveAttack">
        <rdfs:subClassOf rdf:resource="&iotsec;Threat"/>
        <rdfs:comment xml:lang="en">Active attacks involve actions performed by adversaries to gain the control of the network [Gyrard 2014].</rdfs:comment>
    </owl:Class>
    


    <!-- http://www-usr.inf.ufsm.br/~brunomozza/iotsec/iotsec.owl#Antivirus -->

    <owl:Class rdf:about="&iotsec;Antivirus">
        <rdfs:label xml:lang="en">Antivirus</rdfs:label>
        <rdfs:subClassOf rdf:resource="&iotsec;M2MSecurityMechanism"/>
        <rdfs:subClassOf rdf:resource="&iotsec;NetworkManagementSecurityMechanism"/>
        <rdfs:comment xml:lang="en">Anti-viruses softwares applications will reduce viruses and malware on M2M equipment [Gyrard 2014].</rdfs:comment>
        <rdfs:seeAlso xml:lang="en">See Paper: A study of information security for M2M and IoT [Jiang et al. 2010]</rdfs:seeAlso>
    </owl:Class>
    


    <!-- http://www-usr.inf.ufsm.br/~brunomozza/iotsec/iotsec.owl#ApplicationLayer -->

    <owl:Class rdf:about="&iotsec;ApplicationLayer">
        <rdfs:label xml:lang="en">Application Layer</rdfs:label>
        <rdfs:subClassOf rdf:resource="&iotsec;OSIModelLayer"/>
        <rdfs:comment xml:lang="en"></rdfs:comment>
    </owl:Class>
    


    <!-- http://www-usr.inf.ufsm.br/~brunomozza/iotsec/iotsec.owl#Asset -->

    <owl:Class rdf:about="&iotsec;Asset">
        <rdfs:label xml:lang="en">Asset</rdfs:label>
        <rdfs:subClassOf>
            <owl:Restriction>
                <owl:onProperty rdf:resource="&iotsec;requires"/>
                <owl:someValuesFrom rdf:resource="&iotsec;SecurityProperty"/>
            </owl:Restriction>
        </rdfs:subClassOf>
        <rdfs:subClassOf>
            <owl:Restriction>
                <owl:onProperty rdf:resource="&iotsec;hasVulnerability"/>
                <owl:someValuesFrom rdf:resource="&iotsec;Vulnerability"/>
            </owl:Restriction>
        </rdfs:subClassOf>
        <rdfs:comment xml:lang="en">.</rdfs:comment>
    </owl:Class>
    


    <!-- http://www-usr.inf.ufsm.br/~brunomozza/iotsec/iotsec.owl#AsymmetricAlgorithm -->

    <owl:Class rdf:about="&iotsec;AsymmetricAlgorithm">
        <rdfs:label xml:lang="en">Asymmetric algorithm</rdfs:label>
        <rdfs:subClassOf rdf:resource="&iotsec;AuthenticationMethod"/>
        <rdfs:subClassOf rdf:resource="&iotsec;EncryptionAlgorithm"/>
        <rdfs:subClassOf>
            <owl:Restriction>
                <owl:onProperty rdf:resource="&iotsec;hasFeature"/>
                <owl:someValuesFrom rdf:resource="&stac;ExchangeKeyEasy"/>
            </owl:Restriction>
        </rdfs:subClassOf>
        <rdfs:subClassOf>
            <owl:Restriction>
                <owl:onProperty rdf:resource="&iotsec;hasFeature"/>
                <owl:someValuesFrom rdf:resource="&stac;HighEnergyConsuming"/>
            </owl:Restriction>
        </rdfs:subClassOf>
        <rdfs:comment xml:lang="en">The keys used for encryption and decryption are different, allowing for easier key distribution.</rdfs:comment>
        <rdfs:seeAlso rdf:resource="&secberlin;Asymmetric_cryptographic_algorithm"/>
        <rdfs:seeAlso rdf:resource="&maso;Cryptage-asymetrique"/>
        <rdfs:seeAlso rdf:resource="&kimalgorithms;AsymmetricAlgorithm"/>
        <dcterms:hasPart rdf:resource="&stac;IndividualKey"/>
        <dcterms:hasPart rdf:resource="&stac;PrivateKey"/>
        <dcterms:hasPart rdf:resource="&stac;PublicKey"/>
        <rdfs:seeAlso rdf:resource="&securitysw;AsymmetricAlgorithm"/>
        <rdfs:seeAlso rdf:resource="&herzog;Public-KeyEncryption"/>
    </owl:Class>
    


    <!-- http://www-usr.inf.ufsm.br/~brunomozza/iotsec/iotsec.owl#AuthenticationMethod -->

    <owl:Class rdf:about="&iotsec;AuthenticationMethod">
        <rdfs:label xml:lang="en">Authentication Method</rdfs:label>
        <rdfs:subClassOf rdf:resource="&iotsec;SecurityPropertyMethod"/>
        <rdfs:comment xml:lang="en">Authentication prevents unauthorized access to the network [Gyrard 2014].</rdfs:comment>
    </owl:Class>
    


    <!-- http://www-usr.inf.ufsm.br/~brunomozza/iotsec/iotsec.owl#AuthenticationServer -->

    <owl:Class rdf:about="&iotsec;AuthenticationServer">
        <rdfs:label xml:lang="en">Authentication Server (AS)</rdfs:label>
        <rdfs:subClassOf rdf:resource="&iotsec;AuthenticationMethod"/>
        <rdfs:comment xml:lang="en">It identifies the supplicant, checks its credentials, and define privileges and restrictions, and allows or denies it access to the network and services [Gyrard 2014].</rdfs:comment>
    </owl:Class>
    


    <!-- http://www-usr.inf.ufsm.br/~brunomozza/iotsec/iotsec.owl#BlockCipher -->

    <owl:Class rdf:about="&iotsec;BlockCipher">
        <rdfs:label xml:lang="en">Block Cipher</rdfs:label>
        <rdfs:subClassOf rdf:resource="&iotsec;SymmetricAlgorithm"/>
        <rdfs:comment xml:lang="en"></rdfs:comment>
    </owl:Class>
    


    <!-- http://www-usr.inf.ufsm.br/~brunomozza/iotsec/iotsec.owl#BluetoothAttack -->

    <owl:Class rdf:about="&iotsec;BluetoothAttack">
        <rdfs:label xml:lang="en">Bluetooth Attack</rdfs:label>
        <rdfs:subClassOf rdf:resource="&iotsec;Threat"/>
        <rdfs:comment xml:lang="en"></rdfs:comment>
    </owl:Class>
    


    <!-- http://www-usr.inf.ufsm.br/~brunomozza/iotsec/iotsec.owl#BluetoothDevices -->

    <owl:Class rdf:about="&iotsec;BluetoothDevices">
        <rdfs:label xml:lang="en">Bluetooth Devices</rdfs:label>
        <rdfs:subClassOf rdf:resource="&iotsec;BluetoothTechnology"/>
        <rdfs:comment xml:lang="en"></rdfs:comment>
    </owl:Class>
    


    <!-- http://www-usr.inf.ufsm.br/~brunomozza/iotsec/iotsec.owl#BluetoothSecurityAlgorithm -->

    <owl:Class rdf:about="&iotsec;BluetoothSecurityAlgorithm">
        <rdfs:label xml:lang="en">Bluetooth Security Algorithm</rdfs:label>
        <rdfs:subClassOf rdf:resource="&iotsec;SecurityAlgorithm"/>
        <rdfs:comment xml:lang="en"></rdfs:comment>
    </owl:Class>
    


    <!-- http://www-usr.inf.ufsm.br/~brunomozza/iotsec/iotsec.owl#BluetoothSecurityMechanism -->

    <owl:Class rdf:about="&iotsec;BluetoothSecurityMechanism">
        <rdfs:label xml:lang="en">Bluetooth Security Mechanism</rdfs:label>
        <rdfs:subClassOf rdf:resource="&iotsec;SecurityMechanism"/>
        <rdfs:subClassOf>
            <owl:Restriction>
                <owl:onProperty rdf:resource="&iotsec;mitigates"/>
                <owl:someValuesFrom rdf:resource="&iotsec;BluetoothVulnerability"/>
            </owl:Restriction>
        </rdfs:subClassOf>
        <rdfs:comment xml:lang="en"></rdfs:comment>
    </owl:Class>
    


    <!-- http://www-usr.inf.ufsm.br/~brunomozza/iotsec/iotsec.owl#BluetoothTechnology -->

    <owl:Class rdf:about="&iotsec;BluetoothTechnology">
        <rdfs:label xml:lang="en">Bluetooth Technology</rdfs:label>
        <rdfs:subClassOf rdf:resource="&iotsec;Asset"/>
        <rdfs:comment xml:lang="en">A protocol for short-range (up to 100 meters) wireless networks [Gyrard 2014].</rdfs:comment>
        <rdfs:seeAlso rdf:resource="&serviceContext;Bluetooth"/>
        <rdfs:seeAlso rdf:resource="&ct;BluetoothConnectivity"/>
    </owl:Class>
    


    <!-- http://www-usr.inf.ufsm.br/~brunomozza/iotsec/iotsec.owl#BluetoothVulnerability -->

    <owl:Class rdf:about="&iotsec;BluetoothVulnerability">
        <rdfs:label xml:lang="en">Bluetooth Vulnerability</rdfs:label>
        <rdfs:subClassOf rdf:resource="&iotsec;Vulnerability"/>
        <rdfs:subClassOf>
            <owl:Restriction>
                <owl:onProperty rdf:resource="&iotsec;isVulnerabilityOf"/>
                <owl:someValuesFrom rdf:resource="&iotsec;BluetoothTechnology"/>
            </owl:Restriction>
        </rdfs:subClassOf>
        <rdfs:subClassOf>
            <owl:Restriction>
                <owl:onProperty rdf:resource="&iotsec;isMitigateBy"/>
                <owl:someValuesFrom rdf:resource="&iotsec;BluetoothSecurityMechanism"/>
            </owl:Restriction>
        </rdfs:subClassOf>
        <rdfs:comment xml:lang="en"></rdfs:comment>
    </owl:Class>
    


    <!-- http://www-usr.inf.ufsm.br/~brunomozza/iotsec/iotsec.owl#BufferErrors -->

    <owl:Class rdf:about="&iotsec;BufferErrors">
        <rdfs:label xml:lang="en">Buffer Errors</rdfs:label>
        <rdfs:subClassOf rdf:resource="&iotsec;ImproperInputValidation"/>
        <rdfs:comment xml:lang="en">The software performs operations on a memory buffer, but it can read from or write to a memory location that is outside of the intended boundary of the buffer [CWE-119].</rdfs:comment>
        <rdfs:seeAlso xml:lang="en">http://cwe.mitre.org/data/definitions/119.html</rdfs:seeAlso>
    </owl:Class>
    


    <!-- http://www-usr.inf.ufsm.br/~brunomozza/iotsec/iotsec.owl#ChecksumAlgorithm -->

    <owl:Class rdf:about="&iotsec;ChecksumAlgorithm">
        <rdfs:label xml:lang="en">Checksum Algorithm</rdfs:label>
        <rdfs:subClassOf rdf:resource="&iotsec;IntegrityMethod"/>
        <rdfs:comment xml:lang="en"></rdfs:comment>
    </owl:Class>
    


    <!-- http://www-usr.inf.ufsm.br/~brunomozza/iotsec/iotsec.owl#CloudAttack -->

    <owl:Class rdf:about="&iotsec;CloudAttack">
        <rdfs:label xml:lang="en">Cloud Attack</rdfs:label>
        <rdfs:subClassOf rdf:resource="&iotsec;WebAttack"/>
        <rdfs:comment xml:lang="en"></rdfs:comment>
    </owl:Class>
    


    <!-- http://www-usr.inf.ufsm.br/~brunomozza/iotsec/iotsec.owl#CloudTechnology -->

    <owl:Class rdf:about="&iotsec;CloudTechnology">
        <rdfs:label xml:lang="en">Cloud Technology</rdfs:label>
        <rdfs:subClassOf rdf:resource="&iotsec;WebTechnology"/>
        <rdfs:comment xml:lang="en"></rdfs:comment>
    </owl:Class>
    


    <!-- http://www-usr.inf.ufsm.br/~brunomozza/iotsec/iotsec.owl#CloudVulnerability -->

    <owl:Class rdf:about="&iotsec;CloudVulnerability">
        <rdfs:label xml:lang="en">Cloud Vulnerability</rdfs:label>
        <rdfs:subClassOf rdf:resource="&iotsec;WebVulnerability"/>
        <rdfs:comment xml:lang="en"></rdfs:comment>
    </owl:Class>
    


    <!-- http://www-usr.inf.ufsm.br/~brunomozza/iotsec/iotsec.owl#Code -->

    <owl:Class rdf:about="&iotsec;Code">
        <rdfs:label xml:lang="en">Code</rdfs:label>
        <rdfs:subClassOf rdf:resource="&iotsec;SoftwareVulnerability"/>
        <rdfs:comment xml:lang="en">Weaknesses in this category are typically introduced during code development, including specification, design, and implementation [CWE-17].</rdfs:comment>
        <rdfs:seeAlso xml:lang="en">http://cwe.mitre.org/data/definitions/17.html</rdfs:seeAlso>
    </owl:Class>
    


    <!-- http://www-usr.inf.ufsm.br/~brunomozza/iotsec/iotsec.owl#CodeInjection -->

    <owl:Class rdf:about="&iotsec;CodeInjection">
        <rdfs:label xml:lang="en">Code Injection</rdfs:label>
        <rdfs:subClassOf rdf:resource="&iotsec;Injection"/>
        <rdfs:comment xml:lang="en">The software constructs all or part of a code segment using externally-influenced input from an upstream component, but it does not neutralize or incorrectly neutralizes special elements that could modify the syntax or behavior of the intended code segment [CWE-94].</rdfs:comment>
        <rdfs:seeAlso xml:lang="en">http://cwe.mitre.org/data/definitions/94.html</rdfs:seeAlso>
    </owl:Class>
    


    <!-- http://www-usr.inf.ufsm.br/~brunomozza/iotsec/iotsec.owl#CommandInjection -->

    <owl:Class rdf:about="&iotsec;CommandInjection">
        <rdfs:label xml:lang="en">Command Injection</rdfs:label>
        <rdfs:subClassOf rdf:resource="&iotsec;Injection"/>
        <rdfs:comment xml:lang="en">The software constructs all or part of a command using externally-influenced input from an upstream component, but it does not neutralize or incorrectly neutralizes special elements that could modify the intended command when it is sent to a downstream component [CWE-77].</rdfs:comment>
        <rdfs:seeAlso xml:lang="en">http://cwe.mitre.org/data/definitions/77.html</rdfs:seeAlso>
    </owl:Class>
    


    <!-- http://www-usr.inf.ufsm.br/~brunomozza/iotsec/iotsec.owl#Configuration -->

    <owl:Class rdf:about="&iotsec;Configuration">
        <rdfs:label xml:lang="en">Configuration</rdfs:label>
        <rdfs:subClassOf rdf:resource="&iotsec;SoftwareVulnerability"/>
        <rdfs:comment xml:lang="en">Weaknesses in this category are typically introduced during the configuration of the software [CWE-16].</rdfs:comment>
        <rdfs:seeAlso xml:lang="en">http://cwe.mitre.org/data/definitions/16.html</rdfs:seeAlso>
    </owl:Class>
    


    <!-- http://www-usr.inf.ufsm.br/~brunomozza/iotsec/iotsec.owl#CredentialsManagement -->

    <owl:Class rdf:about="&iotsec;CredentialsManagement">
        <rdfs:label xml:lang="en">Credentials Management</rdfs:label>
        <rdfs:subClassOf rdf:resource="&iotsec;SecurityFeatures"/>
        <rdfs:comment xml:lang="en">Weaknesses in this category are related to the management of credentials [CWE-255].</rdfs:comment>
        <rdfs:seeAlso xml:lang="en">http://cwe.mitre.org/data/definitions/255.html</rdfs:seeAlso>
    </owl:Class>
    


    <!-- http://www-usr.inf.ufsm.br/~brunomozza/iotsec/iotsec.owl#CrossSiteRequestForgery -->

    <owl:Class rdf:about="&iotsec;CrossSiteRequestForgery">
        <rdfs:label xml:lang="en">Cross-Site Request Forgery (CSRF)</rdfs:label>
        <rdfs:subClassOf rdf:resource="&iotsec;InsufficientVerificationDataAuthenticity"/>
        <rdfs:comment xml:lang="en">The web application does not, or can not, sufficiently verify whether a well-formed, valid, consistent request was intentionally provided by the user who submitted the request [CWE-352].</rdfs:comment>
        <rdfs:seeAlso xml:lang="en">http://cwe.mitre.org/data/definitions/352.html</rdfs:seeAlso>
    </owl:Class>
    


    <!-- http://www-usr.inf.ufsm.br/~brunomozza/iotsec/iotsec.owl#CrossSiteScripting -->

    <owl:Class rdf:about="&iotsec;CrossSiteScripting">
        <rdfs:label xml:lang="en">Cross-Site Scripting (XSS)</rdfs:label>
        <rdfs:subClassOf rdf:resource="&iotsec;Injection"/>
        <rdfs:comment xml:lang="en">The software does not neutralize or incorrectly neutralizes user-controllable input before it is placed in output that is used as a web page that is served to other users [CWE-79].</rdfs:comment>
        <rdfs:seeAlso xml:lang="en">http://cwe.mitre.org/data/definitions/79.html</rdfs:seeAlso>
    </owl:Class>
    


    <!-- http://www-usr.inf.ufsm.br/~brunomozza/iotsec/iotsec.owl#CryptographicConcept -->

    <owl:Class rdf:about="&iotsec;CryptographicConcept">
        <rdfs:subClassOf rdf:resource="&iotsec;SecurityMechanism"/>
    </owl:Class>
    


    <!-- http://www-usr.inf.ufsm.br/~brunomozza/iotsec/iotsec.owl#CryptographicIssues -->

    <owl:Class rdf:about="&iotsec;CryptographicIssues">
        <rdfs:label xml:lang="en">Cryptographic Issues</rdfs:label>
        <rdfs:subClassOf rdf:resource="&iotsec;SecurityFeatures"/>
        <rdfs:comment xml:lang="en">Weaknesses in this category are related to the use of cryptography [CWE-310].</rdfs:comment>
        <rdfs:seeAlso xml:lang="en">http://cwe.mitre.org/data/definitions/310.html</rdfs:seeAlso>
    </owl:Class>
    


    <!-- http://www-usr.inf.ufsm.br/~brunomozza/iotsec/iotsec.owl#DataHandling -->

    <owl:Class rdf:about="&iotsec;DataHandling">
        <rdfs:label xml:lang="en">Data Handling</rdfs:label>
        <rdfs:subClassOf rdf:resource="&iotsec;SourceCode"/>
        <rdfs:comment xml:lang="en">Weaknesses in this category are typically found in functionality that processes data [CWE-19].</rdfs:comment>
        <rdfs:seeAlso xml:lang="en">http://cwe.mitre.org/data/definitions/19.html</rdfs:seeAlso>
    </owl:Class>
    


    <!-- http://www-usr.inf.ufsm.br/~brunomozza/iotsec/iotsec.owl#DatabaseAttack -->

    <owl:Class rdf:about="&iotsec;DatabaseAttack">
        <rdfs:label xml:lang="en">Database Attack</rdfs:label>
        <rdfs:subClassOf rdf:resource="&iotsec;WebAttack"/>
        <rdfs:comment xml:lang="en"></rdfs:comment>
    </owl:Class>
    


    <!-- http://www-usr.inf.ufsm.br/~brunomozza/iotsec/iotsec.owl#DatabaseTechnology -->

    <owl:Class rdf:about="&iotsec;DatabaseTechnology">
        <rdfs:label xml:lang="en">Database Technology</rdfs:label>
        <rdfs:subClassOf rdf:resource="&iotsec;WebTechnology"/>
        <rdfs:comment xml:lang="en"></rdfs:comment>
    </owl:Class>
    


    <!-- http://www-usr.inf.ufsm.br/~brunomozza/iotsec/iotsec.owl#DigitalCertificate -->

    <owl:Class rdf:about="&iotsec;DigitalCertificate">
        <rdfs:label xml:lang="en">Digital Certificate</rdfs:label>
        <rdfs:subClassOf rdf:resource="&iotsec;AuthenticationMethod"/>
        <rdfs:comment xml:lang="en"></rdfs:comment>
    </owl:Class>
    


    <!-- http://www-usr.inf.ufsm.br/~brunomozza/iotsec/iotsec.owl#DigitalSignature -->

    <owl:Class rdf:about="&iotsec;DigitalSignature">
        <rdfs:label xml:lang="en">Digital Signature</rdfs:label>
        <rdfs:subClassOf rdf:resource="&iotsec;CryptographicConcept"/>
        <rdfs:comment xml:lang="en">The digital signature verifies that the contents of the electronic message have not been altered [Gyrard 2014].</rdfs:comment>
    </owl:Class>
    


    <!-- http://www-usr.inf.ufsm.br/~brunomozza/iotsec/iotsec.owl#ECommerceAttack -->

    <owl:Class rdf:about="&iotsec;ECommerceAttack">
        <rdfs:label xml:lang="en">E-Commerce Attack</rdfs:label>
        <rdfs:subClassOf rdf:resource="&iotsec;WebAttack"/>
        <rdfs:comment xml:lang="en"></rdfs:comment>
    </owl:Class>
    


    <!-- http://www-usr.inf.ufsm.br/~brunomozza/iotsec/iotsec.owl#ECommerceTechnology -->

    <owl:Class rdf:about="&iotsec;ECommerceTechnology">
        <rdfs:label xml:lang="en">E-Commerce Technology</rdfs:label>
        <rdfs:subClassOf rdf:resource="&iotsec;WebTechnology"/>
        <rdfs:comment xml:lang="en"></rdfs:comment>
    </owl:Class>
    


    <!-- http://www-usr.inf.ufsm.br/~brunomozza/iotsec/iotsec.owl#EDGEAttack -->

    <owl:Class rdf:about="&iotsec;EDGEAttack">
        <rdfs:label xml:lang="en">EDGE Attack</rdfs:label>
        <rdfs:subClassOf rdf:resource="&iotsec;Threat"/>
        <rdfs:comment xml:lang="en"></rdfs:comment>
    </owl:Class>
    


    <!-- http://www-usr.inf.ufsm.br/~brunomozza/iotsec/iotsec.owl#EDGESecurityMechanism -->

    <owl:Class rdf:about="&iotsec;EDGESecurityMechanism">
        <rdfs:label xml:lang="en">EDGE Security Mechanism</rdfs:label>
        <rdfs:subClassOf rdf:resource="&iotsec;SecurityMechanism"/>
        <rdfs:comment xml:lang="en"></rdfs:comment>
    </owl:Class>
    


    <!-- http://www-usr.inf.ufsm.br/~brunomozza/iotsec/iotsec.owl#EDGETechnology -->

    <owl:Class rdf:about="&iotsec;EDGETechnology">
        <rdfs:label xml:lang="en">EDGE Technology</rdfs:label>
        <rdfs:subClassOf rdf:resource="&iotsec;Asset"/>
        <rdfs:comment xml:lang="en">2.75G - Enhanced Data Rates for GSM Evolution (EDGE)</rdfs:comment>
        <rdfs:seeAlso rdf:resource="&ct;EDGE"/>
    </owl:Class>
    


    <!-- http://www-usr.inf.ufsm.br/~brunomozza/iotsec/iotsec.owl#EDGEVulnerability -->

    <owl:Class rdf:about="&iotsec;EDGEVulnerability">
        <rdfs:label xml:lang="en">EDGE Vulnerability</rdfs:label>
        <rdfs:subClassOf rdf:resource="&iotsec;Vulnerability"/>
        <rdfs:subClassOf>
            <owl:Restriction>
                <owl:onProperty rdf:resource="&iotsec;isMitigateBy"/>
                <owl:someValuesFrom rdf:resource="&iotsec;EDGESecurityMechanism"/>
            </owl:Restriction>
        </rdfs:subClassOf>
        <rdfs:subClassOf>
            <owl:Restriction>
                <owl:onProperty rdf:resource="&iotsec;isVulnerabilityOf"/>
                <owl:someValuesFrom rdf:resource="&iotsec;EDGETechnology"/>
            </owl:Restriction>
        </rdfs:subClassOf>
        <rdfs:comment xml:lang="en"></rdfs:comment>
    </owl:Class>
    


    <!-- http://www-usr.inf.ufsm.br/~brunomozza/iotsec/iotsec.owl#EncryptionAlgorithm -->

    <owl:Class rdf:about="&iotsec;EncryptionAlgorithm">
        <rdfs:label xml:lang="en">Encryption Algorithm</rdfs:label>
        <rdfs:subClassOf rdf:resource="&iotsec;CryptographicConcept"/>
        <rdfs:subClassOf rdf:resource="&iotsec;SecurityAlgorithm"/>
        <rdfs:comment xml:lang="en"></rdfs:comment>
        <rdfs:comment xml:lang="en">Encryption algorithm ensures the confidentiality property [Gyrard 2014].</rdfs:comment>
    </owl:Class>
    


    <!-- http://www-usr.inf.ufsm.br/~brunomozza/iotsec/iotsec.owl#Environment -->

    <owl:Class rdf:about="&iotsec;Environment">
        <rdfs:label xml:lang="en">Environment</rdfs:label>
        <rdfs:subClassOf rdf:resource="&iotsec;SoftwareVulnerability"/>
        <rdfs:seeAlso>http://cwe.mitre.org/data/definitions/2.html</rdfs:seeAlso>
        <rdfs:comment xml:lang="en"></rdfs:comment>
    </owl:Class>
    


    <!-- http://www-usr.inf.ufsm.br/~brunomozza/iotsec/iotsec.owl#EthernetAttack -->

    <owl:Class rdf:about="&iotsec;EthernetAttack">
        <rdfs:label xml:lang="en">Ethernet Attack</rdfs:label>
        <rdfs:subClassOf rdf:resource="&iotsec;Threat"/>
        <rdfs:comment xml:lang="en"></rdfs:comment>
    </owl:Class>
    


    <!-- http://www-usr.inf.ufsm.br/~brunomozza/iotsec/iotsec.owl#EthernetSecurityMechanism -->

    <owl:Class rdf:about="&iotsec;EthernetSecurityMechanism">
        <rdfs:label xml:lang="en">Ethernet Security Mechanism</rdfs:label>
        <rdfs:subClassOf rdf:resource="&iotsec;SecurityMechanism"/>
        <rdfs:comment xml:lang="en"></rdfs:comment>
    </owl:Class>
    


    <!-- http://www-usr.inf.ufsm.br/~brunomozza/iotsec/iotsec.owl#EthernetTechnology -->

    <owl:Class rdf:about="&iotsec;EthernetTechnology">
        <rdfs:label xml:lang="en">Ethernet Technology</rdfs:label>
        <rdfs:subClassOf rdf:resource="&iotsec;Asset"/>
        <rdfs:comment xml:lang="en"></rdfs:comment>
    </owl:Class>
    


    <!-- http://www-usr.inf.ufsm.br/~brunomozza/iotsec/iotsec.owl#EthernetVulnerability -->

    <owl:Class rdf:about="&iotsec;EthernetVulnerability">
        <rdfs:label xml:lang="en">Ethernet Vulnerability</rdfs:label>
        <rdfs:subClassOf rdf:resource="&iotsec;Vulnerability"/>
        <rdfs:subClassOf>
            <owl:Restriction>
                <owl:onProperty rdf:resource="&iotsec;isMitigateBy"/>
                <owl:someValuesFrom rdf:resource="&iotsec;EthernetSecurityMechanism"/>
            </owl:Restriction>
        </rdfs:subClassOf>
        <rdfs:subClassOf>
            <owl:Restriction>
                <owl:onProperty rdf:resource="&iotsec;isVulnerabilityOf"/>
                <owl:someValuesFrom rdf:resource="&iotsec;EthernetTechnology"/>
            </owl:Restriction>
        </rdfs:subClassOf>
        <rdfs:comment xml:lang="en"></rdfs:comment>
    </owl:Class>
    


    <!-- http://www-usr.inf.ufsm.br/~brunomozza/iotsec/iotsec.owl#ExternalAttack -->

    <owl:Class rdf:about="&iotsec;ExternalAttack">
        <rdfs:label xml:lang="en">External Attack</rdfs:label>
        <rdfs:subClassOf rdf:resource="&iotsec;ActiveAttack"/>
        <rdfs:comment xml:lang="en"></rdfs:comment>
        <rdfs:seeAlso xml:lang="en">See Paper: Malicious actions against the GPRS technology [Xenakis 2006]</rdfs:seeAlso>
    </owl:Class>
    


    <!-- http://www-usr.inf.ufsm.br/~brunomozza/iotsec/iotsec.owl#Feature -->

    <owl:Class rdf:about="&iotsec;Feature">
        <rdfs:label xml:lang="en">Feature</rdfs:label>
        <rdfs:comment xml:lang="en"></rdfs:comment>
    </owl:Class>
    


    <!-- http://www-usr.inf.ufsm.br/~brunomozza/iotsec/iotsec.owl#Firewall -->

    <owl:Class rdf:about="&iotsec;Firewall">
        <rdfs:label xml:lang="en">Firewall</rdfs:label>
        <rdfs:subClassOf rdf:resource="&iotsec;SecurityMechanism"/>
        <rdfs:comment xml:lang="en"></rdfs:comment>
    </owl:Class>
    


    <!-- http://www-usr.inf.ufsm.br/~brunomozza/iotsec/iotsec.owl#Flooding -->

    <owl:Class rdf:about="&iotsec;Flooding">
        <rdfs:label xml:lang="en">Flooding</rdfs:label>
        <rdfs:subClassOf rdf:resource="&iotsec;SensorAttack"/>
        <rdfs:comment xml:lang="en">Floodings attacks generally are used to drain the memry resources by sensing the control signals [Gyrard 2014].</rdfs:comment>
        <rdfs:comment xml:lang="en">See Paper: Survey of Security and Privacy Issues of Internet of Things [Borgohain et al. 2015]</rdfs:comment>
    </owl:Class>
    


    <!-- http://www-usr.inf.ufsm.br/~brunomozza/iotsec/iotsec.owl#FrameworkAttack -->

    <owl:Class rdf:about="&iotsec;FrameworkAttack">
        <rdfs:label xml:lang="en">Framework Attack</rdfs:label>
        <rdfs:subClassOf rdf:resource="&iotsec;WebAttack"/>
        <rdfs:comment xml:lang="en"></rdfs:comment>
    </owl:Class>
    


    <!-- http://www-usr.inf.ufsm.br/~brunomozza/iotsec/iotsec.owl#FrameworkSecurityMechanism -->

    <owl:Class rdf:about="&iotsec;FrameworkSecurityMechanism">
        <rdfs:label xml:lang="en">Framework Security Mechanism</rdfs:label>
        <rdfs:subClassOf rdf:resource="&iotsec;WebSecurityMechanism"/>
        <rdfs:subClassOf>
            <owl:Restriction>
                <owl:onProperty rdf:resource="&iotsec;protects"/>
                <owl:someValuesFrom rdf:resource="&iotsec;FrameworkTechnology"/>
            </owl:Restriction>
        </rdfs:subClassOf>
        <rdfs:comment xml:lang="en"></rdfs:comment>
    </owl:Class>
    


    <!-- http://www-usr.inf.ufsm.br/~brunomozza/iotsec/iotsec.owl#FrameworkTechnology -->

    <owl:Class rdf:about="&iotsec;FrameworkTechnology">
        <rdfs:label xml:lang="en">Framework Technology</rdfs:label>
        <rdfs:subClassOf rdf:resource="&iotsec;WebTechnology"/>
        <rdfs:comment xml:lang="en"></rdfs:comment>
    </owl:Class>
    


    <!-- http://www-usr.inf.ufsm.br/~brunomozza/iotsec/iotsec.owl#GPRSAttack -->

    <owl:Class rdf:about="&iotsec;GPRSAttack">
        <rdfs:label xml:lang="en">GPRS Attack</rdfs:label>
        <rdfs:subClassOf rdf:resource="&iotsec;Threat"/>
        <rdfs:comment xml:lang="en"></rdfs:comment>
    </owl:Class>
    


    <!-- http://www-usr.inf.ufsm.br/~brunomozza/iotsec/iotsec.owl#GPRSSecurityAlgorithm -->

    <owl:Class rdf:about="&iotsec;GPRSSecurityAlgorithm">
        <rdfs:label xml:lang="en">GPRS Security Algorithm</rdfs:label>
        <rdfs:subClassOf rdf:resource="&iotsec;GPRSSecurityMechanism"/>
        <rdfs:subClassOf rdf:resource="&iotsec;SecurityAlgorithm"/>
        <rdfs:comment xml:lang="en"></rdfs:comment>
    </owl:Class>
    


    <!-- http://www-usr.inf.ufsm.br/~brunomozza/iotsec/iotsec.owl#GPRSSecurityMechanism -->

    <owl:Class rdf:about="&iotsec;GPRSSecurityMechanism">
        <rdfs:label xml:lang="en">GPRS Security Mechanism</rdfs:label>
        <rdfs:subClassOf rdf:resource="&iotsec;SecurityMechanism"/>
        <rdfs:comment xml:lang="en"></rdfs:comment>
    </owl:Class>
    


    <!-- http://www-usr.inf.ufsm.br/~brunomozza/iotsec/iotsec.owl#GPRSTechnology -->

    <owl:Class rdf:about="&iotsec;GPRSTechnology">
        <rdfs:label xml:lang="en">GPRS Technology</rdfs:label>
        <rdfs:subClassOf rdf:resource="&iotsec;Asset"/>
        <rdfs:comment xml:lang="en">2.5G - General Packet Radio Service (GPRS)</rdfs:comment>
        <rdfs:seeAlso rdf:resource="&ct;GPRS"/>
    </owl:Class>
    


    <!-- http://www-usr.inf.ufsm.br/~brunomozza/iotsec/iotsec.owl#GPRSVulnerability -->

    <owl:Class rdf:about="&iotsec;GPRSVulnerability">
        <rdfs:label xml:lang="en">GPRS Vulnerability</rdfs:label>
        <rdfs:subClassOf rdf:resource="&iotsec;Vulnerability"/>
        <rdfs:subClassOf>
            <owl:Restriction>
                <owl:onProperty rdf:resource="&iotsec;isVulnerabilityOf"/>
                <owl:someValuesFrom rdf:resource="&iotsec;GPRSTechnology"/>
            </owl:Restriction>
        </rdfs:subClassOf>
        <rdfs:subClassOf>
            <owl:Restriction>
                <owl:onProperty rdf:resource="&iotsec;isMitigateBy"/>
                <owl:someValuesFrom rdf:resource="&iotsec;GPRSSecurityMechanism"/>
            </owl:Restriction>
        </rdfs:subClassOf>
        <rdfs:comment xml:lang="en"></rdfs:comment>
    </owl:Class>
    


    <!-- http://www-usr.inf.ufsm.br/~brunomozza/iotsec/iotsec.owl#GSMAttack -->

    <owl:Class rdf:about="&iotsec;GSMAttack">
        <rdfs:label xml:lang="en">GSM Attack</rdfs:label>
        <rdfs:subClassOf rdf:resource="&iotsec;Threat"/>
        <rdfs:comment xml:lang="en"></rdfs:comment>
    </owl:Class>
    


    <!-- http://www-usr.inf.ufsm.br/~brunomozza/iotsec/iotsec.owl#GSMKeyManagement -->

    <owl:Class rdf:about="&iotsec;GSMKeyManagement">
        <rdfs:label xml:lang="en">GSM Key Management</rdfs:label>
        <rdfs:subClassOf rdf:resource="&iotsec;GSMSecurityMechanism"/>
        <rdfs:subClassOf rdf:resource="&iotsec;KeyManagement"/>
        <rdfs:comment xml:lang="en"></rdfs:comment>
    </owl:Class>
    


    <!-- http://www-usr.inf.ufsm.br/~brunomozza/iotsec/iotsec.owl#GSMSecurityAlgorithm -->

    <owl:Class rdf:about="&iotsec;GSMSecurityAlgorithm">
        <rdfs:label xml:lang="en">GSM Security Algorithm</rdfs:label>
        <rdfs:subClassOf rdf:resource="&iotsec;GSMSecurityMechanism"/>
        <rdfs:comment xml:lang="en"></rdfs:comment>
    </owl:Class>
    


    <!-- http://www-usr.inf.ufsm.br/~brunomozza/iotsec/iotsec.owl#GSMSecurityMechanism -->

    <owl:Class rdf:about="&iotsec;GSMSecurityMechanism">
        <rdfs:label xml:lang="en">GSM Security Mechanism</rdfs:label>
        <rdfs:subClassOf rdf:resource="&iotsec;SecurityAlgorithm"/>
        <rdfs:subClassOf rdf:resource="&iotsec;SecurityMechanism"/>
        <rdfs:subClassOf>
            <owl:Restriction>
                <owl:onProperty rdf:resource="&iotsec;mitigates"/>
                <owl:someValuesFrom rdf:resource="&iotsec;GSMVulnerability"/>
            </owl:Restriction>
        </rdfs:subClassOf>
        <rdfs:comment xml:lang="en"></rdfs:comment>
    </owl:Class>
    


    <!-- http://www-usr.inf.ufsm.br/~brunomozza/iotsec/iotsec.owl#GSMSecurityProtocol -->

    <owl:Class rdf:about="&iotsec;GSMSecurityProtocol">
        <rdfs:label xml:lang="en">GSM Security Protocol</rdfs:label>
        <rdfs:subClassOf rdf:resource="&iotsec;GSMSecurityMechanism"/>
        <rdfs:subClassOf rdf:resource="&iotsec;Protocol"/>
        <rdfs:comment xml:lang="en"></rdfs:comment>
    </owl:Class>
    


    <!-- http://www-usr.inf.ufsm.br/~brunomozza/iotsec/iotsec.owl#GSMTechnology -->

    <owl:Class rdf:about="&iotsec;GSMTechnology">
        <rdfs:label xml:lang="en">GSM Technology</rdfs:label>
        <rdfs:subClassOf rdf:resource="&iotsec;Asset"/>
        <rdfs:comment xml:lang="en">2G technology - Global System for Mobile Communication (GSM)</rdfs:comment>
        <rdfs:seeAlso rdf:resource="&serviceContext;GSM"/>
    </owl:Class>
    


    <!-- http://www-usr.inf.ufsm.br/~brunomozza/iotsec/iotsec.owl#GSMVulnerability -->

    <owl:Class rdf:about="&iotsec;GSMVulnerability">
        <rdfs:label xml:lang="en">GSM Vulnerability</rdfs:label>
        <rdfs:subClassOf rdf:resource="&iotsec;Vulnerability"/>
        <rdfs:subClassOf>
            <owl:Restriction>
                <owl:onProperty rdf:resource="&iotsec;isVulnerabilityOf"/>
                <owl:someValuesFrom rdf:resource="&iotsec;GSMTechnology"/>
            </owl:Restriction>
        </rdfs:subClassOf>
        <rdfs:subClassOf>
            <owl:Restriction>
                <owl:onProperty rdf:resource="&iotsec;isMitigateBy"/>
                <owl:someValuesFrom rdf:resource="&iotsec;GSMSecurityMechanism"/>
            </owl:Restriction>
        </rdfs:subClassOf>
        <rdfs:comment xml:lang="en"></rdfs:comment>
    </owl:Class>
    


    <!-- http://www-usr.inf.ufsm.br/~brunomozza/iotsec/iotsec.owl#HSPDAAttack -->

    <owl:Class rdf:about="&iotsec;HSPDAAttack">
        <rdfs:label xml:lang="en">HSPDA Attack</rdfs:label>
        <rdfs:subClassOf rdf:resource="&iotsec;Threat"/>
        <rdfs:comment xml:lang="en"></rdfs:comment>
    </owl:Class>
    


    <!-- http://www-usr.inf.ufsm.br/~brunomozza/iotsec/iotsec.owl#HSPDASecurityMechanism -->

    <owl:Class rdf:about="&iotsec;HSPDASecurityMechanism">
        <rdfs:label xml:lang="en">HSPDA Security Mechanism</rdfs:label>
        <rdfs:subClassOf rdf:resource="&iotsec;SecurityMechanism"/>
        <rdfs:comment xml:lang="en"></rdfs:comment>
    </owl:Class>
    


    <!-- http://www-usr.inf.ufsm.br/~brunomozza/iotsec/iotsec.owl#HSPDATechnology -->

    <owl:Class rdf:about="&iotsec;HSPDATechnology">
        <rdfs:label xml:lang="en">HSPDA Technology</rdfs:label>
        <rdfs:subClassOf rdf:resource="&iotsec;Asset"/>
        <rdfs:comment xml:lang="en"></rdfs:comment>
    </owl:Class>
    


    <!-- http://www-usr.inf.ufsm.br/~brunomozza/iotsec/iotsec.owl#HSPDAVulnerability -->

    <owl:Class rdf:about="&iotsec;HSPDAVulnerability">
        <rdfs:label xml:lang="en">HSPDA Vulnerability</rdfs:label>
        <rdfs:subClassOf rdf:resource="&iotsec;Vulnerability"/>
        <rdfs:subClassOf>
            <owl:Restriction>
                <owl:onProperty rdf:resource="&iotsec;isVulnerabilityOf"/>
                <owl:someValuesFrom rdf:resource="&iotsec;HSPDATechnology"/>
            </owl:Restriction>
        </rdfs:subClassOf>
        <rdfs:subClassOf>
            <owl:Restriction>
                <owl:onProperty rdf:resource="&iotsec;isMitigateBy"/>
                <owl:someValuesFrom rdf:resource="&iotsec;HSPDASecurityMechanism"/>
            </owl:Restriction>
        </rdfs:subClassOf>
        <rdfs:comment xml:lang="en"></rdfs:comment>
    </owl:Class>
    


    <!-- http://www-usr.inf.ufsm.br/~brunomozza/iotsec/iotsec.owl#HashFunction -->

    <owl:Class rdf:about="&iotsec;HashFunction">
        <rdfs:label xml:lang="en">Hash Function</rdfs:label>
        <rdfs:subClassOf rdf:resource="&iotsec;CryptographicConcept"/>
        <rdfs:comment xml:lang="en"></rdfs:comment>
    </owl:Class>
    


    <!-- http://www-usr.inf.ufsm.br/~brunomozza/iotsec/iotsec.owl#Honeypot -->

    <owl:Class rdf:about="&iotsec;Honeypot">
        <rdfs:label xml:lang="en">Honeypot</rdfs:label>
        <rdfs:subClassOf rdf:resource="&iotsec;NetworkManagementSecurityMechanism"/>
        <rdfs:comment xml:lang="en">Honeypots are hosts meant to be attacked either to distract the attackers or to research their techniques [Gyrard 2014].</rdfs:comment>
    </owl:Class>
    


    <!-- http://www-usr.inf.ufsm.br/~brunomozza/iotsec/iotsec.owl#HouseholdAppliances -->

    <owl:Class rdf:about="&iotsec;HouseholdAppliances">
        <rdfs:label xml:lang="en">Household Appliances</rdfs:label>
        <rdfs:subClassOf rdf:resource="&iotsec;BluetoothDevices"/>
        <rdfs:comment xml:lang="en"></rdfs:comment>
    </owl:Class>
    


    <!-- http://www-usr.inf.ufsm.br/~brunomozza/iotsec/iotsec.owl#IDS -->

    <owl:Class rdf:about="&iotsec;IDS">
        <rdfs:label xml:lang="en">Intrusion Detection System (IDS)</rdfs:label>
        <rdfs:subClassOf rdf:resource="&iotsec;NetworkManagementSecurityMechanism"/>
        <rdfs:comment xml:lang="en"></rdfs:comment>
    </owl:Class>
    


    <!-- http://www-usr.inf.ufsm.br/~brunomozza/iotsec/iotsec.owl#IPS -->

    <owl:Class rdf:about="&iotsec;IPS">
        <rdfs:label xml:lang="en">Intrusion Prevention System (IPS)</rdfs:label>
        <rdfs:subClassOf rdf:resource="&iotsec;NetworkManagementSecurityMechanism"/>
        <rdfs:comment xml:lang="en"></rdfs:comment>
    </owl:Class>
    


    <!-- http://www-usr.inf.ufsm.br/~brunomozza/iotsec/iotsec.owl#ImproperAccessControl -->

    <owl:Class rdf:about="&iotsec;ImproperAccessControl">
        <rdfs:label xml:lang="en">Improper Access Control</rdfs:label>
        <rdfs:subClassOf rdf:resource="&iotsec;PermissionsPrivilegesAccessControl"/>
        <rdfs:comment xml:lang="en">The software does not restrict or incorrectly restricts access to a resource from an unauthorized actor [CWE-284].</rdfs:comment>
        <rdfs:seeAlso xml:lang="en">http://cwe.mitre.org/data/definitions/284.html</rdfs:seeAlso>
    </owl:Class>
    


    <!-- http://www-usr.inf.ufsm.br/~brunomozza/iotsec/iotsec.owl#ImproperAuthentication -->

    <owl:Class rdf:about="&iotsec;ImproperAuthentication">
        <rdfs:label xml:lang="en">Authentication Issues</rdfs:label>
        <rdfs:subClassOf rdf:resource="&iotsec;SecurityFeatures"/>
        <rdfs:comment xml:lang="en">When an actor claims to have a given identity, the software does not prove or insufficiently proves that the claim is correct [CWE-287].</rdfs:comment>
        <rdfs:seeAlso xml:lang="en">http://cwe.mitre.org/data/definitions/287.html</rdfs:seeAlso>
    </owl:Class>
    


    <!-- http://www-usr.inf.ufsm.br/~brunomozza/iotsec/iotsec.owl#ImproperInputValidation -->

    <owl:Class rdf:about="&iotsec;ImproperInputValidation">
        <rdfs:label xml:lang="en">Input Validation</rdfs:label>
        <rdfs:subClassOf rdf:resource="&iotsec;DataHandling"/>
        <rdfs:comment xml:lang="en">The product does not validate or incorrectly validates input that can affect the control flow or data flow of a program [CWE-20].</rdfs:comment>
        <rdfs:seeAlso xml:lang="en">http://cwe.mitre.org/data/definitions/20.html</rdfs:seeAlso>
    </owl:Class>
    


    <!-- http://www-usr.inf.ufsm.br/~brunomozza/iotsec/iotsec.owl#IndicatorPoorCodeQuality -->

    <owl:Class rdf:about="&iotsec;IndicatorPoorCodeQuality">
        <rdfs:label xml:lang="en">Indicator of Poor Code Quality</rdfs:label>
        <rdfs:subClassOf rdf:resource="&iotsec;SourceCode"/>
        <rdfs:comment xml:lang="en">The code has features that do not directly introduce a weakness or vulnerability, but indicate that the product has not been carefully developed or maintained [CWE-398].</rdfs:comment>
        <rdfs:seeAlso xml:lang="en">http://cwe.mitre.org/data/definitions/398.html</rdfs:seeAlso>
    </owl:Class>
    


    <!-- http://www-usr.inf.ufsm.br/~brunomozza/iotsec/iotsec.owl#InformationLeakDisclosure -->

    <owl:Class rdf:about="&iotsec;InformationLeakDisclosure">
        <rdfs:label xml:lang="en">Information Leak / Disclosure</rdfs:label>
        <rdfs:subClassOf rdf:resource="&iotsec;InformationManagementErrors"/>
        <rdfs:comment xml:lang="en">An information exposure is the intentional or unintentional disclosure of information to an actor that is not explicitly authorized to have access to that information [CWE-200].</rdfs:comment>
        <rdfs:seeAlso xml:lang="en">http://cwe.mitre.org/data/definitions/200.html</rdfs:seeAlso>
    </owl:Class>
    


    <!-- http://www-usr.inf.ufsm.br/~brunomozza/iotsec/iotsec.owl#InformationManagementErrors -->

    <owl:Class rdf:about="&iotsec;InformationManagementErrors">
        <rdfs:label xml:lang="en">Information Management Errors</rdfs:label>
        <rdfs:subClassOf rdf:resource="&iotsec;DataHandling"/>
        <rdfs:comment xml:lang="en">Weaknesses in this category are related to improper handling of sensitive information [CWE-199].</rdfs:comment>
        <rdfs:seeAlso xml:lang="en">http://cwe.mitre.org/data/definitions/199.html</rdfs:seeAlso>
    </owl:Class>
    


    <!-- http://www-usr.inf.ufsm.br/~brunomozza/iotsec/iotsec.owl#Injection -->

    <owl:Class rdf:about="&iotsec;Injection">
        <rdfs:label xml:lang="en">Injection</rdfs:label>
        <rdfs:subClassOf rdf:resource="&iotsec;ImproperInputValidation"/>
        <rdfs:comment xml:lang="en">Injection flaws, such as SQL, OS, and LDAP injection occur when untrusted data is sent to an interpreter as part of a command or query. The attacker’s hostile data can trick the interpreter into executing unintended commands or accessing data without proper authorization [OWASP Top Ten 2013].</rdfs:comment>
        <rdfs:comment xml:lang="en">The software constructs all or part of a command, data structure, or record using externally-influenced input from an upstream component, but it does not neutralize or incorrectly neutralizes special elements that could modify how it is parsed or interpreted when it is sent to a downstream component [CWE-74].</rdfs:comment>
        <rdfs:seeAlso xml:lang="en">http://cwe.mitre.org/data/definitions/74.html</rdfs:seeAlso>
    </owl:Class>
    


    <!-- http://www-usr.inf.ufsm.br/~brunomozza/iotsec/iotsec.owl#InsufficientVerificationDataAuthenticity -->

    <owl:Class rdf:about="&iotsec;InsufficientVerificationDataAuthenticity">
        <rdfs:label xml:lang="en">Insufficient Verification of Data Authenticity</rdfs:label>
        <rdfs:subClassOf rdf:resource="&iotsec;SecurityFeatures"/>
        <rdfs:comment xml:lang="en">The software does not sufficiently verify the origin or authenticity of data, in a way that causes it to accept invalid data [CWE-345].</rdfs:comment>
        <rdfs:seeAlso xml:lang="en">http://cwe.mitre.org/data/definitions/345.html</rdfs:seeAlso>
    </owl:Class>
    


    <!-- http://www-usr.inf.ufsm.br/~brunomozza/iotsec/iotsec.owl#IntegrityMethod -->

    <owl:Class rdf:about="&iotsec;IntegrityMethod">
        <rdfs:label xml:lang="en">Integrity Method</rdfs:label>
        <rdfs:subClassOf rdf:resource="&iotsec;SecurityPropertyMethod"/>
        <rdfs:comment xml:lang="en">Data integrity guarantees that the transmitted messages are not modified by attackers, either due to malicious intent or by accident.</rdfs:comment>
    </owl:Class>
    


    <!-- http://www-usr.inf.ufsm.br/~brunomozza/iotsec/iotsec.owl#InternalAttack -->

    <owl:Class rdf:about="&iotsec;InternalAttack">
        <rdfs:label xml:lang="en">Internal Attack</rdfs:label>
        <rdfs:subClassOf rdf:resource="&iotsec;ActiveAttack"/>
        <rdfs:comment xml:lang="en">Internal attacks are launched from compromised nodes, are much more sophisticated than external attacks [Gyrard 2014].</rdfs:comment>
        <rdfs:seeAlso xml:lang="en">See Paper: Malicious actions against the GPRS technology [Xenakis 2006]</rdfs:seeAlso>
    </owl:Class>
    


    <!-- http://www-usr.inf.ufsm.br/~brunomozza/iotsec/iotsec.owl#KeyManagement -->

    <owl:Class rdf:about="&iotsec;KeyManagement">
        <rdfs:label xml:lang="en">Key Management</rdfs:label>
        <rdfs:subClassOf rdf:resource="&iotsec;CryptographicConcept"/>
        <rdfs:comment xml:lang="en">Key management protocols are fundamental requirements to develop a secure application. These protocols are used to set up and distribute various kinds of cryptographic keys to nodes in the network [Gyrard 2014].</rdfs:comment>
    </owl:Class>
    


    <!-- http://www-usr.inf.ufsm.br/~brunomozza/iotsec/iotsec.owl#LTEArchitecture -->

    <owl:Class rdf:about="&iotsec;LTEArchitecture">
        <rdfs:label xml:lang="en">LTE Architecture</rdfs:label>
        <rdfs:subClassOf rdf:resource="&stac;Architecture"/>
        <rdfs:comment xml:lang="en"></rdfs:comment>
    </owl:Class>
    


    <!-- http://www-usr.inf.ufsm.br/~brunomozza/iotsec/iotsec.owl#LTEArchitectureComponent -->

    <owl:Class rdf:about="&iotsec;LTEArchitectureComponent">
        <rdfs:label xml:lang="en">LTE Architecture component</rdfs:label>
        <rdfs:subClassOf rdf:resource="&iotsec;LTEArchitecture"/>
        <rdfs:comment xml:lang="en"></rdfs:comment>
    </owl:Class>
    


    <!-- http://www-usr.inf.ufsm.br/~brunomozza/iotsec/iotsec.owl#LTEAttack -->

    <owl:Class rdf:about="&iotsec;LTEAttack">
        <rdfs:label xml:lang="en">LTE Attack</rdfs:label>
        <rdfs:subClassOf rdf:resource="&iotsec;Threat"/>
        <rdfs:comment xml:lang="en"></rdfs:comment>
    </owl:Class>
    


    <!-- http://www-usr.inf.ufsm.br/~brunomozza/iotsec/iotsec.owl#LTESecurityMechanism -->

    <owl:Class rdf:about="&iotsec;LTESecurityMechanism">
        <rdfs:label xml:lang="en">LTE Security Mechanism</rdfs:label>
        <rdfs:subClassOf rdf:resource="&iotsec;SecurityMechanism"/>
        <rdfs:comment xml:lang="en"></rdfs:comment>
    </owl:Class>
    


    <!-- http://www-usr.inf.ufsm.br/~brunomozza/iotsec/iotsec.owl#LTETechnology -->

    <owl:Class rdf:about="&iotsec;LTETechnology">
        <rdfs:label xml:lang="en">LTE Technology</rdfs:label>
        <rdfs:subClassOf rdf:resource="&iotsec;Asset"/>
        <rdfs:comment xml:lang="en"></rdfs:comment>
    </owl:Class>
    


    <!-- http://www-usr.inf.ufsm.br/~brunomozza/iotsec/iotsec.owl#LTEVulnerability -->

    <owl:Class rdf:about="&iotsec;LTEVulnerability">
        <rdfs:label xml:lang="en">LTE Vulnerability</rdfs:label>
        <rdfs:subClassOf rdf:resource="&iotsec;Vulnerability"/>
        <rdfs:subClassOf>
            <owl:Restriction>
                <owl:onProperty rdf:resource="&iotsec;isVulnerabilityOf"/>
                <owl:someValuesFrom rdf:resource="&iotsec;LTETechnology"/>
            </owl:Restriction>
        </rdfs:subClassOf>
        <rdfs:subClassOf>
            <owl:Restriction>
                <owl:onProperty rdf:resource="&iotsec;isMitigateBy"/>
                <owl:someValuesFrom rdf:resource="&iotsec;LTESecurityMechanism"/>
            </owl:Restriction>
        </rdfs:subClassOf>
        <rdfs:comment xml:lang="en"></rdfs:comment>
    </owl:Class>
    


    <!-- http://www-usr.inf.ufsm.br/~brunomozza/iotsec/iotsec.owl#LinkFollowing -->

    <owl:Class rdf:about="&iotsec;LinkFollowing">
        <rdfs:label xml:lang="en">Link Following</rdfs:label>
        <rdfs:subClassOf rdf:resource="&iotsec;PathEquivalence"/>
        <rdfs:comment xml:lang="en">The software attempts to access a file based on the filename, but it does not properly prevent that filename from identifying a link or shortcut that resolves to an unintended resource [CWE-59].</rdfs:comment>
        <rdfs:seeAlso xml:lang="en">http://cwe.mitre.org/data/definitions/59.html</rdfs:seeAlso>
    </owl:Class>
    


    <!-- http://www-usr.inf.ufsm.br/~brunomozza/iotsec/iotsec.owl#Location -->

    <owl:Class rdf:about="&iotsec;Location">
        <rdfs:label xml:lang="en">Location</rdfs:label>
        <rdfs:subClassOf rdf:resource="&iotsec;SoftwareVulnerability"/>
        <rdfs:comment xml:lang="en">Weaknesses in this category are organized based on which phase they are introduced during the software development and deployment process [CWE-1].</rdfs:comment>
        <rdfs:seeAlso xml:lang="en">http://cwe.mitre.org/data/definitions/1.html</rdfs:seeAlso>
    </owl:Class>
    


    <!-- http://www-usr.inf.ufsm.br/~brunomozza/iotsec/iotsec.owl#LoginPassword -->

    <owl:Class rdf:about="&iotsec;LoginPassword">
        <rdfs:label xml:lang="en">Login/Password</rdfs:label>
        <rdfs:subClassOf rdf:resource="&iotsec;AccessControlMethod"/>
        <rdfs:subClassOf rdf:resource="&iotsec;AuthenticationMethod"/>
        <rdfs:comment xml:lang="en">The simple form of authentication is providing a user name and password which is mainly the case in internet based authentication (e.g. email, online shopping, etc).</rdfs:comment>
    </owl:Class>
    


    <!-- http://www-usr.inf.ufsm.br/~brunomozza/iotsec/iotsec.owl#M2MAttack -->

    <owl:Class rdf:about="&iotsec;M2MAttack">
        <rdfs:label xml:lang="en">M2M Attack</rdfs:label>
        <rdfs:subClassOf rdf:resource="&iotsec;Threat"/>
        <rdfs:comment xml:lang="en"></rdfs:comment>
    </owl:Class>
    


    <!-- http://www-usr.inf.ufsm.br/~brunomozza/iotsec/iotsec.owl#M2MSecurityMechanism -->

    <owl:Class rdf:about="&iotsec;M2MSecurityMechanism">
        <rdfs:label xml:lang="en">M2M Security Mechanism</rdfs:label>
        <rdfs:subClassOf rdf:resource="&iotsec;SecurityMechanism"/>
        <rdfs:comment xml:lang="en"></rdfs:comment>
    </owl:Class>
    


    <!-- http://www-usr.inf.ufsm.br/~brunomozza/iotsec/iotsec.owl#M2MTechnology -->

    <owl:Class rdf:about="&iotsec;M2MTechnology">
        <rdfs:label xml:lang="en">M2M Technology</rdfs:label>
        <rdfs:subClassOf rdf:resource="&iotsec;Asset"/>
        <rdfs:comment xml:lang="en"></rdfs:comment>
    </owl:Class>
    


    <!-- http://www-usr.inf.ufsm.br/~brunomozza/iotsec/iotsec.owl#M2MVulnerability -->

    <owl:Class rdf:about="&iotsec;M2MVulnerability">
        <rdfs:label xml:lang="en">M2M Vulnerability</rdfs:label>
        <rdfs:subClassOf rdf:resource="&iotsec;Vulnerability"/>
        <rdfs:subClassOf>
            <owl:Restriction>
                <owl:onProperty rdf:resource="&iotsec;isVulnerabilityOf"/>
                <owl:someValuesFrom rdf:resource="&iotsec;M2MTechnology"/>
            </owl:Restriction>
        </rdfs:subClassOf>
        <rdfs:subClassOf>
            <owl:Restriction>
                <owl:onProperty rdf:resource="&iotsec;isMitigateBy"/>
                <owl:someValuesFrom rdf:resource="&iotsec;M2MSecurityMechanism"/>
            </owl:Restriction>
        </rdfs:subClassOf>
        <rdfs:comment xml:lang="en"></rdfs:comment>
    </owl:Class>
    


    <!-- http://www-usr.inf.ufsm.br/~brunomozza/iotsec/iotsec.owl#MAC -->

    <owl:Class rdf:about="&iotsec;MAC">
        <rdfs:label xml:lang="en">Message Authentication Code (MAC)</rdfs:label>
        <rdfs:subClassOf rdf:resource="&iotsec;AuthenticationMethod"/>
        <rdfs:subClassOf rdf:resource="&iotsec;IntegrityMethod"/>
        <rdfs:comment xml:lang="en">MAC is a short piece of information used to authenticate a message and check the integrity.</rdfs:comment>
    </owl:Class>
    


    <!-- http://www-usr.inf.ufsm.br/~brunomozza/iotsec/iotsec.owl#MITMAttack -->

    <owl:Class rdf:about="&iotsec;MITMAttack">
        <rdfs:label xml:lang="en">Man-in-the-Middle Attack</rdfs:label>
        <rdfs:subClassOf rdf:resource="&iotsec;BluetoothAttack"/>
        <rdfs:comment xml:lang="en"></rdfs:comment>
    </owl:Class>
    


    <!-- http://www-usr.inf.ufsm.br/~brunomozza/iotsec/iotsec.owl#ManetAttack -->

    <owl:Class rdf:about="&iotsec;ManetAttack">
        <rdfs:label xml:lang="en">Manet Attack</rdfs:label>
        <rdfs:subClassOf rdf:resource="&iotsec;Threat"/>
        <rdfs:comment xml:lang="en">Manet (Mobile ad hoc network) is a self-configuring network of mobile devices connected [Gyrard 2014].</rdfs:comment>
    </owl:Class>
    


    <!-- http://www-usr.inf.ufsm.br/~brunomozza/iotsec/iotsec.owl#ManetSecurityMechanism -->

    <owl:Class rdf:about="&iotsec;ManetSecurityMechanism">
        <rdfs:label xml:lang="en">Manet Security Mechanism</rdfs:label>
        <rdfs:subClassOf rdf:resource="&iotsec;SecurityMechanism"/>
        <rdfs:subClassOf>
            <owl:Restriction>
                <owl:onProperty rdf:resource="&iotsec;mitigates"/>
                <owl:someValuesFrom rdf:resource="&iotsec;ManetVulnerability"/>
            </owl:Restriction>
        </rdfs:subClassOf>
        <rdfs:comment xml:lang="en"></rdfs:comment>
    </owl:Class>
    


    <!-- http://www-usr.inf.ufsm.br/~brunomozza/iotsec/iotsec.owl#ManetTechnology -->

    <owl:Class rdf:about="&iotsec;ManetTechnology">
        <rdfs:label xml:lang="en">Manet Technology</rdfs:label>
        <rdfs:subClassOf rdf:resource="&iotsec;Asset"/>
        <rdfs:comment xml:lang="en"></rdfs:comment>
    </owl:Class>
    


    <!-- http://www-usr.inf.ufsm.br/~brunomozza/iotsec/iotsec.owl#ManetVulnerability -->

    <owl:Class rdf:about="&iotsec;ManetVulnerability">
        <rdfs:label xml:lang="en">Manet Vulnerability</rdfs:label>
        <rdfs:subClassOf rdf:resource="&iotsec;Vulnerability"/>
        <rdfs:subClassOf>
            <owl:Restriction>
                <owl:onProperty rdf:resource="&iotsec;isVulnerabilityOf"/>
                <owl:someValuesFrom rdf:resource="&iotsec;ManetTechnology"/>
            </owl:Restriction>
        </rdfs:subClassOf>
        <rdfs:subClassOf>
            <owl:Restriction>
                <owl:onProperty rdf:resource="&iotsec;isMitigateBy"/>
                <owl:someValuesFrom rdf:resource="&iotsec;ManetSecurityMechanism"/>
            </owl:Restriction>
        </rdfs:subClassOf>
        <rdfs:comment xml:lang="en"></rdfs:comment>
    </owl:Class>
    


    <!-- http://www-usr.inf.ufsm.br/~brunomozza/iotsec/iotsec.owl#MeshArchitecture -->

    <owl:Class rdf:about="&iotsec;MeshArchitecture">
        <rdfs:label xml:lang="en">Mesh Architecture</rdfs:label>
        <rdfs:subClassOf rdf:resource="&stac;Architecture"/>
        <rdfs:subClassOf>
            <owl:Restriction>
                <owl:onProperty rdf:resource="&iotsec;hasFeature"/>
                <owl:someValuesFrom rdf:resource="&stac;LowCostDeployment"/>
            </owl:Restriction>
        </rdfs:subClassOf>
        <rdfs:subClassOf>
            <owl:Restriction>
                <owl:onProperty rdf:resource="&iotsec;hasFeature"/>
                <owl:someValuesFrom rdf:resource="&stac;Flexible"/>
            </owl:Restriction>
        </rdfs:subClassOf>
        <rdfs:subClassOf>
            <owl:Restriction>
                <owl:onProperty rdf:resource="&iotsec;hasFeature"/>
                <owl:someValuesFrom rdf:resource="&stac;Scalable"/>
            </owl:Restriction>
        </rdfs:subClassOf>
        <rdfs:comment xml:lang="en"></rdfs:comment>
    </owl:Class>
    


    <!-- http://www-usr.inf.ufsm.br/~brunomozza/iotsec/iotsec.owl#MeshArchitectureComponent -->

    <owl:Class rdf:about="&iotsec;MeshArchitectureComponent">
        <rdfs:label xml:lang="en">Mesh Architecture component</rdfs:label>
        <rdfs:subClassOf rdf:resource="&iotsec;MeshArchitecture"/>
        <rdfs:comment xml:lang="en"></rdfs:comment>
    </owl:Class>
    


    <!-- http://www-usr.inf.ufsm.br/~brunomozza/iotsec/iotsec.owl#MeshAttack -->

    <owl:Class rdf:about="&iotsec;MeshAttack">
        <rdfs:label xml:lang="en">Mesh Attack</rdfs:label>
        <rdfs:subClassOf rdf:resource="&iotsec;Threat"/>
        <rdfs:comment xml:lang="en"></rdfs:comment>
    </owl:Class>
    


    <!-- http://www-usr.inf.ufsm.br/~brunomozza/iotsec/iotsec.owl#MeshKeyManagement -->

    <owl:Class rdf:about="&iotsec;MeshKeyManagement">
        <rdfs:label xml:lang="en">Mesh Key Management</rdfs:label>
        <rdfs:subClassOf rdf:resource="&iotsec;KeyManagement"/>
        <rdfs:subClassOf rdf:resource="&iotsec;MeshSecurityMechanism"/>
        <rdfs:comment xml:lang="en"></rdfs:comment>
    </owl:Class>
    


    <!-- http://www-usr.inf.ufsm.br/~brunomozza/iotsec/iotsec.owl#MeshSecurityMechanism -->

    <owl:Class rdf:about="&iotsec;MeshSecurityMechanism">
        <rdfs:label xml:lang="en">Mesh Security Mechanism</rdfs:label>
        <rdfs:subClassOf rdf:resource="&iotsec;SecurityMechanism"/>
        <rdfs:comment xml:lang="en"></rdfs:comment>
    </owl:Class>
    


    <!-- http://www-usr.inf.ufsm.br/~brunomozza/iotsec/iotsec.owl#MeshSecurityProtocol -->

    <owl:Class rdf:about="&iotsec;MeshSecurityProtocol">
        <rdfs:subClassOf rdf:resource="&iotsec;MeshSecurityMechanism"/>
        <rdfs:subClassOf rdf:resource="&iotsec;Protocol"/>
    </owl:Class>
    


    <!-- http://www-usr.inf.ufsm.br/~brunomozza/iotsec/iotsec.owl#MeshTechnology -->

    <owl:Class rdf:about="&iotsec;MeshTechnology">
        <rdfs:subClassOf rdf:resource="&iotsec;Asset"/>
    </owl:Class>
    


    <!-- http://www-usr.inf.ufsm.br/~brunomozza/iotsec/iotsec.owl#MeshVulnerability -->

    <owl:Class rdf:about="&iotsec;MeshVulnerability">
        <rdfs:label xml:lang="en">Mesh Vulnerability</rdfs:label>
        <rdfs:subClassOf rdf:resource="&iotsec;Vulnerability"/>
        <rdfs:subClassOf>
            <owl:Restriction>
                <owl:onProperty rdf:resource="&iotsec;isMitigateBy"/>
                <owl:someValuesFrom rdf:resource="&iotsec;MeshSecurityMechanism"/>
            </owl:Restriction>
        </rdfs:subClassOf>
        <rdfs:subClassOf>
            <owl:Restriction>
                <owl:onProperty rdf:resource="&iotsec;isVulnerabilityOf"/>
                <owl:someValuesFrom rdf:resource="&iotsec;MeshTechnology"/>
            </owl:Restriction>
        </rdfs:subClassOf>
        <rdfs:comment xml:lang="en"></rdfs:comment>
    </owl:Class>
    


    <!-- http://www-usr.inf.ufsm.br/~brunomozza/iotsec/iotsec.owl#MessageEncryptionTool -->

    <owl:Class rdf:about="&iotsec;MessageEncryptionTool">
        <rdfs:label xml:lang="en">Message Encryption Tool</rdfs:label>
        <rdfs:subClassOf rdf:resource="&iotsec;SecurityTool"/>
        <rdfs:comment xml:lang="en"></rdfs:comment>
    </owl:Class>
    


    <!-- http://www-usr.inf.ufsm.br/~brunomozza/iotsec/iotsec.owl#ModeOperation -->

    <owl:Class rdf:about="&iotsec;ModeOperation">
        <rdfs:label xml:lang="en">Mode Operation</rdfs:label>
        <rdfs:subClassOf rdf:resource="&iotsec;BlockCipher"/>
        <rdfs:comment xml:lang="en"></rdfs:comment>
    </owl:Class>
    


    <!-- http://www-usr.inf.ufsm.br/~brunomozza/iotsec/iotsec.owl#NegativeFeature -->

    <owl:Class rdf:about="&iotsec;NegativeFeature">
        <rdfs:label xml:lang="en">Negative Feature</rdfs:label>
        <rdfs:subClassOf rdf:resource="&iotsec;Feature"/>
        <rdfs:comment xml:lang="en">Negative Feature of security mechanisms</rdfs:comment>
    </owl:Class>
    


    <!-- http://www-usr.inf.ufsm.br/~brunomozza/iotsec/iotsec.owl#NetworkManagementAttack -->

    <owl:Class rdf:about="&iotsec;NetworkManagementAttack">
        <rdfs:label xml:lang="en">Network Management Attack</rdfs:label>
        <rdfs:subClassOf rdf:resource="&iotsec;Threat"/>
        <rdfs:comment xml:lang="en"></rdfs:comment>
    </owl:Class>
    


    <!-- http://www-usr.inf.ufsm.br/~brunomozza/iotsec/iotsec.owl#NetworkManagementSecurityMechanism -->

    <owl:Class rdf:about="&iotsec;NetworkManagementSecurityMechanism">
        <rdfs:label xml:lang="en">Network Management Security Mechanism</rdfs:label>
        <rdfs:subClassOf rdf:resource="&iotsec;SecurityMechanism"/>
        <rdfs:comment xml:lang="en"></rdfs:comment>
    </owl:Class>
    


    <!-- http://www-usr.inf.ufsm.br/~brunomozza/iotsec/iotsec.owl#NetworkManagementSecurityTool -->

    <owl:Class rdf:about="&iotsec;NetworkManagementSecurityTool">
        <rdfs:label xml:lang="en">Network Management Security Tool</rdfs:label>
        <rdfs:subClassOf rdf:resource="&iotsec;NetworkManagementSecurityMechanism"/>
        <rdfs:comment xml:lang="en"></rdfs:comment>
    </owl:Class>
    


    <!-- http://www-usr.inf.ufsm.br/~brunomozza/iotsec/iotsec.owl#NetworkManagementTechnology -->

    <owl:Class rdf:about="&iotsec;NetworkManagementTechnology">
        <rdfs:label xml:lang="en">Network Management Technology</rdfs:label>
        <rdfs:subClassOf rdf:resource="&iotsec;Asset"/>
        <rdfs:comment xml:lang="en"></rdfs:comment>
    </owl:Class>
    


    <!-- http://www-usr.inf.ufsm.br/~brunomozza/iotsec/iotsec.owl#NumberErrors -->

    <owl:Class rdf:about="&iotsec;NumberErrors">
        <rdfs:label xml:lang="en">Number Errors</rdfs:label>
        <rdfs:subClassOf rdf:resource="&iotsec;DataHandling"/>
        <rdfs:comment xml:lang="en">Weaknesses in this category are related to improper calculation or conversion of numbers [CWE-189].</rdfs:comment>
        <rdfs:seeAlso xml:lang="en">http://cwe.mitre.org/data/definitions/189.html</rdfs:seeAlso>
    </owl:Class>
    


    <!-- http://www-usr.inf.ufsm.br/~brunomozza/iotsec/iotsec.owl#OSCommandInjection -->

    <owl:Class rdf:about="&iotsec;OSCommandInjection">
        <rdfs:label xml:lang="en">OS Command Injection</rdfs:label>
        <rdfs:subClassOf rdf:resource="&iotsec;CommandInjection"/>
        <rdfs:comment xml:lang="en">The software constructs all or part of an OS command using externally-influenced input from an upstream component, but it does not neutralize or incorrectly neutralizes special elements that could modify the intended OS command when it is sent to a downstream component [CWE-78].</rdfs:comment>
        <rdfs:seeAlso xml:lang="en">http://cwe.mitre.org/data/definitions/78.html</rdfs:seeAlso>
    </owl:Class>
    


    <!-- http://www-usr.inf.ufsm.br/~brunomozza/iotsec/iotsec.owl#OSIModel -->

    <owl:Class rdf:about="&iotsec;OSIModel">
        <rdfs:label xml:lang="en"></rdfs:label>
        <owl:equivalentClass>
            <owl:Class>
                <owl:oneOf rdf:parseType="Collection">
                    <rdf:Description rdf:about="&iotsec;LinkLayer"/>
                    <rdf:Description rdf:about="&iotsec;ApplicationLayer"/>
                    <rdf:Description rdf:about="&iotsec;PhysicalLayer"/>
                    <rdf:Description rdf:about="&iotsec;SessionLayer"/>
                    <rdf:Description rdf:about="&iotsec;NetworkLayer"/>
                    <rdf:Description rdf:about="&iotsec;PresentationLayer"/>
                    <rdf:Description rdf:about="&iotsec;TransportLayer"/>
                </owl:oneOf>
            </owl:Class>
        </owl:equivalentClass>
        <rdfs:comment xml:lang="en"></rdfs:comment>
    </owl:Class>
    


    <!-- http://www-usr.inf.ufsm.br/~brunomozza/iotsec/iotsec.owl#OSIModelLayer -->

    <owl:Class rdf:about="&iotsec;OSIModelLayer">
        <rdfs:label xml:lang="en">OSI Model Layer</rdfs:label>
        <rdfs:comment xml:lang="en"></rdfs:comment>
    </owl:Class>
    


    <!-- http://www-usr.inf.ufsm.br/~brunomozza/iotsec/iotsec.owl#Obfuscation -->

    <owl:Class rdf:about="&iotsec;Obfuscation">
        <rdfs:label xml:lang="en">Obfuscation</rdfs:label>
        <rdfs:subClassOf rdf:resource="&iotsec;SecurityTool"/>
        <rdfs:subClassOf>
            <owl:Restriction>
                <owl:onProperty rdf:resource="&iotsec;occursInLayer"/>
                <owl:someValuesFrom rdf:resource="&iotsec;ApplicationLayer"/>
            </owl:Restriction>
        </rdfs:subClassOf>
        <rdfs:comment xml:lang="en"></rdfs:comment>
    </owl:Class>
    


    <!-- http://www-usr.inf.ufsm.br/~brunomozza/iotsec/iotsec.owl#OperatingSystemAttack -->

    <owl:Class rdf:about="&iotsec;OperatingSystemAttack">
        <rdfs:label xml:lang="en">Operating System Attack</rdfs:label>
        <rdfs:subClassOf rdf:resource="&iotsec;NetworkManagementAttack"/>
        <rdfs:comment xml:lang="en"></rdfs:comment>
    </owl:Class>
    


    <!-- http://www-usr.inf.ufsm.br/~brunomozza/iotsec/iotsec.owl#OperatingSystemSecurityMechanism -->

    <owl:Class rdf:about="&iotsec;OperatingSystemSecurityMechanism">
        <rdfs:label xml:lang="en">Operating System Security Mechanism</rdfs:label>
        <rdfs:subClassOf rdf:resource="&iotsec;NetworkManagementSecurityMechanism"/>
        <rdfs:comment xml:lang="en"></rdfs:comment>
    </owl:Class>
    


    <!-- http://www-usr.inf.ufsm.br/~brunomozza/iotsec/iotsec.owl#OperatingSystemTechnology -->

    <owl:Class rdf:about="&iotsec;OperatingSystemTechnology">
        <rdfs:label xml:lang="en">Operating System Technology</rdfs:label>
        <rdfs:subClassOf rdf:resource="&iotsec;Asset"/>
        <rdfs:comment xml:lang="en"></rdfs:comment>
    </owl:Class>
    


    <!-- http://www-usr.inf.ufsm.br/~brunomozza/iotsec/iotsec.owl#PassiveAttack -->

    <owl:Class rdf:about="&iotsec;PassiveAttack">
        <rdfs:label xml:lang="en">Passive Attack</rdfs:label>
        <rdfs:subClassOf rdf:resource="&iotsec;Threat"/>
        <rdfs:comment xml:lang="en">Malicious users violate the confidentiality  of the information exchanged over the network [Gyrard 2014].</rdfs:comment>
        <rdfs:seeAlso xml:lang="en">See Paper: Malicious actions against the GPRS technology [Xenakis 2006]</rdfs:seeAlso>
    </owl:Class>
    


    <!-- http://www-usr.inf.ufsm.br/~brunomozza/iotsec/iotsec.owl#PathEquivalence -->

    <owl:Class rdf:about="&iotsec;PathEquivalence">
        <rdfs:label xml:lang="en">Path Equivalence</rdfs:label>
        <rdfs:subClassOf rdf:resource="&iotsec;ImproperInputValidation"/>
        <rdfs:comment xml:lang="en">Weaknesses in this category can be used to access files outside of a restricted directory (path traversal) or to perform operations on files that would otherwise be restricted (path equivalence) [CWE-21].</rdfs:comment>
        <rdfs:seeAlso xml:lang="en">http://cwe.mitre.org/data/definitions/21.html</rdfs:seeAlso>
    </owl:Class>
    


    <!-- http://www-usr.inf.ufsm.br/~brunomozza/iotsec/iotsec.owl#PathTraversal -->

    <owl:Class rdf:about="&iotsec;PathTraversal">
        <rdfs:label xml:lang="en">Path Traversal</rdfs:label>
        <rdfs:subClassOf rdf:resource="&iotsec;PathEquivalence"/>
        <rdfs:comment xml:lang="en">The software uses external input to construct a pathname that is intended to identify a file or directory that is located underneath a restricted parent directory, but the software does not properly neutralize special elements within the pathname that can cause the pathname to resolve to a location that is outside of the restricted directory [CWE-22].</rdfs:comment>
        <rdfs:seeAlso xml:lang="en">http://cwe.mitre.org/data/definitions/22.html</rdfs:seeAlso>
    </owl:Class>
    


    <!-- http://www-usr.inf.ufsm.br/~brunomozza/iotsec/iotsec.owl#PermissionsPrivilegesAccessControl -->

    <owl:Class rdf:about="&iotsec;PermissionsPrivilegesAccessControl">
        <rdfs:label xml:lang="en">Permissions, Privileges, and Access Control</rdfs:label>
        <rdfs:subClassOf rdf:resource="&iotsec;SecurityFeatures"/>
        <rdfs:comment xml:lang="en">Weaknesses in this category are related to the management of permissions, privileges, and other security features that are used to perform access control [CWE-264].</rdfs:comment>
        <rdfs:seeAlso xml:lang="en">http://cwe.mitre.org/data/definitions/264.html</rdfs:seeAlso>
    </owl:Class>
    


    <!-- http://www-usr.inf.ufsm.br/~brunomozza/iotsec/iotsec.owl#PolymorphicVirus -->

    <owl:Class rdf:about="&iotsec;PolymorphicVirus">
        <rdfs:label xml:lang="en">Polymorphic Virus</rdfs:label>
        <rdfs:subClassOf rdf:resource="&iotsec;Virus"/>
        <rdfs:comment xml:lang="en"></rdfs:comment>
    </owl:Class>
    


    <!-- http://www-usr.inf.ufsm.br/~brunomozza/iotsec/iotsec.owl#PositiveFeature -->

    <owl:Class rdf:about="&iotsec;PositiveFeature">
        <rdfs:label xml:lang="en">Positive Feature</rdfs:label>
        <rdfs:subClassOf rdf:resource="&iotsec;Feature"/>
        <rdfs:comment xml:lang="en">Positive Feature of security mechanisms</rdfs:comment>
    </owl:Class>
    


    <!-- http://www-usr.inf.ufsm.br/~brunomozza/iotsec/iotsec.owl#ProgrammingLanguageAttack -->

    <owl:Class rdf:about="&iotsec;ProgrammingLanguageAttack">
        <rdfs:label xml:lang="en">Programming Language Attack</rdfs:label>
        <rdfs:subClassOf rdf:resource="&iotsec;WebAttack"/>
        <rdfs:comment xml:lang="en"></rdfs:comment>
    </owl:Class>
    


    <!-- http://www-usr.inf.ufsm.br/~brunomozza/iotsec/iotsec.owl#ProgrammingLanguageSecurityMechanism -->

    <owl:Class rdf:about="&iotsec;ProgrammingLanguageSecurityMechanism">
        <rdfs:label xml:lang="en">Programming Language Security Mechanism</rdfs:label>
        <rdfs:subClassOf rdf:resource="&iotsec;WebSecurityMechanism"/>
        <rdfs:subClassOf>
            <owl:Restriction>
                <owl:onProperty rdf:resource="&iotsec;protects"/>
                <owl:someValuesFrom rdf:resource="&iotsec;ProgrammingLanguageTechnology"/>
            </owl:Restriction>
        </rdfs:subClassOf>
        <rdfs:comment xml:lang="en"></rdfs:comment>
    </owl:Class>
    


    <!-- http://www-usr.inf.ufsm.br/~brunomozza/iotsec/iotsec.owl#ProgrammingLanguageTechnology -->

    <owl:Class rdf:about="&iotsec;ProgrammingLanguageTechnology">
        <rdfs:label xml:lang="en">Programming Language Technology</rdfs:label>
        <rdfs:subClassOf rdf:resource="&iotsec;WebTechnology"/>
        <rdfs:comment xml:lang="en"></rdfs:comment>
    </owl:Class>
    


    <!-- http://www-usr.inf.ufsm.br/~brunomozza/iotsec/iotsec.owl#Protocol -->

    <owl:Class rdf:about="&iotsec;Protocol">
        <rdfs:label xml:lang="en">Protocol</rdfs:label>
        <rdfs:subClassOf rdf:resource="&iotsec;SecurityMechanism"/>
        <rdfs:comment xml:lang="en"></rdfs:comment>
    </owl:Class>
    


    <!-- http://www-usr.inf.ufsm.br/~brunomozza/iotsec/iotsec.owl#Proxy -->

    <owl:Class rdf:about="&iotsec;Proxy">
        <rdfs:label xml:lang="en">Proxy</rdfs:label>
        <rdfs:subClassOf rdf:resource="&iotsec;NetworkManagementSecurityMechanism"/>
        <rdfs:comment xml:lang="en">A proxy analyzes application commands, performs authentication and keeps logs [Gyrard 2014].</rdfs:comment>
    </owl:Class>
    


    <!-- http://www-usr.inf.ufsm.br/~brunomozza/iotsec/iotsec.owl#RaceConditions -->

    <owl:Class rdf:about="&iotsec;RaceConditions">
        <rdfs:label xml:lang="en">Race Conditions</rdfs:label>
        <rdfs:subClassOf rdf:resource="&iotsec;TimeState"/>
        <rdfs:comment xml:lang="en">The program contains a code sequence that can run concurrently with other code, and the code sequence requires temporary, exclusive access to a shared resource, but a timing window exists in which the shared resource can be modified by another code sequence that is operating concurrently [CWE-362].</rdfs:comment>
        <rdfs:seeAlso xml:lang="en">http://cwe.mitre.org/data/definitions/362.html</rdfs:seeAlso>
    </owl:Class>
    


    <!-- http://www-usr.inf.ufsm.br/~brunomozza/iotsec/iotsec.owl#ResourceManagementErros -->

    <owl:Class rdf:about="&iotsec;ResourceManagementErros">
        <rdfs:label xml:lang="en">Resource Management Errors</rdfs:label>
        <rdfs:subClassOf rdf:resource="&iotsec;IndicatorPoorCodeQuality"/>
        <rdfs:comment xml:lang="en">Weaknesses in this category are related to improper management of system resources [CWE-399].</rdfs:comment>
        <rdfs:seeAlso xml:lang="en">http://cwe.mitre.org/data/definitions/399.html</rdfs:seeAlso>
    </owl:Class>
    


    <!-- http://www-usr.inf.ufsm.br/~brunomozza/iotsec/iotsec.owl#ReverseProxy -->

    <owl:Class rdf:about="&iotsec;ReverseProxy">
        <rdfs:label xml:lang="en">Reverse Proxy</rdfs:label>
        <rdfs:subClassOf rdf:resource="&iotsec;NetworkManagementSecurityMechanism"/>
        <rdfs:comment xml:lang="en"></rdfs:comment>
    </owl:Class>
    


    <!-- http://www-usr.inf.ufsm.br/~brunomozza/iotsec/iotsec.owl#RfidAttack -->

    <owl:Class rdf:about="&iotsec;RfidAttack">
        <rdfs:label xml:lang="en">RFID Attack</rdfs:label>
        <rdfs:subClassOf rdf:resource="&iotsec;Threat"/>
        <rdfs:comment xml:lang="en"></rdfs:comment>
    </owl:Class>
    


    <!-- http://www-usr.inf.ufsm.br/~brunomozza/iotsec/iotsec.owl#RfidSecurityMechanism -->

    <owl:Class rdf:about="&iotsec;RfidSecurityMechanism">
        <rdfs:label xml:lang="en">RFID Security Mechanism</rdfs:label>
        <rdfs:subClassOf rdf:resource="&iotsec;SecurityMechanism"/>
        <rdfs:comment xml:lang="en"></rdfs:comment>
    </owl:Class>
    


    <!-- http://www-usr.inf.ufsm.br/~brunomozza/iotsec/iotsec.owl#RfidTechnology -->

    <owl:Class rdf:about="&iotsec;RfidTechnology">
        <rdfs:label xml:lang="en">RFID Technology</rdfs:label>
        <rdfs:subClassOf rdf:resource="&iotsec;Asset"/>
        <rdfs:comment xml:lang="en"></rdfs:comment>
    </owl:Class>
    


    <!-- http://www-usr.inf.ufsm.br/~brunomozza/iotsec/iotsec.owl#RfidVulnerability -->

    <owl:Class rdf:about="&iotsec;RfidVulnerability">
        <rdfs:label xml:lang="en">RFID Vulnerability</rdfs:label>
        <rdfs:subClassOf rdf:resource="&iotsec;Vulnerability"/>
        <rdfs:subClassOf>
            <owl:Restriction>
                <owl:onProperty rdf:resource="&iotsec;isMitigateBy"/>
                <owl:someValuesFrom rdf:resource="&iotsec;RfidSecurityMechanism"/>
            </owl:Restriction>
        </rdfs:subClassOf>
        <rdfs:subClassOf>
            <owl:Restriction>
                <owl:onProperty rdf:resource="&iotsec;isVulnerabilityOf"/>
                <owl:someValuesFrom rdf:resource="&iotsec;RfidTechnology"/>
            </owl:Restriction>
        </rdfs:subClassOf>
        <rdfs:comment xml:lang="en"></rdfs:comment>
    </owl:Class>
    


    <!-- http://www-usr.inf.ufsm.br/~brunomozza/iotsec/iotsec.owl#Risk -->

    <owl:Class rdf:about="&iotsec;Risk">
        <rdfs:label xml:lang="en">Risk</rdfs:label>
        <rdfs:comment xml:lang="en"></rdfs:comment>
    </owl:Class>
    


    <!-- http://www-usr.inf.ufsm.br/~brunomozza/iotsec/iotsec.owl#SQLInjection -->

    <owl:Class rdf:about="&iotsec;SQLInjection">
        <rdfs:label xml:lang="en">SQL Injection</rdfs:label>
        <rdfs:subClassOf rdf:resource="&iotsec;Injection"/>
        <rdfs:comment xml:lang="en">The software constructs all or part of an SQL command using externally-influenced input from an upstream component, but it does not neutralize or incorrectly neutralizes special elements that could modify the intended SQL command when it is sent to a downstream component [CWE-89].</rdfs:comment>
        <rdfs:seeAlso xml:lang="en">http://cwe.mitre.org/data/definitions/89.html</rdfs:seeAlso>
    </owl:Class>
    


    <!-- http://www-usr.inf.ufsm.br/~brunomozza/iotsec/iotsec.owl#SecurityAlgorithm -->

    <owl:Class rdf:about="&iotsec;SecurityAlgorithm">
        <rdfs:label xml:lang="en">Security Algorithm</rdfs:label>
        <rdfs:subClassOf rdf:resource="&iotsec;SecurityMechanism"/>
        <rdfs:comment xml:lang="en"></rdfs:comment>
    </owl:Class>
    


    <!-- http://www-usr.inf.ufsm.br/~brunomozza/iotsec/iotsec.owl#SecurityFeatures -->

    <owl:Class rdf:about="&iotsec;SecurityFeatures">
        <rdfs:label xml:lang="en">Security Features</rdfs:label>
        <rdfs:subClassOf rdf:resource="&iotsec;SourceCode"/>
        <rdfs:comment xml:lang="en">Software security is not security software. Here we&apos;re concerned with topics like authentication, access control, confidentiality, cryptography, and privilege management [CWE-254].</rdfs:comment>
        <rdfs:seeAlso xml:lang="en">http://cwe.mitre.org/data/definitions/254.html</rdfs:seeAlso>
    </owl:Class>
    


    <!-- http://www-usr.inf.ufsm.br/~brunomozza/iotsec/iotsec.owl#SecurityMagazine -->

    <owl:Class rdf:about="&iotsec;SecurityMagazine">
        <rdfs:label xml:lang="en">Security Magazine</rdfs:label>
        <rdfs:subClassOf rdf:resource="&iotsec;SecurityMechanism"/>
        <rdfs:comment xml:lang="en"></rdfs:comment>
    </owl:Class>
    


    <!-- http://www-usr.inf.ufsm.br/~brunomozza/iotsec/iotsec.owl#SecurityMechanism -->

    <owl:Class rdf:about="&iotsec;SecurityMechanism">
        <rdfs:label xml:lang="en">Security Mechanism</rdfs:label>
        <rdfs:subClassOf>
            <owl:Restriction>
                <owl:onProperty rdf:resource="&iotsec;hasType"/>
                <owl:someValuesFrom rdf:resource="&iotsec;TypeofDefense"/>
            </owl:Restriction>
        </rdfs:subClassOf>
        <rdfs:subClassOf>
            <owl:Restriction>
                <owl:onProperty rdf:resource="&iotsec;mitigates"/>
                <owl:someValuesFrom rdf:resource="&iotsec;Vulnerability"/>
            </owl:Restriction>
        </rdfs:subClassOf>
        <rdfs:subClassOf>
            <owl:Restriction>
                <owl:onProperty rdf:resource="&iotsec;protects"/>
                <owl:someValuesFrom rdf:resource="&iotsec;Asset"/>
            </owl:Restriction>
        </rdfs:subClassOf>
        <rdfs:subClassOf>
            <owl:Restriction>
                <owl:onProperty rdf:resource="&iotsec;hasPart"/>
                <owl:someValuesFrom rdf:resource="&iotsec;SecurityMechanism"/>
            </owl:Restriction>
        </rdfs:subClassOf>
        <rdfs:subClassOf>
            <owl:Restriction>
                <owl:onProperty rdf:resource="&iotsec;isSecurityMechanismOf"/>
                <owl:someValuesFrom rdf:resource="&iotsec;Threat"/>
            </owl:Restriction>
        </rdfs:subClassOf>
        <rdfs:subClassOf>
            <owl:Restriction>
                <owl:onProperty rdf:resource="&iotsec;satisfies"/>
                <owl:someValuesFrom rdf:resource="&iotsec;SecurityProperty"/>
            </owl:Restriction>
        </rdfs:subClassOf>
        <rdfs:subClassOf>
            <owl:Restriction>
                <owl:onProperty rdf:resource="&iotsec;hasFeature"/>
                <owl:someValuesFrom rdf:resource="&iotsec;Feature"/>
            </owl:Restriction>
        </rdfs:subClassOf>
        <rdfs:comment xml:lang="en"></rdfs:comment>
    </owl:Class>
    


    <!-- http://www-usr.inf.ufsm.br/~brunomozza/iotsec/iotsec.owl#SecurityProperty -->

    <owl:Class rdf:about="&iotsec;SecurityProperty">
        <rdfs:label xml:lang="en">Security Property</rdfs:label>
        <rdfs:comment xml:lang="en"></rdfs:comment>
    </owl:Class>
    


    <!-- http://www-usr.inf.ufsm.br/~brunomozza/iotsec/iotsec.owl#SecurityPropertyMethod -->

    <owl:Class rdf:about="&iotsec;SecurityPropertyMethod">
        <rdfs:label xml:lang="en">Security Property Method</rdfs:label>
        <rdfs:subClassOf rdf:resource="&iotsec;SecurityMechanism"/>
        <rdfs:comment xml:lang="en"></rdfs:comment>
    </owl:Class>
    


    <!-- http://www-usr.inf.ufsm.br/~brunomozza/iotsec/iotsec.owl#SecurityTool -->

    <owl:Class rdf:about="&iotsec;SecurityTool">
        <rdfs:label xml:lang="en">Security Tool</rdfs:label>
        <rdfs:subClassOf rdf:resource="&iotsec;SecurityMechanism"/>
        <rdfs:comment xml:lang="en"></rdfs:comment>
    </owl:Class>
    


    <!-- http://www-usr.inf.ufsm.br/~brunomozza/iotsec/iotsec.owl#SensorAttack -->

    <owl:Class rdf:about="&iotsec;SensorAttack">
        <rdfs:label xml:lang="en">Sensor Attack</rdfs:label>
        <rdfs:subClassOf rdf:resource="&iotsec;Threat"/>
        <rdfs:comment xml:lang="en"></rdfs:comment>
    </owl:Class>
    


    <!-- http://www-usr.inf.ufsm.br/~brunomozza/iotsec/iotsec.owl#SensorKeyManagement -->

    <owl:Class rdf:about="&iotsec;SensorKeyManagement">
        <rdfs:label xml:lang="en">Sensor Key Management</rdfs:label>
        <rdfs:subClassOf rdf:resource="&iotsec;KeyManagement"/>
        <rdfs:comment xml:lang="en"></rdfs:comment>
    </owl:Class>
    


    <!-- http://www-usr.inf.ufsm.br/~brunomozza/iotsec/iotsec.owl#SensorSecurityMechanism -->

    <owl:Class rdf:about="&iotsec;SensorSecurityMechanism">
        <rdfs:label xml:lang="en">Sensor Security Mechanism</rdfs:label>
        <rdfs:subClassOf rdf:resource="&iotsec;SecurityMechanism"/>
        <rdfs:comment xml:lang="en"></rdfs:comment>
    </owl:Class>
    


    <!-- http://www-usr.inf.ufsm.br/~brunomozza/iotsec/iotsec.owl#SensorSecurityProtocol -->

    <owl:Class rdf:about="&iotsec;SensorSecurityProtocol">
        <rdfs:label xml:lang="en">Sensor Security Protocol</rdfs:label>
        <rdfs:subClassOf rdf:resource="&iotsec;Protocol"/>
        <rdfs:subClassOf rdf:resource="&iotsec;SensorSecurityMechanism"/>
        <rdfs:comment xml:lang="en"></rdfs:comment>
    </owl:Class>
    


    <!-- http://www-usr.inf.ufsm.br/~brunomozza/iotsec/iotsec.owl#SensorTechnology -->

    <owl:Class rdf:about="&iotsec;SensorTechnology">
        <rdfs:label xml:lang="en">Sensor Technology</rdfs:label>
        <rdfs:subClassOf rdf:resource="&iotsec;Asset"/>
        <rdfs:comment xml:lang="en"></rdfs:comment>
    </owl:Class>
    


    <!-- http://www-usr.inf.ufsm.br/~brunomozza/iotsec/iotsec.owl#SensorVulnerability -->

    <owl:Class rdf:about="&iotsec;SensorVulnerability">
        <rdfs:label xml:lang="en">Sensor Vulnerability</rdfs:label>
        <rdfs:subClassOf rdf:resource="&iotsec;Vulnerability"/>
        <rdfs:subClassOf>
            <owl:Restriction>
                <owl:onProperty rdf:resource="&iotsec;isMitigateBy"/>
                <owl:someValuesFrom rdf:resource="&iotsec;SensorSecurityMechanism"/>
            </owl:Restriction>
        </rdfs:subClassOf>
        <rdfs:subClassOf>
            <owl:Restriction>
                <owl:onProperty rdf:resource="&iotsec;isVulnerabilityOf"/>
                <owl:someValuesFrom rdf:resource="&iotsec;SensorTechnology"/>
            </owl:Restriction>
        </rdfs:subClassOf>
        <rdfs:comment xml:lang="en"></rdfs:comment>
    </owl:Class>
    


    <!-- http://www-usr.inf.ufsm.br/~brunomozza/iotsec/iotsec.owl#ServerAttack -->

    <owl:Class rdf:about="&iotsec;ServerAttack">
        <rdfs:label xml:lang="en">Server Attack</rdfs:label>
        <rdfs:subClassOf rdf:resource="&iotsec;NetworkManagementAttack"/>
        <rdfs:comment xml:lang="en"></rdfs:comment>
    </owl:Class>
    


    <!-- http://www-usr.inf.ufsm.br/~brunomozza/iotsec/iotsec.owl#ServerSecurityMechanism -->

    <owl:Class rdf:about="&iotsec;ServerSecurityMechanism">
        <rdfs:label xml:lang="en">Server Security Mechanism</rdfs:label>
        <rdfs:subClassOf rdf:resource="&iotsec;NetworkManagementSecurityMechanism"/>
        <rdfs:comment xml:lang="en"></rdfs:comment>
    </owl:Class>
    


    <!-- http://www-usr.inf.ufsm.br/~brunomozza/iotsec/iotsec.owl#ServerTechnology -->

    <owl:Class rdf:about="&iotsec;ServerTechnology">
        <rdfs:label xml:lang="en">Server Technology</rdfs:label>
        <rdfs:subClassOf rdf:resource="&iotsec;Asset"/>
        <rdfs:comment xml:lang="en"></rdfs:comment>
    </owl:Class>
    


    <!-- http://www-usr.inf.ufsm.br/~brunomozza/iotsec/iotsec.owl#SeverityScale -->

    <owl:Class rdf:about="&iotsec;SeverityScale">
        <rdfs:label xml:lang="en">Severity Scale</rdfs:label>
        <rdfs:comment xml:lang="en"></rdfs:comment>
    </owl:Class>
    


    <!-- http://www-usr.inf.ufsm.br/~brunomozza/iotsec/iotsec.owl#SoftwareVulnerability -->

    <owl:Class rdf:about="&iotsec;SoftwareVulnerability">
        <rdfs:label xml:lang="en"> Software Vulnerability</rdfs:label>
        <rdfs:subClassOf rdf:resource="&iotsec;Vulnerability"/>
        <rdfs:comment xml:lang="en"></rdfs:comment>
    </owl:Class>
    


    <!-- http://www-usr.inf.ufsm.br/~brunomozza/iotsec/iotsec.owl#SourceCode -->

    <owl:Class rdf:about="&iotsec;SourceCode">
        <rdfs:label xml:lang="en">Source Code</rdfs:label>
        <rdfs:subClassOf rdf:resource="&iotsec;Code"/>
        <rdfs:comment xml:lang="en">Weaknesses in this category are typically found within source code [CWE-18].</rdfs:comment>
        <rdfs:seeAlso xml:lang="en">http://cwe.mitre.org/data/definitions/18.html</rdfs:seeAlso>
    </owl:Class>
    


    <!-- http://www-usr.inf.ufsm.br/~brunomozza/iotsec/iotsec.owl#Spam -->

    <owl:Class rdf:about="&iotsec;Spam">
        <rdfs:label xml:lang="en">Spam</rdfs:label>
        <rdfs:subClassOf rdf:resource="&iotsec;WebAttack"/>
        <rdfs:comment xml:lang="en"></rdfs:comment>
    </owl:Class>
    


    <!-- http://www-usr.inf.ufsm.br/~brunomozza/iotsec/iotsec.owl#Spyware -->

    <owl:Class rdf:about="&iotsec;Spyware">
        <rdfs:label xml:lang="en">Spyware</rdfs:label>
        <rdfs:subClassOf rdf:resource="&iotsec;WebAttack"/>
        <rdfs:comment xml:lang="en"></rdfs:comment>
    </owl:Class>
    


    <!-- http://www-usr.inf.ufsm.br/~brunomozza/iotsec/iotsec.owl#StreamCipher -->

    <owl:Class rdf:about="&iotsec;StreamCipher">
        <rdfs:label xml:lang="en">Stream Cipher</rdfs:label>
        <rdfs:subClassOf rdf:resource="&iotsec;SymmetricAlgorithm"/>
        <rdfs:comment xml:lang="en"></rdfs:comment>
    </owl:Class>
    


    <!-- http://www-usr.inf.ufsm.br/~brunomozza/iotsec/iotsec.owl#SymmetricAlgorithm -->

    <owl:Class rdf:about="&iotsec;SymmetricAlgorithm">
        <rdfs:label xml:lang="en">Symmetric Algorithm</rdfs:label>
        <rdfs:subClassOf rdf:resource="&iotsec;EncryptionAlgorithm"/>
        <rdfs:comment xml:lang="en"></rdfs:comment>
    </owl:Class>
    


    <!-- http://www-usr.inf.ufsm.br/~brunomozza/iotsec/iotsec.owl#SymmetricKey -->

    <owl:Class rdf:about="&iotsec;SymmetricKey">
        <rdfs:label xml:lang="en">Symmetric Key</rdfs:label>
        <rdfs:subClassOf rdf:resource="&iotsec;GSMKeyManagement"/>
        <rdfs:comment xml:lang="en">Symmetric key: the same key is used for encryption and decryption.</rdfs:comment>
    </owl:Class>
    


    <!-- http://www-usr.inf.ufsm.br/~brunomozza/iotsec/iotsec.owl#SymmetricSensorKey -->

    <owl:Class rdf:about="&iotsec;SymmetricSensorKey">
        <rdfs:label xml:lang="en">Symmetric Sensor Key</rdfs:label>
        <rdfs:subClassOf rdf:resource="&iotsec;SensorKeyManagement"/>
        <rdfs:comment xml:lang="en"></rdfs:comment>
    </owl:Class>
    


    <!-- http://www-usr.inf.ufsm.br/~brunomozza/iotsec/iotsec.owl#Threat -->

    <owl:Class rdf:about="&iotsec;Threat">
        <rdfs:label xml:lang="en">Threat</rdfs:label>
        <rdfs:subClassOf>
            <owl:Restriction>
                <owl:onProperty rdf:resource="&iotsec;occursInLayer"/>
                <owl:someValuesFrom rdf:resource="&iotsec;OSIModel"/>
            </owl:Restriction>
        </rdfs:subClassOf>
        <rdfs:subClassOf>
            <owl:Restriction>
                <owl:onProperty rdf:resource="&iotsec;affects"/>
                <owl:someValuesFrom rdf:resource="&iotsec;SecurityProperty"/>
            </owl:Restriction>
        </rdfs:subClassOf>
        <rdfs:subClassOf>
            <owl:Restriction>
                <owl:onProperty rdf:resource="&iotsec;threatens"/>
                <owl:someValuesFrom rdf:resource="&iotsec;Vulnerability"/>
            </owl:Restriction>
        </rdfs:subClassOf>
        <rdfs:comment xml:lang="en"></rdfs:comment>
    </owl:Class>
    


    <!-- http://www-usr.inf.ufsm.br/~brunomozza/iotsec/iotsec.owl#TimeState -->

    <owl:Class rdf:about="&iotsec;TimeState">
        <rdfs:label xml:lang="en">Time and State</rdfs:label>
        <rdfs:subClassOf rdf:resource="&iotsec;SourceCode"/>
        <rdfs:comment xml:lang="en">Weaknesses in this category are related to the improper management of time and state in an environment that supports simultaneous or near-simultaneous computation by multiple systems, processes, or threads [CWE-361].</rdfs:comment>
        <rdfs:seeAlso xml:lang="en">http://cwe.mitre.org/data/definitions/361.html</rdfs:seeAlso>
    </owl:Class>
    


    <!-- http://www-usr.inf.ufsm.br/~brunomozza/iotsec/iotsec.owl#Trojan -->

    <owl:Class rdf:about="&iotsec;Trojan">
        <rdfs:label xml:lang="en">Trojan</rdfs:label>
        <rdfs:subClassOf rdf:resource="&iotsec;Virus"/>
        <rdfs:comment xml:lang="en"></rdfs:comment>
        <rdfs:comment xml:lang="en">A Trojan horse is a malicious piece of software hidden in a program that performs normal tasks. Program that does something malicious (such as capturing passwords) when run by an unsuspecting user [Gyrard 2014].</rdfs:comment>
        <rdfs:seeAlso xml:lang="en">See Paper: Malicious actions against the GPRS technology [Xenakis 2006]</rdfs:seeAlso>
    </owl:Class>
    


    <!-- http://www-usr.inf.ufsm.br/~brunomozza/iotsec/iotsec.owl#TypeofDefense -->

    <owl:Class rdf:about="&iotsec;TypeofDefense">
        <rdfs:label xml:lang="en">Type of Defense</rdfs:label>
        <rdfs:comment xml:lang="en"></rdfs:comment>
    </owl:Class>
    


    <!-- http://www-usr.inf.ufsm.br/~brunomozza/iotsec/iotsec.owl#UMTSArchitecture -->

    <owl:Class rdf:about="&iotsec;UMTSArchitecture">
        <rdfs:label xml:lang="en">UMTS Architecture</rdfs:label>
        <rdfs:subClassOf rdf:resource="&stac;Architecture"/>
        <rdfs:comment xml:lang="en"></rdfs:comment>
    </owl:Class>
    


    <!-- http://www-usr.inf.ufsm.br/~brunomozza/iotsec/iotsec.owl#UMTSArchitectureComponent -->

    <owl:Class rdf:about="&iotsec;UMTSArchitectureComponent">
        <rdfs:label xml:lang="en">UMTS Architecture component</rdfs:label>
        <rdfs:subClassOf rdf:resource="&iotsec;UMTSArchitecture"/>
        <rdfs:comment xml:lang="en"></rdfs:comment>
    </owl:Class>
    


    <!-- http://www-usr.inf.ufsm.br/~brunomozza/iotsec/iotsec.owl#UMTSAttack -->

    <owl:Class rdf:about="&iotsec;UMTSAttack">
        <rdfs:label xml:lang="en">UTMS Attack</rdfs:label>
        <rdfs:subClassOf rdf:resource="&iotsec;Threat"/>
        <rdfs:comment xml:lang="en"></rdfs:comment>
    </owl:Class>
    


    <!-- http://www-usr.inf.ufsm.br/~brunomozza/iotsec/iotsec.owl#UMTSKeyManagement -->

    <owl:Class rdf:about="&iotsec;UMTSKeyManagement">
        <rdfs:label xml:lang="en">UMTS Key Management</rdfs:label>
        <rdfs:subClassOf rdf:resource="&iotsec;KeyManagement"/>
        <rdfs:comment xml:lang="en"></rdfs:comment>
    </owl:Class>
    


    <!-- http://www-usr.inf.ufsm.br/~brunomozza/iotsec/iotsec.owl#UMTSSecurityAlgorithm -->

    <owl:Class rdf:about="&iotsec;UMTSSecurityAlgorithm">
        <rdfs:label xml:lang="en">UMTS Security Algorithm</rdfs:label>
        <rdfs:subClassOf rdf:resource="&iotsec;SecurityAlgorithm"/>
        <rdfs:subClassOf rdf:resource="&iotsec;UMTSSecurityMechanism"/>
        <rdfs:comment xml:lang="en"></rdfs:comment>
    </owl:Class>
    


    <!-- http://www-usr.inf.ufsm.br/~brunomozza/iotsec/iotsec.owl#UMTSSecurityKeyManagement -->

    <owl:Class rdf:about="&iotsec;UMTSSecurityKeyManagement">
        <rdfs:label xml:lang="en">UMTS Security Key Management</rdfs:label>
        <rdfs:subClassOf rdf:resource="&iotsec;UMTSSecurityMechanism"/>
        <rdfs:comment xml:lang="en"></rdfs:comment>
    </owl:Class>
    


    <!-- http://www-usr.inf.ufsm.br/~brunomozza/iotsec/iotsec.owl#UMTSSecurityMechanism -->

    <owl:Class rdf:about="&iotsec;UMTSSecurityMechanism">
        <rdfs:label xml:lang="en">UTMS Security Mechanism</rdfs:label>
        <rdfs:subClassOf rdf:resource="&iotsec;SecurityMechanism"/>
        <rdfs:comment xml:lang="en"></rdfs:comment>
    </owl:Class>
    


    <!-- http://www-usr.inf.ufsm.br/~brunomozza/iotsec/iotsec.owl#UMTSSecurityProtocol -->

    <owl:Class rdf:about="&iotsec;UMTSSecurityProtocol">
        <rdfs:label xml:lang="en">UMTS Security Protocol</rdfs:label>
        <rdfs:subClassOf rdf:resource="&iotsec;Protocol"/>
        <rdfs:subClassOf rdf:resource="&iotsec;UMTSSecurityMechanism"/>
        <rdfs:comment xml:lang="en"></rdfs:comment>
    </owl:Class>
    


    <!-- http://www-usr.inf.ufsm.br/~brunomozza/iotsec/iotsec.owl#UMTSTechnology -->

    <owl:Class rdf:about="&iotsec;UMTSTechnology">
        <rdfs:label xml:lang="en">UMTS Technology</rdfs:label>
        <rdfs:subClassOf rdf:resource="&iotsec;Asset"/>
        <rdfs:comment xml:lang="en">3G technology - Universal Mobile Telecommunications System (UMTS)</rdfs:comment>
        <rdfs:seeAlso rdf:resource="&serviceContext;UMTS"/>
        <rdfs:seeAlso rdf:resource="&ct;UMTS"/>
    </owl:Class>
    


    <!-- http://www-usr.inf.ufsm.br/~brunomozza/iotsec/iotsec.owl#UMTSVulnerability -->

    <owl:Class rdf:about="&iotsec;UMTSVulnerability">
        <rdfs:label xml:lang="en">UMTS Vulnerability</rdfs:label>
        <rdfs:subClassOf rdf:resource="&iotsec;Vulnerability"/>
        <rdfs:subClassOf>
            <owl:Restriction>
                <owl:onProperty rdf:resource="&iotsec;isMitigateBy"/>
                <owl:someValuesFrom rdf:resource="&iotsec;UMTSSecurityMechanism"/>
            </owl:Restriction>
        </rdfs:subClassOf>
        <rdfs:subClassOf>
            <owl:Restriction>
                <owl:onProperty rdf:resource="&iotsec;isVulnerabilityOf"/>
                <owl:someValuesFrom rdf:resource="&iotsec;UMTSTechnology"/>
            </owl:Restriction>
        </rdfs:subClassOf>
        <rdfs:comment xml:lang="en"></rdfs:comment>
    </owl:Class>
    


    <!-- http://www-usr.inf.ufsm.br/~brunomozza/iotsec/iotsec.owl#UncontrolledFormatString -->

    <owl:Class rdf:about="&iotsec;UncontrolledFormatString">
        <rdfs:label xml:lang="en">Uncontrolled Format String</rdfs:label>
        <rdfs:subClassOf rdf:resource="&iotsec;Injection"/>
        <rdfs:comment xml:lang="en">The software uses externally-controlled format strings in printf-style functions, which can lead to buffer overflows or data representation problems [CWE-134].</rdfs:comment>
        <rdfs:seeAlso xml:lang="en">http://cwe.mitre.org/data/definitions/134.html</rdfs:seeAlso>
    </owl:Class>
    


    <!-- http://www-usr.inf.ufsm.br/~brunomozza/iotsec/iotsec.owl#UwbAttack -->

    <owl:Class rdf:about="&iotsec;UwbAttack">
        <rdfs:label xml:lang="en">Uweb Attack</rdfs:label>
        <rdfs:subClassOf rdf:resource="&iotsec;Threat"/>
        <rdfs:comment xml:lang="en"></rdfs:comment>
    </owl:Class>
    


    <!-- http://www-usr.inf.ufsm.br/~brunomozza/iotsec/iotsec.owl#UwbSecurityMechanism -->

    <owl:Class rdf:about="&iotsec;UwbSecurityMechanism">
        <rdfs:label xml:lang="en">Uwb Security Mechanism</rdfs:label>
        <rdfs:subClassOf rdf:resource="&iotsec;SecurityMechanism"/>
        <rdfs:comment xml:lang="en"></rdfs:comment>
    </owl:Class>
    


    <!-- http://www-usr.inf.ufsm.br/~brunomozza/iotsec/iotsec.owl#UwbTechnology -->

    <owl:Class rdf:about="&iotsec;UwbTechnology">
        <rdfs:label xml:lang="en">Uwb Technology</rdfs:label>
        <rdfs:subClassOf rdf:resource="&iotsec;Asset"/>
        <rdfs:comment xml:lang="en"></rdfs:comment>
    </owl:Class>
    


    <!-- http://www-usr.inf.ufsm.br/~brunomozza/iotsec/iotsec.owl#UwbVulnerability -->

    <owl:Class rdf:about="&iotsec;UwbVulnerability">
        <rdfs:label xml:lang="en"> Uwb Vulnerability</rdfs:label>
        <rdfs:subClassOf rdf:resource="&iotsec;Vulnerability"/>
        <rdfs:subClassOf>
            <owl:Restriction>
                <owl:onProperty rdf:resource="&iotsec;isVulnerabilityOf"/>
                <owl:someValuesFrom rdf:resource="&iotsec;UwbTechnology"/>
            </owl:Restriction>
        </rdfs:subClassOf>
        <rdfs:subClassOf>
            <owl:Restriction>
                <owl:onProperty rdf:resource="&iotsec;isMitigateBy"/>
                <owl:someValuesFrom rdf:resource="&iotsec;UwbSecurityMechanism"/>
            </owl:Restriction>
        </rdfs:subClassOf>
        <rdfs:comment xml:lang="en"></rdfs:comment>
    </owl:Class>
    


    <!-- http://www-usr.inf.ufsm.br/~brunomozza/iotsec/iotsec.owl#Virus -->

    <owl:Class rdf:about="&iotsec;Virus">
        <rdfs:label xml:lang="en">Virus</rdfs:label>
        <rdfs:subClassOf rdf:resource="&iotsec;GPRSAttack"/>
        <rdfs:subClassOf rdf:resource="&iotsec;NetworkManagementAttack"/>
        <rdfs:subClassOf rdf:resource="&iotsec;RfidAttack"/>
        <rdfs:subClassOf rdf:resource="&iotsec;WebAttack"/>
        <rdfs:comment xml:lang="en"></rdfs:comment>
        <rdfs:seeAlso xml:lang="en">See Paper: Malicious actions against the GPRS technology [Xenakis 2006], 
	Paper: Survey of Security and Privacy Issues of Internet of Things [Borgohain et al. 2015]</rdfs:seeAlso>
    </owl:Class>
    


    <!-- http://www-usr.inf.ufsm.br/~brunomozza/iotsec/iotsec.owl#Vulnerability -->

    <owl:Class rdf:about="&iotsec;Vulnerability">
        <rdfs:label xml:lang="en">Vulnerability</rdfs:label>
        <rdfs:subClassOf>
            <owl:Restriction>
                <owl:onProperty rdf:resource="&iotsec;hasSeverity"/>
                <owl:someValuesFrom rdf:resource="&iotsec;SeverityScale"/>
            </owl:Restriction>
        </rdfs:subClassOf>
        <rdfs:subClassOf>
            <owl:Restriction>
                <owl:onProperty rdf:resource="&iotsec;generates"/>
                <owl:someValuesFrom rdf:resource="&iotsec;Risk"/>
            </owl:Restriction>
        </rdfs:subClassOf>
        <rdfs:comment xml:lang="en"></rdfs:comment>
    </owl:Class>
    


    <!-- http://www-usr.inf.ufsm.br/~brunomozza/iotsec/iotsec.owl#WebAttack -->

    <owl:Class rdf:about="&iotsec;WebAttack">
        <rdfs:label xml:lang="en">Web Attack</rdfs:label>
        <rdfs:subClassOf rdf:resource="&iotsec;Threat"/>
        <rdfs:comment xml:lang="en"></rdfs:comment>
    </owl:Class>
    


    <!-- http://www-usr.inf.ufsm.br/~brunomozza/iotsec/iotsec.owl#WebSecurityMechanism -->

    <owl:Class rdf:about="&iotsec;WebSecurityMechanism">
        <rdfs:label xml:lang="en">Web Security Mechanism</rdfs:label>
        <rdfs:subClassOf rdf:resource="&iotsec;SecurityMechanism"/>
        <rdfs:subClassOf>
            <owl:Restriction>
                <owl:onProperty rdf:resource="&iotsec;mitigates"/>
                <owl:someValuesFrom rdf:resource="&iotsec;WebVulnerability"/>
            </owl:Restriction>
        </rdfs:subClassOf>
        <rdfs:comment xml:lang="en"></rdfs:comment>
    </owl:Class>
    


    <!-- http://www-usr.inf.ufsm.br/~brunomozza/iotsec/iotsec.owl#WebSecurityProtocol -->

    <owl:Class rdf:about="&iotsec;WebSecurityProtocol">
        <rdfs:label xml:lang="en">Web Security Protocol</rdfs:label>
        <rdfs:subClassOf rdf:resource="&iotsec;Protocol"/>
        <rdfs:subClassOf rdf:resource="&iotsec;WebSecurityMechanism"/>
        <rdfs:comment xml:lang="en"></rdfs:comment>
    </owl:Class>
    


    <!-- http://www-usr.inf.ufsm.br/~brunomozza/iotsec/iotsec.owl#WebService -->

    <owl:Class rdf:about="&iotsec;WebService">
        <rdfs:label xml:lang="en">Web Service</rdfs:label>
        <rdfs:subClassOf rdf:resource="&iotsec;WebTechnology"/>
        <rdfs:comment xml:lang="en"></rdfs:comment>
    </owl:Class>
    


    <!-- http://www-usr.inf.ufsm.br/~brunomozza/iotsec/iotsec.owl#WebServiceAttack -->

    <owl:Class rdf:about="&iotsec;WebServiceAttack">
        <rdfs:label xml:lang="en">Web Service Attack</rdfs:label>
        <rdfs:subClassOf rdf:resource="&iotsec;WebAttack"/>
        <rdfs:comment xml:lang="en"></rdfs:comment>
    </owl:Class>
    


    <!-- http://www-usr.inf.ufsm.br/~brunomozza/iotsec/iotsec.owl#WebTechnology -->

    <owl:Class rdf:about="&iotsec;WebTechnology">
        <rdfs:label xml:lang="en">Web Technology</rdfs:label>
        <rdfs:subClassOf rdf:resource="&iotsec;Asset"/>
        <rdfs:comment xml:lang="en"></rdfs:comment>
    </owl:Class>
    


    <!-- http://www-usr.inf.ufsm.br/~brunomozza/iotsec/iotsec.owl#WebVulnerability -->

    <owl:Class rdf:about="&iotsec;WebVulnerability">
        <rdfs:label xml:lang="en">Web Vulnerability</rdfs:label>
        <rdfs:subClassOf rdf:resource="&iotsec;Vulnerability"/>
        <rdfs:subClassOf>
            <owl:Restriction>
                <owl:onProperty rdf:resource="&iotsec;isMitigateBy"/>
                <owl:someValuesFrom rdf:resource="&iotsec;WebSecurityMechanism"/>
            </owl:Restriction>
        </rdfs:subClassOf>
        <rdfs:subClassOf>
            <owl:Restriction>
                <owl:onProperty rdf:resource="&iotsec;isVulnerabilityOf"/>
                <owl:someValuesFrom rdf:resource="&iotsec;WebTechnology"/>
            </owl:Restriction>
        </rdfs:subClassOf>
        <rdfs:comment xml:lang="en"></rdfs:comment>
    </owl:Class>
    


    <!-- http://www-usr.inf.ufsm.br/~brunomozza/iotsec/iotsec.owl#WifiArchitecture -->

    <owl:Class rdf:about="&iotsec;WifiArchitecture">
        <rdfs:label xml:lang="en">Wifi Architecture</rdfs:label>
        <rdfs:subClassOf rdf:resource="&stac;Architecture"/>
        <rdfs:comment xml:lang="en"></rdfs:comment>
    </owl:Class>
    


    <!-- http://www-usr.inf.ufsm.br/~brunomozza/iotsec/iotsec.owl#WifiArchitectureComponent -->

    <owl:Class rdf:about="&iotsec;WifiArchitectureComponent">
        <rdfs:label xml:lang="en">Wifi Architecture component</rdfs:label>
        <rdfs:subClassOf rdf:resource="&iotsec;WifiArchitecture"/>
        <rdfs:comment xml:lang="en"></rdfs:comment>
    </owl:Class>
    


    <!-- http://www-usr.inf.ufsm.br/~brunomozza/iotsec/iotsec.owl#WifiAttack -->

    <owl:Class rdf:about="&iotsec;WifiAttack">
        <rdfs:label xml:lang="en">WiFi Attack</rdfs:label>
        <rdfs:subClassOf rdf:resource="&iotsec;Threat"/>
        <rdfs:comment xml:lang="en"></rdfs:comment>
    </owl:Class>
    


    <!-- http://www-usr.inf.ufsm.br/~brunomozza/iotsec/iotsec.owl#WifiAttackTool -->

    <owl:Class rdf:about="&iotsec;WifiAttackTool">
        <rdfs:label xml:lang="en">Wifi Attack Tool</rdfs:label>
        <rdfs:subClassOf rdf:resource="&iotsec;SecurityTool"/>
        <rdfs:comment xml:lang="en"></rdfs:comment>
    </owl:Class>
    


    <!-- http://www-usr.inf.ufsm.br/~brunomozza/iotsec/iotsec.owl#WifiKeyManagement -->

    <owl:Class rdf:about="&iotsec;WifiKeyManagement">
        <rdfs:label xml:lang="en">WiFi Key Management</rdfs:label>
        <rdfs:subClassOf rdf:resource="&iotsec;KeyManagement"/>
        <rdfs:subClassOf rdf:resource="&iotsec;WifiSecurityMechanism"/>
        <rdfs:comment xml:lang="en"></rdfs:comment>
    </owl:Class>
    


    <!-- http://www-usr.inf.ufsm.br/~brunomozza/iotsec/iotsec.owl#WifiSecurityMechanism -->

    <owl:Class rdf:about="&iotsec;WifiSecurityMechanism">
        <rdfs:label xml:lang="en">WiFi Security Mechanism</rdfs:label>
        <rdfs:subClassOf rdf:resource="&iotsec;SecurityMechanism"/>
        <rdfs:comment xml:lang="en"></rdfs:comment>
    </owl:Class>
    


    <!-- http://www-usr.inf.ufsm.br/~brunomozza/iotsec/iotsec.owl#WifiSecurityProtocol -->

    <owl:Class rdf:about="&iotsec;WifiSecurityProtocol">
        <rdfs:label xml:lang="en">WiFi Security Protocol</rdfs:label>
        <rdfs:subClassOf rdf:resource="&iotsec;Protocol"/>
        <rdfs:subClassOf rdf:resource="&iotsec;WifiSecurityMechanism"/>
        <rdfs:comment xml:lang="en"></rdfs:comment>
    </owl:Class>
    


    <!-- http://www-usr.inf.ufsm.br/~brunomozza/iotsec/iotsec.owl#WifiTechnology -->

    <owl:Class rdf:about="&iotsec;WifiTechnology">
        <rdfs:label xml:lang="en">WiFi Technology</rdfs:label>
        <rdfs:subClassOf rdf:resource="&iotsec;Asset"/>
        <rdfs:comment xml:lang="en"></rdfs:comment>
        <rdfs:seeAlso rdf:resource="&ct;WiFiConnectivity"/>
    </owl:Class>
    


    <!-- http://www-usr.inf.ufsm.br/~brunomozza/iotsec/iotsec.owl#WifiVulnerability -->

    <owl:Class rdf:about="&iotsec;WifiVulnerability">
        <rdfs:label xml:lang="en">WiFi Vulnerability</rdfs:label>
        <rdfs:subClassOf rdf:resource="&iotsec;Vulnerability"/>
        <rdfs:subClassOf>
            <owl:Restriction>
                <owl:onProperty rdf:resource="&iotsec;isMitigateBy"/>
                <owl:someValuesFrom rdf:resource="&iotsec;WifiSecurityMechanism"/>
            </owl:Restriction>
        </rdfs:subClassOf>
        <rdfs:subClassOf>
            <owl:Restriction>
                <owl:onProperty rdf:resource="&iotsec;isVulnerabilityOf"/>
                <owl:someValuesFrom rdf:resource="&iotsec;WifiTechnology"/>
            </owl:Restriction>
        </rdfs:subClassOf>
        <rdfs:comment xml:lang="en"></rdfs:comment>
    </owl:Class>
    


    <!-- http://www-usr.inf.ufsm.br/~brunomozza/iotsec/iotsec.owl#WimaxArchitecture -->

    <owl:Class rdf:about="&iotsec;WimaxArchitecture">
        <rdfs:label xml:lang="en">WiMAX Architecture</rdfs:label>
        <rdfs:subClassOf rdf:resource="&stac;Architecture"/>
        <rdfs:comment xml:lang="en"></rdfs:comment>
    </owl:Class>
    


    <!-- http://www-usr.inf.ufsm.br/~brunomozza/iotsec/iotsec.owl#WimaxArchitectureComponent -->

    <owl:Class rdf:about="&iotsec;WimaxArchitectureComponent">
        <rdfs:label xml:lang="en">Wimax Architecture component</rdfs:label>
        <rdfs:subClassOf rdf:resource="&iotsec;WimaxArchitecture"/>
        <rdfs:comment xml:lang="en"></rdfs:comment>
    </owl:Class>
    


    <!-- http://www-usr.inf.ufsm.br/~brunomozza/iotsec/iotsec.owl#WimaxAttack -->

    <owl:Class rdf:about="&iotsec;WimaxAttack">
        <rdfs:label xml:lang="en">Wimax Attack</rdfs:label>
        <rdfs:subClassOf rdf:resource="&iotsec;Threat"/>
        <rdfs:comment xml:lang="en"></rdfs:comment>
    </owl:Class>
    


    <!-- http://www-usr.inf.ufsm.br/~brunomozza/iotsec/iotsec.owl#WimaxKeyManagement -->

    <owl:Class rdf:about="&iotsec;WimaxKeyManagement">
        <rdfs:label xml:lang="en">Wimax Key Management</rdfs:label>
        <rdfs:subClassOf rdf:resource="&iotsec;KeyManagement"/>
        <rdfs:subClassOf rdf:resource="&iotsec;WimaxSecurityMechanism"/>
        <rdfs:comment xml:lang="en"></rdfs:comment>
    </owl:Class>
    


    <!-- http://www-usr.inf.ufsm.br/~brunomozza/iotsec/iotsec.owl#WimaxSecurityMechanism -->

    <owl:Class rdf:about="&iotsec;WimaxSecurityMechanism">
        <rdfs:label xml:lang="en">Wimax Security Mechanism</rdfs:label>
        <rdfs:subClassOf rdf:resource="&iotsec;SecurityMechanism"/>
        <rdfs:subClassOf>
            <owl:Restriction>
                <owl:onProperty rdf:resource="&iotsec;mitigates"/>
                <owl:someValuesFrom rdf:resource="&iotsec;WimaxVulnerability"/>
            </owl:Restriction>
        </rdfs:subClassOf>
        <rdfs:comment xml:lang="en"></rdfs:comment>
    </owl:Class>
    


    <!-- http://www-usr.inf.ufsm.br/~brunomozza/iotsec/iotsec.owl#WimaxSecurityProtocol -->

    <owl:Class rdf:about="&iotsec;WimaxSecurityProtocol">
        <rdfs:label xml:lang="en">Wimax Security Protocol</rdfs:label>
        <rdfs:subClassOf rdf:resource="&iotsec;Protocol"/>
        <rdfs:subClassOf rdf:resource="&iotsec;WimaxSecurityMechanism"/>
        <rdfs:comment xml:lang="en"></rdfs:comment>
    </owl:Class>
    


    <!-- http://www-usr.inf.ufsm.br/~brunomozza/iotsec/iotsec.owl#WimaxTechnology -->

    <owl:Class rdf:about="&iotsec;WimaxTechnology">
        <rdfs:label xml:lang="en">Wimax Technology</rdfs:label>
        <rdfs:subClassOf rdf:resource="&iotsec;Asset"/>
        <rdfs:comment xml:lang="en"></rdfs:comment>
        <rdfs:seeAlso rdf:resource="&ct;WiMAXConnectivity"/>
    </owl:Class>
    


    <!-- http://www-usr.inf.ufsm.br/~brunomozza/iotsec/iotsec.owl#WimaxVulnerability -->

    <owl:Class rdf:about="&iotsec;WimaxVulnerability">
        <rdfs:label xml:lang="en">Wimax Vulnerability</rdfs:label>
        <rdfs:subClassOf rdf:resource="&iotsec;Vulnerability"/>
        <rdfs:subClassOf>
            <owl:Restriction>
                <owl:onProperty rdf:resource="&iotsec;isMitigateBy"/>
                <owl:someValuesFrom rdf:resource="&iotsec;WimaxSecurityMechanism"/>
            </owl:Restriction>
        </rdfs:subClassOf>
        <rdfs:subClassOf>
            <owl:Restriction>
                <owl:onProperty rdf:resource="&iotsec;isVulnerabilityOf"/>
                <owl:someValuesFrom rdf:resource="&iotsec;WimaxTechnology"/>
            </owl:Restriction>
        </rdfs:subClassOf>
        <rdfs:comment xml:lang="en"></rdfs:comment>
    </owl:Class>
    


    <!-- http://www-usr.inf.ufsm.br/~brunomozza/iotsec/iotsec.owl#Worm -->

    <owl:Class rdf:about="&iotsec;Worm">
        <rdfs:label xml:lang="en">Worm</rdfs:label>
        <rdfs:subClassOf rdf:resource="&iotsec;WebAttack"/>
        <rdfs:seeAlso xml:lang="en">See Paper: Malicious actions against the GPRS technology [Xenakis 2006]</rdfs:seeAlso>
        <rdfs:comment xml:lang="en">Worms are self-propagating pieces of malicious software. They propagate from one computer/device to another via a network link [Gyrard 2014].</rdfs:comment>
    </owl:Class>
    


    <!-- http://www-usr.inf.ufsm.br/~brunomozza/iotsec/iotsec.owl#ZigbeeAttack -->

    <owl:Class rdf:about="&iotsec;ZigbeeAttack">
        <rdfs:label xml:lang="en">Zigbee Attack</rdfs:label>
        <rdfs:subClassOf rdf:resource="&iotsec;Threat"/>
        <rdfs:comment xml:lang="en"></rdfs:comment>
    </owl:Class>
    


    <!-- http://www-usr.inf.ufsm.br/~brunomozza/iotsec/iotsec.owl#ZigbeeSecurityMechanism -->

    <owl:Class rdf:about="&iotsec;ZigbeeSecurityMechanism">
        <rdfs:label xml:lang="en">Zigbee Security Mechanism</rdfs:label>
        <rdfs:subClassOf rdf:resource="&iotsec;SecurityMechanism"/>
        <rdfs:comment xml:lang="en"></rdfs:comment>
    </owl:Class>
    


    <!-- http://www-usr.inf.ufsm.br/~brunomozza/iotsec/iotsec.owl#ZigbeeTechnology -->

    <owl:Class rdf:about="&iotsec;ZigbeeTechnology">
        <rdfs:label xml:lang="en">Zigbee Technology</rdfs:label>
        <rdfs:subClassOf rdf:resource="&iotsec;Asset"/>
        <rdfs:comment xml:lang="en"></rdfs:comment>
    </owl:Class>
    


    <!-- http://www-usr.inf.ufsm.br/~brunomozza/iotsec/iotsec.owl#ZigbeeVulnerability -->

    <owl:Class rdf:about="&iotsec;ZigbeeVulnerability">
        <rdfs:label xml:lang="en">Zigbee Vulnerability</rdfs:label>
        <rdfs:subClassOf rdf:resource="&iotsec;Vulnerability"/>
        <rdfs:subClassOf>
            <owl:Restriction>
                <owl:onProperty rdf:resource="&iotsec;isVulnerabilityOf"/>
                <owl:someValuesFrom rdf:resource="&iotsec;ZigbeeTechnology"/>
            </owl:Restriction>
        </rdfs:subClassOf>
        <rdfs:subClassOf>
            <owl:Restriction>
                <owl:onProperty rdf:resource="&iotsec;isMitigateBy"/>
                <owl:someValuesFrom rdf:resource="&iotsec;ZigbeeSecurityMechanism"/>
            </owl:Restriction>
        </rdfs:subClassOf>
        <rdfs:comment xml:lang="en"></rdfs:comment>
    </owl:Class>
    


    <!-- 
    ///////////////////////////////////////////////////////////////////////////////////////
    //
    // Individuals
    //
    ///////////////////////////////////////////////////////////////////////////////////////
     -->

    


    <!-- http://preciosa.informatik.hu-berlin.de/ontology/security.owl3DES -->

    <owl:NamedIndividual rdf:about="&secberlin;3DES">
        <rdf:type rdf:resource="&iotsec;BlockCipher"/>
        <owl:sameAs rdf:resource="&iotsec;TripleDES"/>
    </owl:NamedIndividual>
    


    <!-- http://preciosa.informatik.hu-berlin.de/ontology/security.owlAES -->

    <owl:NamedIndividual rdf:about="&secberlin;AES">
        <rdf:type rdf:resource="&iotsec;BlockCipher"/>
        <owl:sameAs rdf:resource="&iotsec;AES"/>
    </owl:NamedIndividual>
    


    <!-- http://preciosa.informatik.hu-berlin.de/ontology/security.owlAccountability -->

    <owl:NamedIndividual rdf:about="&secberlin;Accountability">
        <owl:sameAs rdf:resource="&iotsec;Accountability"/>
    </owl:NamedIndividual>
    


    <!-- http://preciosa.informatik.hu-berlin.de/ontology/security.owlAuthorization -->

    <owl:NamedIndividual rdf:about="&secberlin;Authorization">
        <owl:sameAs rdf:resource="&iotsec;Authorization"/>
    </owl:NamedIndividual>
    


    <!-- http://preciosa.informatik.hu-berlin.de/ontology/security.owlBlowfish -->

    <owl:NamedIndividual rdf:about="&secberlin;Blowfish">
        <owl:sameAs rdf:resource="&iotsec;Blowfish"/>
    </owl:NamedIndividual>
    


    <!-- http://preciosa.informatik.hu-berlin.de/ontology/security.owlDES -->

    <owl:NamedIndividual rdf:about="&secberlin;DES">
        <owl:sameAs rdf:resource="&iotsec;DES"/>
    </owl:NamedIndividual>
    


    <!-- http://preciosa.informatik.hu-berlin.de/ontology/security.owlEllipticCurveCryptography -->

    <owl:NamedIndividual rdf:about="&secberlin;EllipticCurveCryptography">
        <owl:sameAs rdf:resource="&iotsec;ECC"/>
    </owl:NamedIndividual>
    


    <!-- http://preciosa.informatik.hu-berlin.de/ontology/security.owlRC4 -->

    <owl:NamedIndividual rdf:about="&secberlin;RC4">
        <owl:sameAs rdf:resource="&iotsec;RC4"/>
    </owl:NamedIndividual>
    


    <!-- http://securitytoolbox.appspot.com/MASO#AES -->

    <owl:NamedIndividual rdf:about="&maso;AES">
        <owl:sameAs rdf:resource="&iotsec;AES"/>
    </owl:NamedIndividual>
    


    <!-- http://securitytoolbox.appspot.com/MASO#Blowfish -->

    <owl:NamedIndividual rdf:about="&maso;Blowfish">
        <owl:sameAs rdf:resource="&iotsec;Blowfish"/>
    </owl:NamedIndividual>
    


    <!-- http://securitytoolbox.appspot.com/MASO#CAST -->

    <owl:NamedIndividual rdf:about="&maso;CAST">
        <owl:sameAs rdf:resource="&iotsec;CAST"/>
    </owl:NamedIndividual>
    


    <!-- http://securitytoolbox.appspot.com/MASO#Confiance -->

    <owl:NamedIndividual rdf:about="&maso;Confiance">
        <owl:sameAs rdf:resource="&iotsec;Trust"/>
    </owl:NamedIndividual>
    


    <!-- http://securitytoolbox.appspot.com/MASO#Confidentialite -->

    <owl:NamedIndividual rdf:about="&maso;Confidentialite">
        <owl:sameAs rdf:resource="&iotsec;Confidentiality"/>
    </owl:NamedIndividual>
    


    <!-- http://securitytoolbox.appspot.com/MASO#DES -->

    <owl:NamedIndividual rdf:about="&maso;DES">
        <owl:sameAs rdf:resource="&iotsec;DES"/>
    </owl:NamedIndividual>
    


    <!-- http://securitytoolbox.appspot.com/MASO#Disponibilite -->

    <owl:NamedIndividual rdf:about="&maso;Disponibilite">
        <owl:sameAs rdf:resource="&iotsec;Availability"/>
    </owl:NamedIndividual>
    


    <!-- http://securitytoolbox.appspot.com/MASO#ElGamal -->

    <owl:NamedIndividual rdf:about="&maso;ElGamal">
        <owl:sameAs rdf:resource="&iotsec;ElGamal"/>
    </owl:NamedIndividual>
    


    <!-- http://securitytoolbox.appspot.com/MASO#Elliptic_curve -->

    <owl:NamedIndividual rdf:about="&maso;Elliptic_curve">
        <owl:sameAs rdf:resource="&iotsec;ECC"/>
    </owl:NamedIndividual>
    


    <!-- http://securitytoolbox.appspot.com/MASO#IDEA -->

    <owl:NamedIndividual rdf:about="&maso;IDEA">
        <owl:sameAs rdf:resource="&iotsec;IDEA"/>
    </owl:NamedIndividual>
    


    <!-- http://securitytoolbox.appspot.com/MASO#Integrite -->

    <owl:NamedIndividual rdf:about="&maso;Integrite">
        <owl:sameAs rdf:resource="&iotsec;Integrity"/>
    </owl:NamedIndividual>
    


    <!-- http://securitytoolbox.appspot.com/MASO#MD5 -->

    <owl:NamedIndividual rdf:about="&maso;MD5">
        <owl:sameAs rdf:resource="&iotsec;MD5"/>
    </owl:NamedIndividual>
    


    <!-- http://securitytoolbox.appspot.com/MASO#Non-repudiation -->

    <owl:NamedIndividual rdf:about="&maso;Non-repudiation">
        <owl:sameAs rdf:resource="&iotsec;NonRepudiation"/>
    </owl:NamedIndividual>
    


    <!-- http://securitytoolbox.appspot.com/MASO#RSA -->

    <owl:NamedIndividual rdf:about="&maso;RSA">
        <owl:sameAs rdf:resource="&iotsec;RSA"/>
    </owl:NamedIndividual>
    


    <!-- http://securitytoolbox.appspot.com/MASO#Twofish -->

    <owl:NamedIndividual rdf:about="&maso;Twofish">
        <owl:sameAs rdf:resource="&iotsec;Twofish"/>
    </owl:NamedIndividual>
    


    <!-- http://securitytoolbox.appspot.com/MASO#_3DES -->

    <owl:NamedIndividual rdf:about="&maso;_3DES">
        <owl:sameAs rdf:resource="&iotsec;TripleDES"/>
    </owl:NamedIndividual>
    


    <!-- http://securitytoolbox.appspot.com/securityAlgorithms#AES -->

    <owl:NamedIndividual rdf:about="&kimalgorithms;AES">
        <owl:sameAs rdf:resource="&iotsec;AES"/>
    </owl:NamedIndividual>
    


    <!-- http://securitytoolbox.appspot.com/securityAlgorithms#Blowfish -->

    <owl:NamedIndividual rdf:about="&kimalgorithms;Blowfish">
        <owl:sameAs rdf:resource="&iotsec;Blowfish"/>
    </owl:NamedIndividual>
    


    <!-- http://securitytoolbox.appspot.com/securityAlgorithms#CAST -->

    <owl:NamedIndividual rdf:about="&kimalgorithms;CAST">
        <owl:sameAs rdf:resource="&iotsec;CAST"/>
    </owl:NamedIndividual>
    


    <!-- http://securitytoolbox.appspot.com/securityAlgorithms#DES -->

    <owl:NamedIndividual rdf:about="&kimalgorithms;DES">
        <owl:sameAs rdf:resource="&iotsec;DES"/>
    </owl:NamedIndividual>
    


    <!-- http://securitytoolbox.appspot.com/securityAlgorithms#ECC -->

    <owl:NamedIndividual rdf:about="&kimalgorithms;ECC">
        <owl:sameAs rdf:resource="&iotsec;ECC"/>
    </owl:NamedIndividual>
    


    <!-- http://securitytoolbox.appspot.com/securityAlgorithms#MD5 -->

    <owl:NamedIndividual rdf:about="&kimalgorithms;MD5">
        <owl:sameAs rdf:resource="&iotsec;MD5"/>
    </owl:NamedIndividual>
    


    <!-- http://securitytoolbox.appspot.com/securityAlgorithms#RC4 -->

    <owl:NamedIndividual rdf:about="&kimalgorithms;RC4">
        <owl:sameAs rdf:resource="&iotsec;RC4"/>
    </owl:NamedIndividual>
    


    <!-- http://securitytoolbox.appspot.com/securityAlgorithms#RIPE-MD -->

    <owl:NamedIndividual rdf:about="&kimalgorithms;RIPE-MD">
        <owl:sameAs rdf:resource="&iotsec;RIPE-MD"/>
    </owl:NamedIndividual>
    


    <!-- http://securitytoolbox.appspot.com/securityAlgorithms#RSA -->

    <owl:NamedIndividual rdf:about="&kimalgorithms;RSA">
        <owl:sameAs rdf:resource="&iotsec;RSA"/>
    </owl:NamedIndividual>
    


    <!-- http://securitytoolbox.appspot.com/securityAlgorithms#SHA-1 -->

    <owl:NamedIndividual rdf:about="&kimalgorithms;SHA-1">
        <owl:sameAs rdf:resource="&iotsec;SHA"/>
    </owl:NamedIndividual>
    


    <!-- http://securitytoolbox.appspot.com/securityAlgorithms#Skipjack -->

    <owl:NamedIndividual rdf:about="&kimalgorithms;Skipjack">
        <owl:sameAs rdf:resource="&iotsec;Skipjack"/>
    </owl:NamedIndividual>
    


    <!-- http://securitytoolbox.appspot.com/securityAlgorithms#TripleDES -->

    <owl:NamedIndividual rdf:about="&kimalgorithms;TripleDES">
        <owl:sameAs rdf:resource="&iotsec;TripleDES"/>
    </owl:NamedIndividual>
    


    <!-- http://securitytoolbox.appspot.com/securityMain#Anonymity -->

    <owl:NamedIndividual rdf:about="&kim;Anonymity">
        <owl:sameAs rdf:resource="&iotsec;Anonymity"/>
    </owl:NamedIndividual>
    


    <!-- http://securitytoolbox.appspot.com/securityMain#Authorization -->

    <owl:NamedIndividual rdf:about="&kim;Authorization">
        <owl:sameAs rdf:resource="&iotsec;Authorization"/>
    </owl:NamedIndividual>
    


    <!-- http://securitytoolbox.appspot.com/securityMain#Availability -->

    <owl:NamedIndividual rdf:about="&kim;Availability">
        <owl:sameAs rdf:resource="&iotsec;Availability"/>
    </owl:NamedIndividual>
    


    <!-- http://securitytoolbox.appspot.com/securityMain#Confidentiality -->

    <owl:NamedIndividual rdf:about="&kim;Confidentiality">
        <owl:sameAs rdf:resource="&iotsec;Confidentiality"/>
    </owl:NamedIndividual>
    


    <!-- http://securitytoolbox.appspot.com/securityMain#MessageIntegrity -->

    <owl:NamedIndividual rdf:about="&kim;MessageIntegrity">
        <owl:sameAs rdf:resource="&iotsec;Integrity"/>
    </owl:NamedIndividual>
    


    <!-- http://securitytoolbox.appspot.com/securityMain#Trust -->

    <owl:NamedIndividual rdf:about="&kim;Trust">
        <owl:sameAs rdf:resource="&iotsec;Trust"/>
    </owl:NamedIndividual>
    


    <!-- http://securitytoolbox.appspot.com/stac#A3 -->

    <owl:NamedIndividual rdf:about="&stac;A3">
        <rdf:type rdf:resource="&iotsec;GSMSecurityAlgorithm"/>
        <rdfs:label xml:lang="en">A3</rdfs:label>
        <rdfs:comment xml:lang="en">See Paper: Malicious actions against the GPRS technology [Xenakis 2006]</rdfs:comment>
        <rdfs:comment xml:lang="en">The A3 algorithm is the authentication algorithm for GSM networks. The A3 algorithm resides on the SIM card and at the AuC/HLR. The main purpose of this algorithm is to authenticate the identity of a mobile subscriber.</rdfs:comment>
        <iotsec:satisfies rdf:resource="&iotsec;Authentication"/>
    </owl:NamedIndividual>
    


    <!-- http://securitytoolbox.appspot.com/stac#A5_3 -->

    <owl:NamedIndividual rdf:about="&stac;A5_3">
        <rdf:type rdf:resource="&iotsec;GSMSecurityAlgorithm"/>
        <rdf:type rdf:resource="&iotsec;StreamCipher"/>
        <rdfs:label xml:lang="en">A5</rdfs:label>
        <rdfs:comment xml:lang="en">A5 is an encryption algorithm to encrypt the communication between the mobile phone and the base station (BTS Base Station Transceiver).</rdfs:comment>
        <iotsec:satisfies rdf:resource="&iotsec;Confidentiality"/>
        <dcterms:hasPart rdf:resource="&iotsec;Kasumi"/>
    </owl:NamedIndividual>
    


    <!-- http://securitytoolbox.appspot.com/stac#A8 -->

    <owl:NamedIndividual rdf:about="&stac;A8">
        <rdf:type rdf:resource="&iotsec;GSMKeyManagement"/>
        <rdf:type rdf:resource="&iotsec;GSMSecurityAlgorithm"/>
        <rdfs:label xml:lang="en">A8</rdfs:label>
        <rdfs:comment xml:lang="en">A8 algorithm is the ciphering key generation algorithm.</rdfs:comment>
        <iotsec:satisfies rdf:resource="&iotsec;Authentication"/>
    </owl:NamedIndividual>
    


    <!-- http://securitytoolbox.appspot.com/stac#AAAServer -->

    <owl:NamedIndividual rdf:about="&stac;AAAServer">
        <rdf:type rdf:resource="&iotsec;GSMSecurityMechanism"/>
        <rdf:type rdf:resource="&iotsec;ManetSecurityMechanism"/>
        <rdf:type rdf:resource="&iotsec;MeshSecurityMechanism"/>
        <rdfs:label xml:lang="en">Authentication, Authorization, Accounting (AAA)</rdfs:label>
        <rdfs:comment xml:lang="en">Security architecture for distributed systems.</rdfs:comment>
        <iotsec:satisfies rdf:resource="&iotsec;Accountability"/>
        <iotsec:satisfies rdf:resource="&iotsec;Authentication"/>
        <iotsec:satisfies rdf:resource="&iotsec;Authorization"/>
    </owl:NamedIndividual>
    


    <!-- http://securitytoolbox.appspot.com/stac#ACL -->

    <owl:NamedIndividual rdf:about="&stac;ACL">
        <rdf:type rdf:resource="&iotsec;NetworkManagementSecurityMechanism"/>
        <rdfs:label xml:lang="en">Access Control List (ACL)</rdfs:label>
        <rdfs:comment xml:lang="en"></rdfs:comment>
        <iotsec:satisfies rdf:resource="&iotsec;AccessControl"/>
        <iotsec:protectsInLayer rdf:resource="&iotsec;NetworkLayer"/>
        <iotsec:protectsInLayer rdf:resource="&iotsec;TransportLayer"/>
    </owl:NamedIndividual>
    


    <!-- http://securitytoolbox.appspot.com/stac#AES -->

    <owl:NamedIndividual rdf:about="&stac;AES">
        <owl:sameAs rdf:resource="&stac;Rijndael"/>
        <owl:sameAs rdf:resource="&iotsec;AES"/>
    </owl:NamedIndividual>
    


    <!-- http://securitytoolbox.appspot.com/stac#AIDE -->

    <owl:NamedIndividual rdf:about="&stac;AIDE">
        <rdf:type rdf:resource="&iotsec;IDS"/>
        <rdfs:label xml:lang="en">Advanced Intrusion Detection Environment (AIDE)</rdfs:label>
        <rdfs:comment xml:lang="en"></rdfs:comment>
        <iotsec:protectsInLayer rdf:resource="&iotsec;ApplicationLayer"/>
        <iotsec:satisfies rdf:resource="&iotsec;Availability"/>
        <iotsec:hasFeature rdf:resource="&iotsec;Free"/>
    </owl:NamedIndividual>
    


    <!-- http://securitytoolbox.appspot.com/stac#AInterface -->

    <owl:NamedIndividual rdf:about="&stac;AInterface">
        <rdf:type rdf:resource="&stac;GSMArchitectureComponent"/>
        <rdfs:label xml:lang="en">AInterface</rdfs:label>
        <rdfs:comment xml:lang="en">The BSS communicates with the MSC across the A interface.</rdfs:comment>
    </owl:NamedIndividual>
    


    <!-- http://securitytoolbox.appspot.com/stac#AKA -->

    <owl:NamedIndividual rdf:about="&stac;AKA">
        <rdf:type rdf:resource="&iotsec;UMTSSecurityProtocol"/>
        <rdfs:label xml:lang="en">AKA (Authentication and Key Agreement)</rdfs:label>
        <rdfs:comment xml:lang="en"></rdfs:comment>
        <rdfs:comment xml:lang="en">See Paper: Securing 4G networks with y-communication using AKA protocol [Rana 2011]</rdfs:comment>
        <iotsec:satisfies rdf:resource="&iotsec;Authentication"/>
        <iotsec:protectsInLayer rdf:resource="&iotsec;LinkLayer"/>
        <dcterms:hasPart rdf:resource="&iotsec;f3"/>
        <dcterms:hasPart rdf:resource="&iotsec;f4"/>
    </owl:NamedIndividual>
    


    <!-- http://securitytoolbox.appspot.com/stac#ARPPoisoning -->

    <owl:NamedIndividual rdf:about="&stac;ARPPoisoning">
        <rdf:type rdf:resource="&iotsec;Flooding"/>
        <rdfs:label xml:lang="en">ARP Poisoning/ ARP Spoofing</rdfs:label>
        <rdfs:comment xml:lang="en">Is a technique whereby an attacker sends fake (&quot;spoofed&quot;) ARP messages. ARP (Address Resolution Protocol) is the protocol which convert MAC address into IP address.</rdfs:comment>
    </owl:NamedIndividual>
    


    <!-- http://securitytoolbox.appspot.com/stac#AVG -->

    <owl:NamedIndividual rdf:about="&stac;AVG">
        <rdf:type rdf:resource="&iotsec;Antivirus"/>
        <rdfs:label xml:lang="en">AVG</rdfs:label>
        <rdfs:comment xml:lang="en"></rdfs:comment>
        <iotsec:hasFeature rdf:resource="&iotsec;Free"/>
        <iotsec:satisfies rdf:resource="&iotsec;Integrity"/>
    </owl:NamedIndividual>
    


    <!-- http://securitytoolbox.appspot.com/stac#AccessPoint -->

    <owl:NamedIndividual rdf:about="&stac;AccessPoint">
        <rdf:type rdf:resource="&iotsec;WifiArchitectureComponent"/>
        <rdfs:label xml:lang="en">Access Point (AP)</rdfs:label>
        <rdfs:comment xml:lang="en">An AP is a hardware device that allows wireless communication devices (e.g., PDAs or mobile computers) to connect to a wireless network. An AP connects to a wired network, and provides a bridge for data communication between wireless and wired devices.</rdfs:comment>
    </owl:NamedIndividual>
    


    <!-- http://securitytoolbox.appspot.com/stac#Accountability -->

    <owl:NamedIndividual rdf:about="&stac;Accountability">
        <rdf:type rdf:resource="&iotsec;SecurityProperty"/>
        <rdfs:label xml:lang="en">Accountability</rdfs:label>
        <rdfs:comment xml:lang="en">Accountability is the requirement that actions of an entity may be traced uniquely to that entity.</rdfs:comment>
        <owl:sameAs rdf:resource="&iotsec;Accountability"/>
        <owl:sameAs rdf:resource="&herzog;Accountability"/>
    </owl:NamedIndividual>
    


    <!-- http://securitytoolbox.appspot.com/stac#AcegiSecuritySystem -->

    <owl:NamedIndividual rdf:about="&stac;AcegiSecuritySystem">
        <rdf:type rdf:resource="&iotsec;FrameworkSecurityMechanism"/>
        <rdfs:label xml:lang="en">Acegi Security System</rdfs:label>
        <rdfs:comment xml:lang="en">Acegi Security System is an aspect-oriented framework for incorporating security requirements into software. Acegi is build on top of Spring, the well-known Java framework. Spring does not implement its aspect-oriented features on the language level but though the use of dynamic byte code generation, thereby leaving the Java language intact. Acegi uses these aspect-oriented features to offer support for authentication and authorization services.</rdfs:comment>
        <iotsec:satisfies rdf:resource="&iotsec;Authentication"/>
        <iotsec:satisfies rdf:resource="&iotsec;Authorization"/>
    </owl:NamedIndividual>
    


    <!-- http://securitytoolbox.appspot.com/stac#AcknowledgmentSpoofing -->

    <owl:NamedIndividual rdf:about="&stac;AcknowledgmentSpoofing">
        <rdf:type rdf:resource="&iotsec;SensorAttack"/>
        <rdfs:label xml:lang="en">Acknowledgment Spoofing</rdfs:label>
        <rdfs:comment xml:lang="en"></rdfs:comment>
        <rdfs:comment xml:lang="en">An adversary spoofs link layer acknowledgment (ACK) packets of neighboring nodes. By spoofing such packets, an adversary can convince the sender that &quot;a weak link is strong or that a dead or disabled node is alive.&quot;</rdfs:comment>
        <iotsec:threatens rdf:resource="&iotsec;Authentication"/>
        <iotsec:occursInLayer rdf:resource="&iotsec;NetworkLayer"/>
    </owl:NamedIndividual>
    


    <!-- http://securitytoolbox.appspot.com/stac#AdHocMode -->

    <owl:NamedIndividual rdf:about="&stac;AdHocMode">
        <rdf:type rdf:resource="&iotsec;WifiArchitectureComponent"/>
        <rdfs:label xml:lang="en">Ad Hoc Mode</rdfs:label>
        <rdfs:comment xml:lang="en">It consists of at least two wireless stations where no access point is involved in their communication.</rdfs:comment>
    </owl:NamedIndividual>
    


    <!-- http://securitytoolbox.appspot.com/stac#AdaptiveChosenPlaintext -->

    <owl:NamedIndividual rdf:about="&stac;AdaptiveChosenPlaintext">
        <rdf:type rdf:resource="&iotsec;Threat"/>
        <rdfs:label xml:lang="en">Adaptive Chosen Plaintext</rdfs:label>
        <rdfs:comment xml:lang="en">The attacker can gets ciphers of chosen plaintexts before and after challenge.</rdfs:comment>
    </owl:NamedIndividual>
    


    <!-- http://securitytoolbox.appspot.com/stac#AdaptiveChosenPlaintextCiphertext -->

    <owl:NamedIndividual rdf:about="&stac;AdaptiveChosenPlaintextCiphertext">
        <rdf:type rdf:resource="&iotsec;Threat"/>
        <rdfs:label xml:lang="en">Adaptive Chosen Plaintext Ciphertext</rdfs:label>
        <rdfs:comment xml:lang="en">The attacker can decipher chosen ciphertexts before and after the challenge (apart fro; this letter).</rdfs:comment>
    </owl:NamedIndividual>
    


    <!-- http://securitytoolbox.appspot.com/stac#Adware -->

    <owl:NamedIndividual rdf:about="&stac;Adware">
        <rdf:type rdf:resource="&iotsec;WebAttack"/>
        <rdfs:label xml:lang="en">Adware</rdfs:label>
        <rdfs:comment xml:lang="en"></rdfs:comment>
        <iotsec:occursInLayer rdf:resource="&iotsec;ApplicationLayer"/>
    </owl:NamedIndividual>
    


    <!-- http://securitytoolbox.appspot.com/stac#Aerosol -->

    <owl:NamedIndividual rdf:about="&stac;Aerosol">
        <rdf:type rdf:resource="&iotsec;WifiAttackTool"/>
        <rdfs:label xml:lang="en">Aerosol</rdfs:label>
        <rdfs:comment xml:lang="en"></rdfs:comment>
    </owl:NamedIndividual>
    


    <!-- http://securitytoolbox.appspot.com/stac#AirCrack -->

    <owl:NamedIndividual rdf:about="&stac;AirCrack">
        <rdf:type rdf:resource="&iotsec;WifiAttackTool"/>
        <rdfs:label xml:lang="en">Air Crack</rdfs:label>
        <rdfs:comment xml:lang="en">Air Crack is a suite of tools for WEP and WPA cracking. It implments the best known cracking algorithms to recover wireless keys once enough encrypted packets have been gathered.</rdfs:comment>
    </owl:NamedIndividual>
    


    <!-- http://securitytoolbox.appspot.com/stac#AirSnort -->

    <owl:NamedIndividual rdf:about="&stac;AirSnort">
        <rdf:type rdf:resource="&iotsec;WifiAttackTool"/>
        <rdfs:label xml:lang="en">AirSnort</rdfs:label>
        <rdfs:comment xml:lang="en"></rdfs:comment>
    </owl:NamedIndividual>
    


    <!-- http://securitytoolbox.appspot.com/stac#Altered -->

    <owl:NamedIndividual rdf:about="&stac;Altered">
        <rdf:type rdf:resource="&iotsec;SensorAttack"/>
        <rdfs:label xml:lang="en">Altered</rdfs:label>
        <rdfs:comment xml:lang="en">Routing information exchanged between sensor nodes is altered by an attacker.</rdfs:comment>
        <iotsec:occursInLayer rdf:resource="&iotsec;NetworkLayer"/>
    </owl:NamedIndividual>
    


    <!-- http://securitytoolbox.appspot.com/stac#Android -->

    <owl:NamedIndividual rdf:about="&stac;Android">
        <rdf:type rdf:resource="&iotsec;OperatingSystemTechnology"/>
        <rdf:type rdf:resource="&iotsec;ProgrammingLanguageTechnology"/>
        <rdfs:label xml:lang="en">Android</rdfs:label>
        <rdfs:comment xml:lang="en"></rdfs:comment>
    </owl:NamedIndividual>
    


    <!-- http://securitytoolbox.appspot.com/stac#Anonymity -->

    <owl:NamedIndividual rdf:about="&stac;Anonymity">
        <rdf:type rdf:resource="&iotsec;SecurityProperty"/>
        <rdfs:label xml:lang="en">Anonymity</rdfs:label>
        <rdfs:comment xml:lang="en">Anonimity hides the source of a packet during communication.</rdfs:comment>
        <rdfs:comment xml:lang="en">Anonymity protects user identity, making it hard to track the whereabouts of a certain user.</rdfs:comment>
        <owl:sameAs rdf:resource="&denker;Anonymity"/>
        <owl:sameAs rdf:resource="&herzog;Anonymity"/>
    </owl:NamedIndividual>
    


    <!-- http://securitytoolbox.appspot.com/stac#AnonymityKeyAK -->

    <owl:NamedIndividual rdf:about="&stac;AnonymityKeyAK">
        <rdf:type rdf:resource="&iotsec;UMTSArchitectureComponent"/>
        <rdfs:label xml:lang="en">Anonymity Key (AK)</rdfs:label>
        <rdfs:comment xml:lang="en"></rdfs:comment>
    </owl:NamedIndividual>
    


    <!-- http://securitytoolbox.appspot.com/stac#ApplicationLayer -->

    <owl:NamedIndividual rdf:about="&stac;ApplicationLayer">
        <rdf:type rdf:resource="&iotsec;OSIModelLayer"/>
        <rdfs:label xml:lang="en">Application Layer</rdfs:label>
        <rdfs:comment xml:lang="en">The application layer is the layer closest to end users, which means bot the ISO application layer and the users interact directly with the software applications.</rdfs:comment>
    </owl:NamedIndividual>
    


    <!-- http://securitytoolbox.appspot.com/stac#Auc -->

    <owl:NamedIndividual rdf:about="&stac;Auc">
        <rdf:type rdf:resource="&stac;GSMArchitectureComponent"/>
        <rdfs:label xml:lang="en">Authentication Center (AuC)</rdfs:label>
        <rdfs:comment xml:lang="en">AuC includes information for identifying authorized users of the GSM or GPRS network and thus prevent unauthorized use of the network.</rdfs:comment>
        <dcterms:hasPart rdf:resource="&iotsec;A3"/>
        <dcterms:hasPart rdf:resource="&iotsec;A8"/>
    </owl:NamedIndividual>
    


    <!-- http://securitytoolbox.appspot.com/stac#Authentication -->

    <owl:NamedIndividual rdf:about="&stac;Authentication">
        <rdf:type rdf:resource="&iotsec;SecurityProperty"/>
        <rdfs:label xml:lang="en">Authentication</rdfs:label>
        <rdfs:comment xml:lang="en">Authentication prevents unauthorized access to the network.</rdfs:comment>
        <owl:sameAs rdf:resource="&securitysw;Authentication"/>
        <owl:sameAs rdf:resource="&denker;Authentication"/>
        <owl:sameAs rdf:resource="&herzog;Authentication"/>
    </owl:NamedIndividual>
    


    <!-- http://securitytoolbox.appspot.com/stac#AuthenticationTokenAUTN -->

    <owl:NamedIndividual rdf:about="&stac;AuthenticationTokenAUTN">
        <rdf:type rdf:resource="&iotsec;UMTSArchitectureComponent"/>
        <rdfs:label xml:lang="en">Authentication Token (AUTN)</rdfs:label>
        <rdfs:comment xml:lang="en">It is verified bu the user to authenticate the network.</rdfs:comment>
    </owl:NamedIndividual>
    


    <!-- http://securitytoolbox.appspot.com/stac#AuthenticationVector -->

    <owl:NamedIndividual rdf:about="&stac;AuthenticationVector">
        <rdf:type rdf:resource="&iotsec;UMTSArchitectureComponent"/>
        <rdfs:label xml:lang="en">Authentication Vector (AV)</rdfs:label>
        <rdfs:comment xml:lang="en"></rdfs:comment>
        <dcterms:hasPart rdf:resource="&iotsec;f1"/>
        <dcterms:hasPart rdf:resource="&iotsec;f2"/>
        <dcterms:hasPart rdf:resource="&iotsec;f3"/>
        <dcterms:hasPart rdf:resource="&iotsec;f4"/>
        <dcterms:hasPart rdf:resource="&iotsec;f5"/>
    </owl:NamedIndividual>
    


    <!-- http://securitytoolbox.appspot.com/stac#Authorization -->

    <owl:NamedIndividual rdf:about="&stac;Authorization">
        <rdf:type rdf:resource="&iotsec;SecurityProperty"/>
        <rdfs:label xml:lang="en">Authorization</rdfs:label>
        <rdfs:comment xml:lang="en">Only authorized persons can access to network services or resources.</rdfs:comment>
        <owl:sameAs rdf:resource="&denker;Authorization"/>
        <owl:sameAs rdf:resource="&herzog;Authorisation"/>
    </owl:NamedIndividual>
    


    <!-- http://securitytoolbox.appspot.com/stac#Availability -->

    <owl:NamedIndividual rdf:about="&stac;Availability">
        <rdf:type rdf:resource="&iotsec;SecurityProperty"/>
        <rdfs:label xml:lang="en">Availability</rdfs:label>
        <rdfs:comment xml:lang="en">Availability ensures that services and information can be accessed at the time when they are required. Data availability ensures that the network is alive and that data are accessible.</rdfs:comment>
        <owl:sameAs rdf:resource="&securitysw;Availability"/>
        <owl:sameAs rdf:resource="&herzog;Availability"/>
    </owl:NamedIndividual>
    


    <!-- http://securitytoolbox.appspot.com/stac#Avast -->

    <owl:NamedIndividual rdf:about="&stac;Avast">
        <rdf:type rdf:resource="&iotsec;Antivirus"/>
        <rdfs:label xml:lang="en">Avast</rdfs:label>
        <rdfs:comment xml:lang="en"></rdfs:comment>
        <iotsec:hasFeature rdf:resource="&iotsec;Free"/>
        <iotsec:satisfies rdf:resource="&iotsec;Integrity"/>
    </owl:NamedIndividual>
    


    <!-- http://securitytoolbox.appspot.com/stac#BLS -->

    <owl:NamedIndividual rdf:about="&stac;BLS">
        <rdf:type rdf:resource="&iotsec;DigitalSignature"/>
        <rdfs:label xml:lang="en">Boneh-Lynn-Shacham (BLS)</rdfs:label>
        <rdfs:comment xml:lang="en"></rdfs:comment>
        <iotsec:satisfies rdf:resource="&iotsec;Authentication"/>
        <iotsec:satisfies rdf:resource="&iotsec;Integrity"/>
        <iotsec:satisfies rdf:resource="&iotsec;NonRepudiation"/>
    </owl:NamedIndividual>
    


    <!-- http://securitytoolbox.appspot.com/stac#BackTrack -->

    <owl:NamedIndividual rdf:about="&stac;BackTrack">
        <rdf:type rdf:resource="&iotsec;NetworkManagementSecurityTool"/>
        <rdfs:label xml:lang="en">BackTrack</rdfs:label>
        <rdfs:comment xml:lang="en">BackTrack is a distribution based on the Debian GNU/Linux distribution aimed at digital forensics and penetration testing use.</rdfs:comment>
    </owl:NamedIndividual>
    


    <!-- http://securitytoolbox.appspot.com/stac#Backdoor -->

    <owl:NamedIndividual rdf:about="&stac;Backdoor">
        <rdf:type rdf:resource="&iotsec;WebAttack"/>
        <rdfs:label xml:lang="en">Backdoor</rdfs:label>
        <rdfs:comment xml:lang="en"></rdfs:comment>
        <iotsec:occursInLayer rdf:resource="&iotsec;ApplicationLayer"/>
    </owl:NamedIndividual>
    


    <!-- http://securitytoolbox.appspot.com/stac#BaseStationController -->

    <owl:NamedIndividual rdf:about="&stac;BaseStationController">
        <rdf:type rdf:resource="&stac;GSMArchitectureComponent"/>
        <rdfs:label xml:lang="en">Base Station Controller (BSC)</rdfs:label>
        <rdfs:comment xml:lang="en">The BSC is responsible for the switching between several BTSs, and for the switching of radio channels.</rdfs:comment>
    </owl:NamedIndividual>
    


    <!-- http://securitytoolbox.appspot.com/stac#BaseStationSubsystem -->

    <owl:NamedIndividual rdf:about="&stac;BaseStationSubsystem">
        <rdf:type rdf:resource="&stac;GSMArchitectureComponent"/>
        <rdfs:label xml:lang="en">Base Station Subsystem (BSS)</rdfs:label>
        <rdfs:comment xml:lang="en">Base Station Subsystem (BSS) controls the radio link with the Mobile Station (MS).</rdfs:comment>
        <dcterms:hasPart rdf:resource="&iotsec;BaseStationController"/>
        <dcterms:hasPart rdf:resource="&iotsec;BaseTransceiverStation"/>
    </owl:NamedIndividual>
    


    <!-- http://securitytoolbox.appspot.com/stac#BaseTransceiverStation -->

    <owl:NamedIndividual rdf:about="&stac;BaseTransceiverStation">
        <rdf:type rdf:resource="&stac;GSMArchitectureComponent"/>
        <rdfs:label xml:lang="en">Base Transceiver Station (BTS)</rdfs:label>
        <rdfs:comment xml:lang="en">The BTS is the radio equipment that transmits and receives information over the air to provide communication with the mobile station.</rdfs:comment>
    </owl:NamedIndividual>
    


    <!-- http://securitytoolbox.appspot.com/stac#BasicServiceSet -->

    <owl:NamedIndividual rdf:about="&stac;BasicServiceSet">
        <rdf:type rdf:resource="&iotsec;WifiArchitectureComponent"/>
        <rdfs:label xml:lang="en">Basic Service Set (BSS)</rdfs:label>
        <rdfs:comment xml:lang="en"></rdfs:comment>
    </owl:NamedIndividual>
    


    <!-- http://securitytoolbox.appspot.com/stac#BitDefender -->

    <owl:NamedIndividual rdf:about="&stac;BitDefender">
        <rdf:type rdf:resource="&iotsec;Antivirus"/>
        <rdf:type rdf:resource="&iotsec;Firewall"/>
        <rdfs:label xml:lang="en">BitDefender</rdfs:label>
        <rdfs:comment xml:lang="en"></rdfs:comment>
        <iotsec:satisfies rdf:resource="&iotsec;Integrity"/>
    </owl:NamedIndividual>
    


    <!-- http://securitytoolbox.appspot.com/stac#BlackHole -->

    <owl:NamedIndividual rdf:about="&stac;BlackHole">
        <rdf:type rdf:resource="&iotsec;ManetAttack"/>
        <rdf:type rdf:resource="&iotsec;SensorAttack"/>
        <rdfs:label xml:lang="en">BlackHole</rdfs:label>
        <rdfs:comment xml:lang="en"></rdfs:comment>
        <iotsec:occursInLayer rdf:resource="&iotsec;NetworkLayer"/>
        <owl:sameAs rdf:resource="&iotsec;Sinkhole"/>
    </owl:NamedIndividual>
    


    <!-- http://securitytoolbox.appspot.com/stac#Blaster -->

    <owl:NamedIndividual rdf:about="&stac;Blaster">
        <rdf:type rdf:resource="&iotsec;DatabaseAttack"/>
        <rdf:type rdf:resource="&iotsec;OperatingSystemAttack"/>
        <rdf:type rdf:resource="&iotsec;Worm"/>
        <rdfs:label xml:lang="en">BlasterWorm worm.</rdfs:label>
        <rdfs:comment xml:lang="en">BlasterWorm is a Windows 2000 vulnerability.</rdfs:comment>
    </owl:NamedIndividual>
    


    <!-- http://securitytoolbox.appspot.com/stac#Blowfish -->

    <owl:NamedIndividual rdf:about="&stac;Blowfish">
        <rdf:type rdf:resource="&iotsec;BlockCipher"/>
        <rdf:type rdf:resource="&iotsec;ManetSecurityMechanism"/>
        <rdfs:label xml:lang="en">Blowfish</rdfs:label>
        <rdfs:comment xml:lang="en"></rdfs:comment>
        <iotsec:satisfies rdf:resource="&iotsec;Confidentiality"/>
    </owl:NamedIndividual>
    


    <!-- http://securitytoolbox.appspot.com/stac#Bluebugging -->

    <owl:NamedIndividual rdf:about="&stac;Bluebugging">
        <rdf:type rdf:resource="&iotsec;BluetoothAttack"/>
        <rdfs:label xml:lang="en">Bluebugging</rdfs:label>
        <rdfs:comment xml:lang="en"></rdfs:comment>
    </owl:NamedIndividual>
    


    <!-- http://securitytoolbox.appspot.com/stac#Bluejacking -->

    <owl:NamedIndividual rdf:about="&stac;Bluejacking">
        <rdf:type rdf:resource="&iotsec;BluetoothAttack"/>
        <rdfs:label xml:lang="en">Bluejacking</rdfs:label>
        <rdfs:comment xml:lang="en">Bluejacking is the sending of either a picture or a message from one user through Bluetooth.</rdfs:comment>
    </owl:NamedIndividual>
    


    <!-- http://securitytoolbox.appspot.com/stac#Bluepot -->

    <owl:NamedIndividual rdf:about="&stac;Bluepot">
        <rdf:type rdf:resource="&iotsec;BluetoothSecurityMechanism"/>
        <rdf:type rdf:resource="&iotsec;Honeypot"/>
        <rdfs:label xml:lang="en">Bluepot</rdfs:label>
        <rdfs:comment xml:lang="en">Bluepot: a honeypot for bluetooth attacks.</rdfs:comment>
    </owl:NamedIndividual>
    


    <!-- http://securitytoolbox.appspot.com/stac#Bluesmack -->

    <owl:NamedIndividual rdf:about="&stac;Bluesmack">
        <rdf:type rdf:resource="&iotsec;BluetoothAttack"/>
        <rdfs:label xml:lang="en">Bluesmack</rdfs:label>
        <rdfs:comment xml:lang="en"></rdfs:comment>
    </owl:NamedIndividual>
    


    <!-- http://securitytoolbox.appspot.com/stac#Bluesnarf -->

    <owl:NamedIndividual rdf:about="&stac;Bluesnarf">
        <rdf:type rdf:resource="&iotsec;BluetoothAttack"/>
        <rdfs:label xml:lang="en">Bluesnarf</rdfs:label>
        <rdfs:comment xml:lang="en"></rdfs:comment>
    </owl:NamedIndividual>
    


    <!-- http://securitytoolbox.appspot.com/stac#Bot -->

    <owl:NamedIndividual rdf:about="&stac;Bot">
        <rdf:type rdf:resource="&iotsec;WebAttack"/>
        <rdfs:label xml:lang="en">Bot</rdfs:label>
        <rdfs:comment xml:lang="en"></rdfs:comment>
        <iotsec:occursInLayer rdf:resource="&iotsec;ApplicationLayer"/>
    </owl:NamedIndividual>
    


    <!-- http://securitytoolbox.appspot.com/stac#Bro -->

    <owl:NamedIndividual rdf:about="&stac;Bro">
        <rdf:type rdf:resource="&iotsec;IDS"/>
        <rdf:type rdf:resource="&iotsec;IPS"/>
        <rdfs:label xml:lang="en">Bro</rdfs:label>
        <rdfs:comment xml:lang="en"></rdfs:comment>
        <iotsec:protectsInLayer rdf:resource="&iotsec;ApplicationLayer"/>
        <iotsec:satisfies rdf:resource="&iotsec;Availability"/>
    </owl:NamedIndividual>
    


    <!-- http://securitytoolbox.appspot.com/stac#BruteForce -->

    <owl:NamedIndividual rdf:about="&stac;BruteForce">
        <rdf:type rdf:resource="&iotsec;DatabaseAttack"/>
        <rdf:type rdf:resource="&iotsec;WebAttack"/>
        <rdfs:label xml:lang="en">Brute Force</rdfs:label>
        <rdfs:comment xml:lang="en"></rdfs:comment>
        <iotsec:hasSecurityMechanism rdf:resource="&stac;AuthenticationMethod"/>
        <iotsec:occursInLayer rdf:resource="&iotsec;ApplicationLayer"/>
        <iotsec:threatens rdf:resource="&iotsec;Authentication"/>
    </owl:NamedIndividual>
    


    <!-- http://securitytoolbox.appspot.com/stac#BufferOverflow -->

    <owl:NamedIndividual rdf:about="&stac;BufferOverflow">
        <rdf:type rdf:resource="&iotsec;WebAttack"/>
        <rdfs:label xml:lang="en">Buffer Overflow</rdfs:label>
        <rdfs:comment xml:lang="en"></rdfs:comment>
        <iotsec:occursInLayer rdf:resource="&iotsec;ApplicationLayer"/>
    </owl:NamedIndividual>
    


    <!-- http://securitytoolbox.appspot.com/stac#ByzantineAttack -->

    <owl:NamedIndividual rdf:about="&stac;ByzantineAttack">
        <rdf:type rdf:resource="&iotsec;ManetAttack"/>
        <rdf:type rdf:resource="&iotsec;MeshAttack"/>
        <rdfs:label xml:lang="en">Byzantine Attack</rdfs:label>
        <rdfs:comment xml:lang="en">It is an invalid operation of the network initiated by malicious nodes where the presence of compromised routing and compromised nodes are not detected.</rdfs:comment>
        <iotsec:occursInLayer rdf:resource="&iotsec;NetworkLayer"/>
    </owl:NamedIndividual>
    


    <!-- http://securitytoolbox.appspot.com/stac#CAML -->

    <owl:NamedIndividual rdf:about="&stac;CAML">
        <rdf:type rdf:resource="&iotsec;ProgrammingLanguageTechnology"/>
        <rdfs:label xml:lang="en">CAML</rdfs:label>
        <rdfs:comment xml:lang="en"></rdfs:comment>
    </owl:NamedIndividual>
    


    <!-- http://securitytoolbox.appspot.com/stac#CAST -->

    <owl:NamedIndividual rdf:about="&stac;CAST">
        <rdf:type rdf:resource="&iotsec;BlockCipher"/>
        <rdf:type rdf:resource="&iotsec;ManetSecurityMechanism"/>
        <rdfs:label xml:lang="en">CAST</rdfs:label>
        <rdfs:comment xml:lang="en"></rdfs:comment>
        <iotsec:satisfies rdf:resource="&iotsec;Confidentiality"/>
    </owl:NamedIndividual>
    


    <!-- http://securitytoolbox.appspot.com/stac#CBC -->

    <owl:NamedIndividual rdf:about="&stac;CBC">
        <rdf:type rdf:resource="&iotsec;ModeOperation"/>
        <rdfs:label xml:lang="en">Cipher-block chaining (CBC)</rdfs:label>
        <rdfs:comment xml:lang="en"></rdfs:comment>
    </owl:NamedIndividual>
    


    <!-- http://securitytoolbox.appspot.com/stac#CBC-MAC -->

    <owl:NamedIndividual rdf:about="&stac;CBC-MAC">
        <rdf:type rdf:resource="&iotsec;MAC"/>
        <rdf:type rdf:resource="&iotsec;ManetSecurityMechanism"/>
        <rdfs:label xml:lang="en">Cipher Bloch Chaining - Message Authentication Code (CBC-MAC)</rdfs:label>
        <rdfs:comment xml:lang="en"></rdfs:comment>
    </owl:NamedIndividual>
    


    <!-- http://securitytoolbox.appspot.com/stac#CCMP -->

    <owl:NamedIndividual rdf:about="&stac;CCMP">
        <rdf:type rdf:resource="&iotsec;WifiArchitectureComponent"/>
        <rdfs:label xml:lang="en">Counter Mode with Cipher Block Chaining Message Authentication Code Protocol (CCMP)</rdfs:label>
        <rdfs:comment xml:lang="en"></rdfs:comment>
        <dcterms:hasPart rdf:resource="&iotsec;AEC"/>
        <dcterms:hasPart rdf:resource="&iotsec;CBC"/>
        <dcterms:hasPart rdf:resource="&iotsec;CTR"/>
        <iotsec:satisfies rdf:resource="&iotsec;Confidentiality"/>
        <iotsec:satisfies rdf:resource="&iotsec;Integrity"/>
        <dcterms:hasPart rdf:resource="&iotsec;MIC"/>
    </owl:NamedIndividual>
    


    <!-- http://securitytoolbox.appspot.com/stac#CFB -->

    <owl:NamedIndividual rdf:about="&stac;CFB">
        <rdf:type rdf:resource="&iotsec;ModeOperation"/>
        <rdfs:label xml:lang="en">Cipher Feedback (CFB)</rdfs:label>
        <rdfs:comment xml:lang="en"></rdfs:comment>
    </owl:NamedIndividual>
    


    <!-- http://securitytoolbox.appspot.com/stac#CHAP -->

    <owl:NamedIndividual rdf:about="&stac;CHAP">
        <rdf:type rdf:resource="&iotsec;ManetSecurityMechanism"/>
        <rdf:type rdf:resource="&iotsec;Protocol"/>
        <rdfs:label xml:lang="en">Challenge-Handshake Authentication Protocol (CHAP)</rdfs:label>
        <rdfs:comment xml:lang="en">Is an authentication protocol that uses a password.</rdfs:comment>
        <iotsec:satisfies rdf:resource="&iotsec;Authentication"/>
        <iotsec:protectsInLayer rdf:resource="&iotsec;LinkLayer"/>
    </owl:NamedIndividual>
    


    <!-- http://securitytoolbox.appspot.com/stac#COMP128 -->

    <owl:NamedIndividual rdf:about="&stac;COMP128">
        <rdf:type rdf:resource="&iotsec;GSMSecurityAlgorithm"/>
        <rdfs:label xml:lang="en">COMP128</rdfs:label>
        <rdfs:comment xml:lang="en">COMP128 is an implementation of the A3 and A8 algorithms defined in the GSM standard.</rdfs:comment>
        <rdfs:comment xml:lang="en">See Paper: Malicious actions against the GPRS technology [Xenakis 2006]</rdfs:comment>
        <iotsec:hasFeature rdf:resource="&iotsec;Deprecated"/>
    </owl:NamedIndividual>
    


    <!-- http://securitytoolbox.appspot.com/stac#CPlusPlus -->

    <owl:NamedIndividual rdf:about="&stac;CPlusPlus">
        <rdf:type rdf:resource="&iotsec;ProgrammingLanguageTechnology"/>
        <rdfs:label xml:lang="en">C++</rdfs:label>
        <rdfs:comment xml:lang="en"></rdfs:comment>
    </owl:NamedIndividual>
    


    <!-- http://securitytoolbox.appspot.com/stac#CRC-32 -->

    <owl:NamedIndividual rdf:about="&stac;CRC-32">
        <rdf:type rdf:resource="&iotsec;ChecksumAlgorithm"/>
        <rdf:type rdf:resource="&iotsec;ManetSecurityMechanism"/>
        <rdfs:label xml:lang="en">CRC-32</rdfs:label>
        <rdfs:comment xml:lang="en"></rdfs:comment>
        <iotsec:satisfies rdf:resource="&iotsec;Integrity"/>
    </owl:NamedIndividual>
    


    <!-- http://securitytoolbox.appspot.com/stac#CSRF -->

    <owl:NamedIndividual rdf:about="&stac;CSRF">
        <rdf:type rdf:resource="&iotsec;WebAttack"/>
        <rdfs:label xml:lang="en">Cross Site Request Forgery (CSRF)</rdfs:label>
        <rdfs:comment xml:lang="en"></rdfs:comment>
        <iotsec:occursInLayer rdf:resource="&iotsec;ApplicationLayer"/>
    </owl:NamedIndividual>
    


    <!-- http://securitytoolbox.appspot.com/stac#CTR -->

    <owl:NamedIndividual rdf:about="&stac;CTR">
        <rdf:type rdf:resource="&iotsec;ModeOperation"/>
        <rdfs:label xml:lang="en">Counter</rdfs:label>
        <rdfs:comment xml:lang="en"></rdfs:comment>
    </owl:NamedIndividual>
    


    <!-- http://securitytoolbox.appspot.com/stac#ChosenCiphertext -->

    <owl:NamedIndividual rdf:about="&stac;ChosenCiphertext">
        <rdf:type rdf:resource="&iotsec;Threat"/>
        <rdfs:label xml:lang="en">Chosen Ciphertext</rdfs:label>
        <rdfs:comment xml:lang="en">The attacker can decipher chosen ciphertexts before the challenge.</rdfs:comment>
    </owl:NamedIndividual>
    


    <!-- http://securitytoolbox.appspot.com/stac#ChosenPlaintext -->

    <owl:NamedIndividual rdf:about="&stac;ChosenPlaintext">
        <rdf:type rdf:resource="&iotsec;Threat"/>
        <rdfs:label xml:lang="en">Chosen Plaintext</rdfs:label>
        <rdfs:comment xml:lang="en">The attacker can get ciphers of chosen plaintexts but only before the plaintext to attack (called challenge).</rdfs:comment>
    </owl:NamedIndividual>
    


    <!-- http://securitytoolbox.appspot.com/stac#CipherKeyCK -->

    <owl:NamedIndividual rdf:about="&stac;CipherKeyCK">
        <rdf:type rdf:resource="&iotsec;UMTSArchitectureComponent"/>
        <rdfs:label xml:lang="en">Cipher Key (CK)</rdfs:label>
        <rdfs:comment xml:lang="en"></rdfs:comment>
    </owl:NamedIndividual>
    


    <!-- http://securitytoolbox.appspot.com/stac#CiphertextOnly -->

    <owl:NamedIndividual rdf:about="&stac;CiphertextOnly">
        <rdf:type rdf:resource="&iotsec;Threat"/>
        <rdfs:label xml:lang="en">Ciphertext Only</rdfs:label>
        <rdfs:comment xml:lang="en">The attacker only knows the ciphertext.</rdfs:comment>
    </owl:NamedIndividual>
    


    <!-- http://securitytoolbox.appspot.com/stac#CircuitSwitched -->

    <owl:NamedIndividual rdf:about="&stac;CircuitSwitched">
        <rdf:type rdf:resource="&iotsec;UMTSArchitectureComponent"/>
        <rdfs:label xml:lang="en">Circuit Switched</rdfs:label>
        <rdfs:comment xml:lang="en"></rdfs:comment>
        <dcterms:hasPart rdf:resource="&iotsec;MSC"/>
        <dcterms:hasPart rdf:resource="&iotsec;VLR"/>
    </owl:NamedIndividual>
    


    <!-- http://securitytoolbox.appspot.com/stac#ClientPuzzle -->

    <owl:NamedIndividual rdf:about="&stac;ClientPuzzle">
        <rdf:type rdf:resource="&iotsec;SensorSecurityMechanism"/>
        <rdfs:label xml:lang="en">Client Puzzle</rdfs:label>
        <rdfs:comment xml:lang="en"></rdfs:comment>
        <iotsec:protectsInLayer rdf:resource="&iotsec;TransportLayer"/>
    </owl:NamedIndividual>
    


    <!-- http://securitytoolbox.appspot.com/stac#ClusterKey -->

    <owl:NamedIndividual rdf:about="&stac;ClusterKey">
        <rdf:type rdf:resource="&iotsec;SymmetricSensorKey"/>
        <rdfs:label xml:lang="en">Cluster Key</rdfs:label>
        <rdfs:comment xml:lang="en">A cluster key is a key shared by a node and all its neighbors, and it is mainly used for securing locally broadcast messages, e.g., routing control information, or securing sensor messages which can benefit from passive participation.</rdfs:comment>
    </owl:NamedIndividual>
    


    <!-- http://securitytoolbox.appspot.com/stac#Collision -->

    <owl:NamedIndividual rdf:about="&stac;Collision">
        <rdf:type rdf:resource="&iotsec;RfidAttack"/>
        <rdf:type rdf:resource="&iotsec;SensorAttack"/>
        <rdf:type rdf:resource="&iotsec;UMTSAttack"/>
        <rdfs:label xml:lang="en">Collision</rdfs:label>
        <rdfs:comment xml:lang="en">An attacker may intentionally violate the communication protocol and continually transmit messages in an attempt to generate collisions ans also deplete a sensor node by forcing too many retransmissions. When two nodes transmit packets of data on the same frequency channel, it can lead to discard of the affected data packet for re-transmission.</rdfs:comment>
        <rdfs:comment xml:lang="en">See Paper: Survey of Security and Privacy Issues of Internet of Things [Borgohain et al. 2015], Paper: MILENAGE: An example of good UMTS Security [Massari 2009?]</rdfs:comment>
        <iotsec:hasSecurityMechanism rdf:resource="&iotsec;CollisionDetection"/>
        <iotsec:hasSecurityMechanism rdf:resource="&iotsec;ErrorCorrectingCode"/>
        <iotsec:occursInLayer rdf:resource="&iotsec;LinkLayer"/>
    </owl:NamedIndividual>
    


    <!-- http://securitytoolbox.appspot.com/stac#CollisionDetection -->

    <owl:NamedIndividual rdf:about="&stac;CollisionDetection">
        <rdf:type rdf:resource="&iotsec;SensorSecurityMechanism"/>
        <rdfs:label xml:lang="en">Collision Detection</rdfs:label>
        <rdfs:comment xml:lang="en"></rdfs:comment>
        <iotsec:protectsInLayer rdf:resource="&iotsec;LinkLayer"/>
    </owl:NamedIndividual>
    


    <!-- http://securitytoolbox.appspot.com/stac#CommonElement -->

    <owl:NamedIndividual rdf:about="&stac;CommonElement">
        <rdf:type rdf:resource="&iotsec;UMTSArchitectureComponent"/>
        <rdfs:label xml:lang="en">Common Element</rdfs:label>
        <rdfs:comment xml:lang="en"></rdfs:comment>
        <dcterms:hasPart rdf:resource="&iotsec;AuC"/>
        <dcterms:hasPart rdf:resource="&iotsec;EIR"/>
        <dcterms:hasPart rdf:resource="&iotsec;HLR"/>
    </owl:NamedIndividual>
    


    <!-- http://securitytoolbox.appspot.com/stac#Comodo -->

    <owl:NamedIndividual rdf:about="&stac;Comodo">
        <rdf:type rdf:resource="&iotsec;Firewall"/>
        <rdfs:label xml:lang="en">ZoneAlarm</rdfs:label>
        <rdfs:comment xml:lang="en"></rdfs:comment>
        <iotsec:satisfies rdf:resource="&iotsec;AccessControl"/>
        <iotsec:hasFeature rdf:resource="&iotsec;Free"/>
    </owl:NamedIndividual>
    


    <!-- http://securitytoolbox.appspot.com/stac#Confidentiality -->

    <owl:NamedIndividual rdf:about="&stac;Confidentiality">
        <rdf:type rdf:resource="&iotsec;SecurityProperty"/>
        <rdfs:label xml:lang="en">Confidentiality/Privacy </rdfs:label>
        <rdfs:comment xml:lang="en">Confidentiality means that only destined user must be able to read data. </rdfs:comment>
        <owl:sameAs rdf:resource="&securitysw;Confidentiality"/>
        <owl:sameAs rdf:resource="&denker;Confidentiality"/>
        <owl:sameAs rdf:resource="&herzog;Confidentiality"/>
    </owl:NamedIndividual>
    


    <!-- http://securitytoolbox.appspot.com/stac#Contiki -->

    <owl:NamedIndividual rdf:about="&stac;Contiki">
        <rdf:type rdf:resource="&iotsec;OperatingSystemTechnology"/>
        <rdf:type rdf:resource="&iotsec;SensorTechnology"/>
        <rdfs:label xml:lang="en">Contiki</rdfs:label>
        <rdfs:comment xml:lang="en">Contiki is an operating system for sensors.</rdfs:comment>
    </owl:NamedIndividual>
    


    <!-- http://securitytoolbox.appspot.com/stac#ContikiSec -->

    <owl:NamedIndividual rdf:about="&stac;ContikiSec">
        <rdf:type rdf:resource="&iotsec;SensorSecurityProtocol"/>
        <rdfs:label xml:lang="en">ContikiSec</rdfs:label>
        <rdfs:comment xml:lang="en"></rdfs:comment>
        <rdfs:comment xml:lang="en">See Paper ContikiSec: a secure network layer for wireless sensor networks under the contiki operating system [Casado et al. 2009]</rdfs:comment>
        <dcterms:hasPart rdf:resource="&iotsec;AES"/>
        <iotsec:satisfies rdf:resource="&iotsec;Authentication"/>
        <dcterms:hasPart rdf:resource="&iotsec;CBC"/>
        <iotsec:satisfies rdf:resource="&iotsec;Confidentiality"/>
        <iotsec:satisfies rdf:resource="&iotsec;Integrity"/>
    </owl:NamedIndividual>
    


    <!-- http://securitytoolbox.appspot.com/stac#CoreNetwork -->

    <owl:NamedIndividual rdf:about="&stac;CoreNetwork">
        <rdf:type rdf:resource="&iotsec;UMTSArchitectureComponent"/>
        <rdfs:label xml:lang="en">Core Network (CN)</rdfs:label>
        <rdfs:comment xml:lang="en">The CN provides switching, routing and transit for user traffic and contains the databases and network management.</rdfs:comment>
        <dcterms:hasPart rdf:resource="&iotsec;CircuitSwitched"/>
        <dcterms:hasPart rdf:resource="&iotsec;CommonElement"/>
        <dcterms:hasPart rdf:resource="&iotsec;PacketSwitched"/>
    </owl:NamedIndividual>
    


    <!-- http://securitytoolbox.appspot.com/stac#DB2 -->

    <owl:NamedIndividual rdf:about="&stac;DB2">
        <rdf:type rdf:resource="&iotsec;DatabaseTechnology"/>
        <rdfs:label xml:lang="en">DB2</rdfs:label>
        <rdfs:comment xml:lang="en"></rdfs:comment>
    </owl:NamedIndividual>
    


    <!-- http://securitytoolbox.appspot.com/stac#DES -->

    <owl:NamedIndividual rdf:about="&stac;DES">
        <rdf:type rdf:resource="&iotsec;BlockCipher"/>
        <rdf:type rdf:resource="&iotsec;ManetSecurityMechanism"/>
        <rdfs:label xml:lang="en">DES</rdfs:label>
        <rdfs:comment xml:lang="en"></rdfs:comment>
        <iotsec:satisfies rdf:resource="&iotsec;Confidentiality"/>
        <iotsec:hasFeature rdf:resource="&iotsec;Deprecated"/>
        <iotsec:isReplacedBy rdf:resource="&iotsec;TripleDES"/>
    </owl:NamedIndividual>
    


    <!-- http://securitytoolbox.appspot.com/stac#DMZ -->

    <owl:NamedIndividual rdf:about="&stac;DMZ">
        <rdf:type rdf:resource="&iotsec;NetworkManagementSecurityMechanism"/>
        <rdfs:label xml:lang="en">Demilitarized zone (DMZ)</rdfs:label>
        <rdfs:comment xml:lang="en"></rdfs:comment>
        <iotsec:protectsInLayer rdf:resource="&iotsec;ApplicationLayer"/>
    </owl:NamedIndividual>
    


    <!-- http://securitytoolbox.appspot.com/stac#DNSCachePoisoning -->

    <owl:NamedIndividual rdf:about="&stac;DNSCachePoisoning">
        <rdf:type rdf:resource="&iotsec;Threat"/>
        <rdfs:label xml:lang="en">DNS Cache Poisoning</rdfs:label>
        <rdfs:comment xml:lang="en"></rdfs:comment>
    </owl:NamedIndividual>
    


    <!-- http://securitytoolbox.appspot.com/stac#DNSFlood -->

    <owl:NamedIndividual rdf:about="&stac;DNSFlood">
        <rdf:type rdf:resource="&iotsec;Threat"/>
        <rdfs:label xml:lang="en">DNS Flood</rdfs:label>
        <rdfs:comment xml:lang="en"></rdfs:comment>
    </owl:NamedIndividual>
    


    <!-- http://securitytoolbox.appspot.com/stac#DSA -->

    <owl:NamedIndividual rdf:about="&stac;DSA">
        <rdf:type rdf:resource="&iotsec;DigitalSignature"/>
        <rdfs:label xml:lang="en">Digital Sinature Algorithm (DSA)</rdfs:label>
        <rdfs:comment xml:lang="en"></rdfs:comment>
        <iotsec:satisfies rdf:resource="&iotsec;Authentication"/>
        <iotsec:satisfies rdf:resource="&iotsec;Integrity"/>
        <iotsec:satisfies rdf:resource="&iotsec;NonRepudiation"/>
    </owl:NamedIndividual>
    


    <!-- http://securitytoolbox.appspot.com/stac#DSA_Mesh -->

    <owl:NamedIndividual rdf:about="&stac;DSA_Mesh">
        <rdf:type rdf:resource="&iotsec;MeshSecurityMechanism"/>
        <rdfs:label xml:lang="en">DSA-Mesh</rdfs:label>
        <rdfs:comment xml:lang="en"></rdfs:comment>
        <iotsec:satisfies rdf:resource="&iotsec;AccessControl"/>
        <iotsec:satisfies rdf:resource="&iotsec;Confidentiality"/>
        <iotsec:satisfies rdf:resource="&iotsec;Integrity"/>
    </owl:NamedIndividual>
    


    <!-- http://securitytoolbox.appspot.com/stac#DSS -->

    <owl:NamedIndividual rdf:about="&stac;DSS">
        <rdf:type rdf:resource="&iotsec;DigitalSignature"/>
        <rdfs:label xml:lang="en">Digital Sinature Standard (DSS)</rdfs:label>
        <rdfs:comment xml:lang="en"></rdfs:comment>
        <iotsec:satisfies rdf:resource="&iotsec;Authentication"/>
        <iotsec:satisfies rdf:resource="&iotsec;Integrity"/>
        <iotsec:satisfies rdf:resource="&iotsec;NonRepudiation"/>
    </owl:NamedIndividual>
    


    <!-- http://securitytoolbox.appspot.com/stac#DataFreshness -->

    <owl:NamedIndividual rdf:about="&stac;DataFreshness">
        <rdf:type rdf:resource="&iotsec;SecurityProperty"/>
        <rdfs:label xml:lang="en">Data Freshness, Replay Protection</rdfs:label>
        <rdfs:comment xml:lang="en">Data freshness suggests that the data is recent, and it ensures that no old messages have been replayed.</rdfs:comment>
    </owl:NamedIndividual>
    


    <!-- http://securitytoolbox.appspot.com/stac#Deprecated -->

    <owl:NamedIndividual rdf:about="&stac;Deprecated">
        <rdf:type rdf:resource="&iotsec;NegativeFeature"/>
        <rdfs:label xml:lang="en">Deprecated</rdfs:label>
        <rdfs:comment xml:lang="en">A security algorithm is deprecated when it has been cracked.</rdfs:comment>
    </owl:NamedIndividual>
    


    <!-- http://securitytoolbox.appspot.com/stac#Desynchronization -->

    <owl:NamedIndividual rdf:about="&stac;Desynchronization">
        <rdf:type rdf:resource="&iotsec;SensorAttack"/>
        <rdfs:label xml:lang="en">Desynchronization</rdfs:label>
        <rdfs:comment xml:lang="en">In de-synchronized attack, attacker may disrupts the established link between two legitimate two ends nodes by re-synchronizing their transmission.</rdfs:comment>
        <rdfs:comment xml:lang="en">See Paper: Survey of Security and Privacy Issues of Internet of Things [Borgohain et al. 2015]</rdfs:comment>
        <iotsec:threatens rdf:resource="&iotsec;Authentication"/>
        <iotsec:hasSecurityMechanism rdf:resource="&iotsec;ClientPuzzle"/>
        <iotsec:occursInLayer rdf:resource="&iotsec;TransportLayer"/>
    </owl:NamedIndividual>
    


    <!-- http://securitytoolbox.appspot.com/stac#Diameter -->

    <owl:NamedIndividual rdf:about="&stac;Diameter">
        <rdf:type rdf:resource="&iotsec;AuthenticationServer"/>
        <rdf:type rdf:resource="&iotsec;WifiSecurityMechanism"/>
        <rdfs:label xml:lang="en">Diameter</rdfs:label>
        <rdfs:comment xml:lang="en">Diameter is evolving to improve RADIUS to provide better security.</rdfs:comment>
        <iotsec:satisfies rdf:resource="&iotsec;Authentication"/>
    </owl:NamedIndividual>
    


    <!-- http://securitytoolbox.appspot.com/stac#Dictionnary -->

    <owl:NamedIndividual rdf:about="&stac;Dictionnary">
        <rdf:type rdf:resource="&iotsec;WebAttack"/>
        <rdfs:label xml:lang="en">Dictionnary Attack</rdfs:label>
        <rdfs:comment xml:lang="en"></rdfs:comment>
        <iotsec:occursInLayer rdf:resource="&iotsec;ApplicationLayer"/>
    </owl:NamedIndividual>
    


    <!-- http://securitytoolbox.appspot.com/stac#DiffieHellman -->

    <owl:NamedIndividual rdf:about="&stac;DiffieHellman">
        <rdf:type rdf:resource="&iotsec;KeyManagement"/>
        <rdfs:label xml:lang="en">Diffie Hellman</rdfs:label>
        <rdfs:comment xml:lang="en"></rdfs:comment>
        <iotsec:satisfies rdf:resource="&iotsec;Authentication"/>
    </owl:NamedIndividual>
    


    <!-- http://securitytoolbox.appspot.com/stac#DirectionalAntenna -->

    <owl:NamedIndividual rdf:about="&stac;DirectionalAntenna">
        <rdf:type rdf:resource="&iotsec;M2MSecurityMechanism"/>
        <rdf:type rdf:resource="&iotsec;SensorSecurityMechanism"/>
        <rdfs:label xml:lang="en">Directional Antenna</rdfs:label>
        <rdfs:comment xml:lang="en"></rdfs:comment>
    </owl:NamedIndividual>
    


    <!-- http://securitytoolbox.appspot.com/stac#DoS -->

    <owl:NamedIndividual rdf:about="&stac;DoS">
        <rdf:type rdf:resource="&iotsec;DatabaseAttack"/>
        <rdf:type rdf:resource="&iotsec;GPRSAttack"/>
        <rdf:type rdf:resource="&iotsec;ManetAttack"/>
        <rdf:type rdf:resource="&iotsec;NetworkManagementAttack"/>
        <rdf:type rdf:resource="&iotsec;RfidAttack"/>
        <rdf:type rdf:resource="&iotsec;SensorAttack"/>
        <rdf:type rdf:resource="&iotsec;Threat"/>
        <rdf:type rdf:resource="&iotsec;UMTSAttack"/>
        <rdf:type rdf:resource="&iotsec;WimaxAttack"/>
        <rdfs:label xml:lang="en">Denial of Service (DoS)</rdfs:label>
        <rdfs:comment xml:lang="en">A DoS attack is any event that diminishes or eliminates a network&apos;s capacity to perform its expected function. Paper: Denial of Service in Sensor Networks  [Wood et al. 2002]. A DoS threats are harmful to every application. The DoS attack tries to exhaust the resources available to the victim node, by sending extra unnecessary packets and thus prevents legitimate network users from accessing services or resources to which they are entitled.</rdfs:comment>
        <rdfs:comment xml:lang="en">See Paper: UMTS Security: Security in Core Network and UTRAN [Abid et al. 2002]. See Paper: Malicious actions against the GPRS technology [Xenakis 2006], Paper: Survey of Security and Privacy Issues of Internet of Things [Borgohain et al. 2015]</rdfs:comment>
        <iotsec:isVulnerabilityOf rdf:resource="&stac;Technology"/>
        <iotsec:occursInLayer rdf:resource="&iotsec;ApplicationLayer"/>
        <iotsec:hasSecurityMechanism rdf:resource="&iotsec;ClientPuzzle"/>
        <iotsec:hasSecurityMechanism rdf:resource="&iotsec;IPS"/>
        <iotsec:occursInLayer rdf:resource="&iotsec;NetworkLayer"/>
        <iotsec:hasSecurityMechanism rdf:resource="&iotsec;PANA"/>
        <iotsec:occursInLayer rdf:resource="&iotsec;TransportLayer"/>
    </owl:NamedIndividual>
    


    <!-- http://securitytoolbox.appspot.com/stac#DotNet -->

    <owl:NamedIndividual rdf:about="&stac;DotNet">
        <rdf:type rdf:resource="&iotsec;ProgrammingLanguageTechnology"/>
        <rdfs:label xml:lang="en">.Net</rdfs:label>
        <rdfs:comment xml:lang="en"></rdfs:comment>
    </owl:NamedIndividual>
    


    <!-- http://securitytoolbox.appspot.com/stac#E0 -->

    <owl:NamedIndividual rdf:about="&stac;E0">
        <rdf:type rdf:resource="&iotsec;BluetoothSecurityAlgorithm"/>
        <rdf:type rdf:resource="&iotsec;StreamCipher"/>
        <rdfs:label xml:lang="en">E0</rdfs:label>
        <rdfs:comment xml:lang="en">E0 is a stream cipher used in the Bluetooth protocol.</rdfs:comment>
    </owl:NamedIndividual>
    


    <!-- http://securitytoolbox.appspot.com/stac#EAP -->

    <owl:NamedIndividual rdf:about="&stac;EAP">
        <rdf:type rdf:resource="&iotsec;WifiSecurityProtocol"/>
        <rdf:type rdf:resource="&iotsec;WimaxSecurityProtocol"/>
        <rdfs:label xml:lang="en">EAP (Extensible Authentication Protocol)</rdfs:label>
        <rdfs:comment xml:lang="en">EAP is a generic authentication protocol used in wireless networks.</rdfs:comment>
        <iotsec:satisfies rdf:resource="&iotsec;Authentication"/>
    </owl:NamedIndividual>
    


    <!-- http://securitytoolbox.appspot.com/stac#EAPOL -->

    <owl:NamedIndividual rdf:about="&stac;EAPOL">
        <rdf:type rdf:resource="&iotsec;WifiSecurityProtocol"/>
        <rdfs:label xml:lang="en">EAP Over LAN (EAPOL)</rdfs:label>
        <rdfs:comment xml:lang="en"></rdfs:comment>
        <iotsec:satisfies rdf:resource="&iotsec;Authentication"/>
    </owl:NamedIndividual>
    


    <!-- http://securitytoolbox.appspot.com/stac#EAP_AKA -->

    <owl:NamedIndividual rdf:about="&stac;EAP_AKA">
        <rdf:type rdf:resource="&iotsec;UMTSSecurityProtocol"/>
        <rdf:type rdf:resource="&iotsec;WimaxSecurityProtocol"/>
        <rdfs:label xml:lang="en">EAP-AKA (EAP-Authentication and Key Agreement)</rdfs:label>
        <rdfs:comment xml:lang="en"></rdfs:comment>
        <iotsec:satisfies rdf:resource="&iotsec;Authentication"/>
    </owl:NamedIndividual>
    


    <!-- http://securitytoolbox.appspot.com/stac#EAP_MD5 -->

    <owl:NamedIndividual rdf:about="&stac;EAP_MD5">
        <rdf:type rdf:resource="&iotsec;WifiSecurityProtocol"/>
        <rdfs:label xml:lang="en">EAP-MD5 (EAP-Authentication and Key Agreement)</rdfs:label>
        <rdfs:comment xml:lang="en"></rdfs:comment>
        <iotsec:satisfies rdf:resource="&iotsec;Authentication"/>
    </owl:NamedIndividual>
    


    <!-- http://securitytoolbox.appspot.com/stac#EAP_SIM -->

    <owl:NamedIndividual rdf:about="&stac;EAP_SIM">
        <rdf:type rdf:resource="&iotsec;GSMSecurityProtocol"/>
        <rdfs:label xml:lang="en">EAP-SIM (Extensible Authentication Protocol - Subscriber Identity Module)</rdfs:label>
        <rdfs:comment xml:lang="en"></rdfs:comment>
        <iotsec:satisfies rdf:resource="&iotsec;Authentication"/>
    </owl:NamedIndividual>
    


    <!-- http://securitytoolbox.appspot.com/stac#EAP_TLS -->

    <owl:NamedIndividual rdf:about="&stac;EAP_TLS">
        <rdf:type rdf:resource="&iotsec;WifiSecurityProtocol"/>
        <rdf:type rdf:resource="&iotsec;WimaxSecurityProtocol"/>
        <rdfs:label xml:lang="en">EAP-TLS (Extensible Authentication Protocol - Transport Layer Security)</rdfs:label>
        <rdfs:comment xml:lang="en"></rdfs:comment>
        <iotsec:satisfies rdf:resource="&iotsec;Authentication"/>
    </owl:NamedIndividual>
    


    <!-- http://securitytoolbox.appspot.com/stac#EAP_TTLS -->

    <owl:NamedIndividual rdf:about="&stac;EAP_TTLS">
        <rdf:type rdf:resource="&iotsec;WifiSecurityProtocol"/>
        <rdf:type rdf:resource="&iotsec;WimaxSecurityProtocol"/>
        <rdfs:label xml:lang="en">EAP-TTLS (EAP-Tunelled-TLS)</rdfs:label>
        <rdfs:comment xml:lang="en">EAP-TTLS is used to support establishment of secure connections in a roaming environment and protection of user credentials.</rdfs:comment>
        <iotsec:hasFeature rdf:resource="&stac;Flexible"/>
        <iotsec:satisfies rdf:resource="&iotsec;Authentication"/>
    </owl:NamedIndividual>
    


    <!-- http://securitytoolbox.appspot.com/stac#ECB -->

    <owl:NamedIndividual rdf:about="&stac;ECB">
        <rdf:type rdf:resource="&iotsec;ModeOperation"/>
        <rdfs:label xml:lang="en">Electonic Code Book (ECB)</rdfs:label>
        <rdfs:comment xml:lang="en"></rdfs:comment>
    </owl:NamedIndividual>
    


    <!-- http://securitytoolbox.appspot.com/stac#ECC -->

    <owl:NamedIndividual rdf:about="&stac;ECC">
        <rdf:type rdf:resource="&iotsec;AsymmetricAlgorithm"/>
        <rdf:type rdf:resource="&iotsec;KeyManagement"/>
        <rdf:type rdf:resource="&iotsec;ManetSecurityMechanism"/>
        <rdfs:label xml:lang="en">Elliptic Curve Cryptography (ECC)</rdfs:label>
        <rdfs:comment xml:lang="en">Elliptic curve cryptography (ECC) is an approach to public-key cryptography based on the algebraic structure of elliptic curves. Because the RSA algorithm is rather inefficient in its use of key length, ECC has been proposed.</rdfs:comment>
        <iotsec:satisfies rdf:resource="&iotsec;Authentication"/>
        <iotsec:satisfies rdf:resource="&iotsec;Confidentiality"/>
    </owl:NamedIndividual>
    


    <!-- http://securitytoolbox.appspot.com/stac#ECDDSA -->

    <owl:NamedIndividual rdf:about="&stac;ECDDSA">
        <rdf:type rdf:resource="&iotsec;DigitalSignature"/>
        <rdfs:label xml:lang="en">Elliptic Curve Digital Sinature Algorithm (ECDSA)</rdfs:label>
        <rdfs:comment xml:lang="en">ECDSA is a variant of the DSA which uses ECC.</rdfs:comment>
        <iotsec:satisfies rdf:resource="&iotsec;Authentication"/>
        <iotsec:satisfies rdf:resource="&iotsec;Integrity"/>
        <iotsec:satisfies rdf:resource="&iotsec;NonRepudiation"/>
    </owl:NamedIndividual>
    


    <!-- http://securitytoolbox.appspot.com/stac#EIR -->

    <owl:NamedIndividual rdf:about="&stac;EIR">
        <rdf:type rdf:resource="&stac;GSMArchitectureComponent"/>
        <rdfs:label xml:lang="en">Equipment Identity Register (EIR)</rdfs:label>
        <rdfs:comment xml:lang="en">The EIR contains a list of valid mobile equipment.</rdfs:comment>
    </owl:NamedIndividual>
    


    <!-- http://securitytoolbox.appspot.com/stac#EPC -->

    <owl:NamedIndividual rdf:about="&stac;EPC">
        <rdf:type rdf:resource="&iotsec;LTEArchitectureComponent"/>
        <rdfs:label xml:lang="en">Evolved Packet Core (EPC)</rdfs:label>
        <rdfs:comment xml:lang="en"></rdfs:comment>
    </owl:NamedIndividual>
    


    <!-- http://securitytoolbox.appspot.com/stac#EUTRAN -->

    <owl:NamedIndividual rdf:about="&stac;EUTRAN">
        <rdf:type rdf:resource="&iotsec;LTEArchitectureComponent"/>
        <rdfs:label xml:lang="en">Evolved UMTS Terresrial Radio Access Network (E-UTRAN)</rdfs:label>
        <rdfs:comment xml:lang="en"></rdfs:comment>
    </owl:NamedIndividual>
    


    <!-- http://securitytoolbox.appspot.com/stac#Eavesdropping -->

    <owl:NamedIndividual rdf:about="&stac;Eavesdropping">
        <rdf:type rdf:resource="&iotsec;M2MAttack"/>
        <rdf:type rdf:resource="&iotsec;ManetAttack"/>
        <rdf:type rdf:resource="&iotsec;MeshAttack"/>
        <rdf:type rdf:resource="&iotsec;RfidAttack"/>
        <rdf:type rdf:resource="&iotsec;Threat"/>
        <rdf:type rdf:resource="&iotsec;UMTSAttack"/>
        <rdf:type rdf:resource="&iotsec;WifiAttack"/>
        <rdf:type rdf:resource="&iotsec;WimaxAttack"/>
        <rdfs:label xml:lang="en">Eavesdropping</rdfs:label>
        <rdfs:comment xml:lang="en">Eavesdropping is the act of secretly listening to the private conversation of others without their consent. Two-way authentication and encryption altgorithm can prevent from this attack.</rdfs:comment>
        <rdfs:comment xml:lang="en">See Paper: A study of information security for M2M and IoT [Jiang et al. 2010], Paper: Survey of Security and Privacy Issues of Internet of Things [Borgohain et al. 2015]</rdfs:comment>
        <iotsec:isVulnerabilityOf rdf:resource="&stac;BluetoothTechnology"/>
        <iotsec:isVulnerabilityOf rdf:resource="&stac;EDGETechnology"/>
        <iotsec:hasSecurityMechanism rdf:resource="&stac;EncryptionAlgorithm"/>
        <iotsec:isVulnerabilityOf rdf:resource="&stac;EthernetTechnology"/>
        <iotsec:isVulnerabilityOf rdf:resource="&stac;GPRSTechnology"/>
        <iotsec:isVulnerabilityOf rdf:resource="&stac;GSMTechnology"/>
        <iotsec:isVulnerabilityOf rdf:resource="&stac;HSDPATechnology"/>
        <iotsec:isVulnerabilityOf rdf:resource="&stac;LTETechnology"/>
        <iotsec:isVulnerabilityOf rdf:resource="&stac;M2MTechnology"/>
        <iotsec:isVulnerabilityOf rdf:resource="&stac;ManetTechnology"/>
        <iotsec:isVulnerabilityOf rdf:resource="&stac;MeshTechnology"/>
        <iotsec:hasSecurityMechanism rdf:resource="&stac;MutualAuthentication"/>
        <iotsec:isVulnerabilityOf rdf:resource="&stac;RFIDTechnology"/>
        <iotsec:isVulnerabilityOf rdf:resource="&stac;SensorTechnology"/>
        <iotsec:isVulnerabilityOf rdf:resource="&stac;UMTSTechnology"/>
        <iotsec:isVulnerabilityOf rdf:resource="&stac;UWBTechnology"/>
        <iotsec:isVulnerabilityOf rdf:resource="&stac;WifiTechnology"/>
        <iotsec:isVulnerabilityOf rdf:resource="&stac;WimaxTechnology"/>
        <iotsec:isVulnerabilityOf rdf:resource="&stac;ZigbeeTechnology"/>
        <iotsec:threatens rdf:resource="&iotsec;Authentication"/>
        <iotsec:hasSecurityMechanism rdf:resource="&iotsec;DirectionalAntenna"/>
        <iotsec:hasSecurityMechanism rdf:resource="&iotsec;HTTPS"/>
        <iotsec:hasSecurityMechanism rdf:resource="&iotsec;Kerberos"/>
        <iotsec:hasSecurityMechanism rdf:resource="&iotsec;PANA"/>
        <iotsec:occursInLayer rdf:resource="&iotsec;PhysicalLayer"/>
        <iotsec:hasSecurityMechanism rdf:resource="&iotsec;VPN"/>
    </owl:NamedIndividual>
    


    <!-- http://securitytoolbox.appspot.com/stac#ElGamal -->

    <owl:NamedIndividual rdf:about="&stac;ElGamal">
        <rdf:type rdf:resource="&iotsec;AsymmetricAlgorithm"/>
        <rdf:type rdf:resource="&iotsec;ManetSecurityMechanism"/>
        <rdfs:label xml:lang="en">ElGamal</rdfs:label>
        <rdfs:comment xml:lang="en"></rdfs:comment>
        <owl:sameAs rdf:resource="&securitysw;ElGammelAlgorithm"/>
        <iotsec:satisfies rdf:resource="&iotsec;Authentication"/>
        <iotsec:satisfies rdf:resource="&iotsec;Confidentiality"/>
    </owl:NamedIndividual>
    


    <!-- http://securitytoolbox.appspot.com/stac#ErrorCorrectingCode -->

    <owl:NamedIndividual rdf:about="&stac;ErrorCorrectingCode">
        <rdf:type rdf:resource="&iotsec;SensorSecurityMechanism"/>
        <rdfs:label xml:lang="en">Error Correcting Code</rdfs:label>
        <rdfs:comment xml:lang="en"></rdfs:comment>
        <iotsec:protectsInLayer rdf:resource="&iotsec;LinkLayer"/>
    </owl:NamedIndividual>
    


    <!-- http://securitytoolbox.appspot.com/stac#Ettercap -->

    <owl:NamedIndividual rdf:about="&stac;Ettercap">
        <rdf:type rdf:resource="&iotsec;NetworkManagementSecurityTool"/>
        <rdfs:label xml:lang="en">Ettercap</rdfs:label>
        <rdfs:comment xml:lang="en">Ettercap is a free and open source network security tool for man-in-the-middle attacks on LAN. It can be used for computer network protocol analysis and security auditing.  It is capable of intercepting traffic on a network segment, capturing passwords, and conducting active eavesdropping against a number of common protocols.</rdfs:comment>
        <iotsec:hasFeature rdf:resource="&iotsec;Free"/>
        <iotsec:hasFeature rdf:resource="&iotsec;Opensource"/>
    </owl:NamedIndividual>
    


    <!-- http://securitytoolbox.appspot.com/stac#ExchangeKeyEasy -->

    <owl:NamedIndividual rdf:about="&stac;ExchangeKeyEasy">
        <rdf:type rdf:resource="&iotsec;PositiveFeature"/>
    </owl:NamedIndividual>
    


    <!-- http://securitytoolbox.appspot.com/stac#ExchangeKeyNotEasy -->

    <owl:NamedIndividual rdf:about="&stac;ExchangeKeyNotEasy">
        <rdf:type rdf:resource="&iotsec;NegativeFeature"/>
        <rdfs:label xml:lang="en">Exchange Key not easy</rdfs:label>
        <rdfs:comment xml:lang="en"></rdfs:comment>
    </owl:NamedIndividual>
    


    <!-- http://securitytoolbox.appspot.com/stac#Exhaustion -->

    <owl:NamedIndividual rdf:about="&stac;Exhaustion">
        <rdf:type rdf:resource="&iotsec;SensorAttack"/>
        <rdfs:label xml:lang="en">Battery exhaustion</rdfs:label>
        <rdfs:comment xml:lang="en">Exhaustion of the node&apos;s battery due to repeated retransmission. In exhaustion attacks the battery source is self-sacrificing, since wireless nodes most of the time maintains the channel active.</rdfs:comment>
        <rdfs:comment xml:lang="en">See Paper: Survey of Security and Privacy Issues of Internet of Things [Borgohain et al. 2015]</rdfs:comment>
        <iotsec:occursInLayer rdf:resource="&iotsec;LinkLayer"/>
        <iotsec:hasSecurityMechanism rdf:resource="&iotsec;RateLimitation"/>
        <iotsec:hasSecurityMechanism rdf:resource="&iotsec;TimeDivisionMultiplexing"/>
    </owl:NamedIndividual>
    


    <!-- http://securitytoolbox.appspot.com/stac#Exploit -->

    <owl:NamedIndividual rdf:about="&stac;Exploit">
        <rdf:type rdf:resource="&iotsec;WebAttack"/>
        <rdfs:label xml:lang="en">Exploit</rdfs:label>
        <rdfs:comment xml:lang="en"></rdfs:comment>
        <iotsec:occursInLayer rdf:resource="&iotsec;ApplicationLayer"/>
    </owl:NamedIndividual>
    


    <!-- http://securitytoolbox.appspot.com/stac#ExploitVulnarability -->

    <owl:NamedIndividual rdf:about="&stac;ExploitVulnarability">
        <rdf:type rdf:resource="&iotsec;DatabaseAttack"/>
        <rdfs:label xml:lang="en">Exploit Vulnarability</rdfs:label>
        <rdfs:comment xml:lang="en"></rdfs:comment>
    </owl:NamedIndividual>
    


    <!-- http://securitytoolbox.appspot.com/stac#Firewall -->

    <owl:NamedIndividual rdf:about="&stac;Firewall">
        <rdf:type rdf:resource="&iotsec;NetworkManagementSecurityMechanism"/>
        <rdf:type rdf:resource="&iotsec;UMTSSecurityMechanism"/>
    </owl:NamedIndividual>
    


    <!-- http://securitytoolbox.appspot.com/stac#Flexible -->

    <owl:NamedIndividual rdf:about="&stac;Flexible">
        <rdf:type rdf:resource="&iotsec;PositiveFeature"/>
    </owl:NamedIndividual>
    


    <!-- http://securitytoolbox.appspot.com/stac#ForgeryAttack -->

    <owl:NamedIndividual rdf:about="&stac;ForgeryAttack">
        <rdf:type rdf:resource="&iotsec;WimaxAttack"/>
        <rdfs:label xml:lang="en">Forgery Attack</rdfs:label>
        <rdfs:comment xml:lang="en"></rdfs:comment>
        <iotsec:hasSecurityMechanism rdf:resource="&iotsec;HMAC"/>
    </owl:NamedIndividual>
    


    <!-- http://securitytoolbox.appspot.com/stac#Free -->

    <owl:NamedIndividual rdf:about="&stac;Free">
        <rdf:type rdf:resource="&iotsec;PositiveFeature"/>
        <rdfs:label xml:lang="en">Free</rdfs:label>
        <rdfs:comment xml:lang="en"></rdfs:comment>
    </owl:NamedIndividual>
    


    <!-- http://securitytoolbox.appspot.com/stac#GAE -->

    <owl:NamedIndividual rdf:about="&stac;GAE">
        <rdf:type rdf:resource="&iotsec;ServerTechnology"/>
        <rdfs:label xml:lang="en">Google Application Engine (GAE)</rdfs:label>
        <rdfs:comment xml:lang="en"></rdfs:comment>
    </owl:NamedIndividual>
    


    <!-- http://securitytoolbox.appspot.com/stac#GEA3 -->

    <owl:NamedIndividual rdf:about="&stac;GEA3">
        <rdf:type rdf:resource="&iotsec;GPRSSecurityAlgorithm"/>
        <rdf:type rdf:resource="&iotsec;StreamCipher"/>
        <rdfs:label xml:lang="en">GEA3 (GPRS Encryption Algorithm)</rdfs:label>
        <rdfs:comment xml:lang="en">See Paper: Malicious actions against the GPRS technology [Xenakis 2006]</rdfs:comment>
        <rdfs:comment xml:lang="en">The GEA3 algorithm is integrated in the Mobile Equipment and is used for encryption the data during a data transfer under the ciphering key, Kc.</rdfs:comment>
        <dcterms:hasPart rdf:resource="&iotsec;Kasumi"/>
    </owl:NamedIndividual>
    


    <!-- http://securitytoolbox.appspot.com/stac#GGSN -->

    <owl:NamedIndividual rdf:about="&stac;GGSN">
        <rdf:type rdf:resource="&stac;GPRSArchitectureComponent"/>
        <rdfs:label xml:lang="en">Gateway GPRS Support Node (GGSN)</rdfs:label>
        <rdfs:comment xml:lang="en">The GGSN provides connection with external packet switched networks such as Internet or private networks.</rdfs:comment>
    </owl:NamedIndividual>
    


    <!-- http://securitytoolbox.appspot.com/stac#GMK -->

    <owl:NamedIndividual rdf:about="&stac;GMK">
        <rdf:type rdf:resource="&iotsec;WifiKeyManagement"/>
        <rdfs:label xml:lang="en">Group Master Key (GMK)</rdfs:label>
        <rdfs:comment xml:lang="en"></rdfs:comment>
        <iotsec:satisfies rdf:resource="&iotsec;Authentication"/>
    </owl:NamedIndividual>
    


    <!-- http://securitytoolbox.appspot.com/stac#GPG -->

    <owl:NamedIndividual rdf:about="&stac;GPG">
        <rdf:type rdf:resource="&iotsec;MessageEncryptionTool"/>
        <rdf:type rdf:resource="&iotsec;SecurityMechanism"/>
        <rdfs:label xml:lang="en">Gnu Privacy Guard (GPG)</rdfs:label>
        <rdfs:comment xml:lang="en"></rdfs:comment>
        <iotsec:satisfies rdf:resource="&iotsec;Confidentiality"/>
        <iotsec:hasFeature rdf:resource="&iotsec;Free"/>
    </owl:NamedIndividual>
    


    <!-- http://securitytoolbox.appspot.com/stac#GPRSMobileStation -->

    <owl:NamedIndividual rdf:about="&stac;GPRSMobileStation">
        <rdf:type rdf:resource="&stac;GPRSArchitectureComponent"/>
        <rdfs:label xml:lang="en">GPRS Mobile Station</rdfs:label>
        <rdfs:comment xml:lang="en"></rdfs:comment>
        <dcterms:hasPart rdf:resource="&iotsec;MobileTerminal"/>
        <dcterms:hasPart rdf:resource="&iotsec;TerminalEquipment"/>
    </owl:NamedIndividual>
    


    <!-- http://securitytoolbox.appspot.com/stac#GPRS_A5 -->

    <owl:NamedIndividual rdf:about="&stac;GPRS_A5">
        <rdf:type rdf:resource="&iotsec;GPRSSecurityAlgorithm"/>
        <rdf:type rdf:resource="&iotsec;StreamCipher"/>
        <rdfs:label xml:lang="en">GPRS_A5</rdfs:label>
        <rdfs:comment xml:lang="en"></rdfs:comment>
    </owl:NamedIndividual>
    


    <!-- http://securitytoolbox.appspot.com/stac#GSMDatabase -->

    <owl:NamedIndividual rdf:about="&stac;GSMDatabase">
        <rdf:type rdf:resource="&stac;GSMArchitectureComponent"/>
        <rdfs:label xml:lang="en">GSM Database</rdfs:label>
        <rdfs:comment xml:lang="en"></rdfs:comment>
    </owl:NamedIndividual>
    


    <!-- http://securitytoolbox.appspot.com/stac#GSMMobileStation -->

    <owl:NamedIndividual rdf:about="&stac;GSMMobileStation">
        <rdf:type rdf:resource="&stac;GSMArchitectureComponent"/>
        <rdfs:label xml:lang="en">GSM Mobile Station (MS)</rdfs:label>
        <rdfs:comment xml:lang="en"></rdfs:comment>
        <dcterms:hasPart rdf:resource="&iotsec;MobileEquipment"/>
        <dcterms:hasPart rdf:resource="&iotsec;SIM"/>
    </owl:NamedIndividual>
    


    <!-- http://securitytoolbox.appspot.com/stac#Glassfish -->

    <owl:NamedIndividual rdf:about="&stac;Glassfish">
        <rdf:type rdf:resource="&iotsec;ServerTechnology"/>
        <rdfs:label xml:lang="en">Glassfish</rdfs:label>
        <rdfs:comment xml:lang="en"></rdfs:comment>
    </owl:NamedIndividual>
    


    <!-- http://securitytoolbox.appspot.com/stac#GroupKey -->

    <owl:NamedIndividual rdf:about="&stac;GroupKey">
        <rdf:type rdf:resource="&iotsec;SymmetricSensorKey"/>
        <rdfs:label xml:lang="en">Group Key</rdfs:label>
        <rdfs:comment xml:lang="en">This is globally shared key that is used by the base station for encrypting messages that are broadcast to the whole group.</rdfs:comment>
    </owl:NamedIndividual>
    


    <!-- http://securitytoolbox.appspot.com/stac#HBase -->

    <owl:NamedIndividual rdf:about="&stac;HBase">
        <rdf:type rdf:resource="&iotsec;DatabaseTechnology"/>
        <rdfs:label xml:lang="en">HBase</rdfs:label>
        <rdfs:comment xml:lang="en"></rdfs:comment>
    </owl:NamedIndividual>
    


    <!-- http://securitytoolbox.appspot.com/stac#HLR -->

    <owl:NamedIndividual rdf:about="&stac;HLR">
        <rdf:type rdf:resource="&stac;GSMArchitectureComponent"/>
        <rdfs:label xml:lang="en">Home Location Register (HLR)</rdfs:label>
        <rdfs:comment xml:lang="en">HLR is the database that holds subscription information for every person.</rdfs:comment>
    </owl:NamedIndividual>
    


    <!-- http://securitytoolbox.appspot.com/stac#HMAC -->

    <owl:NamedIndividual rdf:about="&stac;HMAC">
        <rdf:type rdf:resource="&iotsec;HashFunction"/>
        <rdf:type rdf:resource="&iotsec;ManetSecurityMechanism"/>
        <rdfs:label xml:lang="en">Hash-based Message Authentication Code (HMAC)</rdfs:label>
        <rdfs:comment xml:lang="en"></rdfs:comment>
        <iotsec:satisfies rdf:resource="&iotsec;Authentication"/>
        <iotsec:satisfies rdf:resource="&iotsec;Integrity"/>
    </owl:NamedIndividual>
    


    <!-- http://securitytoolbox.appspot.com/stac#HTTPS -->

    <owl:NamedIndividual rdf:about="&stac;HTTPS">
        <rdf:type rdf:resource="&iotsec;WebSecurityProtocol"/>
        <rdfs:label xml:lang="en">HyperText Transfer Protocol Secure (HTTPS)</rdfs:label>
        <rdfs:comment xml:lang="en">HTTPS is a widely used to secure the communication against eavesdroppers and thus providing confidentiality.</rdfs:comment>
        <iotsec:protectsInLayer rdf:resource="&iotsec;ApplicationLayer"/>
        <iotsec:satisfies rdf:resource="&iotsec;Authentication"/>
        <iotsec:satisfies rdf:resource="&iotsec;Confidentiality"/>
        <dcterms:hasPart rdf:resource="&iotsec;SSL"/>
        <dcterms:hasPart rdf:resource="&iotsec;X_509"/>
    </owl:NamedIndividual>
    


    <!-- http://securitytoolbox.appspot.com/stac#HackInSight -->

    <owl:NamedIndividual rdf:about="&stac;HackInSight">
        <rdf:type rdf:resource="&iotsec;SecurityMagazine"/>
        <rdfs:label xml:lang="en">HackInSight</rdfs:label>
        <rdfs:comment xml:lang="en"></rdfs:comment>
    </owl:NamedIndividual>
    


    <!-- http://securitytoolbox.appspot.com/stac#Hadoop -->

    <owl:NamedIndividual rdf:about="&stac;Hadoop">
        <rdf:type rdf:resource="&iotsec;FrameworkTechnology"/>
        <rdfs:label xml:lang="en">Hadoop</rdfs:label>
        <rdfs:comment xml:lang="en"></rdfs:comment>
    </owl:NamedIndividual>
    


    <!-- http://securitytoolbox.appspot.com/stac#HelloFlood -->

    <owl:NamedIndividual rdf:about="&stac;HelloFlood">
        <rdf:type rdf:resource="&iotsec;ManetAttack"/>
        <rdf:type rdf:resource="&iotsec;SensorAttack"/>
        <rdfs:label xml:lang="en">Hello Flood</rdfs:label>
        <rdfs:comment xml:lang="en">See Paper: Survey of Security and Privacy Issues of Internet of Things [Borgohain et al. 2015], Paper: Routing security in sensor networks: Hello Flood Attack and Defense [Hamid et al. 2006]</rdfs:comment>
        <rdfs:comment xml:lang="en">The Hello Flood attack uses HELLO packets as a weapon to convince the sensors in Wireless Sensor Networks.</rdfs:comment>
        <iotsec:hasSecurityMechanism rdf:resource="&iotsec;IdentityVerification"/>
        <iotsec:occursInLayer rdf:resource="&iotsec;NetworkLayer"/>
    </owl:NamedIndividual>
    


    <!-- http://securitytoolbox.appspot.com/stac#Helomoto -->

    <owl:NamedIndividual rdf:about="&stac;Helomoto">
        <rdf:type rdf:resource="&iotsec;BluetoothAttack"/>
        <rdfs:label xml:lang="en">Helomoto</rdfs:label>
        <rdfs:comment xml:lang="en"></rdfs:comment>
    </owl:NamedIndividual>
    


    <!-- http://securitytoolbox.appspot.com/stac#Hibernate -->

    <owl:NamedIndividual rdf:about="&stac;Hibernate">
        <rdf:type rdf:resource="&iotsec;FrameworkTechnology"/>
        <rdfs:label xml:lang="en">Hibernate</rdfs:label>
        <rdfs:comment xml:lang="en"></rdfs:comment>
    </owl:NamedIndividual>
    


    <!-- http://securitytoolbox.appspot.com/stac#HidingNode -->

    <owl:NamedIndividual rdf:about="&stac;HidingNode">
        <rdf:type rdf:resource="&iotsec;SecurityMechanism"/>
        <rdfs:label xml:lang="en">Hiding Node</rdfs:label>
        <rdfs:comment xml:lang="en"></rdfs:comment>
        <iotsec:protectsInLayer rdf:resource="&iotsec;PhysicalLayer"/>
    </owl:NamedIndividual>
    


    <!-- http://securitytoolbox.appspot.com/stac#HighCostDeployment -->

    <owl:NamedIndividual rdf:about="&stac;HighCostDeployment">
        <rdf:type rdf:resource="&iotsec;NegativeFeature"/>
        <rdfs:label xml:lang="en">High Cost Deployment</rdfs:label>
        <rdfs:comment xml:lang="en"></rdfs:comment>
    </owl:NamedIndividual>
    


    <!-- http://securitytoolbox.appspot.com/stac#HighEnergyConsuming -->

    <owl:NamedIndividual rdf:about="&stac;HighEnergyConsuming">
        <rdf:type rdf:resource="&iotsec;NegativeFeature"/>
    </owl:NamedIndividual>
    


    <!-- http://securitytoolbox.appspot.com/stac#HijackIMSI -->

    <owl:NamedIndividual rdf:about="&stac;HijackIMSI">
        <rdf:type rdf:resource="&iotsec;UMTSAttack"/>
        <rdfs:label xml:lang="en">Hijack IMSI</rdfs:label>
        <rdfs:comment xml:lang="en"></rdfs:comment>
    </owl:NamedIndividual>
    


    <!-- http://securitytoolbox.appspot.com/stac#HoneyBOT -->

    <owl:NamedIndividual rdf:about="&stac;HoneyBOT">
        <rdf:type rdf:resource="&iotsec;Honeypot"/>
        <rdfs:label xml:lang="en">HoneyBOT</rdfs:label>
        <rdfs:comment xml:lang="en">HoneyBOT is a honeypot.</rdfs:comment>
    </owl:NamedIndividual>
    


    <!-- http://securitytoolbox.appspot.com/stac#Honeyd -->

    <owl:NamedIndividual rdf:about="&stac;Honeyd">
        <rdf:type rdf:resource="&iotsec;Honeypot"/>
        <rdfs:label xml:lang="en">Honeyd</rdfs:label>
        <rdfs:comment xml:lang="en">Honeyd is a honeypot.</rdfs:comment>
    </owl:NamedIndividual>
    


    <!-- http://securitytoolbox.appspot.com/stac#HtAccess -->

    <owl:NamedIndividual rdf:about="&stac;HtAccess">
        <rdf:type rdf:resource="&iotsec;NetworkManagementSecurityMechanism"/>
        <rdf:type rdf:resource="&iotsec;WebSecurityMechanism"/>
        <rdfs:label xml:lang="en">HtAccess</rdfs:label>
        <rdfs:comment xml:lang="en">A .htaccess file is a directory-level configuration file supported by several web servers, that allows for decentralized management of web server configuration. They are placed inside the web tree, and are able to override a subset of the server&apos;s global configuration for the directory that they are in, and all sub-directories</rdfs:comment>
        <iotsec:protectsInLayer rdf:resource="&iotsec;ApplicationLayer"/>
        <iotsec:satisfies rdf:resource="&iotsec;Authentication"/>
    </owl:NamedIndividual>
    


    <!-- http://securitytoolbox.appspot.com/stac#IBSS -->

    <owl:NamedIndividual rdf:about="&stac;IBSS">
        <rdf:type rdf:resource="&iotsec;WifiArchitectureComponent"/>
        <rdfs:label xml:lang="en">Integrated Basic Service Set (IBSS)</rdfs:label>
        <rdfs:comment xml:lang="en"></rdfs:comment>
    </owl:NamedIndividual>
    


    <!-- http://securitytoolbox.appspot.com/stac#IDEA -->

    <owl:NamedIndividual rdf:about="&stac;IDEA">
        <rdf:type rdf:resource="&iotsec;BlockCipher"/>
        <rdf:type rdf:resource="&iotsec;ManetSecurityMechanism"/>
        <rdfs:label xml:lang="en">International Data Encryption Algorithm (IDEA)</rdfs:label>
        <rdfs:comment xml:lang="en"></rdfs:comment>
        <iotsec:satisfies rdf:resource="&iotsec;Confidentiality"/>
    </owl:NamedIndividual>
    


    <!-- http://securitytoolbox.appspot.com/stac#IKE -->

    <owl:NamedIndividual rdf:about="&stac;IKE">
        <rdf:type rdf:resource="&iotsec;KeyManagement"/>
        <rdf:type rdf:resource="&iotsec;Protocol"/>
        <rdfs:label xml:lang="en">Internet Key Exchange (IKE)</rdfs:label>
        <rdfs:comment xml:lang="en">IKE uses asymmetric algorithms (public key cryptography) where secret key for secure communication can be exchanged over an insecure channel.</rdfs:comment>
        <iotsec:satisfies rdf:resource="&iotsec;Authentication"/>
        <dcterms:hasPart rdf:resource="&iotsec;DiffieHellman"/>
    </owl:NamedIndividual>
    


    <!-- http://securitytoolbox.appspot.com/stac#IMEI -->

    <owl:NamedIndividual rdf:about="&stac;IMEI">
        <rdf:type rdf:resource="&stac;GSMArchitectureComponent"/>
        <rdfs:label xml:lang="en">International Mobile Equipment Identity (IMEI)</rdfs:label>
        <rdfs:comment xml:lang="en"></rdfs:comment>
    </owl:NamedIndividual>
    


    <!-- http://securitytoolbox.appspot.com/stac#IMSI -->

    <owl:NamedIndividual rdf:about="&stac;IMSI">
        <rdf:type rdf:resource="&stac;GSMArchitectureComponent"/>
        <rdfs:label xml:lang="en">International Mobile Subscriber Identity (IMSI)</rdfs:label>
        <rdfs:comment xml:lang="en">The IMSI is a unique identifier for a mobile subscriber in a GSM and UMTS network. It is stored in the SIM card of the mobile station.</rdfs:comment>
    </owl:NamedIndividual>
    


    <!-- http://securitytoolbox.appspot.com/stac#IPFlooding -->

    <owl:NamedIndividual rdf:about="&stac;IPFlooding">
        <rdf:type rdf:resource="&iotsec;Flooding"/>
        <rdfs:label xml:lang="en">IP Flooding</rdfs:label>
        <rdfs:comment xml:lang="en"></rdfs:comment>
    </owl:NamedIndividual>
    


    <!-- http://securitytoolbox.appspot.com/stac#ISAKMP -->

    <owl:NamedIndividual rdf:about="&stac;ISAKMP">
        <rdf:type rdf:resource="&iotsec;KeyManagement"/>
        <rdf:type rdf:resource="&iotsec;Protocol"/>
        <rdfs:label xml:lang="en">Internet Security Association and Key Management Protocol (ISAKMP)</rdfs:label>
        <rdfs:comment xml:lang="en">ISAKMP is a protocol defined for establishing Security Associations (SA) and cryptographic keys in an Internet environment.</rdfs:comment>
        <iotsec:protectsInLayer rdf:resource="&iotsec;ApplicationLayer"/>
        <iotsec:satisfies rdf:resource="&iotsec;Authentication"/>
    </owl:NamedIndividual>
    


    <!-- http://securitytoolbox.appspot.com/stac#IdentityVerification -->

    <owl:NamedIndividual rdf:about="&stac;IdentityVerification">
        <rdf:type rdf:resource="&iotsec;SensorSecurityMechanism"/>
        <rdfs:label xml:lang="en">Identity Verification</rdfs:label>
        <rdfs:comment xml:lang="en">This protocol verifies bi-directionality of a link between two nodes.</rdfs:comment>
        <iotsec:protectsInLayer rdf:resource="&iotsec;NetworkLayer"/>
    </owl:NamedIndividual>
    


    <!-- http://securitytoolbox.appspot.com/stac#IndividualKey -->

    <owl:NamedIndividual rdf:about="&stac;IndividualKey">
        <rdf:type rdf:resource="&iotsec;SymmetricSensorKey"/>
        <rdfs:label xml:lang="en">Individual Key</rdfs:label>
        <rdfs:comment xml:lang="en">Every node has a unique key that it shares pairwise with the base station. This key is used for secure communication between a node and the base station. Similarly, the base station can use this key to encrypt any sensitive information.</rdfs:comment>
    </owl:NamedIndividual>
    


    <!-- http://securitytoolbox.appspot.com/stac#InfrastructureMode -->

    <owl:NamedIndividual rdf:about="&stac;InfrastructureMode">
        <rdf:type rdf:resource="&iotsec;WifiArchitectureComponent"/>
        <rdfs:label xml:lang="en">Infrastructure Mode</rdfs:label>
        <rdfs:comment xml:lang="en">It consists of a number of wireless stations and access points.</rdfs:comment>
        <dcterms:hasPart rdf:resource="&iotsec;AccessPoint"/>
        <dcterms:hasPart rdf:resource="&iotsec;BasicServiceSet"/>
        <dcterms:hasPart rdf:resource="&iotsec;IBSS"/>
        <dcterms:hasPart rdf:resource="&iotsec;SSID"/>
        <dcterms:hasPart rdf:resource="&iotsec;WifiMobileStation"/>
    </owl:NamedIndividual>
    


    <!-- http://securitytoolbox.appspot.com/stac#Integrity -->

    <owl:NamedIndividual rdf:about="&stac;Integrity">
        <rdf:type rdf:resource="&iotsec;SecurityProperty"/>
        <rdfs:label xml:lang="en">Integrity</rdfs:label>
        <rdfs:comment xml:lang="en">Data integrity guarantees that the transmitted messages are not modified by attackers, either due to malicious intent or by accident.</rdfs:comment>
        <rdfs:comment xml:lang="en">Integrity means that no data is altered during the communication.</rdfs:comment>
        <owl:sameAs rdf:resource="&securitysw;Integrity"/>
        <owl:sameAs rdf:resource="&denker;DataIntegrity"/>
        <owl:sameAs rdf:resource="&herzog;Integrity"/>
    </owl:NamedIndividual>
    


    <!-- http://securitytoolbox.appspot.com/stac#IntegrityKeyIK -->

    <owl:NamedIndividual rdf:about="&stac;IntegrityKeyIK">
        <rdf:type rdf:resource="&iotsec;UMTSArchitectureComponent"/>
        <rdfs:label xml:lang="en">Integrity Key (IK)</rdfs:label>
        <rdfs:comment xml:lang="en"></rdfs:comment>
    </owl:NamedIndividual>
    


    <!-- http://securitytoolbox.appspot.com/stac#Ipsec -->

    <owl:NamedIndividual rdf:about="&stac;Ipsec">
        <rdf:type rdf:resource="&iotsec;ManetSecurityMechanism"/>
        <rdf:type rdf:resource="&iotsec;Protocol"/>
        <rdfs:label xml:lang="en">Internet Security Protocol (Ipsec)</rdfs:label>
        <rdfs:comment xml:lang="en">IPSec improves the security at the network layer of the IP based core network.</rdfs:comment>
        <rdfs:comment xml:lang="en">See Paper: UMTS Security: Security in Core Network and UTRAN [Abid et al. 2002]</rdfs:comment>
        <dcterms:hasPart rdf:resource="&iotsec;AH"/>
        <iotsec:satisfies rdf:resource="&iotsec;Authentication"/>
        <iotsec:satisfies rdf:resource="&iotsec;Confidentiality"/>
        <dcterms:hasPart rdf:resource="&iotsec;ESP"/>
        <dcterms:hasPart rdf:resource="&iotsec;IKE"/>
        <iotsec:satisfies rdf:resource="&iotsec;Integrity"/>
        <iotsec:protectsInLayer rdf:resource="&iotsec;NetworkLayer"/>
    </owl:NamedIndividual>
    


    <!-- http://securitytoolbox.appspot.com/stac#IurInterface -->

    <owl:NamedIndividual rdf:about="&stac;IurInterface">
        <rdf:type rdf:resource="&iotsec;UMTSArchitectureComponent"/>
        <rdfs:label xml:lang="en">Iur Interface</rdfs:label>
        <rdfs:comment xml:lang="en">Connection between two RNCs.</rdfs:comment>
    </owl:NamedIndividual>
    


    <!-- http://securitytoolbox.appspot.com/stac#JAAS -->

    <owl:NamedIndividual rdf:about="&stac;JAAS">
        <rdf:type rdf:resource="&iotsec;ProgrammingLanguageSecurityMechanism"/>
        <rdfs:label xml:lang="en">Java Authentication and Authorization Service (JAAS)</rdfs:label>
        <rdfs:comment xml:lang="en"></rdfs:comment>
    </owl:NamedIndividual>
    


    <!-- http://securitytoolbox.appspot.com/stac#JCE -->

    <owl:NamedIndividual rdf:about="&stac;JCE">
        <rdf:type rdf:resource="&iotsec;ProgrammingLanguageSecurityMechanism"/>
        <rdfs:label xml:lang="en">Java Cryptography Extension (JCE)</rdfs:label>
        <rdfs:comment xml:lang="en"></rdfs:comment>
    </owl:NamedIndividual>
    


    <!-- http://securitytoolbox.appspot.com/stac#JHoney -->

    <owl:NamedIndividual rdf:about="&stac;JHoney">
        <rdf:type rdf:resource="&iotsec;Honeypot"/>
        <rdfs:label xml:lang="en">JHoney</rdfs:label>
        <rdfs:comment xml:lang="en">JHoney is a honeypot tool for Linux written in Java.</rdfs:comment>
    </owl:NamedIndividual>
    


    <!-- http://securitytoolbox.appspot.com/stac#JSR82 -->

    <owl:NamedIndividual rdf:about="&stac;JSR82">
        <rdf:type rdf:resource="&iotsec;BluetoothSecurityMechanism"/>
        <rdf:type rdf:resource="&iotsec;ProgrammingLanguageSecurityMechanism"/>
        <rdfs:label xml:lang="en">JSR-82</rdfs:label>
        <rdfs:comment xml:lang="en">JSR-82 is the official Java Blutooth Application Programming Interface (API)</rdfs:comment>
    </owl:NamedIndividual>
    


    <!-- http://securitytoolbox.appspot.com/stac#Jamming -->

    <owl:NamedIndividual rdf:about="&stac;Jamming">
        <rdf:type rdf:resource="&iotsec;ManetAttack"/>
        <rdf:type rdf:resource="&iotsec;RfidAttack"/>
        <rdf:type rdf:resource="&iotsec;SensorAttack"/>
        <rdf:type rdf:resource="&iotsec;Threat"/>
        <rdf:type rdf:resource="&iotsec;WimaxAttack"/>
        <rdf:type rdf:resource="&iotsec;ZigbeeAttack"/>
        <rdfs:label xml:lang="en">Jamming</rdfs:label>
        <rdfs:comment xml:lang="en">Jamming is the interference with the Radio Frequency (RF) used by the nodes in a network in the physical layer. It prevents the nodes to communicate with each other.</rdfs:comment>
        <rdfs:comment xml:lang="en">See Paper: Survey of Security and Privacy Issues of Internet of Things [Borgohain et al. 2015]</rdfs:comment>
        <iotsec:isVulnerabilityOf rdf:resource="&stac;BluetoothTechnology"/>
        <iotsec:isVulnerabilityOf rdf:resource="&stac;EDGETechnology"/>
        <iotsec:isVulnerabilityOf rdf:resource="&stac;GPRSTechnology"/>
        <iotsec:isVulnerabilityOf rdf:resource="&stac;GSMTechnology"/>
        <iotsec:isVulnerabilityOf rdf:resource="&stac;HSDPATechnology"/>
        <iotsec:isVulnerabilityOf rdf:resource="&stac;LTETechnology"/>
        <iotsec:isVulnerabilityOf rdf:resource="&stac;M2MTechnology"/>
        <iotsec:isVulnerabilityOf rdf:resource="&stac;ManetTechnology"/>
        <iotsec:isVulnerabilityOf rdf:resource="&stac;MeshTechnology"/>
        <iotsec:isVulnerabilityOf rdf:resource="&stac;RFIDTechnology"/>
        <iotsec:isVulnerabilityOf rdf:resource="&stac;SensorTechnology"/>
        <iotsec:isVulnerabilityOf rdf:resource="&stac;UMTSTechnology"/>
        <iotsec:isVulnerabilityOf rdf:resource="&stac;UWBTechnology"/>
        <iotsec:isVulnerabilityOf rdf:resource="&stac;WifiTechnology"/>
        <iotsec:isVulnerabilityOf rdf:resource="&stac;WimaxTechnology"/>
        <iotsec:isVulnerabilityOf rdf:resource="&stac;ZigbeeTechnology"/>
        <iotsec:occursInLayer rdf:resource="&iotsec;PhysicalLayer"/>
        <iotsec:hasSecurityMechanism rdf:resource="&iotsec;RadioSpectrumMonitoringEquipment"/>
        <iotsec:hasSecurityMechanism rdf:resource="&iotsec;SpreadSpectrumCommunication"/>
    </owl:NamedIndividual>
    


    <!-- http://securitytoolbox.appspot.com/stac#Java -->

    <owl:NamedIndividual rdf:about="&stac;Java">
        <rdf:type rdf:resource="&iotsec;ProgrammingLanguageTechnology"/>
        <rdfs:label xml:lang="en">Java</rdfs:label>
        <rdfs:comment xml:lang="en"></rdfs:comment>
    </owl:NamedIndividual>
    


    <!-- http://securitytoolbox.appspot.com/stac#Javascript -->

    <owl:NamedIndividual rdf:about="&stac;Javascript">
        <rdf:type rdf:resource="&iotsec;ProgrammingLanguageTechnology"/>
        <rdfs:label xml:lang="en">Javascript</rdfs:label>
        <rdfs:comment xml:lang="en"></rdfs:comment>
    </owl:NamedIndividual>
    


    <!-- http://securitytoolbox.appspot.com/stac#Jena -->

    <owl:NamedIndividual rdf:about="&stac;Jena">
        <rdf:type rdf:resource="&iotsec;FrameworkTechnology"/>
        <rdfs:label xml:lang="en">Jena</rdfs:label>
        <rdfs:comment xml:lang="en"></rdfs:comment>
    </owl:NamedIndividual>
    


    <!-- http://securitytoolbox.appspot.com/stac#JohnTheRipper -->

    <owl:NamedIndividual rdf:about="&stac;JohnTheRipper">
        <rdf:type rdf:resource="&iotsec;NetworkManagementSecurityTool"/>
        <rdfs:label xml:lang="en">John the Ripper</rdfs:label>
        <rdfs:comment xml:lang="en">John the Ripper is a fast password cracker.</rdfs:comment>
    </owl:NamedIndividual>
    


    <!-- http://securitytoolbox.appspot.com/stac#KEK -->

    <owl:NamedIndividual rdf:about="&stac;KEK">
        <rdf:type rdf:resource="&iotsec;WimaxKeyManagement"/>
        <rdfs:label xml:lang="en">Key Encryption Key (KEK)</rdfs:label>
        <rdfs:comment xml:lang="en"></rdfs:comment>
        <iotsec:satisfies rdf:resource="&iotsec;Authentication"/>
    </owl:NamedIndividual>
    


    <!-- http://securitytoolbox.appspot.com/stac#Kapersky -->

    <owl:NamedIndividual rdf:about="&stac;Kapersky">
        <rdf:type rdf:resource="&iotsec;Antivirus"/>
        <rdf:type rdf:resource="&iotsec;Firewall"/>
        <rdfs:label xml:lang="en">Kapersky</rdfs:label>
        <rdfs:comment xml:lang="en"></rdfs:comment>
        <iotsec:satisfies rdf:resource="&iotsec;AccessControl"/>
        <iotsec:hasFeature rdf:resource="&iotsec;NotFree"/>
    </owl:NamedIndividual>
    


    <!-- http://securitytoolbox.appspot.com/stac#Kasumi -->

    <owl:NamedIndividual rdf:about="&stac;Kasumi">
        <rdf:type rdf:resource="&iotsec;BlockCipher"/>
        <rdf:type rdf:resource="&iotsec;ManetSecurityMechanism"/>
        <rdfs:label xml:lang="en">Kasumi</rdfs:label>
        <rdfs:comment xml:lang="en"></rdfs:comment>
        <dcterms:hasPart rdf:resource="&iotsec;CBC"/>
        <iotsec:satisfies rdf:resource="&iotsec;Confidentiality"/>
        <iotsec:satisfies rdf:resource="&iotsec;Integrity"/>
    </owl:NamedIndividual>
    


    <!-- http://securitytoolbox.appspot.com/stac#Kc -->

    <owl:NamedIndividual rdf:about="&stac;Kc">
        <rdf:type rdf:resource="&iotsec;SymmetricKey"/>
        <rdfs:label xml:lang="en">Kc</rdfs:label>
        <rdfs:comment xml:lang="en"></rdfs:comment>
    </owl:NamedIndividual>
    


    <!-- http://securitytoolbox.appspot.com/stac#Kerberos -->

    <owl:NamedIndividual rdf:about="&stac;Kerberos">
        <rdf:type rdf:resource="&iotsec;Protocol"/>
        <rdfs:label xml:lang="en">Kerberos</rdfs:label>
        <rdfs:comment xml:lang="en"></rdfs:comment>
        <iotsec:satisfies rdf:resource="&iotsec;Authentication"/>
        <dcterms:hasPart rdf:resource="&iotsec;NeedhamSchroeder"/>
    </owl:NamedIndividual>
    


    <!-- http://securitytoolbox.appspot.com/stac#KeyLoger -->

    <owl:NamedIndividual rdf:about="&stac;KeyLoger">
        <rdf:type rdf:resource="&iotsec;WebAttack"/>
        <rdfs:label xml:lang="en">KeyLoger</rdfs:label>
        <rdfs:comment xml:lang="en"></rdfs:comment>
        <iotsec:occursInLayer rdf:resource="&iotsec;ApplicationLayer"/>
    </owl:NamedIndividual>
    


    <!-- http://securitytoolbox.appspot.com/stac#KnownPlaintext -->

    <owl:NamedIndividual rdf:about="&stac;KnownPlaintext">
        <rdf:type rdf:resource="&iotsec;Threat"/>
        <rdfs:label xml:lang="en">Known Plaintext</rdfs:label>
        <rdfs:comment xml:lang="en">The attacker knows pairs of plaintext and ciphertext.</rdfs:comment>
    </owl:NamedIndividual>
    


    <!-- http://securitytoolbox.appspot.com/stac#LDAP -->

    <owl:NamedIndividual rdf:about="&stac;LDAP">
        <rdf:type rdf:resource="&iotsec;WebSecurityProtocol"/>
        <rdfs:label xml:lang="en">Lightweight Directory Access Protocol (LDAP)</rdfs:label>
        <rdfs:comment xml:lang="en"></rdfs:comment>
        <iotsec:protectsInLayer rdf:resource="&iotsec;ApplicationLayer"/>
        <iotsec:satisfies rdf:resource="&iotsec;Authentication"/>
    </owl:NamedIndividual>
    


    <!-- http://securitytoolbox.appspot.com/stac#LEAP -->

    <owl:NamedIndividual rdf:about="&stac;LEAP">
        <rdf:type rdf:resource="&iotsec;WifiSecurityProtocol"/>
        <rdfs:label xml:lang="en">LEAP (Lightweight Extensible Authentication Protocol)</rdfs:label>
        <rdfs:comment xml:lang="en"></rdfs:comment>
        <iotsec:satisfies rdf:resource="&iotsec;Authentication"/>
    </owl:NamedIndividual>
    


    <!-- http://securitytoolbox.appspot.com/stac#LEAP_sensor -->

    <owl:NamedIndividual rdf:about="&stac;LEAP_sensor">
        <rdf:type rdf:resource="&iotsec;SensorKeyManagement"/>
        <rdfs:label xml:lang="en">Localized encryption and authentication protocol (LEAP)</rdfs:label>
        <rdfs:comment xml:lang="en">LEAP is a famous key management used in sensor networks. </rdfs:comment>
        <rdfs:comment xml:lang="en">See Paper: LEAP: Efficient security mechanisms for large-scale distributed sensor networks [Zhu et al. 2004]</rdfs:comment>
        <iotsec:satisfies rdf:resource="&iotsec;Authentication"/>
        <dcterms:hasPart rdf:resource="&iotsec;ClusterKey"/>
        <iotsec:satisfies rdf:resource="&iotsec;Confidentiality"/>
        <dcterms:hasPart rdf:resource="&iotsec;GroupKey"/>
        <dcterms:hasPart rdf:resource="&iotsec;IndividualKey"/>
        <dcterms:hasPart rdf:resource="&iotsec;PairwiseKey"/>
    </owl:NamedIndividual>
    


    <!-- http://securitytoolbox.appspot.com/stac#LISP -->

    <owl:NamedIndividual rdf:about="&stac;LISP">
        <rdf:type rdf:resource="&iotsec;SensorSecurityProtocol"/>
        <rdfs:label xml:lang="en">LiSP</rdfs:label>
        <rdfs:comment xml:lang="en"></rdfs:comment>
        <rdfs:comment xml:lang="en">See Paper: LiSP: A lightweight Security Protcol for Wireless Sensor Networks [Park et al. 2004]</rdfs:comment>
        <iotsec:satisfies rdf:resource="&iotsec;AccessControl"/>
        <iotsec:satisfies rdf:resource="&iotsec;Availability"/>
        <iotsec:satisfies rdf:resource="&iotsec;Confidentiality"/>
        <iotsec:satisfies rdf:resource="&iotsec;Integrity"/>
    </owl:NamedIndividual>
    


    <!-- http://securitytoolbox.appspot.com/stac#LLSP -->

    <owl:NamedIndividual rdf:about="&stac;LLSP">
        <rdf:type rdf:resource="&iotsec;SensorSecurityProtocol"/>
        <rdfs:label xml:lang="en">Link-Layer Security Protocol (LLSP)</rdfs:label>
        <rdfs:comment xml:lang="en"></rdfs:comment>
        <rdfs:comment xml:lang="en">See Paper: An energy efficient Link-Layer Security Protocol for wireless sensor networks [Lighfoot et al. 2004]</rdfs:comment>
        <dcterms:hasPart rdf:resource="&iotsec;AES"/>
        <iotsec:satisfies rdf:resource="&iotsec;Authentication"/>
        <dcterms:hasPart rdf:resource="&iotsec;CBC"/>
        <iotsec:satisfies rdf:resource="&iotsec;Confidentiality"/>
        <iotsec:satisfies rdf:resource="&iotsec;DataFreshness"/>
        <iotsec:protectsInLayer rdf:resource="&iotsec;LinkLayer"/>
        <iotsec:satisfies rdf:resource="&iotsec;SemanticSecurity"/>
    </owl:NamedIndividual>
    


    <!-- http://securitytoolbox.appspot.com/stac#LinkLayer -->

    <owl:NamedIndividual rdf:about="&stac;LinkLayer">
        <rdf:type rdf:resource="&iotsec;OSIModelLayer"/>
        <rdfs:label xml:lang="en">Link Layer</rdfs:label>
        <rdfs:comment xml:lang="en">The link layer is responsible for a reliable link between two nodes, by detecting and correcting errors that may occur in the physical layer.</rdfs:comment>
    </owl:NamedIndividual>
    


    <!-- http://securitytoolbox.appspot.com/stac#Linux -->

    <owl:NamedIndividual rdf:about="&stac;Linux">
        <rdf:type rdf:resource="&iotsec;OperatingSystemTechnology"/>
        <rdfs:label xml:lang="en">Linux</rdfs:label>
        <rdfs:comment xml:lang="en"></rdfs:comment>
    </owl:NamedIndividual>
    


    <!-- http://securitytoolbox.appspot.com/stac#LoveBug -->

    <owl:NamedIndividual rdf:about="&stac;LoveBug">
        <rdf:type rdf:resource="&iotsec;Virus"/>
        <rdfs:label xml:lang="en">Love Bug</rdfs:label>
        <rdfs:comment xml:lang="en"></rdfs:comment>
    </owl:NamedIndividual>
    


    <!-- http://securitytoolbox.appspot.com/stac#LowCostDeployment -->

    <owl:NamedIndividual rdf:about="&stac;LowCostDeployment">
        <rdf:type rdf:resource="&iotsec;PositiveFeature"/>
    </owl:NamedIndividual>
    


    <!-- http://securitytoolbox.appspot.com/stac#LowEnergyConsuming -->

    <owl:NamedIndividual rdf:about="&stac;LowEnergyConsuming">
        <rdf:type rdf:resource="&iotsec;PositiveFeature"/>
        <rdfs:label xml:lang="en">Low Energy Consuming</rdfs:label>
        <rdfs:comment xml:lang="en"></rdfs:comment>
    </owl:NamedIndividual>
    


    <!-- http://securitytoolbox.appspot.com/stac#MACAddressFiltering -->

    <owl:NamedIndividual rdf:about="&stac;MACAddressFiltering">
        <rdf:type rdf:resource="&iotsec;NetworkManagementSecurityMechanism"/>
        <rdfs:label xml:lang="en">MAC Address Filtering</rdfs:label>
        <rdfs:comment xml:lang="en">If a client&apos;s MAC address is not included in the list, the client will not be allowed to access the network.</rdfs:comment>
    </owl:NamedIndividual>
    


    <!-- http://securitytoolbox.appspot.com/stac#MAPSec -->

    <owl:NamedIndividual rdf:about="&stac;MAPSec">
        <rdf:type rdf:resource="&iotsec;Protocol"/>
        <rdf:type rdf:resource="&iotsec;UMTSSecurityMechanism"/>
        <rdfs:label xml:lang="en">Mobile Application Part (MAPSec)</rdfs:label>
        <rdfs:comment xml:lang="en">MAPSec protects existing signalling protocols and applications</rdfs:comment>
        <rdfs:comment xml:lang="en">See Paper: UMTS Security: Security in Core Network and UTRAN [Abid et al. 2002].</rdfs:comment>
        <iotsec:protectsInLayer rdf:resource="&iotsec;ApplicationLayer"/>
        <iotsec:satisfies rdf:resource="&iotsec;Confidentiality"/>
        <iotsec:satisfies rdf:resource="&iotsec;Integrity"/>
        <dcterms:hasPart rdf:resource="&iotsec;MapsecSA"/>
    </owl:NamedIndividual>
    


    <!-- http://securitytoolbox.appspot.com/stac#MD5 -->

    <owl:NamedIndividual rdf:about="&stac;MD5">
        <rdf:type rdf:resource="&iotsec;HashFunction"/>
        <rdf:type rdf:resource="&iotsec;ManetSecurityMechanism"/>
        <rdf:type rdf:resource="&iotsec;StreamCipher"/>
        <rdfs:label xml:lang="en">Message Digest 5 (MD5)</rdfs:label>
        <rdfs:comment xml:lang="en"></rdfs:comment>
        <owl:sameAs rdf:resource="&securitysw;MD5"/>
        <iotsec:satisfies rdf:resource="&iotsec;Authentication"/>
        <iotsec:satisfies rdf:resource="&iotsec;Integrity"/>
    </owl:NamedIndividual>
    


    <!-- http://securitytoolbox.appspot.com/stac#MILENAGE -->

    <owl:NamedIndividual rdf:about="&stac;MILENAGE">
        <rdf:type rdf:resource="&iotsec;UMTSSecurityAlgorithm"/>
        <rdfs:label xml:lang="en">MILENAGE</rdfs:label>
        <rdfs:comment xml:lang="en">Is a recommendation for AKA algorithms. MILENAGE is based on AES or Rijndael.</rdfs:comment>
        <rdfs:comment xml:lang="en">Paper: MILENAGE: An example of good UMTS Security [Massari 2009?]</rdfs:comment>
        <iotsec:hasFeature rdf:resource="&iotsec;Deprecated"/>
        <dcterms:hasPart rdf:resource="&iotsec;Rijndael"/>
    </owl:NamedIndividual>
    


    <!-- http://securitytoolbox.appspot.com/stac#MITM -->

    <owl:NamedIndividual rdf:about="&stac;MITM">
        <rdf:type rdf:resource="&iotsec;GPRSAttack"/>
        <rdf:type rdf:resource="&iotsec;RfidAttack"/>
        <rdf:type rdf:resource="&iotsec;Threat"/>
        <rdf:type rdf:resource="&iotsec;UMTSAttack"/>
        <rdfs:label xml:lang="en">Man-in-the-Middle (MITM) attack</rdfs:label>
        <rdfs:comment xml:lang="en">An attacker intrudes into the communication between the endpoints on a network to inject false information and intercept the data transferred between them. The attack allows an intruder to impersonate a valid GSM base station to a UMTS subscriber regardless of the fact that UMTS authentication and key agreement are used.</rdfs:comment>
        <rdfs:comment xml:lang="en">See Paper: Survey of Security and Privacy Issues of Internet of Things [Borgohain et al. 2015], Paper: A Man-in-the-Middle Attack on UMTS [Meyer 2004]. See Paper: Malicious actions against the GPRS technology [Xenakis 2006]</rdfs:comment>
        <iotsec:isVulnerabilityOf rdf:resource="&stac;BluetoothTechnology"/>
        <iotsec:hasSecurityMechanism rdf:resource="&stac;DigitalCertificate"/>
        <iotsec:isVulnerabilityOf rdf:resource="&stac;EDGETechnology"/>
        <iotsec:isVulnerabilityOf rdf:resource="&stac;EthernetTechnology"/>
        <iotsec:isVulnerabilityOf rdf:resource="&stac;GPRSTechnology"/>
        <iotsec:isVulnerabilityOf rdf:resource="&stac;GSMTechnology"/>
        <iotsec:isVulnerabilityOf rdf:resource="&stac;HSDPATechnology"/>
        <iotsec:isVulnerabilityOf rdf:resource="&stac;LTETechnology"/>
        <iotsec:isVulnerabilityOf rdf:resource="&stac;M2MTechnology"/>
        <iotsec:isVulnerabilityOf rdf:resource="&stac;ManetTechnology"/>
        <iotsec:isVulnerabilityOf rdf:resource="&stac;MeshTechnology"/>
        <iotsec:isVulnerabilityOf rdf:resource="&stac;RFIDTechnology"/>
        <iotsec:isVulnerabilityOf rdf:resource="&stac;SensorTechnology"/>
        <iotsec:isVulnerabilityOf rdf:resource="&stac;UMTSTechnology"/>
        <iotsec:isVulnerabilityOf rdf:resource="&stac;UWBTechnology"/>
        <iotsec:isVulnerabilityOf rdf:resource="&stac;WifiTechnology"/>
        <iotsec:isVulnerabilityOf rdf:resource="&stac;WimaxTechnology"/>
        <iotsec:isVulnerabilityOf rdf:resource="&stac;ZigbeeTechnology"/>
        <iotsec:hasSecurityMechanism rdf:resource="&iotsec;HTTPS"/>
        <iotsec:hasSecurityMechanism rdf:resource="&iotsec;PANA"/>
    </owl:NamedIndividual>
    


    <!-- http://securitytoolbox.appspot.com/stac#MSC -->

    <owl:NamedIndividual rdf:about="&stac;MSC">
        <rdf:type rdf:resource="&stac;GSMArchitectureComponent"/>
        <rdfs:label xml:lang="en">Mobile services Switching Center (MSC)</rdfs:label>
        <rdfs:comment xml:lang="en">Mobile services Switching Center (MSC) performs the switching of calls between the mobile users (mobile and fixed) one. The MSC also handles the mobility management operations.</rdfs:comment>
    </owl:NamedIndividual>
    


    <!-- http://securitytoolbox.appspot.com/stac#Mac -->

    <owl:NamedIndividual rdf:about="&stac;Mac">
        <rdf:type rdf:resource="&iotsec;OperatingSystemTechnology"/>
        <rdfs:label xml:lang="en">Mac</rdfs:label>
        <rdfs:comment xml:lang="en"></rdfs:comment>
    </owl:NamedIndividual>
    


    <!-- http://securitytoolbox.appspot.com/stac#MacAfee -->

    <owl:NamedIndividual rdf:about="&stac;MacAfee">
        <rdf:type rdf:resource="&iotsec;Antivirus"/>
        <rdf:type rdf:resource="&iotsec;Firewall"/>
        <rdfs:label xml:lang="en">MacAfee</rdfs:label>
        <rdfs:comment xml:lang="en"></rdfs:comment>
        <iotsec:satisfies rdf:resource="&iotsec;AccessControl"/>
        <iotsec:hasFeature rdf:resource="&iotsec;NotFree"/>
    </owl:NamedIndividual>
    


    <!-- http://securitytoolbox.appspot.com/stac#MapsecSA -->

    <owl:NamedIndividual rdf:about="&stac;MapsecSA">
        <rdf:type rdf:resource="&iotsec;UMTSSecurityMechanism"/>
        <rdfs:label xml:lang="en">MAPSec SA (Security Association)</rdfs:label>
        <rdfs:comment xml:lang="en">The SA contains cryptographic keys, key lifetimes, etc.</rdfs:comment>
    </owl:NamedIndividual>
    


    <!-- http://securitytoolbox.appspot.com/stac#MerkleHellman -->

    <owl:NamedIndividual rdf:about="&stac;MerkleHellman">
        <rdf:type rdf:resource="&iotsec;AsymmetricAlgorithm"/>
        <rdf:type rdf:resource="&iotsec;ManetSecurityMechanism"/>
        <rdfs:label xml:lang="en">Merkle-Hellman</rdfs:label>
        <rdfs:comment xml:lang="en"></rdfs:comment>
        <iotsec:satisfies rdf:resource="&iotsec;Authentication"/>
        <iotsec:satisfies rdf:resource="&iotsec;Confidentiality"/>
    </owl:NamedIndividual>
    


    <!-- http://securitytoolbox.appspot.com/stac#MeshAccessPoint -->

    <owl:NamedIndividual rdf:about="&stac;MeshAccessPoint">
        <rdf:type rdf:resource="&iotsec;MeshArchitectureComponent"/>
        <rdfs:label xml:lang="en">Mesh Access Point (MAP)</rdfs:label>
        <rdfs:comment xml:lang="en"></rdfs:comment>
    </owl:NamedIndividual>
    


    <!-- http://securitytoolbox.appspot.com/stac#MeshArchitecture -->

    <owl:NamedIndividual rdf:about="&stac;MeshArchitecture">
        <owl:sameAs rdf:resource="&iotsec;MeshArchitecture"/>
    </owl:NamedIndividual>
    


    <!-- http://securitytoolbox.appspot.com/stac#MeshClient -->

    <owl:NamedIndividual rdf:about="&stac;MeshClient">
        <rdf:type rdf:resource="&iotsec;MeshArchitectureComponent"/>
        <rdfs:label xml:lang="en">Mesh Client (MC)</rdfs:label>
        <rdfs:comment xml:lang="en"></rdfs:comment>
    </owl:NamedIndividual>
    


    <!-- http://securitytoolbox.appspot.com/stac#MeshGateway -->

    <owl:NamedIndividual rdf:about="&stac;MeshGateway">
        <rdf:type rdf:resource="&iotsec;MeshArchitectureComponent"/>
        <rdfs:label xml:lang="en">Mesh Gateway (MG)</rdfs:label>
        <rdfs:comment xml:lang="en">MGs provide connectivity to the wired infrastructure.</rdfs:comment>
    </owl:NamedIndividual>
    


    <!-- http://securitytoolbox.appspot.com/stac#MeshPointPortal -->

    <owl:NamedIndividual rdf:about="&stac;MeshPointPortal">
        <rdf:type rdf:resource="&iotsec;MeshArchitectureComponent"/>
        <rdfs:label xml:lang="en">Mesh Point Portal (MPP)</rdfs:label>
        <rdfs:comment xml:lang="en">Each Mesh Point chooses which Portal to use to get access to the external world.</rdfs:comment>
    </owl:NamedIndividual>
    


    <!-- http://securitytoolbox.appspot.com/stac#MeshRouter -->

    <owl:NamedIndividual rdf:about="&stac;MeshRouter">
        <rdf:type rdf:resource="&iotsec;MeshArchitectureComponent"/>
        <rdfs:label xml:lang="en">Mesh Router (MR)</rdfs:label>
        <rdfs:comment xml:lang="en">Mesh routers provide access to mobile users, like AP in Wifi.</rdfs:comment>
    </owl:NamedIndividual>
    


    <!-- http://securitytoolbox.appspot.com/stac#Metasploit -->

    <owl:NamedIndividual rdf:about="&stac;Metasploit">
        <rdf:type rdf:resource="&iotsec;NetworkManagementSecurityTool"/>
        <rdfs:label xml:lang="en">Metasploit</rdfs:label>
        <rdfs:comment xml:lang="en">The Metasploit Project is a computer security project that provides information about security vulnerabilities and aids in penetration testing and IDS signature development.</rdfs:comment>
        <iotsec:hasFeature rdf:resource="&iotsec;Free"/>
        <iotsec:hasFeature rdf:resource="&iotsec;Opensource"/>
    </owl:NamedIndividual>
    


    <!-- http://securitytoolbox.appspot.com/stac#MicaZ -->

    <owl:NamedIndividual rdf:about="&stac;MicaZ">
        <rdf:type rdf:resource="&iotsec;SensorTechnology"/>
        <rdfs:label xml:lang="en">MicaZ</rdfs:label>
        <rdfs:comment xml:lang="en">The MicaZ platform is largely diffused in the Wireless Sensor Networks community due to the reduced power consumption.</rdfs:comment>
    </owl:NamedIndividual>
    


    <!-- http://securitytoolbox.appspot.com/stac#Michael -->

    <owl:NamedIndividual rdf:about="&stac;Michael">
        <rdf:type rdf:resource="&iotsec;AsymmetricAlgorithm"/>
        <rdf:type rdf:resource="&iotsec;ManetSecurityMechanism"/>
        <rdfs:label xml:lang="en">Michael</rdfs:label>
        <rdfs:comment xml:lang="en"></rdfs:comment>
        <iotsec:satisfies rdf:resource="&iotsec;Authentication"/>
        <iotsec:satisfies rdf:resource="&iotsec;Confidentiality"/>
    </owl:NamedIndividual>
    


    <!-- http://securitytoolbox.appspot.com/stac#MiniSec -->

    <owl:NamedIndividual rdf:about="&stac;MiniSec">
        <rdf:type rdf:resource="&iotsec;SensorSecurityProtocol"/>
        <rdfs:label xml:lang="en">MiniSec</rdfs:label>
        <rdfs:comment xml:lang="en"></rdfs:comment>
        <rdfs:comment xml:lang="en">See Paper MiniSec: A secure Sensor Network Communication Architecture  [Perrig et al. 2007]</rdfs:comment>
        <iotsec:satisfies rdf:resource="&iotsec;Authentication"/>
        <iotsec:satisfies rdf:resource="&iotsec;Confidentiality"/>
        <iotsec:satisfies rdf:resource="&iotsec;DataFreshness"/>
        <iotsec:protectsInLayer rdf:resource="&iotsec;NetworkLayer"/>
        <dcterms:hasPart rdf:resource="&iotsec;OCB"/>
        <dcterms:hasPart rdf:resource="&iotsec;Skipjack"/>
    </owl:NamedIndividual>
    


    <!-- http://securitytoolbox.appspot.com/stac#Misc -->

    <owl:NamedIndividual rdf:about="&stac;Misc">
        <rdf:type rdf:resource="&iotsec;SecurityMagazine"/>
        <rdfs:label xml:lang="en">Misc (Multi-System and Internet Security Cookbook)</rdfs:label>
        <rdfs:comment xml:lang="en"></rdfs:comment>
    </owl:NamedIndividual>
    


    <!-- http://securitytoolbox.appspot.com/stac#MobiSec -->

    <owl:NamedIndividual rdf:about="&stac;MobiSec">
        <rdf:type rdf:resource="&iotsec;MeshSecurityMechanism"/>
        <rdfs:label xml:lang="en">MobiSEC</rdfs:label>
        <rdfs:comment xml:lang="en"></rdfs:comment>
    </owl:NamedIndividual>
    


    <!-- http://securitytoolbox.appspot.com/stac#MobileEquipment -->

    <owl:NamedIndividual rdf:about="&stac;MobileEquipment">
        <rdf:type rdf:resource="&stac;GSMArchitectureComponent"/>
        <rdfs:label xml:lang="en">Mobile Equipment (ME)</rdfs:label>
        <rdfs:comment xml:lang="en">Mobile Equipment (ME) is the mobile phone</rdfs:comment>
        <dcterms:hasPart rdf:resource="&iotsec;IMEI"/>
    </owl:NamedIndividual>
    


    <!-- http://securitytoolbox.appspot.com/stac#MobileStationIsdnNumber -->

    <owl:NamedIndividual rdf:about="&stac;MobileStationIsdnNumber">
        <rdf:type rdf:resource="&stac;GSMArchitectureComponent"/>
        <rdfs:label xml:lang="en">Mobile Station ISDN Number</rdfs:label>
        <rdfs:comment xml:lang="en"></rdfs:comment>
    </owl:NamedIndividual>
    


    <!-- http://securitytoolbox.appspot.com/stac#MobileTerminal -->

    <owl:NamedIndividual rdf:about="&stac;MobileTerminal">
        <rdf:type rdf:resource="&stac;GPRSArchitectureComponent"/>
        <rdfs:label xml:lang="en">MobileTerminal</rdfs:label>
        <rdfs:comment xml:lang="en"></rdfs:comment>
    </owl:NamedIndividual>
    


    <!-- http://securitytoolbox.appspot.com/stac#MongoDB -->

    <owl:NamedIndividual rdf:about="&stac;MongoDB">
        <rdf:type rdf:resource="&iotsec;DatabaseTechnology"/>
        <rdfs:label xml:lang="en">MongoDB</rdfs:label>
        <rdfs:comment xml:lang="en"></rdfs:comment>
    </owl:NamedIndividual>
    


    <!-- http://securitytoolbox.appspot.com/stac#Morris -->

    <owl:NamedIndividual rdf:about="&stac;Morris">
        <rdf:type rdf:resource="&iotsec;Worm"/>
        <rdfs:label xml:lang="en">Morris</rdfs:label>
        <rdfs:comment xml:lang="en"></rdfs:comment>
    </owl:NamedIndividual>
    


    <!-- http://securitytoolbox.appspot.com/stac#MultiPathRouting -->

    <owl:NamedIndividual rdf:about="&stac;MultiPathRouting">
        <rdf:type rdf:resource="&iotsec;SensorSecurityMechanism"/>
        <rdfs:label xml:lang="en">Multi Path Routing</rdfs:label>
        <rdfs:comment xml:lang="en"></rdfs:comment>
        <iotsec:protectsInLayer rdf:resource="&iotsec;NetworkLayer"/>
    </owl:NamedIndividual>
    


    <!-- http://securitytoolbox.appspot.com/stac#MySQL -->

    <owl:NamedIndividual rdf:about="&stac;MySQL">
        <rdf:type rdf:resource="&iotsec;DatabaseTechnology"/>
        <rdfs:label xml:lang="en">MySQL</rdfs:label>
        <rdfs:comment xml:lang="en"></rdfs:comment>
    </owl:NamedIndividual>
    


    <!-- http://securitytoolbox.appspot.com/stac#NSS -->

    <owl:NamedIndividual rdf:about="&stac;NSS">
        <rdf:type rdf:resource="&stac;GSMArchitectureComponent"/>
        <rdfs:label xml:lang="en">Network Subsystem (NSS)</rdfs:label>
        <rdfs:comment xml:lang="en">The NSS provides switching services between GSM and external networks.</rdfs:comment>
        <dcterms:hasPart rdf:resource="&iotsec;HLR"/>
        <dcterms:hasPart rdf:resource="&iotsec;MSC"/>
        <dcterms:hasPart rdf:resource="&iotsec;VLR"/>
    </owl:NamedIndividual>
    


    <!-- http://securitytoolbox.appspot.com/stac#NeedhamSchroeder -->

    <owl:NamedIndividual rdf:about="&stac;NeedhamSchroeder">
        <rdf:type rdf:resource="&iotsec;Protocol"/>
        <rdfs:label xml:lang="en">Needham-Schroeder</rdfs:label>
        <rdfs:comment xml:lang="en"></rdfs:comment>
    </owl:NamedIndividual>
    


    <!-- http://securitytoolbox.appspot.com/stac#Nessus -->

    <owl:NamedIndividual rdf:about="&stac;Nessus">
        <rdf:type rdf:resource="&iotsec;NetworkManagementSecurityTool"/>
        <rdfs:label xml:lang="en">Nessus</rdfs:label>
        <rdfs:comment xml:lang="en">Nessus is a vulnerability scanner. Its goal is to detect potential vulnerabilities on the tested systems.</rdfs:comment>
        <iotsec:hasFeature rdf:resource="&iotsec;NotFree"/>
    </owl:NamedIndividual>
    


    <!-- http://securitytoolbox.appspot.com/stac#NetworkLayer -->

    <owl:NamedIndividual rdf:about="&stac;NetworkLayer">
        <rdf:type rdf:resource="&iotsec;OSIModelLayer"/>
        <rdfs:label xml:lang="en">NetworkLayer</rdfs:label>
        <rdfs:comment xml:lang="en">The network layer handles the adressing and routing of the data.</rdfs:comment>
    </owl:NamedIndividual>
    


    <!-- http://securitytoolbox.appspot.com/stac#Nmap -->

    <owl:NamedIndividual rdf:about="&stac;Nmap">
        <rdf:type rdf:resource="&iotsec;NetworkManagementSecurityTool"/>
        <rdfs:label xml:lang="en">Nmap</rdfs:label>
        <rdfs:comment xml:lang="en">Nmap is a security scanner</rdfs:comment>
    </owl:NamedIndividual>
    


    <!-- http://securitytoolbox.appspot.com/stac#NoSQL -->

    <owl:NamedIndividual rdf:about="&stac;NoSQL">
        <rdf:type rdf:resource="&iotsec;DatabaseTechnology"/>
        <rdfs:label xml:lang="en">NoSQL</rdfs:label>
        <rdfs:comment xml:lang="en"></rdfs:comment>
    </owl:NamedIndividual>
    


    <!-- http://securitytoolbox.appspot.com/stac#NodeB -->

    <owl:NamedIndividual rdf:about="&stac;NodeB">
        <rdf:type rdf:resource="&iotsec;UMTSArchitectureComponent"/>
        <rdfs:label xml:lang="en">NodeB</rdfs:label>
        <rdfs:comment xml:lang="en">Node-Bs are the bases stations of the UMTS network. A node B is mainly responsible for the transmission and reception of data.</rdfs:comment>
    </owl:NamedIndividual>
    


    <!-- http://securitytoolbox.appspot.com/stac#NodeCapture -->

    <owl:NamedIndividual rdf:about="&stac;NodeCapture">
        <rdf:type rdf:resource="&iotsec;M2MAttack"/>
        <rdf:type rdf:resource="&iotsec;MeshAttack"/>
        <rdf:type rdf:resource="&iotsec;SensorAttack"/>
        <rdfs:label xml:lang="en">Node capture/Compromise/NodeReplication</rdfs:label>
        <rdfs:comment xml:lang="en">A node can be completely captured and manipulated by the adversary. Paper: An evaluation of security protocols on wireless sensor network [Ahmed et al. 2009]</rdfs:comment>
        <rdfs:comment xml:lang="en">Resilience against node capture is one of the most challeging problems in sensor networks.</rdfs:comment>
        <iotsec:hasSecurityMechanism rdf:resource="&iotsec;HidingNode"/>
        <iotsec:occursInLayer rdf:resource="&iotsec;PhysicalLayer"/>
        <iotsec:hasSecurityMechanism rdf:resource="&iotsec;TamperResistantHarware"/>
    </owl:NamedIndividual>
    


    <!-- http://securitytoolbox.appspot.com/stac#NonRepudiation -->

    <owl:NamedIndividual rdf:about="&stac;NonRepudiation">
        <rdf:type rdf:resource="&iotsec;SecurityProperty"/>
        <rdfs:label xml:lang="en">Non Repudiation</rdfs:label>
        <rdfs:comment xml:lang="en">Non repudiation means that a sender is unable to deny having sent a message or infoomation.</rdfs:comment>
        <owl:sameAs rdf:resource="&securitysw;NonRepudiation"/>
        <owl:sameAs rdf:resource="&herzog;Non-Repudiation"/>
    </owl:NamedIndividual>
    


    <!-- http://securitytoolbox.appspot.com/stac#Norton -->

    <owl:NamedIndividual rdf:about="&stac;Norton">
        <rdf:type rdf:resource="&iotsec;Antivirus"/>
        <rdf:type rdf:resource="&iotsec;Firewall"/>
        <rdfs:label xml:lang="en">Norton</rdfs:label>
        <rdfs:comment xml:lang="en"></rdfs:comment>
        <iotsec:satisfies rdf:resource="&iotsec;Integrity"/>
        <iotsec:hasFeature rdf:resource="&iotsec;NotFree"/>
    </owl:NamedIndividual>
    


    <!-- http://securitytoolbox.appspot.com/stac#NotFlexible -->

    <owl:NamedIndividual rdf:about="&stac;NotFlexible">
        <rdf:type rdf:resource="&iotsec;NegativeFeature"/>
        <rdfs:label xml:lang="en">Not Flexible</rdfs:label>
        <rdfs:comment xml:lang="en"></rdfs:comment>
    </owl:NamedIndividual>
    


    <!-- http://securitytoolbox.appspot.com/stac#NotFree -->

    <owl:NamedIndividual rdf:about="&stac;NotFree">
        <rdf:type rdf:resource="&iotsec;NegativeFeature"/>
        <rdfs:label xml:lang="en">NotFree</rdfs:label>
        <rdfs:comment xml:lang="en"></rdfs:comment>
    </owl:NamedIndividual>
    


    <!-- http://securitytoolbox.appspot.com/stac#NotScalable -->

    <owl:NamedIndividual rdf:about="&stac;NotScalable">
        <rdf:type rdf:resource="&iotsec;NegativeFeature"/>
        <rdfs:label xml:lang="en">Not Scalable</rdfs:label>
        <rdfs:comment xml:lang="en">Cannot scale for larger networks.</rdfs:comment>
    </owl:NamedIndividual>
    


    <!-- http://securitytoolbox.appspot.com/stac#NotSuitableHeterogeneousTechnology -->

    <owl:NamedIndividual rdf:about="&stac;NotSuitableHeterogeneousTechnology">
        <rdf:type rdf:resource="&iotsec;NegativeFeature"/>
        <rdfs:label xml:lang="en">Not suitable for heterogeneous technologies</rdfs:label>
        <rdfs:comment xml:lang="en"></rdfs:comment>
    </owl:NamedIndividual>
    


    <!-- http://securitytoolbox.appspot.com/stac#OAuth -->

    <owl:NamedIndividual rdf:about="&stac;OAuth">
        <rdf:type rdf:resource="&iotsec;WebSecurityMechanism"/>
        <rdfs:label xml:lang="en">OAuth</rdfs:label>
        <rdfs:comment xml:lang="en">OAuth is an authentication server, an open standard for authorization.</rdfs:comment>
        <iotsec:satisfies rdf:resource="&iotsec;Authorization"/>
    </owl:NamedIndividual>
    


    <!-- http://securitytoolbox.appspot.com/stac#OCB -->

    <owl:NamedIndividual rdf:about="&stac;OCB">
        <rdf:type rdf:resource="&iotsec;ModeOperation"/>
        <rdfs:label xml:lang="en">Offset Codebook (OCB)</rdfs:label>
        <rdfs:comment xml:lang="en"></rdfs:comment>
        <iotsec:satisfies rdf:resource="&iotsec;Authentication"/>
        <iotsec:satisfies rdf:resource="&iotsec;Confidentiality"/>
    </owl:NamedIndividual>
    


    <!-- http://securitytoolbox.appspot.com/stac#OFB -->

    <owl:NamedIndividual rdf:about="&stac;OFB">
        <rdf:type rdf:resource="&iotsec;ModeOperation"/>
        <rdfs:label xml:lang="en">Output Feddback Mode(OFB)</rdfs:label>
        <rdfs:comment xml:lang="en"></rdfs:comment>
    </owl:NamedIndividual>
    


    <!-- http://securitytoolbox.appspot.com/stac#OMAC -->

    <owl:NamedIndividual rdf:about="&stac;OMAC">
        <rdf:type rdf:resource="&iotsec;MAC"/>
        <rdf:type rdf:resource="&iotsec;ManetSecurityMechanism"/>
        <rdfs:label xml:lang="en">One-key Message Authentication Code (OMAC)</rdfs:label>
        <rdfs:comment xml:lang="en"></rdfs:comment>
        <dcterms:hasPart rdf:resource="&iotsec;AES"/>
        <iotsec:satisfies rdf:resource="&iotsec;DataFreshness"/>
    </owl:NamedIndividual>
    


    <!-- http://securitytoolbox.appspot.com/stac#OMC -->

    <owl:NamedIndividual rdf:about="&stac;OMC">
        <rdf:type rdf:resource="&stac;GSMArchitectureComponent"/>
        <rdfs:label xml:lang="en">Operations and Maintenance Center (OMC)</rdfs:label>
        <rdfs:comment xml:lang="en">Operations and Maintenance Center (OMC) supervises the proper operation and setup of the network.</rdfs:comment>
    </owl:NamedIndividual>
    


    <!-- http://securitytoolbox.appspot.com/stac#OSS -->

    <owl:NamedIndividual rdf:about="&stac;OSS">
        <rdf:type rdf:resource="&stac;GSMArchitectureComponent"/>
        <rdfs:label xml:lang="en">Operation Support Subsystem (OSS)</rdfs:label>
        <rdfs:comment xml:lang="en"></rdfs:comment>
        <dcterms:hasPart rdf:resource="&iotsec;Auc"/>
        <dcterms:hasPart rdf:resource="&iotsec;EIR"/>
        <dcterms:hasPart rdf:resource="&iotsec;OMC"/>
    </owl:NamedIndividual>
    


    <!-- http://securitytoolbox.appspot.com/stac#Oakley -->

    <owl:NamedIndividual rdf:about="&stac;Oakley">
        <rdf:type rdf:resource="&iotsec;KeyManagement"/>
        <rdf:type rdf:resource="&iotsec;Protocol"/>
        <rdfs:label xml:lang="en">Oakley (Oakley Key Determination Protocol)</rdfs:label>
        <rdfs:comment xml:lang="en">Oakley is a key-agreement protocol</rdfs:comment>
        <iotsec:satisfies rdf:resource="&iotsec;Authentication"/>
        <dcterms:hasPart rdf:resource="&iotsec;DiffieHellman"/>
    </owl:NamedIndividual>
    


    <!-- http://securitytoolbox.appspot.com/stac#ObjectiveC -->

    <owl:NamedIndividual rdf:about="&stac;ObjectiveC">
        <rdf:type rdf:resource="&iotsec;ProgrammingLanguageTechnology"/>
        <rdfs:label xml:lang="en">ObjectiveC</rdfs:label>
        <rdfs:comment xml:lang="en"></rdfs:comment>
    </owl:NamedIndividual>
    


    <!-- http://securitytoolbox.appspot.com/stac#OpenID -->

    <owl:NamedIndividual rdf:about="&stac;OpenID">
        <rdf:type rdf:resource="&iotsec;WebSecurityMechanism"/>
        <rdfs:label xml:lang="en">OpenID</rdfs:label>
        <rdfs:comment xml:lang="en">OpenID is an open standard that allows users to be authenticated by certain co-operating sites using a third party service, eliminating the need for webmasters to provide their own ad hoc systems and allowing users to consolidate their digital identities. </rdfs:comment>
        <iotsec:satisfies rdf:resource="&iotsec;Authentication"/>
        <iotsec:hasFeature rdf:resource="&iotsec;Popular"/>
    </owl:NamedIndividual>
    


    <!-- http://securitytoolbox.appspot.com/stac#OpenPGP -->

    <owl:NamedIndividual rdf:about="&stac;OpenPGP">
        <rdf:type rdf:resource="&iotsec;SecurityMechanism"/>
        <rdfs:label xml:lang="en">OpenPGP</rdfs:label>
        <rdfs:comment xml:lang="en"></rdfs:comment>
        <iotsec:protectsInLayer rdf:resource="&iotsec;ApplicationLayer"/>
        <iotsec:satisfies rdf:resource="&iotsec;Authentication"/>
        <iotsec:satisfies rdf:resource="&iotsec;Confidentiality"/>
        <iotsec:satisfies rdf:resource="&iotsec;Integrity"/>
    </owl:NamedIndividual>
    


    <!-- http://securitytoolbox.appspot.com/stac#Opensource -->

    <owl:NamedIndividual rdf:about="&stac;Opensource">
        <rdf:type rdf:resource="&iotsec;PositiveFeature"/>
        <rdfs:label xml:lang="en">Opensource</rdfs:label>
        <rdfs:comment xml:lang="en"></rdfs:comment>
    </owl:NamedIndividual>
    


    <!-- http://securitytoolbox.appspot.com/stac#OperatorNetwork -->

    <owl:NamedIndividual rdf:about="&stac;OperatorNetwork">
        <rdf:type rdf:resource="&iotsec;WimaxArchitectureComponent"/>
        <rdfs:label xml:lang="en">OperatorNetwork</rdfs:label>
        <rdfs:comment xml:lang="en"></rdfs:comment>
    </owl:NamedIndividual>
    


    <!-- http://securitytoolbox.appspot.com/stac#Oracle -->

    <owl:NamedIndividual rdf:about="&stac;Oracle">
        <rdf:type rdf:resource="&iotsec;DatabaseTechnology"/>
        <rdfs:label xml:lang="en">Oracle</rdfs:label>
        <rdfs:comment xml:lang="en"></rdfs:comment>
    </owl:NamedIndividual>
    


    <!-- http://securitytoolbox.appspot.com/stac#P3P -->

    <owl:NamedIndividual rdf:about="&stac;P3P">
        <rdf:type rdf:resource="&iotsec;SecurityMechanism"/>
        <rdfs:label xml:lang="en">Platform for Privacy Preferences (P3P)</rdfs:label>
        <rdfs:comment xml:lang="en">Provides a language for description of privacy preferences.</rdfs:comment>
        <iotsec:satisfies rdf:resource="&iotsec;Confidentiality"/>
    </owl:NamedIndividual>
    


    <!-- http://securitytoolbox.appspot.com/stac#PANA -->

    <owl:NamedIndividual rdf:about="&stac;PANA">
        <rdf:type rdf:resource="&iotsec;MeshSecurityProtocol"/>
        <rdf:type rdf:resource="&iotsec;SecurityMechanism"/>
        <rdfs:label xml:lang="en">Protocol for Carrying Authentication for Network Access (PANA)</rdfs:label>
        <rdfs:comment xml:lang="en">PANA is applicable to any network technologies.</rdfs:comment>
        <rdfs:comment xml:lang="en">Paper: Evaluation of security attacks on UMTS authentication mechanism [Mobarhan 2012]</rdfs:comment>
        <dcterms:hasPart rdf:resource="&iotsec;EAP"/>
        <iotsec:protectsInLayer rdf:resource="&iotsec;NetworkLayer"/>
        <iotsec:hasFeature rdf:resource="&iotsec;SuitableHeterogeneousTechnology"/>
    </owl:NamedIndividual>
    


    <!-- http://securitytoolbox.appspot.com/stac#PAP -->

    <owl:NamedIndividual rdf:about="&stac;PAP">
        <rdf:type rdf:resource="&iotsec;Protocol"/>
        <rdfs:label xml:lang="en">Password Authentication Protocol (PAP)</rdfs:label>
        <rdfs:comment xml:lang="en">Is an authentication protocol that uses a password.</rdfs:comment>
        <iotsec:satisfies rdf:resource="&iotsec;Authentication"/>
        <iotsec:protectsInLayer rdf:resource="&iotsec;LinkLayer"/>
    </owl:NamedIndividual>
    


    <!-- http://securitytoolbox.appspot.com/stac#PCBC -->

    <owl:NamedIndividual rdf:about="&stac;PCBC">
        <rdf:type rdf:resource="&iotsec;ModeOperation"/>
        <rdfs:label xml:lang="en">Propagating Cipher-Block Chaining (PCBC)</rdfs:label>
        <rdfs:comment xml:lang="en"></rdfs:comment>
    </owl:NamedIndividual>
    


    <!-- http://securitytoolbox.appspot.com/stac#PEAP -->

    <owl:NamedIndividual rdf:about="&stac;PEAP">
        <rdf:type rdf:resource="&iotsec;WifiSecurityProtocol"/>
        <rdfs:label xml:lang="en">PEAP (Protected Extensible Authentication Protocol)</rdfs:label>
        <rdfs:comment xml:lang="en"></rdfs:comment>
        <iotsec:hasFeature rdf:resource="&stac;NotFlexible"/>
        <iotsec:satisfies rdf:resource="&iotsec;Authentication"/>
    </owl:NamedIndividual>
    


    <!-- http://securitytoolbox.appspot.com/stac#PGP -->

    <owl:NamedIndividual rdf:about="&stac;PGP">
        <rdf:type rdf:resource="&iotsec;MessageEncryptionTool"/>
        <rdf:type rdf:resource="&iotsec;SecurityMechanism"/>
        <rdfs:label xml:lang="en">Pretty Good Privacy (PGP)</rdfs:label>
        <rdfs:comment xml:lang="en">PGP is a data encryption and decryption computer program that provides privacy and authentication for data communication.</rdfs:comment>
        <iotsec:satisfies rdf:resource="&iotsec;Confidentiality"/>
        <iotsec:hasFeature rdf:resource="&iotsec;NotFree"/>
    </owl:NamedIndividual>
    


    <!-- http://securitytoolbox.appspot.com/stac#PHP -->

    <owl:NamedIndividual rdf:about="&stac;PHP">
        <rdf:type rdf:resource="&iotsec;ProgrammingLanguageTechnology"/>
        <rdfs:label xml:lang="en">PHP</rdfs:label>
        <rdfs:comment xml:lang="en"></rdfs:comment>
    </owl:NamedIndividual>
    


    <!-- http://securitytoolbox.appspot.com/stac#PIKE -->

    <owl:NamedIndividual rdf:about="&stac;PIKE">
        <rdf:type rdf:resource="&iotsec;KeyManagement"/>
        <rdfs:label xml:lang="en">Peer intermediates scheme for key establishment protocol (PIKE)</rdfs:label>
        <rdfs:comment xml:lang="en"></rdfs:comment>
        <iotsec:satisfies rdf:resource="&iotsec;Authentication"/>
    </owl:NamedIndividual>
    


    <!-- http://securitytoolbox.appspot.com/stac#PIN -->

    <owl:NamedIndividual rdf:about="&stac;PIN">
        <rdf:type rdf:resource="&stac;GSMArchitectureComponent"/>
        <rdfs:label xml:lang="en">Personal Identification Number (PIN)</rdfs:label>
        <rdfs:comment xml:lang="en">PIN: a secret numeric password shared between a user and a system that can be used to authenticate the user to the system.</rdfs:comment>
        <iotsec:satisfies rdf:resource="&iotsec;Authentication"/>
    </owl:NamedIndividual>
    


    <!-- http://securitytoolbox.appspot.com/stac#PKM -->

    <owl:NamedIndividual rdf:about="&stac;PKM">
        <rdf:type rdf:resource="&iotsec;WimaxKeyManagement"/>
        <rdfs:label xml:lang="en">Privacy and Key Management Protocol (PKM)</rdfs:label>
        <rdfs:comment xml:lang="en"></rdfs:comment>
        <dcterms:hasPart rdf:resource="&iotsec;AES"/>
        <iotsec:satisfies rdf:resource="&iotsec;Authentication"/>
        <dcterms:hasPart rdf:resource="&iotsec;RSA"/>
        <dcterms:hasPart rdf:resource="&iotsec;X_509"/>
    </owl:NamedIndividual>
    


    <!-- http://securitytoolbox.appspot.com/stac#PMAC -->

    <owl:NamedIndividual rdf:about="&stac;PMAC">
        <rdf:type rdf:resource="&iotsec;MAC"/>
        <rdf:type rdf:resource="&iotsec;ManetSecurityMechanism"/>
        <rdfs:label xml:lang="en">Parrallelizable Message Authentication Code (PMAC)</rdfs:label>
        <rdfs:comment xml:lang="en"></rdfs:comment>
    </owl:NamedIndividual>
    


    <!-- http://securitytoolbox.appspot.com/stac#PMK -->

    <owl:NamedIndividual rdf:about="&stac;PMK">
        <rdf:type rdf:resource="&iotsec;MeshKeyManagement"/>
        <rdf:type rdf:resource="&iotsec;WifiKeyManagement"/>
        <rdfs:label xml:lang="en">Pairwise Master Key (PMK)</rdfs:label>
        <rdfs:comment xml:lang="en"></rdfs:comment>
        <iotsec:satisfies rdf:resource="&iotsec;Authentication"/>
    </owl:NamedIndividual>
    


    <!-- http://securitytoolbox.appspot.com/stac#PSK -->

    <owl:NamedIndividual rdf:about="&stac;PSK">
        <rdf:type rdf:resource="&iotsec;WifiKeyManagement"/>
        <rdfs:label xml:lang="en">Pre Shared Key (PSK)</rdfs:label>
        <rdfs:comment xml:lang="en"></rdfs:comment>
        <iotsec:satisfies rdf:resource="&iotsec;Authentication"/>
    </owl:NamedIndividual>
    


    <!-- http://securitytoolbox.appspot.com/stac#PTK -->

    <owl:NamedIndividual rdf:about="&stac;PTK">
        <rdf:type rdf:resource="&iotsec;WifiKeyManagement"/>
        <rdfs:label xml:lang="en">Pairwise Transient Key (PTK)</rdfs:label>
        <rdfs:comment xml:lang="en"></rdfs:comment>
        <iotsec:satisfies rdf:resource="&iotsec;Authentication"/>
    </owl:NamedIndividual>
    


    <!-- http://securitytoolbox.appspot.com/stac#PacketLeaches -->

    <owl:NamedIndividual rdf:about="&stac;PacketLeaches">
        <rdf:type rdf:resource="&iotsec;SensorSecurityMechanism"/>
        <rdfs:label xml:lang="en">Packet Leaches</rdfs:label>
        <rdfs:comment xml:lang="en"></rdfs:comment>
        <iotsec:protectsInLayer rdf:resource="&iotsec;NetworkLayer"/>
    </owl:NamedIndividual>
    


    <!-- http://securitytoolbox.appspot.com/stac#PacketSwitched -->

    <owl:NamedIndividual rdf:about="&stac;PacketSwitched">
        <rdf:type rdf:resource="&iotsec;UMTSArchitectureComponent"/>
        <rdfs:label xml:lang="en">Packet Switched</rdfs:label>
        <rdfs:comment xml:lang="en"></rdfs:comment>
        <dcterms:hasPart rdf:resource="&iotsec;SGSN"/>
    </owl:NamedIndividual>
    


    <!-- http://securitytoolbox.appspot.com/stac#PairwiseKey -->

    <owl:NamedIndividual rdf:about="&stac;PairwiseKey">
        <rdf:type rdf:resource="&iotsec;SymmetricSensorKey"/>
        <rdfs:label xml:lang="en">Pairwise Key</rdfs:label>
        <rdfs:comment xml:lang="en">Every node shares a pairwise key with each of its immediate neighbors. IN LEAP, pairwise keys are used for securing communications that require privacy or source authentication. In many sensor networks, the immediate neighbors of a sensor node cannot be predicted in advance; consequently, these pairwise shared keys will need to be established after the network is deployed.</rdfs:comment>
    </owl:NamedIndividual>
    


    <!-- http://securitytoolbox.appspot.com/stac#ParkingLot -->

    <owl:NamedIndividual rdf:about="&stac;ParkingLot">
        <rdf:type rdf:resource="&iotsec;WifiAttack"/>
        <rdfs:label xml:lang="en">Parking Lot</rdfs:label>
        <rdfs:comment xml:lang="en">Signals can be intercepted outside buildings.</rdfs:comment>
    </owl:NamedIndividual>
    


    <!-- http://securitytoolbox.appspot.com/stac#PhysicalLayer -->

    <owl:NamedIndividual rdf:about="&stac;PhysicalLayer">
        <rdf:type rdf:resource="&iotsec;OSIModelLayer"/>
        <rdfs:label xml:lang="en">Physical Layer</rdfs:label>
        <rdfs:comment xml:lang="en">The physical layer defines the electrical and physical specifications of the data connection.</rdfs:comment>
    </owl:NamedIndividual>
    


    <!-- http://securitytoolbox.appspot.com/stac#Pointcheval-Stern -->

    <owl:NamedIndividual rdf:about="&stac;Pointcheval-Stern">
        <rdf:type rdf:resource="&iotsec;DigitalSignature"/>
        <rdfs:label xml:lang="en">Pointcheval-Stern</rdfs:label>
        <rdfs:comment xml:lang="en"></rdfs:comment>
        <iotsec:satisfies rdf:resource="&iotsec;Authentication"/>
        <iotsec:satisfies rdf:resource="&iotsec;Integrity"/>
        <iotsec:satisfies rdf:resource="&iotsec;NonRepudiation"/>
    </owl:NamedIndividual>
    


    <!-- http://securitytoolbox.appspot.com/stac#Popular -->

    <owl:NamedIndividual rdf:about="&stac;Popular">
        <rdf:type rdf:resource="&iotsec;PositiveFeature"/>
        <rdfs:label xml:lang="en">Popular</rdfs:label>
        <rdfs:comment xml:lang="en"></rdfs:comment>
    </owl:NamedIndividual>
    


    <!-- http://securitytoolbox.appspot.com/stac#PostgreSQL -->

    <owl:NamedIndividual rdf:about="&stac;PostgreSQL">
        <rdf:type rdf:resource="&iotsec;DatabaseTechnology"/>
        <rdfs:label xml:lang="en">PostgreSQL</rdfs:label>
        <rdfs:comment xml:lang="en"></rdfs:comment>
    </owl:NamedIndividual>
    


    <!-- http://securitytoolbox.appspot.com/stac#Prelude -->

    <owl:NamedIndividual rdf:about="&stac;Prelude">
        <rdf:type rdf:resource="&iotsec;IDS"/>
        <rdfs:label xml:lang="en">Prelude</rdfs:label>
        <rdfs:comment xml:lang="en"></rdfs:comment>
        <iotsec:protectsInLayer rdf:resource="&iotsec;ApplicationLayer"/>
        <iotsec:satisfies rdf:resource="&iotsec;Availability"/>
    </owl:NamedIndividual>
    


    <!-- http://securitytoolbox.appspot.com/stac#PresentationLayer -->

    <owl:NamedIndividual rdf:about="&stac;PresentationLayer">
        <rdf:type rdf:resource="&iotsec;OSIModelLayer"/>
        <rdfs:label xml:lang="en">Presentation Layer</rdfs:label>
        <rdfs:comment xml:lang="en">The presentation layer is usually part of an operating system (OS) and converts incoming and outgoing data from one presentation format to another.</rdfs:comment>
    </owl:NamedIndividual>
    


    <!-- http://securitytoolbox.appspot.com/stac#ProGuard -->

    <owl:NamedIndividual rdf:about="&stac;ProGuard">
        <rdf:type rdf:resource="&iotsec;Obfuscation"/>
        <rdfs:label xml:lang="en">ProGuard</rdfs:label>
        <rdfs:comment xml:lang="en"></rdfs:comment>
    </owl:NamedIndividual>
    


    <!-- http://securitytoolbox.appspot.com/stac#PublicKeyInfrastructure -->

    <owl:NamedIndividual rdf:about="&stac;PublicKeyInfrastructure">
        <rdf:type rdf:resource="&iotsec;AsymmetricAlgorithm"/>
        <rdf:type rdf:resource="&iotsec;DigitalCertificate"/>
        <rdf:type rdf:resource="&iotsec;KeyManagement"/>
        <rdfs:label xml:lang="en">Public Key Infrastructure (PKI)</rdfs:label>
        <rdfs:comment xml:lang="en">Public Key Infrastructure (PKI) is used for authentication.</rdfs:comment>
        <iotsec:protectsInLayer rdf:resource="&iotsec;ApplicationLayer"/>
        <iotsec:satisfies rdf:resource="&iotsec;Authentication"/>
        <iotsec:satisfies rdf:resource="&iotsec;Integrity"/>
        <iotsec:satisfies rdf:resource="&iotsec;NonRepudiation"/>
    </owl:NamedIndividual>
    


    <!-- http://securitytoolbox.appspot.com/stac#Python -->

    <owl:NamedIndividual rdf:about="&stac;Python">
        <rdf:type rdf:resource="&iotsec;ProgrammingLanguageTechnology"/>
        <rdfs:label xml:lang="en">Python</rdfs:label>
        <rdfs:comment xml:lang="en"></rdfs:comment>
    </owl:NamedIndividual>
    


    <!-- http://securitytoolbox.appspot.com/stac#RADIUS -->

    <owl:NamedIndividual rdf:about="&stac;RADIUS">
        <rdf:type rdf:resource="&iotsec;AuthenticationServer"/>
        <rdf:type rdf:resource="&iotsec;ManetSecurityMechanism"/>
        <rdf:type rdf:resource="&iotsec;WifiSecurityMechanism"/>
        <rdfs:label xml:lang="en">Remote Authentication Dial In User Service (RADIUS)</rdfs:label>
        <rdfs:comment xml:lang="en">RADIUS is a client/server protocol.</rdfs:comment>
        <iotsec:satisfies rdf:resource="&iotsec;Accountability"/>
        <iotsec:protectsInLayer rdf:resource="&iotsec;ApplicationLayer"/>
        <iotsec:satisfies rdf:resource="&iotsec;Authentication"/>
        <iotsec:satisfies rdf:resource="&iotsec;Authorization"/>
        <iotsec:isReplacedBy rdf:resource="&iotsec;Diameter"/>
    </owl:NamedIndividual>
    


    <!-- http://securitytoolbox.appspot.com/stac#RAI -->

    <owl:NamedIndividual rdf:about="&stac;RAI">
        <rdf:type rdf:resource="&stac;GPRSArchitectureComponent"/>
        <rdfs:label xml:lang="en">Routing Area Identity (RAI)</rdfs:label>
        <rdfs:comment xml:lang="en"></rdfs:comment>
    </owl:NamedIndividual>
    


    <!-- http://securitytoolbox.appspot.com/stac#RAND -->

    <owl:NamedIndividual rdf:about="&stac;RAND">
        <rdf:type rdf:resource="&stac;GSMArchitectureComponent"/>
        <rdfs:label xml:lang="en">RAND</rdfs:label>
        <rdfs:comment xml:lang="en"></rdfs:comment>
    </owl:NamedIndividual>
    


    <!-- http://securitytoolbox.appspot.com/stac#RC4 -->

    <owl:NamedIndividual rdf:about="&stac;RC4">
        <rdf:type rdf:resource="&iotsec;ManetSecurityMechanism"/>
        <rdf:type rdf:resource="&iotsec;StreamCipher"/>
        <rdfs:label xml:lang="en">Rivest Cypher 4 (RC4)</rdfs:label>
        <rdfs:comment xml:lang="en">RC4 is used in the WEP protocol in WiFi</rdfs:comment>
        <iotsec:satisfies rdf:resource="&iotsec;Confidentiality"/>
        <iotsec:hasFeature rdf:resource="&iotsec;Deprecated"/>
    </owl:NamedIndividual>
    


    <!-- http://securitytoolbox.appspot.com/stac#RC5 -->

    <owl:NamedIndividual rdf:about="&stac;RC5">
        <rdf:type rdf:resource="&iotsec;ManetSecurityMechanism"/>
        <rdf:type rdf:resource="&iotsec;StreamCipher"/>
        <rdfs:label xml:lang="en">RC5</rdfs:label>
        <rdfs:comment xml:lang="en"></rdfs:comment>
        <iotsec:satisfies rdf:resource="&iotsec;Confidentiality"/>
    </owl:NamedIndividual>
    


    <!-- http://securitytoolbox.appspot.com/stac#RC6 -->

    <owl:NamedIndividual rdf:about="&stac;RC6">
        <rdf:type rdf:resource="&iotsec;ManetSecurityMechanism"/>
        <rdf:type rdf:resource="&iotsec;StreamCipher"/>
        <rdfs:label xml:lang="en">RC6</rdfs:label>
        <rdfs:comment xml:lang="en"></rdfs:comment>
        <iotsec:satisfies rdf:resource="&iotsec;Confidentiality"/>
    </owl:NamedIndividual>
    


    <!-- http://securitytoolbox.appspot.com/stac#RIPE-MD -->

    <owl:NamedIndividual rdf:about="&stac;RIPE-MD">
        <rdf:type rdf:resource="&iotsec;HashFunction"/>
        <rdf:type rdf:resource="&iotsec;ManetSecurityMechanism"/>
        <rdfs:label xml:lang="en">Security Hash Algorithm (RIPE-MD)</rdfs:label>
        <rdfs:comment xml:lang="en"></rdfs:comment>
        <owl:sameAs rdf:resource="&securitysw;RIPE-MD"/>
        <iotsec:satisfies rdf:resource="&iotsec;Authentication"/>
        <iotsec:satisfies rdf:resource="&iotsec;Integrity"/>
    </owl:NamedIndividual>
    


    <!-- http://securitytoolbox.appspot.com/stac#RNC -->

    <owl:NamedIndividual rdf:about="&stac;RNC">
        <rdf:type rdf:resource="&iotsec;UMTSArchitectureComponent"/>
        <rdfs:label xml:lang="en">Radio Network Controller (RNC)</rdfs:label>
        <rdfs:comment xml:lang="en">The RNC is responsible for control of the Node-Bs.</rdfs:comment>
    </owl:NamedIndividual>
    


    <!-- http://securitytoolbox.appspot.com/stac#RSA -->

    <owl:NamedIndividual rdf:about="&stac;RSA">
        <rdf:type rdf:resource="&iotsec;AsymmetricAlgorithm"/>
        <rdf:type rdf:resource="&iotsec;DigitalSignature"/>
        <rdf:type rdf:resource="&iotsec;KeyManagement"/>
        <rdf:type rdf:resource="&iotsec;ManetSecurityMechanism"/>
        <rdfs:label xml:lang="en">Rivest Shamir Adleman (RSA)</rdfs:label>
        <rdfs:comment xml:lang="en"></rdfs:comment>
        <owl:sameAs rdf:resource="&securitysw;RSAAlgorithm"/>
        <iotsec:satisfies rdf:resource="&iotsec;Authentication"/>
        <iotsec:satisfies rdf:resource="&iotsec;Confidentiality"/>
    </owl:NamedIndividual>
    


    <!-- http://securitytoolbox.appspot.com/stac#RSN -->

    <owl:NamedIndividual rdf:about="&stac;RSN">
        <rdf:type rdf:resource="&iotsec;WifiArchitectureComponent"/>
        <rdfs:label xml:lang="en">Robust Security Network (RSN)</rdfs:label>
        <rdfs:comment xml:lang="en"></rdfs:comment>
    </owl:NamedIndividual>
    


    <!-- http://securitytoolbox.appspot.com/stac#RSS -->

    <owl:NamedIndividual rdf:about="&stac;RSS">
        <rdf:type rdf:resource="&stac;GSMArchitectureComponent"/>
        <rdfs:label xml:lang="en">Radio Subsystem (RSS)</rdfs:label>
        <rdfs:comment xml:lang="en">The RSS deals with all the radio aspects of a network.</rdfs:comment>
        <dcterms:hasPart rdf:resource="&iotsec;BaseStationSubsystem"/>
        <dcterms:hasPart rdf:resource="&iotsec;GSMMobileStation"/>
    </owl:NamedIndividual>
    


    <!-- http://securitytoolbox.appspot.com/stac#Rabin -->

    <owl:NamedIndividual rdf:about="&stac;Rabin">
        <rdf:type rdf:resource="&iotsec;DigitalSignature"/>
        <rdfs:label xml:lang="en">Rabin</rdfs:label>
        <rdfs:comment xml:lang="en"></rdfs:comment>
        <iotsec:satisfies rdf:resource="&iotsec;Authentication"/>
        <iotsec:satisfies rdf:resource="&iotsec;Integrity"/>
        <iotsec:satisfies rdf:resource="&iotsec;NonRepudiation"/>
    </owl:NamedIndividual>
    


    <!-- http://securitytoolbox.appspot.com/stac#RadioResourceTesting -->

    <owl:NamedIndividual rdf:about="&stac;RadioResourceTesting">
        <rdf:type rdf:resource="&iotsec;SensorSecurityMechanism"/>
        <rdfs:label xml:lang="en">Radio Resource Testing</rdfs:label>
        <rdfs:comment xml:lang="en"></rdfs:comment>
        <iotsec:protectsInLayer rdf:resource="&iotsec;NetworkLayer"/>
    </owl:NamedIndividual>
    


    <!-- http://securitytoolbox.appspot.com/stac#RadioSpectrumMonitoringEquipment -->

    <owl:NamedIndividual rdf:about="&stac;RadioSpectrumMonitoringEquipment">
        <rdf:type rdf:resource="&iotsec;SecurityMechanism"/>
        <rdfs:label xml:lang="en">Radio Spectrum Monitoring Equipment</rdfs:label>
        <rdfs:comment xml:lang="en"></rdfs:comment>
    </owl:NamedIndividual>
    


    <!-- http://securitytoolbox.appspot.com/stac#RandomKeyDistribution -->

    <owl:NamedIndividual rdf:about="&stac;RandomKeyDistribution">
        <rdf:type rdf:resource="&iotsec;KeyManagement"/>
        <rdfs:label xml:lang="en">Random Key Distribution</rdfs:label>
        <rdfs:comment xml:lang="en"></rdfs:comment>
        <iotsec:satisfies rdf:resource="&iotsec;Authentication"/>
    </owl:NamedIndividual>
    


    <!-- http://securitytoolbox.appspot.com/stac#RandomKeyPredistribution -->

    <owl:NamedIndividual rdf:about="&stac;RandomKeyPredistribution">
        <rdf:type rdf:resource="&iotsec;SensorSecurityMechanism"/>
        <rdfs:label xml:lang="en">Random Key Predistribution</rdfs:label>
        <rdfs:comment xml:lang="en">Associates the identity of the node to the keys assigned to it and validate the keys to see if the node is really who it claims to be.</rdfs:comment>
        <iotsec:protectsInLayer rdf:resource="&iotsec;NetworkLayer"/>
    </owl:NamedIndividual>
    


    <!-- http://securitytoolbox.appspot.com/stac#RansomWare -->

    <owl:NamedIndividual rdf:about="&stac;RansomWare">
        <rdf:type rdf:resource="&iotsec;WebAttack"/>
        <rdfs:label xml:lang="en">RansomWare</rdfs:label>
        <rdfs:comment xml:lang="en"></rdfs:comment>
        <iotsec:occursInLayer rdf:resource="&iotsec;ApplicationLayer"/>
    </owl:NamedIndividual>
    


    <!-- http://securitytoolbox.appspot.com/stac#RateLimitation -->

    <owl:NamedIndividual rdf:about="&stac;RateLimitation">
        <rdf:type rdf:resource="&iotsec;SensorSecurityMechanism"/>
        <rdfs:label xml:lang="en">Rate Limitation</rdfs:label>
        <rdfs:comment xml:lang="en"></rdfs:comment>
        <iotsec:protectsInLayer rdf:resource="&iotsec;LinkLayer"/>
    </owl:NamedIndividual>
    


    <!-- http://securitytoolbox.appspot.com/stac#Registration -->

    <owl:NamedIndividual rdf:about="&stac;Registration">
        <rdf:type rdf:resource="&iotsec;SensorSecurityMechanism"/>
        <rdfs:label xml:lang="en">Registration Identity</rdfs:label>
        <rdfs:comment xml:lang="en">Registration of the node identities at a central base station.</rdfs:comment>
        <iotsec:protectsInLayer rdf:resource="&iotsec;NetworkLayer"/>
    </owl:NamedIndividual>
    


    <!-- http://securitytoolbox.appspot.com/stac#RelayStation -->

    <owl:NamedIndividual rdf:about="&stac;RelayStation">
        <rdf:type rdf:resource="&iotsec;WimaxArchitectureComponent"/>
        <rdfs:label xml:lang="en">Relay Station (RS)</rdfs:label>
        <rdfs:comment xml:lang="en"></rdfs:comment>
    </owl:NamedIndividual>
    


    <!-- http://securitytoolbox.appspot.com/stac#ReplayAttack -->

    <owl:NamedIndividual rdf:about="&stac;ReplayAttack">
        <rdf:type rdf:resource="&iotsec;RfidAttack"/>
        <rdf:type rdf:resource="&iotsec;SensorAttack"/>
        <rdf:type rdf:resource="&iotsec;WimaxAttack"/>
        <rdfs:label xml:lang="en">Replay Attack</rdfs:label>
        <rdfs:comment xml:lang="en"></rdfs:comment>
        <rdfs:comment xml:lang="en">See Paper: Survey of Security and Privacy Issues of Internet of Things [Borgohain et al. 2015, Paper: An evaluation of security protocols on wireless sensor network [Ahmed et al. 2009]</rdfs:comment>
        <iotsec:isVulnerabilityOf rdf:resource="&stac;BluetoothTechnology"/>
        <iotsec:isVulnerabilityOf rdf:resource="&stac;EDGETechnology"/>
        <iotsec:isVulnerabilityOf rdf:resource="&stac;EthernetTechnology"/>
        <iotsec:isVulnerabilityOf rdf:resource="&stac;GPRSTechnology"/>
        <iotsec:isVulnerabilityOf rdf:resource="&stac;GSMTechnology"/>
        <iotsec:isVulnerabilityOf rdf:resource="&stac;HSDPATechnology"/>
        <iotsec:isVulnerabilityOf rdf:resource="&stac;LTETechnology"/>
        <iotsec:isVulnerabilityOf rdf:resource="&stac;M2MTechnology"/>
        <iotsec:isVulnerabilityOf rdf:resource="&stac;ManetTechnology"/>
        <iotsec:isVulnerabilityOf rdf:resource="&stac;MeshTechnology"/>
        <iotsec:isVulnerabilityOf rdf:resource="&stac;RFIDTechnology"/>
        <iotsec:isVulnerabilityOf rdf:resource="&stac;SensorTechnology"/>
        <iotsec:isVulnerabilityOf rdf:resource="&stac;UMTSTechnology"/>
        <iotsec:isVulnerabilityOf rdf:resource="&stac;UWBTechnology"/>
        <iotsec:isVulnerabilityOf rdf:resource="&stac;WifiTechnology"/>
        <iotsec:isVulnerabilityOf rdf:resource="&stac;WimaxTechnology"/>
        <iotsec:isVulnerabilityOf rdf:resource="&stac;ZigbeeTechnology"/>
        <iotsec:threatens rdf:resource="&iotsec;Availability"/>
        <iotsec:hasSecurityMechanism rdf:resource="&iotsec;CHAP"/>
        <iotsec:threatens rdf:resource="&iotsec;Freshness"/>
        <iotsec:hasSecurityMechanism rdf:resource="&iotsec;Kerberos"/>
        <iotsec:occursInLayer rdf:resource="&iotsec;NetworkLayer"/>
    </owl:NamedIndividual>
    


    <!-- http://securitytoolbox.appspot.com/stac#ResourceConstraint -->

    <owl:NamedIndividual rdf:about="&stac;ResourceConstraint">
        <rdf:type rdf:resource="&iotsec;Feature"/>
        <rdfs:label xml:lang="en">Resource Constraint</rdfs:label>
        <rdfs:comment xml:lang="en"></rdfs:comment>
    </owl:NamedIndividual>
    


    <!-- http://securitytoolbox.appspot.com/stac#RetroGuard -->

    <owl:NamedIndividual rdf:about="&stac;RetroGuard">
        <rdf:type rdf:resource="&iotsec;Obfuscation"/>
        <rdfs:label xml:lang="en">RetroGuard</rdfs:label>
        <rdfs:comment xml:lang="en"></rdfs:comment>
    </owl:NamedIndividual>
    


    <!-- http://securitytoolbox.appspot.com/stac#Rijndael -->

    <owl:NamedIndividual rdf:about="&stac;Rijndael">
        <rdf:type rdf:resource="&iotsec;BlockCipher"/>
        <rdf:type rdf:resource="&iotsec;ManetSecurityMechanism"/>
        <rdfs:label xml:lang="en">Rijndael</rdfs:label>
        <rdfs:comment xml:lang="en">Its suitability for smart card implementations.</rdfs:comment>
        <iotsec:satisfies rdf:resource="&iotsec;Confidentiality"/>
    </owl:NamedIndividual>
    


    <!-- http://securitytoolbox.appspot.com/stac#Rogue -->

    <owl:NamedIndividual rdf:about="&stac;Rogue">
        <rdf:type rdf:resource="&iotsec;WebAttack"/>
        <rdfs:label xml:lang="en">Rogue</rdfs:label>
        <rdfs:comment xml:lang="en"></rdfs:comment>
        <iotsec:occursInLayer rdf:resource="&iotsec;ApplicationLayer"/>
    </owl:NamedIndividual>
    


    <!-- http://securitytoolbox.appspot.com/stac#RogueAP -->

    <owl:NamedIndividual rdf:about="&stac;RogueAP">
        <rdf:type rdf:resource="&iotsec;WifiAttack"/>
        <rdfs:label xml:lang="en">Rogue Access Point </rdfs:label>
        <rdfs:comment xml:lang="en"></rdfs:comment>
    </owl:NamedIndividual>
    


    <!-- http://securitytoolbox.appspot.com/stac#RogueBaseStation -->

    <owl:NamedIndividual rdf:about="&stac;RogueBaseStation">
        <rdf:type rdf:resource="&iotsec;GSMAttack"/>
        <rdf:type rdf:resource="&iotsec;WimaxAttack"/>
        <rdfs:label xml:lang="en">Rogue Base Station </rdfs:label>
        <rdfs:comment xml:lang="en"></rdfs:comment>
        <iotsec:isVulnerabilityOf rdf:resource="&stac;GSMTechnology"/>
        <iotsec:isVulnerabilityOf rdf:resource="&stac;WimaxTechnology"/>
    </owl:NamedIndividual>
    


    <!-- http://securitytoolbox.appspot.com/stac#RogueReader -->

    <owl:NamedIndividual rdf:about="&stac;RogueReader">
        <rdf:type rdf:resource="&iotsec;RfidAttack"/>
        <rdfs:label xml:lang="en">Rogue Reader </rdfs:label>
        <rdfs:comment xml:lang="en"></rdfs:comment>
    </owl:NamedIndividual>
    


    <!-- http://securitytoolbox.appspot.com/stac#Rootkit -->

    <owl:NamedIndividual rdf:about="&stac;Rootkit">
        <rdf:type rdf:resource="&iotsec;WebAttack"/>
        <rdfs:label xml:lang="en">Rootkit</rdfs:label>
        <rdfs:comment xml:lang="en"></rdfs:comment>
        <iotsec:occursInLayer rdf:resource="&iotsec;ApplicationLayer"/>
    </owl:NamedIndividual>
    


    <!-- http://securitytoolbox.appspot.com/stac#RoutingTableOverflow -->

    <owl:NamedIndividual rdf:about="&stac;RoutingTableOverflow">
        <rdf:type rdf:resource="&iotsec;MeshAttack"/>
        <rdfs:label xml:lang="en">Routing Table Overflow</rdfs:label>
        <rdfs:comment xml:lang="en"></rdfs:comment>
        <iotsec:occursInLayer rdf:resource="&iotsec;NetworkLayer"/>
    </owl:NamedIndividual>
    


    <!-- http://securitytoolbox.appspot.com/stac#RubyOnRails -->

    <owl:NamedIndividual rdf:about="&stac;RubyOnRails">
        <rdf:type rdf:resource="&iotsec;FrameworkTechnology"/>
        <rdfs:label xml:lang="en">Ruby On Rails</rdfs:label>
        <rdfs:comment xml:lang="en"></rdfs:comment>
    </owl:NamedIndividual>
    


    <!-- http://securitytoolbox.appspot.com/stac#Rushing -->

    <owl:NamedIndividual rdf:about="&stac;Rushing">
        <rdf:type rdf:resource="&iotsec;M2MAttack"/>
        <rdfs:label xml:lang="en">Rushing</rdfs:label>
        <rdfs:comment xml:lang="en"></rdfs:comment>
        <iotsec:occursInLayer rdf:resource="&iotsec;NetworkLayer"/>
    </owl:NamedIndividual>
    


    <!-- http://securitytoolbox.appspot.com/stac#SAE -->

    <owl:NamedIndividual rdf:about="&stac;SAE">
        <rdf:type rdf:resource="&iotsec;LoginPassword"/>
        <rdf:type rdf:resource="&iotsec;MeshSecurityMechanism"/>
        <rdfs:label xml:lang="en">Simultaneous Authentication of Equals (SAE)</rdfs:label>
        <rdfs:comment xml:lang="en"></rdfs:comment>
        <dcterms:hasPart rdf:resource="&iotsec;ECC"/>
        <dcterms:hasPart rdf:resource="&iotsec;PMK"/>
    </owl:NamedIndividual>
    


    <!-- http://securitytoolbox.appspot.com/stac#SCHEME -->

    <owl:NamedIndividual rdf:about="&stac;SCHEME">
        <rdf:type rdf:resource="&iotsec;Protocol"/>
        <rdfs:label xml:lang="en">SCHEME</rdfs:label>
        <rdfs:comment xml:lang="en"></rdfs:comment>
    </owl:NamedIndividual>
    


    <!-- http://securitytoolbox.appspot.com/stac#SEAL -->

    <owl:NamedIndividual rdf:about="&stac;SEAL">
        <rdf:type rdf:resource="&iotsec;ManetSecurityMechanism"/>
        <rdf:type rdf:resource="&iotsec;StreamCipher"/>
        <rdfs:label xml:lang="en">Software-Opitmized Encryption algorithm (SEAL)</rdfs:label>
        <rdfs:comment xml:lang="en"></rdfs:comment>
        <iotsec:satisfies rdf:resource="&iotsec;Confidentiality"/>
    </owl:NamedIndividual>
    


    <!-- http://securitytoolbox.appspot.com/stac#SET -->

    <owl:NamedIndividual rdf:about="&stac;SET">
        <rdf:type rdf:resource="&iotsec;WebSecurityMechanism"/>
        <rdfs:label xml:lang="en">Secure Electronic Transaction (SET)</rdfs:label>
        <rdfs:comment xml:lang="en">SET is protocol for securing credit card transactions over insecure networks (e.g., Internet).</rdfs:comment>
        <iotsec:protectsInLayer rdf:resource="&iotsec;ApplicationLayer"/>
        <iotsec:satisfies rdf:resource="&iotsec;Authentication"/>
        <iotsec:satisfies rdf:resource="&iotsec;Confidentiality"/>
        <dcterms:hasPart rdf:resource="&iotsec;DES"/>
        <iotsec:satisfies rdf:resource="&iotsec;Integrity"/>
    </owl:NamedIndividual>
    


    <!-- http://securitytoolbox.appspot.com/stac#SGSN -->

    <owl:NamedIndividual rdf:about="&stac;SGSN">
        <rdf:type rdf:resource="&stac;GPRSArchitectureComponent"/>
        <rdfs:label xml:lang="en">Serving GPRS Support Node (SGSN)</rdfs:label>
        <rdfs:comment xml:lang="en">The SGSN handles the traffic of IP packets addressed to and from a mobile station that is attached within the SGSN service area</rdfs:comment>
    </owl:NamedIndividual>
    


    <!-- http://securitytoolbox.appspot.com/stac#SHA -->

    <owl:NamedIndividual rdf:about="&stac;SHA">
        <rdf:type rdf:resource="&iotsec;HashFunction"/>
        <rdf:type rdf:resource="&iotsec;ManetSecurityMechanism"/>
        <rdfs:label xml:lang="en">Secure Hash Algorithm (SHA)</rdfs:label>
        <rdfs:comment xml:lang="en"></rdfs:comment>
        <owl:sameAs rdf:resource="&securitysw;SHA1"/>
        <iotsec:satisfies rdf:resource="&iotsec;Authentication"/>
        <iotsec:satisfies rdf:resource="&iotsec;Integrity"/>
    </owl:NamedIndividual>
    


    <!-- http://securitytoolbox.appspot.com/stac#SIM -->

    <owl:NamedIndividual rdf:about="&stac;SIM">
        <rdf:type rdf:resource="&stac;GSMArchitectureComponent"/>
        <rdfs:label xml:lang="en">Subscriber Identity Module (SIM)</rdfs:label>
        <rdfs:comment xml:lang="en">SIM cards provide the security mechanism for GSM. SIM cards are like credit cards and identify the user to the GSM network.</rdfs:comment>
        <dcterms:hasPart rdf:resource="&iotsec;A3"/>
        <dcterms:hasPart rdf:resource="&iotsec;A8"/>
        <dcterms:hasPart rdf:resource="&iotsec;IMSI"/>
        <dcterms:hasPart rdf:resource="&iotsec;MobileStationIsdnNumber"/>
    </owl:NamedIndividual>
    


    <!-- http://securitytoolbox.appspot.com/stac#SMIME -->

    <owl:NamedIndividual rdf:about="&stac;SMIME">
        <rdf:type rdf:resource="&iotsec;SecurityMechanism"/>
        <rdfs:label xml:lang="en">Secure/Multipurpose Internet Mail Extension (S/MIME)</rdfs:label>
        <rdfs:comment xml:lang="en"></rdfs:comment>
        <iotsec:protectsInLayer rdf:resource="&iotsec;ApplicationLayer"/>
        <iotsec:satisfies rdf:resource="&iotsec;Authentication"/>
        <iotsec:satisfies rdf:resource="&iotsec;Confidentiality"/>
        <iotsec:satisfies rdf:resource="&iotsec;Integrity"/>
        <iotsec:satisfies rdf:resource="&iotsec;NonRepudiation"/>
    </owl:NamedIndividual>
    


    <!-- http://securitytoolbox.appspot.com/stac#SPINS -->

    <owl:NamedIndividual rdf:about="&stac;SPINS">
        <rdf:type rdf:resource="&iotsec;SensorSecurityProtocol"/>
        <rdfs:label xml:lang="en">SPINS</rdfs:label>
        <rdfs:comment xml:lang="en">See SPINS: Security Protocols for Sensor Networks  [Perrig et al. 2001]</rdfs:comment>
        <iotsec:protectsInLayer rdf:resource="&iotsec;LinkLayer"/>
        <dcterms:hasPart rdf:resource="&iotsec;RC6"/>
        <dcterms:hasPart rdf:resource="&iotsec;SNEP"/>
        <dcterms:hasPart rdf:resource="&iotsec;microTESLA"/>
    </owl:NamedIndividual>
    


    <!-- http://securitytoolbox.appspot.com/stac#SQLInjection -->

    <owl:NamedIndividual rdf:about="&stac;SQLInjection">
        <rdf:type rdf:resource="&iotsec;DatabaseAttack"/>
        <rdf:type rdf:resource="&iotsec;WebAttack"/>
        <rdfs:label xml:lang="en">SQL Injection</rdfs:label>
        <rdfs:comment xml:lang="en"></rdfs:comment>
        <iotsec:hasSecurityMechanism rdf:resource="&stac;Firewall"/>
        <iotsec:occursInLayer rdf:resource="&iotsec;ApplicationLayer"/>
    </owl:NamedIndividual>
    


    <!-- http://securitytoolbox.appspot.com/stac#SQLLite -->

    <owl:NamedIndividual rdf:about="&stac;SQLLite">
        <rdf:type rdf:resource="&iotsec;DatabaseTechnology"/>
        <rdfs:label xml:lang="en">SQLLite</rdfs:label>
        <rdfs:comment xml:lang="en"></rdfs:comment>
    </owl:NamedIndividual>
    


    <!-- http://securitytoolbox.appspot.com/stac#SQLSlammer -->

    <owl:NamedIndividual rdf:about="&stac;SQLSlammer">
        <rdf:type rdf:resource="&iotsec;OperatingSystemAttack"/>
        <rdf:type rdf:resource="&iotsec;Worm"/>
        <rdfs:label xml:lang="en">SQLSlammer worm.</rdfs:label>
        <rdfs:comment xml:lang="en">SQLSlammer worm took advantage of a Microsoft SQL server protocol vulnerability.</rdfs:comment>
    </owl:NamedIndividual>
    


    <!-- http://securitytoolbox.appspot.com/stac#SRES -->

    <owl:NamedIndividual rdf:about="&stac;SRES">
        <rdf:type rdf:resource="&stac;GSMArchitectureComponent"/>
        <rdfs:label xml:lang="en">Signed Response (SRES)</rdfs:label>
        <rdfs:comment xml:lang="en"></rdfs:comment>
    </owl:NamedIndividual>
    


    <!-- http://securitytoolbox.appspot.com/stac#SSH -->

    <owl:NamedIndividual rdf:about="&stac;SSH">
        <rdf:type rdf:resource="&iotsec;Protocol"/>
        <rdf:type rdf:resource="&iotsec;WebSecurityMechanism"/>
        <rdfs:label xml:lang="en">Secure Shell (SSH)</rdfs:label>
        <rdfs:comment xml:lang="en">SSH is the now ubiquitous program for logging into or executing commands on a remote machine. It provides secure encrypted communications between two untrusted hosts over an insecure network.</rdfs:comment>
        <iotsec:protectsInLayer rdf:resource="&iotsec;ApplicationLayer"/>
        <dcterms:hasPart rdf:resource="&iotsec;AsymmetricAlgorithm"/>
        <iotsec:satisfies rdf:resource="&iotsec;Authentication"/>
        <iotsec:satisfies rdf:resource="&iotsec;Confidentiality"/>
        <iotsec:satisfies rdf:resource="&iotsec;Integrity"/>
        <iotsec:hasFeature rdf:resource="&iotsec;Popular"/>
    </owl:NamedIndividual>
    


    <!-- http://securitytoolbox.appspot.com/stac#SSID -->

    <owl:NamedIndividual rdf:about="&stac;SSID">
        <rdf:type rdf:resource="&iotsec;WifiArchitectureComponent"/>
        <rdfs:label xml:lang="en">Service Set Identifier (SSID)</rdfs:label>
        <rdfs:comment xml:lang="en">Different networks are identified by SSIDs, SSID is basically a network name.</rdfs:comment>
        <iotsec:satisfies rdf:resource="&iotsec;AccessControl"/>
    </owl:NamedIndividual>
    


    <!-- http://securitytoolbox.appspot.com/stac#SSL -->

    <owl:NamedIndividual rdf:about="&stac;SSL">
        <rdf:type rdf:resource="&iotsec;ManetSecurityMechanism"/>
        <rdf:type rdf:resource="&iotsec;Protocol"/>
        <rdf:type rdf:resource="&iotsec;WebSecurityMechanism"/>
        <rdfs:label xml:lang="en">Secure Socket Layer (SSL)</rdfs:label>
        <rdfs:comment xml:lang="en">SSL is used by web browsers to secure transactions within web applications. Transport Layer Security (TLS) and its predecessor, Secure Sockets Layer (SSL), are cryptographic protocols which are designed to provide communication security over the Internet. They use X.509 certificates and hence asymmetric cryptography to assure the counterparty with whom they are communicating, and to exchange a symmetric key. </rdfs:comment>
        <iotsec:satisfies rdf:resource="&iotsec;Authentication"/>
        <iotsec:satisfies rdf:resource="&iotsec;Confidentiality"/>
        <iotsec:satisfies rdf:resource="&iotsec;Integrity"/>
        <dcterms:hasPart rdf:resource="&iotsec;PublicKeyInfrastructure"/>
        <iotsec:isReplacedBy rdf:resource="&iotsec;TLS"/>
        <iotsec:protectsInLayer rdf:resource="&iotsec;TransportLayer"/>
    </owl:NamedIndividual>
    


    <!-- http://securitytoolbox.appspot.com/stac#SYNFlooding -->

    <owl:NamedIndividual rdf:about="&stac;SYNFlooding">
        <rdf:type rdf:resource="&iotsec;Flooding"/>
        <rdf:type rdf:resource="&iotsec;ManetAttack"/>
        <rdfs:label xml:lang="en">SYN Flooding</rdfs:label>
        <rdfs:comment xml:lang="en"></rdfs:comment>
        <iotsec:occursInLayer rdf:resource="&iotsec;TransportLayer"/>
    </owl:NamedIndividual>
    


    <!-- http://securitytoolbox.appspot.com/stac#Scalable -->

    <owl:NamedIndividual rdf:about="&stac;Scalable">
        <rdf:type rdf:resource="&iotsec;PositiveFeature"/>
    </owl:NamedIndividual>
    


    <!-- http://securitytoolbox.appspot.com/stac#Schnorr -->

    <owl:NamedIndividual rdf:about="&stac;Schnorr">
        <rdf:type rdf:resource="&iotsec;DigitalSignature"/>
        <rdfs:label xml:lang="en">Schnorr</rdfs:label>
        <rdfs:comment xml:lang="en"></rdfs:comment>
        <iotsec:satisfies rdf:resource="&iotsec;Authentication"/>
        <iotsec:satisfies rdf:resource="&iotsec;Integrity"/>
        <iotsec:satisfies rdf:resource="&iotsec;NonRepudiation"/>
    </owl:NamedIndividual>
    


    <!-- http://securitytoolbox.appspot.com/stac#Scrambling -->

    <owl:NamedIndividual rdf:about="&stac;Scrambling">
        <rdf:type rdf:resource="&iotsec;WimaxAttack"/>
        <rdfs:label xml:lang="en">Scrambling</rdfs:label>
        <rdfs:comment xml:lang="en">Scrambling is a kind of jamming, but for short intervals of time and targeted to specific frames or parts of frames.</rdfs:comment>
        <iotsec:occursInLayer rdf:resource="&iotsec;PhysicalLayer"/>
    </owl:NamedIndividual>
    


    <!-- http://securitytoolbox.appspot.com/stac#SecureUML -->

    <owl:NamedIndividual rdf:about="&stac;SecureUML">
        <rdf:type rdf:resource="&iotsec;FrameworkSecurityMechanism"/>
        <rdfs:label xml:lang="en">SecureUML</rdfs:label>
        <rdfs:comment xml:lang="en"></rdfs:comment>
    </owl:NamedIndividual>
    


    <!-- http://securitytoolbox.appspot.com/stac#Secured -->

    <owl:NamedIndividual rdf:about="&stac;Secured">
        <rdf:type rdf:resource="&iotsec;PositiveFeature"/>
        <rdfs:label xml:lang="en">Secured</rdfs:label>
        <rdfs:comment xml:lang="en"></rdfs:comment>
    </owl:NamedIndividual>
    


    <!-- http://securitytoolbox.appspot.com/stac#SelectiveForwarding -->

    <owl:NamedIndividual rdf:about="&stac;SelectiveForwarding">
        <rdf:type rdf:resource="&iotsec;M2MAttack"/>
        <rdf:type rdf:resource="&iotsec;MeshAttack"/>
        <rdf:type rdf:resource="&iotsec;SensorAttack"/>
        <rdfs:label xml:lang="en">Selective Forwarding</rdfs:label>
        <rdfs:comment xml:lang="en">Malicious nodes may ensure that certain messages are not transmitted by simply forwarding a few packets and dropping the remaining one.</rdfs:comment>
        <rdfs:comment xml:lang="en">See Paper: Survey of Security and Privacy Issues of Internet of Things [Borgohain et al. 2015]</rdfs:comment>
        <iotsec:hasSecurityMechanism rdf:resource="&iotsec;LLSP"/>
        <iotsec:hasSecurityMechanism rdf:resource="&iotsec;MultiPathRouting"/>
        <iotsec:occursInLayer rdf:resource="&iotsec;NetworkLayer"/>
    </owl:NamedIndividual>
    


    <!-- http://securitytoolbox.appspot.com/stac#SemanticSecurity -->

    <owl:NamedIndividual rdf:about="&stac;SemanticSecurity">
        <rdf:type rdf:resource="&iotsec;SecurityProperty"/>
        <rdfs:label xml:lang="en">Semantic Security</rdfs:label>
        <rdfs:comment xml:lang="en">Semantic security ensures that an eavesdropper has no information about the message, even if it sees multiple encryptions of the same messages.</rdfs:comment>
    </owl:NamedIndividual>
    


    <!-- http://securitytoolbox.appspot.com/stac#SequenceNumber -->

    <owl:NamedIndividual rdf:about="&stac;SequenceNumber">
        <rdf:type rdf:resource="&iotsec;UMTSArchitectureComponent"/>
        <rdfs:label xml:lang="en">Sequence Number (SQN)</rdfs:label>
        <rdfs:comment xml:lang="en"></rdfs:comment>
        <iotsec:satisfies rdf:resource="&iotsec;DataFreshness"/>
    </owl:NamedIndividual>
    


    <!-- http://securitytoolbox.appspot.com/stac#Serpent -->

    <owl:NamedIndividual rdf:about="&stac;Serpent">
        <rdf:type rdf:resource="&iotsec;BlockCipher"/>
        <rdf:type rdf:resource="&iotsec;ManetSecurityMechanism"/>
        <rdfs:label xml:lang="en">Serpent</rdfs:label>
        <rdfs:comment xml:lang="en"></rdfs:comment>
        <iotsec:satisfies rdf:resource="&iotsec;Confidentiality"/>
    </owl:NamedIndividual>
    


    <!-- http://securitytoolbox.appspot.com/stac#Sesame -->

    <owl:NamedIndividual rdf:about="&stac;Sesame">
        <rdf:type rdf:resource="&iotsec;FrameworkTechnology"/>
        <rdfs:label xml:lang="en">Sesame</rdfs:label>
        <rdfs:comment xml:lang="en"></rdfs:comment>
    </owl:NamedIndividual>
    


    <!-- http://securitytoolbox.appspot.com/stac#SessionHijacking -->

    <owl:NamedIndividual rdf:about="&stac;SessionHijacking">
        <rdf:type rdf:resource="&iotsec;WebAttack"/>
        <rdfs:label xml:lang="en">Session Hijacking</rdfs:label>
        <rdfs:comment xml:lang="en">To access mobile communication services on the target&apos;s account.</rdfs:comment>
        <iotsec:isVulnerabilityOf rdf:resource="&stac;WebTechnology"/>
        <iotsec:occursInLayer rdf:resource="&iotsec;ApplicationLayer"/>
    </owl:NamedIndividual>
    


    <!-- http://securitytoolbox.appspot.com/stac#SessionLayer -->

    <owl:NamedIndividual rdf:about="&stac;SessionLayer">
        <rdf:type rdf:resource="&iotsec;OSIModelLayer"/>
        <rdfs:label xml:lang="en">Session Layer</rdfs:label>
        <rdfs:comment xml:lang="en">The session layer controls the dialogues between computers.</rdfs:comment>
    </owl:NamedIndividual>
    


    <!-- http://securitytoolbox.appspot.com/stac#Shell -->

    <owl:NamedIndividual rdf:about="&stac;Shell">
        <rdf:type rdf:resource="&iotsec;ProgrammingLanguageTechnology"/>
        <rdfs:label xml:lang="en">Shell</rdfs:label>
        <rdfs:comment xml:lang="en"></rdfs:comment>
    </owl:NamedIndividual>
    


    <!-- http://securitytoolbox.appspot.com/stac#SideChannel -->

    <owl:NamedIndividual rdf:about="&stac;SideChannel">
        <rdf:type rdf:resource="&iotsec;Threat"/>
        <rdfs:label xml:lang="en">Side Channel</rdfs:label>
        <rdfs:comment xml:lang="en">Side channel attack is any attack based on information gained from the physical implementation of a cryptosystem.</rdfs:comment>
    </owl:NamedIndividual>
    


    <!-- http://securitytoolbox.appspot.com/stac#Sinkhole -->

    <owl:NamedIndividual rdf:about="&stac;Sinkhole">
        <rdf:type rdf:resource="&iotsec;M2MAttack"/>
        <rdf:type rdf:resource="&iotsec;MeshAttack"/>
        <rdf:type rdf:resource="&iotsec;SensorAttack"/>
        <rdfs:label xml:lang="en">Sinkhole</rdfs:label>
        <rdfs:comment xml:lang="en">An attacker tries to attract all neighboring nodes to establish routes though a malicious node. Once the attacker is successfuk in the sinkhole attack, then the network, is also open to other attacks, for example, eavesdropping or selective forwarding. Sinkhole attacks are very hard to detect.</rdfs:comment>
        <iotsec:hasSecurityMechanism rdf:resource="&iotsec;LLSP"/>
        <iotsec:occursInLayer rdf:resource="&iotsec;NetworkLayer"/>
        <iotsec:hasSecurityMechanism rdf:resource="&iotsec;Watchdog"/>
    </owl:NamedIndividual>
    


    <!-- http://securitytoolbox.appspot.com/stac#Skipjack -->

    <owl:NamedIndividual rdf:about="&stac;Skipjack">
        <rdf:type rdf:resource="&iotsec;BlockCipher"/>
        <rdf:type rdf:resource="&iotsec;ManetSecurityMechanism"/>
        <rdfs:label xml:lang="en">Skipjack</rdfs:label>
        <rdfs:comment xml:lang="en"></rdfs:comment>
        <iotsec:satisfies rdf:resource="&iotsec;Confidentiality"/>
    </owl:NamedIndividual>
    


    <!-- http://securitytoolbox.appspot.com/stac#SmallFrame -->

    <owl:NamedIndividual rdf:about="&stac;SmallFrame">
        <rdf:type rdf:resource="&iotsec;SensorSecurityMechanism"/>
        <rdfs:label xml:lang="en">Small Frame</rdfs:label>
        <rdfs:comment xml:lang="en">Small frames are used so that an individual node can capture the channel only for a short time.</rdfs:comment>
        <iotsec:protectsInLayer rdf:resource="&iotsec;LinkLayer"/>
    </owl:NamedIndividual>
    


    <!-- http://securitytoolbox.appspot.com/stac#Sniffing -->

    <owl:NamedIndividual rdf:about="&stac;Sniffing">
        <rdf:type rdf:resource="&iotsec;Threat"/>
        <rdf:type rdf:resource="&iotsec;UMTSAttack"/>
        <rdfs:label xml:lang="en">Sniffing</rdfs:label>
        <rdfs:comment xml:lang="en">See Paper: UMTS Security: Security in Core Network and UTRAN [Abid et al. 2002]</rdfs:comment>
        <rdfs:comment xml:lang="en">Sniffing means that hacker aim to collect information (e.g. password)</rdfs:comment>
    </owl:NamedIndividual>
    


    <!-- http://securitytoolbox.appspot.com/stac#Snort -->

    <owl:NamedIndividual rdf:about="&stac;Snort">
        <rdf:type rdf:resource="&iotsec;IDS"/>
        <rdf:type rdf:resource="&iotsec;IPS"/>
        <rdfs:label xml:lang="en">Snort</rdfs:label>
        <rdfs:comment xml:lang="en">Snort is a network intrusion detection and prevention system and excels at traffic analysis and packet logging on IP networks. Snort detects thousands of worms, vulnerability exploit attempts, port scans, and other suspicious behavior.</rdfs:comment>
        <iotsec:protectsInLayer rdf:resource="&iotsec;ApplicationLayer"/>
        <iotsec:satisfies rdf:resource="&iotsec;Availability"/>
        <iotsec:hasFeature rdf:resource="&iotsec;Free"/>
        <iotsec:hasFeature rdf:resource="&iotsec;Opensource"/>
        <iotsec:hasFeature rdf:resource="&iotsec;Popular"/>
    </owl:NamedIndividual>
    


    <!-- http://securitytoolbox.appspot.com/stac#SocialEngineering -->

    <owl:NamedIndividual rdf:about="&stac;SocialEngineering">
        <rdf:type rdf:resource="&iotsec;UMTSAttack"/>
        <rdf:type rdf:resource="&iotsec;WebAttack"/>
        <rdfs:label xml:lang="en">Social Engineering</rdfs:label>
        <rdfs:comment xml:lang="en">See Paper: UMTS Security: Security in Core Network and UTRAN [Abid et al. 2002]</rdfs:comment>
        <rdfs:comment xml:lang="en">Social engineering can be weird calls or mails where the caller explains the need of a user ID and password to an equipment there and the responsible is on holiday or unreachable.</rdfs:comment>
        <iotsec:hasSecurityMechanism rdf:resource="&stac;AuthenticationMethod"/>
        <iotsec:occursInLayer rdf:resource="&iotsec;ApplicationLayer"/>
        <iotsec:threatens rdf:resource="&iotsec;Authentication"/>
    </owl:NamedIndividual>
    


    <!-- http://securitytoolbox.appspot.com/stac#Spoofed -->

    <owl:NamedIndividual rdf:about="&stac;Spoofed">
        <rdf:type rdf:resource="&iotsec;SensorAttack"/>
        <rdfs:label xml:lang="en">Spoofed</rdfs:label>
        <rdfs:comment xml:lang="en">Routing information exchanged between sensor nodes is spoofed by an attacker.</rdfs:comment>
        <iotsec:threatens rdf:resource="&iotsec;Authentication"/>
        <iotsec:occursInLayer rdf:resource="&iotsec;NetworkLayer"/>
    </owl:NamedIndividual>
    


    <!-- http://securitytoolbox.appspot.com/stac#SpoofingAddress -->

    <owl:NamedIndividual rdf:about="&stac;SpoofingAddress">
        <rdf:type rdf:resource="&iotsec;ManetAttack"/>
        <rdf:type rdf:resource="&iotsec;MeshAttack"/>
        <rdf:type rdf:resource="&iotsec;RfidAttack"/>
        <rdf:type rdf:resource="&iotsec;SensorAttack"/>
        <rdf:type rdf:resource="&iotsec;Threat"/>
        <rdf:type rdf:resource="&iotsec;UMTSAttack"/>
        <rdf:type rdf:resource="&iotsec;WifiAttack"/>
        <rdfs:label xml:lang="en">Spoofing/Impersonation IP or MAC Address</rdfs:label>
        <rdfs:comment xml:lang="en">See Survey of Security and Privacy Issues of Internet of Things [Borgohain et al. 2015], Paper: Survey of Security and Privacy Issues of Internet of Things [Borgohain et al. 2015], Paper: UMTS Security: Security in Core Network and UTRAN [Abid et al. 2002]</rdfs:comment>
        <rdfs:comment xml:lang="en">Spoofing means that hackers use someone else&apos;s IP address and receives packets from the other users.</rdfs:comment>
        <iotsec:hasSecurityMechanism rdf:resource="&stac;Firewall"/>
        <iotsec:hasSecurityMechanism rdf:resource="&stac;PANA"/>
        <iotsec:hasSecurityMechanism rdf:resource="&stac;VPN"/>
        <iotsec:threatens rdf:resource="&iotsec;Authentication"/>
        <iotsec:occursInLayer rdf:resource="&iotsec;NetworkLayer"/>
    </owl:NamedIndividual>
    


    <!-- http://securitytoolbox.appspot.com/stac#SpreadSpectrumCommunication -->

    <owl:NamedIndividual rdf:about="&stac;SpreadSpectrumCommunication">
        <rdf:type rdf:resource="&iotsec;SecurityMechanism"/>
        <rdfs:label xml:lang="en">Spread Spectrum Communication</rdfs:label>
        <rdfs:comment xml:lang="en">A modulation technique where the transmission signal is spreading over a wide range of the radio spectrum. Resilience to jamming can be augmented by increasing the power of signals using spreding techniques.</rdfs:comment>
    </owl:NamedIndividual>
    


    <!-- http://securitytoolbox.appspot.com/stac#Spring -->

    <owl:NamedIndividual rdf:about="&stac;Spring">
        <rdf:type rdf:resource="&iotsec;FrameworkTechnology"/>
        <rdfs:label xml:lang="en">Spring</rdfs:label>
        <rdfs:comment xml:lang="en"></rdfs:comment>
        <rdfs:comment xml:lang="en">Spring is a well-known Java framework. Spring does not implement its aspect-oriented features on the language level but though the use of dynamic byte code generation, thereby leaving the Java language intact.</rdfs:comment>
    </owl:NamedIndividual>
    


    <!-- http://securitytoolbox.appspot.com/stac#SpringSecurity -->

    <owl:NamedIndividual rdf:about="&stac;SpringSecurity">
        <rdf:type rdf:resource="&iotsec;FrameworkTechnology"/>
        <rdfs:label xml:lang="en">Spring Security</rdfs:label>
        <rdfs:comment xml:lang="en"></rdfs:comment>
    </owl:NamedIndividual>
    


    <!-- http://securitytoolbox.appspot.com/stac#Squid -->

    <owl:NamedIndividual rdf:about="&stac;Squid">
        <rdf:type rdf:resource="&iotsec;Proxy"/>
        <rdfs:label xml:lang="en">Squid</rdfs:label>
        <rdfs:comment xml:lang="en"></rdfs:comment>
        <iotsec:satisfies rdf:resource="&iotsec;AccessControl"/>
        <iotsec:protectsInLayer rdf:resource="&iotsec;ApplicationLayer"/>
    </owl:NamedIndividual>
    


    <!-- http://securitytoolbox.appspot.com/stac#StealNic -->

    <owl:NamedIndividual rdf:about="&stac;StealNic">
        <rdf:type rdf:resource="&iotsec;WifiAttack"/>
        <rdfs:label xml:lang="en">Steal NIC (Network Interface Card)</rdfs:label>
        <rdfs:comment xml:lang="en">Because ACLs (Access Control Lists) rely on MAC addresses which is a unique identifier for a NIC.</rdfs:comment>
    </owl:NamedIndividual>
    


    <!-- http://securitytoolbox.appspot.com/stac#StolenBackup -->

    <owl:NamedIndividual rdf:about="&stac;StolenBackup">
        <rdf:type rdf:resource="&iotsec;DatabaseAttack"/>
        <rdf:type rdf:resource="&iotsec;Threat"/>
        <rdfs:label xml:lang="en">Stolen Backup</rdfs:label>
        <rdfs:comment xml:lang="en"></rdfs:comment>
    </owl:NamedIndividual>
    


    <!-- http://securitytoolbox.appspot.com/stac#Struts -->

    <owl:NamedIndividual rdf:about="&stac;Struts">
        <rdf:type rdf:resource="&iotsec;FrameworkTechnology"/>
        <rdfs:label xml:lang="en">Struts</rdfs:label>
        <rdfs:comment xml:lang="en"></rdfs:comment>
    </owl:NamedIndividual>
    


    <!-- http://securitytoolbox.appspot.com/stac#SubscriberStation -->

    <owl:NamedIndividual rdf:about="&stac;SubscriberStation">
        <rdf:type rdf:resource="&iotsec;WimaxArchitectureComponent"/>
        <rdfs:label xml:lang="en">Subscriber Station (SS)</rdfs:label>
        <rdfs:comment xml:lang="en"></rdfs:comment>
    </owl:NamedIndividual>
    


    <!-- http://securitytoolbox.appspot.com/stac#SuitableHeterogeneousTechnology -->

    <owl:NamedIndividual rdf:about="&stac;SuitableHeterogeneousTechnology">
        <rdf:type rdf:resource="&iotsec;PositiveFeature"/>
        <rdfs:label xml:lang="en">Suitable for heterogeneous technologies</rdfs:label>
        <rdfs:comment xml:lang="en"></rdfs:comment>
    </owl:NamedIndividual>
    


    <!-- http://securitytoolbox.appspot.com/stac#Suricata -->

    <owl:NamedIndividual rdf:about="&stac;Suricata">
        <rdf:type rdf:resource="&iotsec;IDS"/>
        <rdfs:label xml:lang="en">Suricata</rdfs:label>
        <rdfs:comment xml:lang="en">Suricata is an open source-based intrusion detection system (IDS)</rdfs:comment>
        <iotsec:protectsInLayer rdf:resource="&iotsec;ApplicationLayer"/>
        <iotsec:satisfies rdf:resource="&iotsec;Availability"/>
        <iotsec:hasFeature rdf:resource="&iotsec;Opensource"/>
    </owl:NamedIndividual>
    


    <!-- http://securitytoolbox.appspot.com/stac#Sybil -->

    <owl:NamedIndividual rdf:about="&stac;Sybil">
        <rdf:type rdf:resource="&iotsec;M2MAttack"/>
        <rdf:type rdf:resource="&iotsec;MeshAttack"/>
        <rdf:type rdf:resource="&iotsec;SensorAttack"/>
        <rdfs:label xml:lang="en">Sybil</rdfs:label>
        <rdfs:comment xml:lang="en">See Paper: Survey of Security and Privacy Issues of Internet of Things [Borgohain et al. 2015]</rdfs:comment>
        <rdfs:comment xml:lang="en">The malicious node presents multiple fake identities to other nodes in the network.</rdfs:comment>
        <iotsec:occursInLayer rdf:resource="&iotsec;NetworkLayer"/>
        <iotsec:hasSecurityMechanism rdf:resource="&iotsec;RadioResourceTesting"/>
        <iotsec:hasSecurityMechanism rdf:resource="&iotsec;RandomKeyPredistribution"/>
        <iotsec:hasSecurityMechanism rdf:resource="&iotsec;Registration"/>
        <iotsec:hasSecurityMechanism rdf:resource="&iotsec;SPINS"/>
    </owl:NamedIndividual>
    


    <!-- http://securitytoolbox.appspot.com/stac#SymmetricGSMKey -->

    <owl:NamedIndividual rdf:about="&stac;SymmetricGSMKey">
        <rdf:type rdf:resource="&iotsec;SymmetricKey"/>
        <rdfs:label xml:lang="en">Symmetric GSM Key</rdfs:label>
        <rdfs:comment xml:lang="en"></rdfs:comment>
    </owl:NamedIndividual>
    


    <!-- http://securitytoolbox.appspot.com/stac#TCPFlooding -->

    <owl:NamedIndividual rdf:about="&stac;TCPFlooding">
        <rdf:type rdf:resource="&iotsec;Flooding"/>
        <rdfs:label xml:lang="en">TCP Flooding</rdfs:label>
        <rdfs:comment xml:lang="en">Floodings attacks generally are used to drain the memry resources by sensing the control signals.</rdfs:comment>
        <iotsec:occursInLayer rdf:resource="&iotsec;TransportLayer"/>
    </owl:NamedIndividual>
    


    <!-- http://securitytoolbox.appspot.com/stac#TEK -->

    <owl:NamedIndividual rdf:about="&stac;TEK">
        <rdf:type rdf:resource="&iotsec;WimaxKeyManagement"/>
        <rdfs:label xml:lang="en">Traffic Encryption Key (TEK)</rdfs:label>
        <rdfs:comment xml:lang="en"></rdfs:comment>
        <iotsec:satisfies rdf:resource="&iotsec;Authentication"/>
    </owl:NamedIndividual>
    


    <!-- http://securitytoolbox.appspot.com/stac#TKIP -->

    <owl:NamedIndividual rdf:about="&stac;TKIP">
        <rdf:type rdf:resource="&iotsec;WifiArchitectureComponent"/>
        <rdfs:label xml:lang="en">Temporal Key Integrity Protocol (TKIP)</rdfs:label>
        <rdfs:comment xml:lang="en"></rdfs:comment>
        <iotsec:satisfies rdf:resource="&iotsec;Confidentiality"/>
        <iotsec:hasFeature rdf:resource="&iotsec;Deprecated"/>
        <dcterms:hasPart rdf:resource="&iotsec;EAPOL"/>
        <iotsec:protectsInLayer rdf:resource="&iotsec;LinkLayer"/>
        <dcterms:hasPart rdf:resource="&iotsec;MIC"/>
        <dcterms:hasPart rdf:resource="&iotsec;Michael"/>
        <dcterms:hasPart rdf:resource="&iotsec;RC4"/>
    </owl:NamedIndividual>
    


    <!-- http://securitytoolbox.appspot.com/stac#TLLI -->

    <owl:NamedIndividual rdf:about="&stac;TLLI">
        <rdf:type rdf:resource="&stac;GPRSArchitectureComponent"/>
        <rdfs:label xml:lang="en">Temporary Logical Link Identity (TLLI)</rdfs:label>
        <rdfs:comment xml:lang="en"></rdfs:comment>
    </owl:NamedIndividual>
    


    <!-- http://securitytoolbox.appspot.com/stac#TLS -->

    <owl:NamedIndividual rdf:about="&stac;TLS">
        <rdf:type rdf:resource="&iotsec;Protocol"/>
        <rdf:type rdf:resource="&iotsec;WebSecurityMechanism"/>
        <rdfs:label xml:lang="en">Transport Layer Security (TLS)</rdfs:label>
        <rdfs:comment xml:lang="en">The TLS protocol allows for secure transactions and provides for end-to-end security at the transport layer. TLS is also known as SSL.</rdfs:comment>
        <owl:sameAs rdf:resource="&iotsec;SSL"/>
        <iotsec:protectsInLayer rdf:resource="&iotsec;TransportLayer"/>
    </owl:NamedIndividual>
    


    <!-- http://securitytoolbox.appspot.com/stac#TMSI -->

    <owl:NamedIndividual rdf:about="&stac;TMSI">
        <rdf:type rdf:resource="&stac;GSMArchitectureComponent"/>
        <rdfs:label xml:lang="en">Temporary Mobile Subscriber Identity (TMSI)</rdfs:label>
        <rdfs:comment xml:lang="en">The TMSI is transmitted by the MS (Mobile Station). The purpose of this TMSI is to deny an intruder the possibility of gaining information on the resources used by the subscriber, preventing of tracing the user&apos;s location.</rdfs:comment>
        <iotsec:satisfies rdf:resource="&iotsec;Anonymity"/>
    </owl:NamedIndividual>
    


    <!-- http://securitytoolbox.appspot.com/stac#TagCloning -->

    <owl:NamedIndividual rdf:about="&stac;TagCloning">
        <rdf:type rdf:resource="&iotsec;RfidAttack"/>
        <rdfs:label xml:lang="en">Unauthorized tag cloning</rdfs:label>
        <rdfs:comment xml:lang="en">Once the identification information of a tag is compromised, replication of the tag (cloning) is made possible which can be used to bypass counterfeit security measures.</rdfs:comment>
        <rdfs:comment xml:lang="en">See Paper: Survey of Security and Privacy Issues of Internet of Things [Borgohain et al. 2015]</rdfs:comment>
        <iotsec:threatens rdf:resource="&iotsec;Integrity"/>
    </owl:NamedIndividual>
    


    <!-- http://securitytoolbox.appspot.com/stac#TagDisabling -->

    <owl:NamedIndividual rdf:about="&stac;TagDisabling">
        <rdf:type rdf:resource="&iotsec;RfidAttack"/>
        <rdfs:label xml:lang="en">Unauthorized tag disabling</rdfs:label>
        <rdfs:comment xml:lang="en">See Paper: Survey of Security and Privacy Issues of Internet of Things [Borgohain et al. 2015]</rdfs:comment>
        <rdfs:comment xml:lang="en">Such attacks render a RFID tag to malfunction and misbehave under the scan of a tag reader.</rdfs:comment>
        <iotsec:threatens rdf:resource="&iotsec;Authentication"/>
    </owl:NamedIndividual>
    


    <!-- http://securitytoolbox.appspot.com/stac#TagTracking -->

    <owl:NamedIndividual rdf:about="&stac;TagTracking">
        <rdf:type rdf:resource="&iotsec;RfidAttack"/>
        <rdfs:label xml:lang="en">Unauthorized tag tracking</rdfs:label>
        <rdfs:comment xml:lang="en">A tag can be traced through rogue readers, which may result in giving up of sensistive information like a person&apos;s address.</rdfs:comment>
        <rdfs:comment xml:lang="en">See Paper: Survey of Security and Privacy Issues of Internet of Things [Borgohain et al. 2015]</rdfs:comment>
        <iotsec:threatens rdf:resource="&iotsec;Confidentiality"/>
    </owl:NamedIndividual>
    


    <!-- http://securitytoolbox.appspot.com/stac#TamperResistantHarware -->

    <owl:NamedIndividual rdf:about="&stac;TamperResistantHarware">
        <rdf:type rdf:resource="&iotsec;SecurityMechanism"/>
        <rdfs:label xml:lang="en">Tamper Resistant Harware</rdfs:label>
        <rdfs:comment xml:lang="en"></rdfs:comment>
        <iotsec:protectsInLayer rdf:resource="&iotsec;PhysicalLayer"/>
    </owl:NamedIndividual>
    


    <!-- http://securitytoolbox.appspot.com/stac#Tampering -->

    <owl:NamedIndividual rdf:about="&stac;Tampering">
        <rdf:type rdf:resource="&iotsec;SensorAttack"/>
        <rdfs:label xml:lang="en">Node tampering</rdfs:label>
        <rdfs:comment xml:lang="en">An attacker can tamper with nodes physically and interrogate and compromise them by extracting sensitive information.</rdfs:comment>
        <rdfs:comment xml:lang="en">See Paper: Survey of Security and Privacy Issues of Internet of Things [Borgohain et al. 2015]</rdfs:comment>
        <iotsec:threatens rdf:resource="&iotsec;Confidentiality"/>
        <iotsec:occursInLayer rdf:resource="&iotsec;PhysicalLayer"/>
    </owl:NamedIndividual>
    


    <!-- http://securitytoolbox.appspot.com/stac#Tcpdump -->

    <owl:NamedIndividual rdf:about="&stac;Tcpdump">
        <rdf:type rdf:resource="&iotsec;NetworkManagementSecurityTool"/>
        <rdfs:label xml:lang="en">Tcpdump</rdfs:label>
        <rdfs:comment xml:lang="en"></rdfs:comment>
        <iotsec:isReplacedBy rdf:resource="&iotsec;Wireshark"/>
    </owl:NamedIndividual>
    


    <!-- http://securitytoolbox.appspot.com/stac#TerminalEquipment -->

    <owl:NamedIndividual rdf:about="&stac;TerminalEquipment">
        <rdf:type rdf:resource="&stac;GPRSArchitectureComponent"/>
        <rdfs:label xml:lang="en">Terminal Equipment</rdfs:label>
        <rdfs:comment xml:lang="en"></rdfs:comment>
    </owl:NamedIndividual>
    


    <!-- http://securitytoolbox.appspot.com/stac#TimeDivisionMultiplexing -->

    <owl:NamedIndividual rdf:about="&stac;TimeDivisionMultiplexing">
        <rdf:type rdf:resource="&iotsec;SensorSecurityMechanism"/>
        <rdfs:label xml:lang="en">Time Division Multiplexing</rdfs:label>
        <rdfs:comment xml:lang="en">Time Division Multiplexing gives each node a slot for transmission without requiring arbitration for each frame.</rdfs:comment>
        <iotsec:protectsInLayer rdf:resource="&iotsec;LinkLayer"/>
    </owl:NamedIndividual>
    


    <!-- http://securitytoolbox.appspot.com/stac#TinyOS -->

    <owl:NamedIndividual rdf:about="&stac;TinyOS">
        <rdf:type rdf:resource="&iotsec;OperatingSystemTechnology"/>
        <rdf:type rdf:resource="&iotsec;SensorTechnology"/>
        <rdfs:label xml:lang="en">TinyOS</rdfs:label>
        <rdfs:comment xml:lang="en">TinyOS is an operating system for sensors.</rdfs:comment>
    </owl:NamedIndividual>
    


    <!-- http://securitytoolbox.appspot.com/stac#TinySec -->

    <owl:NamedIndividual rdf:about="&stac;TinySec">
        <rdf:type rdf:resource="&iotsec;SensorSecurityProtocol"/>
        <rdfs:label xml:lang="en">TinySec</rdfs:label>
        <rdfs:comment xml:lang="en">TinySec is a sensor protocol for the link layer.</rdfs:comment>
        <iotsec:satisfies rdf:resource="&iotsec;Authentication"/>
        <iotsec:satisfies rdf:resource="&iotsec;Confidentiality"/>
        <iotsec:satisfies rdf:resource="&iotsec;DataFreshness"/>
        <iotsec:satisfies rdf:resource="&iotsec;Integrity"/>
        <iotsec:protectsInLayer rdf:resource="&iotsec;LinkLayer"/>
        <iotsec:satisfies rdf:resource="&iotsec;SemanticSecurity"/>
        <dcterms:hasPart rdf:resource="&iotsec;Skipjack"/>
        <dcterms:hasPart rdf:resource="&iotsec;TinySec_AE"/>
        <dcterms:hasPart rdf:resource="&iotsec;TinySec_Auth"/>
    </owl:NamedIndividual>
    


    <!-- http://securitytoolbox.appspot.com/stac#Tomcat -->

    <owl:NamedIndividual rdf:about="&stac;Tomcat">
        <rdf:type rdf:resource="&iotsec;ServerTechnology"/>
        <rdfs:label xml:lang="en">Tomcat</rdfs:label>
        <rdfs:comment xml:lang="en"></rdfs:comment>
    </owl:NamedIndividual>
    


    <!-- http://securitytoolbox.appspot.com/stac#TransportLayer -->

    <owl:NamedIndividual rdf:about="&stac;TransportLayer">
        <rdf:type rdf:resource="&iotsec;OSIModelLayer"/>
        <rdfs:label xml:lang="en">Transport Layer</rdfs:label>
        <rdfs:comment xml:lang="en">The transport layer manages packetization of data, then the delivery of the packets, including checking for errors in the data once it arrives.</rdfs:comment>
    </owl:NamedIndividual>
    


    <!-- http://securitytoolbox.appspot.com/stac#TripleDES -->

    <owl:NamedIndividual rdf:about="&stac;TripleDES">
        <rdf:type rdf:resource="&iotsec;BlockCipher"/>
        <rdf:type rdf:resource="&iotsec;ManetSecurityMechanism"/>
        <rdfs:label xml:lang="en">TripleDES</rdfs:label>
        <rdfs:comment xml:lang="en"></rdfs:comment>
        <iotsec:satisfies rdf:resource="&iotsec;Confidentiality"/>
        <owl:sameAs rdf:resource="&iotsec;TripleDES"/>
    </owl:NamedIndividual>
    


    <!-- http://securitytoolbox.appspot.com/stac#TripleStore -->

    <owl:NamedIndividual rdf:about="&stac;TripleStore">
        <rdf:type rdf:resource="&iotsec;DatabaseTechnology"/>
        <rdfs:label xml:lang="en">TripleStore</rdfs:label>
        <rdfs:comment xml:lang="en"></rdfs:comment>
    </owl:NamedIndividual>
    


    <!-- http://securitytoolbox.appspot.com/stac#Trust -->

    <owl:NamedIndividual rdf:about="&stac;Trust">
        <rdf:type rdf:resource="&iotsec;SecurityProperty"/>
        <rdfs:label xml:lang="en">Trust</rdfs:label>
        <rdfs:comment xml:lang="en">Data is reliable?</rdfs:comment>
        <rdfs:comment xml:lang="en">Trust is defined as the degree to which a node should be trustworthy, secure, or reliable during any interaction with the node.</rdfs:comment>
    </owl:NamedIndividual>
    


    <!-- http://securitytoolbox.appspot.com/stac#Twofish -->

    <owl:NamedIndividual rdf:about="&stac;Twofish">
        <rdf:type rdf:resource="&iotsec;BlockCipher"/>
        <rdf:type rdf:resource="&iotsec;ManetSecurityMechanism"/>
        <rdfs:label xml:lang="en">Twofish</rdfs:label>
        <rdfs:comment xml:lang="en"></rdfs:comment>
        <iotsec:satisfies rdf:resource="&iotsec;Confidentiality"/>
    </owl:NamedIndividual>
    


    <!-- http://securitytoolbox.appspot.com/stac#UDPFlooding -->

    <owl:NamedIndividual rdf:about="&stac;UDPFlooding">
        <rdf:type rdf:resource="&iotsec;Flooding"/>
        <rdfs:label xml:lang="en">UDP Flooding</rdfs:label>
        <rdfs:comment xml:lang="en">Floodings attacks generally are used to drain the memry resources by sensing the control signals.</rdfs:comment>
        <iotsec:occursInLayer rdf:resource="&iotsec;TransportLayer"/>
    </owl:NamedIndividual>
    


    <!-- http://securitytoolbox.appspot.com/stac#UMLSec -->

    <owl:NamedIndividual rdf:about="&stac;UMLSec">
        <rdf:type rdf:resource="&iotsec;FrameworkSecurityMechanism"/>
        <rdfs:label xml:lang="en">SecureUML</rdfs:label>
        <rdfs:comment xml:lang="en"></rdfs:comment>
    </owl:NamedIndividual>
    


    <!-- http://securitytoolbox.appspot.com/stac#USIM -->

    <owl:NamedIndividual rdf:about="&stac;USIM">
        <rdf:type rdf:resource="&iotsec;UMTSArchitectureComponent"/>
        <rdfs:label xml:lang="en">Universal Subscriber Identity Module (USIM)</rdfs:label>
        <rdfs:comment xml:lang="en">The keys and algorithms used for authentication and encryption are stored on the USIM.</rdfs:comment>
        <dcterms:hasPart rdf:resource="&iotsec;AKA"/>
        <iotsec:satisfies rdf:resource="&iotsec;Authentication"/>
        <iotsec:satisfies rdf:resource="&iotsec;Confidentiality"/>
        <dcterms:hasPart rdf:resource="&iotsec;IMSI"/>
        <iotsec:satisfies rdf:resource="&iotsec;Integrity"/>
    </owl:NamedIndividual>
    


    <!-- http://securitytoolbox.appspot.com/stac#UTRAN -->

    <owl:NamedIndividual rdf:about="&stac;UTRAN">
        <rdf:type rdf:resource="&iotsec;UMTSArchitectureComponent"/>
        <rdfs:label xml:lang="en">Access Network (UTRAN)</rdfs:label>
        <rdfs:comment xml:lang="en">The UTRAN is the new access network for UMTS networks, it allows connectivity between the UE (User Equipment) and the core network.</rdfs:comment>
        <dcterms:hasPart rdf:resource="&iotsec;NodeB"/>
        <dcterms:hasPart rdf:resource="&iotsec;RNC"/>
    </owl:NamedIndividual>
    


    <!-- http://securitytoolbox.appspot.com/stac#UltraSoft -->

    <owl:NamedIndividual rdf:about="&stac;UltraSoft">
        <rdf:type rdf:resource="&iotsec;Proxy"/>
        <rdfs:label xml:lang="en">UltraSoft</rdfs:label>
        <rdfs:comment xml:lang="en"></rdfs:comment>
        <iotsec:satisfies rdf:resource="&iotsec;AccessControl"/>
        <iotsec:protectsInLayer rdf:resource="&iotsec;ApplicationLayer"/>
    </owl:NamedIndividual>
    


    <!-- http://securitytoolbox.appspot.com/stac#UltraSurf -->

    <owl:NamedIndividual rdf:about="&stac;UltraSurf">
        <rdf:type rdf:resource="&iotsec;Proxy"/>
        <rdfs:label xml:lang="en">UltraSurf</rdfs:label>
        <rdfs:comment xml:lang="en"></rdfs:comment>
        <iotsec:satisfies rdf:resource="&iotsec;AccessControl"/>
        <iotsec:protectsInLayer rdf:resource="&iotsec;ApplicationLayer"/>
    </owl:NamedIndividual>
    


    <!-- http://securitytoolbox.appspot.com/stac#UmInterface -->

    <owl:NamedIndividual rdf:about="&stac;UmInterface">
        <rdf:type rdf:resource="&stac;GSMArchitectureComponent"/>
        <rdfs:label xml:lang="en">Um Interface</rdfs:label>
        <rdfs:comment xml:lang="en">The Mobile Station and the BSS communicate across the Um interface, also known as the radio link or the air interface.</rdfs:comment>
    </owl:NamedIndividual>
    


    <!-- http://securitytoolbox.appspot.com/stac#Unfairness -->

    <owl:NamedIndividual rdf:about="&stac;Unfairness">
        <rdf:type rdf:resource="&iotsec;SensorAttack"/>
        <rdfs:label xml:lang="en">Unfairness</rdfs:label>
        <rdfs:comment xml:lang="en">See Paper: Survey of Security and Privacy Issues of Internet of Things [Borgohain et al. 2015]</rdfs:comment>
        <rdfs:comment xml:lang="en">Unfairness is a weaker form DoS that is done by abusing MAC prority schemes. In unfairness attacks, network performance degrades because medium access control layer priority is generally disrupted accroding to the application requirements.</rdfs:comment>
        <iotsec:occursInLayer rdf:resource="&iotsec;LinkLayer"/>
        <iotsec:hasSecurityMechanism rdf:resource="&iotsec;SmallFrame"/>
    </owl:NamedIndividual>
    


    <!-- http://securitytoolbox.appspot.com/stac#UserEquipment -->

    <owl:NamedIndividual rdf:about="&stac;UserEquipment">
        <rdf:type rdf:resource="&iotsec;LTEArchitecture"/>
        <rdf:type rdf:resource="&iotsec;UMTSArchitectureComponent"/>
        <rdfs:label xml:lang="en">User Equipment (UE)</rdfs:label>
        <rdfs:comment xml:lang="en">The UE is the end device of UMTS network&gt; The user can make a phone call through user equipment. It always contains mobile phone and USIM card.</rdfs:comment>
        <dcterms:hasPart rdf:resource="&iotsec;MobileEquipment"/>
        <dcterms:hasPart rdf:resource="&iotsec;TerminalEquipment"/>
        <dcterms:hasPart rdf:resource="&iotsec;USIM"/>
    </owl:NamedIndividual>
    


    <!-- http://securitytoolbox.appspot.com/stac#UuInterface -->

    <owl:NamedIndividual rdf:about="&stac;UuInterface">
        <rdf:type rdf:resource="&iotsec;UMTSArchitectureComponent"/>
        <rdfs:label xml:lang="en">Uu Interface</rdfs:label>
        <rdfs:comment xml:lang="en">Connections between NodeBs and RNCs.</rdfs:comment>
    </owl:NamedIndividual>
    


    <!-- http://securitytoolbox.appspot.com/stac#VLR -->

    <owl:NamedIndividual rdf:about="&stac;VLR">
        <rdf:type rdf:resource="&stac;GSMArchitectureComponent"/>
        <rdfs:label xml:lang="en">Visitor Location Register (VLR)</rdfs:label>
        <rdfs:comment xml:lang="en">The VLR is a subscriber profile containing temporary information, and is distributed in the network according to geographical locations. The VLR performs the authentication and key agreement procedure.</rdfs:comment>
    </owl:NamedIndividual>
    


    <!-- http://securitytoolbox.appspot.com/stac#VPN -->

    <owl:NamedIndividual rdf:about="&stac;VPN">
        <rdf:type rdf:resource="&iotsec;NetworkManagementSecurityMechanism"/>
        <rdf:type rdf:resource="&iotsec;UMTSSecurityMechanism"/>
        <rdf:type rdf:resource="&iotsec;WebSecurityMechanism"/>
        <rdfs:label xml:lang="en">Virtual Private Network (VPN)</rdfs:label>
        <rdfs:comment xml:lang="en">See Paper: Malicious actions against the GPRS technology [Xenakis 2006]</rdfs:comment>
        <rdfs:comment xml:lang="en">VPN allows a client to use an &quot;untrusted&quot; network (e.g. the Internet or a wireless network) for secure communication.</rdfs:comment>
        <iotsec:satisfies rdf:resource="&iotsec;AccessControl"/>
        <iotsec:protectsInLayer rdf:resource="&iotsec;ApplicationLayer"/>
        <iotsec:satisfies rdf:resource="&iotsec;Authentication"/>
        <iotsec:satisfies rdf:resource="&iotsec;Authorization"/>
        <iotsec:satisfies rdf:resource="&iotsec;Confidentiality"/>
        <dcterms:hasPart rdf:resource="&iotsec;IKE"/>
        <iotsec:satisfies rdf:resource="&iotsec;Integrity"/>
        <dcterms:hasPart rdf:resource="&iotsec;Ipsec"/>
        <iotsec:hasFeature rdf:resource="&iotsec;LowCostDeployment"/>
        <iotsec:hasFeature rdf:resource="&iotsec;Secured"/>
        <iotsec:hasSecurityMechanism rdf:resource="&iotsec;VPN"/>
    </owl:NamedIndividual>
    


    <!-- http://securitytoolbox.appspot.com/stac#VeriSign -->

    <owl:NamedIndividual rdf:about="&stac;VeriSign">
        <rdf:type rdf:resource="&iotsec;WebSecurityMechanism"/>
        <rdfs:label xml:lang="en">VeriSign</rdfs:label>
        <rdfs:comment xml:lang="en"></rdfs:comment>
    </owl:NamedIndividual>
    


    <!-- http://securitytoolbox.appspot.com/stac#Virtuoso -->

    <owl:NamedIndividual rdf:about="&stac;Virtuoso">
        <rdf:type rdf:resource="&iotsec;FrameworkTechnology"/>
        <rdfs:label xml:lang="en">Virtuoso</rdfs:label>
        <rdfs:comment xml:lang="en"></rdfs:comment>
    </owl:NamedIndividual>
    


    <!-- http://securitytoolbox.appspot.com/stac#WAP1 -->

    <owl:NamedIndividual rdf:about="&stac;WAP1">
        <rdf:type rdf:resource="&iotsec;WifiTechnology"/>
        <rdfs:label xml:lang="en">Wireless Application Protocol (WAP1)</rdfs:label>
        <rdfs:comment xml:lang="en">WAP is an open specification which enables mobile users to access the Internet.</rdfs:comment>
        <iotsec:isReplacedBy rdf:resource="&iotsec;WAP2"/>
        <dcterms:hasPart rdf:resource="&iotsec;WTLS"/>
    </owl:NamedIndividual>
    


    <!-- http://securitytoolbox.appspot.com/stac#WAP2 -->

    <owl:NamedIndividual rdf:about="&stac;WAP2">
        <rdf:type rdf:resource="&iotsec;WifiTechnology"/>
        <rdfs:label xml:lang="en">Wireless Application Protocol (WAP2)</rdfs:label>
        <rdfs:comment xml:lang="en">WAP is an open specification which enables mobile users to access the Internet.</rdfs:comment>
        <dcterms:hasPart rdf:resource="&iotsec;TLS"/>
    </owl:NamedIndividual>
    


    <!-- http://securitytoolbox.appspot.com/stac#WEP -->

    <owl:NamedIndividual rdf:about="&stac;WEP">
        <rdf:type rdf:resource="&iotsec;StreamCipher"/>
        <rdf:type rdf:resource="&iotsec;WifiSecurityProtocol"/>
        <rdfs:label xml:lang="en">Wired Equivalent Privacy (WEP)</rdfs:label>
        <rdfs:comment xml:lang="en">WEP is a security protocol to provide encrypted communication between the client and an AP, once the client is authenticated.</rdfs:comment>
        <iotsec:satisfies rdf:resource="&iotsec;Authentication"/>
        <iotsec:hashasModeOperation rdf:resource="&iotsec;CRC-32"/>
        <dcterms:hasPart rdf:resource="&iotsec;CRCValue"/>
        <iotsec:satisfies rdf:resource="&iotsec;Confidentiality"/>
        <iotsec:hasFeature rdf:resource="&iotsec;Deprecated"/>
        <iotsec:hashasModeOperation rdf:resource="&iotsec;ECB"/>
        <iotsec:satisfies rdf:resource="&iotsec;Integrity"/>
        <iotsec:protectsInLayer rdf:resource="&iotsec;LinkLayer"/>
        <iotsec:hasFeature rdf:resource="&iotsec;NotScalable"/>
        <dcterms:hasPart rdf:resource="&iotsec;RC4"/>
        <iotsec:satisfies rdf:resource="&iotsec;SemanticSecurity"/>
        <iotsec:isReplacedBy rdf:resource="&iotsec;WPA1"/>
    </owl:NamedIndividual>
    


    <!-- http://securitytoolbox.appspot.com/stac#WPA1 -->

    <owl:NamedIndividual rdf:about="&stac;WPA1">
        <rdf:type rdf:resource="&iotsec;WifiSecurityProtocol"/>
        <rdfs:label xml:lang="en">Wi-Fi Protected Access (WPA)</rdfs:label>
        <rdfs:comment xml:lang="en">WPA is an authentication system.</rdfs:comment>
        <iotsec:satisfies rdf:resource="&iotsec;Authentication"/>
        <iotsec:satisfies rdf:resource="&iotsec;Confidentiality"/>
        <iotsec:hasFeature rdf:resource="&iotsec;Deprecated"/>
        <dcterms:hasPart rdf:resource="&iotsec;IEEE_802.1X"/>
        <iotsec:satisfies rdf:resource="&iotsec;Integrity"/>
        <dcterms:hasPart rdf:resource="&iotsec;TKIP"/>
        <iotsec:isReplacedBy rdf:resource="&iotsec;WPA2"/>
    </owl:NamedIndividual>
    


    <!-- http://securitytoolbox.appspot.com/stac#WPA2 -->

    <owl:NamedIndividual rdf:about="&stac;WPA2">
        <rdf:type rdf:resource="&iotsec;WifiSecurityProtocol"/>
        <rdfs:label xml:lang="en">Wi-Fi Protected Access (WPA2)</rdfs:label>
        <rdfs:comment xml:lang="en">A wireless security protocol in which only authorised users can access a wireless device.</rdfs:comment>
        <dcterms:hasPart rdf:resource="&iotsec;AES"/>
        <iotsec:satisfies rdf:resource="&iotsec;Authentication"/>
        <dcterms:hasPart rdf:resource="&iotsec;CCMP"/>
        <iotsec:satisfies rdf:resource="&iotsec;Confidentiality"/>
        <dcterms:hasPart rdf:resource="&iotsec;EAP"/>
        <dcterms:hasPart rdf:resource="&iotsec;GMK"/>
        <dcterms:hasPart rdf:resource="&iotsec;IEEE_802.1X"/>
        <iotsec:satisfies rdf:resource="&iotsec;Integrity"/>
        <owl:sameAs rdf:resource="&iotsec;RSN"/>
        <iotsec:hasFeature rdf:resource="&iotsec;Secured"/>
        <dcterms:hasPart rdf:resource="&iotsec;TKIP"/>
    </owl:NamedIndividual>
    


    <!-- http://securitytoolbox.appspot.com/stac#WTLS -->

    <owl:NamedIndividual rdf:about="&stac;WTLS">
        <rdf:type rdf:resource="&iotsec;WifiSecurityProtocol"/>
        <rdfs:label xml:lang="en">Wireless Transport Layer Security (WTLS)</rdfs:label>
        <rdfs:comment xml:lang="en">WTLS secures, authenticates, and encrypts data transmissions between the WAP gateway and mobile devices.</rdfs:comment>
        <iotsec:satisfies rdf:resource="&iotsec;Authentication"/>
        <iotsec:satisfies rdf:resource="&iotsec;Confidentiality"/>
        <iotsec:satisfies rdf:resource="&iotsec;Integrity"/>
        <dcterms:hasPart rdf:resource="&iotsec;RSA"/>
    </owl:NamedIndividual>
    


    <!-- http://securitytoolbox.appspot.com/stac#Watchdog -->

    <owl:NamedIndividual rdf:about="&stac;Watchdog">
        <rdf:type rdf:resource="&iotsec;SensorSecurityMechanism"/>
        <rdfs:label xml:lang="en">Watchdog</rdfs:label>
        <rdfs:comment xml:lang="en"></rdfs:comment>
        <iotsec:protectsInLayer rdf:resource="&iotsec;NetworkLayer"/>
    </owl:NamedIndividual>
    


    <!-- http://securitytoolbox.appspot.com/stac#WaterTorture -->

    <owl:NamedIndividual rdf:about="&stac;WaterTorture">
        <rdf:type rdf:resource="&iotsec;WimaxAttack"/>
        <rdfs:label xml:lang="en">Water Torture Attack</rdfs:label>
        <rdfs:comment xml:lang="en">Pushes a Subscriber Station (SS) to drain its battery or consume computing resources by sending bogus frames.</rdfs:comment>
    </owl:NamedIndividual>
    


    <!-- http://securitytoolbox.appspot.com/stac#WepCrack -->

    <owl:NamedIndividual rdf:about="&stac;WepCrack">
        <rdf:type rdf:resource="&iotsec;WifiAttackTool"/>
        <rdfs:label xml:lang="en">WEP Crack</rdfs:label>
        <rdfs:comment xml:lang="en"></rdfs:comment>
    </owl:NamedIndividual>
    


    <!-- http://securitytoolbox.appspot.com/stac#WifiMobileStation -->

    <owl:NamedIndividual rdf:about="&stac;WifiMobileStation">
        <rdf:type rdf:resource="&iotsec;WifiArchitectureComponent"/>
        <rdfs:label xml:lang="en">Wifi Mobile Station (STA)</rdfs:label>
        <rdfs:comment xml:lang="en"></rdfs:comment>
    </owl:NamedIndividual>
    


    <!-- http://securitytoolbox.appspot.com/stac#WimaxBaseStation -->

    <owl:NamedIndividual rdf:about="&stac;WimaxBaseStation">
        <rdf:type rdf:resource="&iotsec;WimaxArchitectureComponent"/>
        <rdfs:label xml:lang="en">WiMAX Base Station (BS)</rdfs:label>
        <rdfs:comment xml:lang="en"></rdfs:comment>
    </owl:NamedIndividual>
    


    <!-- http://securitytoolbox.appspot.com/stac#WimaxMobileStation -->

    <owl:NamedIndividual rdf:about="&stac;WimaxMobileStation">
        <rdf:type rdf:resource="&iotsec;WimaxArchitectureComponent"/>
        <rdfs:label xml:lang="en">WiMAX Mobile Station (MS)</rdfs:label>
        <rdfs:comment xml:lang="en"></rdfs:comment>
    </owl:NamedIndividual>
    


    <!-- http://securitytoolbox.appspot.com/stac#Windows -->

    <owl:NamedIndividual rdf:about="&stac;Windows">
        <rdf:type rdf:resource="&iotsec;OperatingSystemTechnology"/>
        <rdfs:label xml:lang="en">Windows</rdfs:label>
        <rdfs:comment xml:lang="en"></rdfs:comment>
    </owl:NamedIndividual>
    


    <!-- http://securitytoolbox.appspot.com/stac#WindowsDefender -->

    <owl:NamedIndividual rdf:about="&stac;WindowsDefender">
        <rdf:type rdf:resource="&iotsec;Antivirus"/>
        <rdfs:label xml:lang="en">WindowsDefender</rdfs:label>
        <rdfs:comment xml:lang="en"></rdfs:comment>
        <iotsec:hasFeature rdf:resource="&iotsec;Free"/>
        <iotsec:satisfies rdf:resource="&iotsec;Integrity"/>
    </owl:NamedIndividual>
    


    <!-- http://securitytoolbox.appspot.com/stac#Wireshark -->

    <owl:NamedIndividual rdf:about="&stac;Wireshark">
        <rdf:type rdf:resource="&iotsec;NetworkManagementSecurityTool"/>
        <rdfs:label xml:lang="en">Wireshark or Ethereal</rdfs:label>
        <rdfs:comment xml:lang="en">Wireshark is a network protocol packet analyzer. It allows you to examine data from a live network of from a capture file on disk. </rdfs:comment>
        <iotsec:hasFeature rdf:resource="&iotsec;Free"/>
        <iotsec:hasFeature rdf:resource="&iotsec;Opensource"/>
    </owl:NamedIndividual>
    


    <!-- http://securitytoolbox.appspot.com/stac#Wormhole -->

    <owl:NamedIndividual rdf:about="&stac;Wormhole">
        <rdf:type rdf:resource="&iotsec;M2MAttack"/>
        <rdf:type rdf:resource="&iotsec;ManetAttack"/>
        <rdf:type rdf:resource="&iotsec;MeshAttack"/>
        <rdf:type rdf:resource="&iotsec;SensorAttack"/>
        <rdfs:label xml:lang="en">Wormhole</rdfs:label>
        <rdfs:comment xml:lang="en">An attacker tunnels messages from one location to another location. The attacker then replays those messages from the latter location.</rdfs:comment>
        <rdfs:comment xml:lang="en">See Paper: Survey of Security and Privacy Issues of Internet of Things [Borgohain et al. 2015]</rdfs:comment>
        <iotsec:hasSecurityMechanism rdf:resource="&iotsec;DirectionalAntenna"/>
        <iotsec:occursInLayer rdf:resource="&iotsec;NetworkLayer"/>
        <iotsec:hasSecurityMechanism rdf:resource="&iotsec;PacketLeaches"/>
        <iotsec:hasSecurityMechanism rdf:resource="&iotsec;Timestamp"/>
    </owl:NamedIndividual>
    


    <!-- http://securitytoolbox.appspot.com/stac#XRES -->

    <owl:NamedIndividual rdf:about="&stac;XRES">
        <rdf:type rdf:resource="&iotsec;UMTSArchitectureComponent"/>
        <rdfs:label xml:lang="en">Expected Response (XRES)</rdfs:label>
        <rdfs:comment xml:lang="en"></rdfs:comment>
    </owl:NamedIndividual>
    


    <!-- http://securitytoolbox.appspot.com/stac#XSS -->

    <owl:NamedIndividual rdf:about="&stac;XSS">
        <rdf:type rdf:resource="&iotsec;WebAttack"/>
        <rdfs:label xml:lang="en">Cross Site Scripting (XSS)</rdfs:label>
        <rdfs:comment xml:lang="en"></rdfs:comment>
        <iotsec:hasSecurityMechanism rdf:resource="&stac;Firewall"/>
        <iotsec:occursInLayer rdf:resource="&iotsec;ApplicationLayer"/>
    </owl:NamedIndividual>
    


    <!-- http://securitytoolbox.appspot.com/stac#X_509 -->

    <owl:NamedIndividual rdf:about="&stac;X_509">
        <rdf:type rdf:resource="&iotsec;DigitalCertificate"/>
        <rdfs:label xml:lang="en">X_509</rdfs:label>
        <rdfs:comment xml:lang="en">X.509 specifies standard formats for public key certificates, certificate revocation lists, attribute certificates, and a certification path validation algorithm.</rdfs:comment>
        <iotsec:satisfies rdf:resource="&iotsec;AccessControl"/>
        <iotsec:satisfies rdf:resource="&iotsec;Authentication"/>
    </owl:NamedIndividual>
    


    <!-- http://securitytoolbox.appspot.com/stac#YGuard -->

    <owl:NamedIndividual rdf:about="&stac;YGuard">
        <rdf:type rdf:resource="&iotsec;Obfuscation"/>
        <rdfs:label xml:lang="en">YGuard</rdfs:label>
        <rdfs:comment xml:lang="en"></rdfs:comment>
    </owl:NamedIndividual>
    


    <!-- http://securitytoolbox.appspot.com/stac#ZoneAlarm -->

    <owl:NamedIndividual rdf:about="&stac;ZoneAlarm">
        <rdf:type rdf:resource="&iotsec;Firewall"/>
        <rdfs:label xml:lang="en">ZoneAlarm</rdfs:label>
        <rdfs:comment xml:lang="en"></rdfs:comment>
        <iotsec:satisfies rdf:resource="&iotsec;AccessControl"/>
        <iotsec:hasFeature rdf:resource="&iotsec;Free"/>
    </owl:NamedIndividual>
    


    <!-- http://securitytoolbox.appspot.com/stac#eNodeB -->

    <owl:NamedIndividual rdf:about="&stac;eNodeB">
        <rdf:type rdf:resource="&iotsec;LTEArchitectureComponent"/>
        <rdfs:label xml:lang="en">eNodeB</rdfs:label>
        <rdfs:comment xml:lang="en"></rdfs:comment>
    </owl:NamedIndividual>
    


    <!-- http://securitytoolbox.appspot.com/stac#eScan -->

    <owl:NamedIndividual rdf:about="&stac;eScan">
        <rdf:type rdf:resource="&iotsec;Firewall"/>
        <rdfs:label xml:lang="en">eScan</rdfs:label>
        <rdfs:comment xml:lang="en"></rdfs:comment>
        <iotsec:satisfies rdf:resource="&iotsec;AccessControl"/>
    </owl:NamedIndividual>
    


    <!-- http://securitytoolbox.appspot.com/stac#f1 -->

    <owl:NamedIndividual rdf:about="&stac;f1">
        <rdf:type rdf:resource="&iotsec;UMTSSecurityAlgorithm"/>
        <rdfs:label xml:lang="en">f1</rdfs:label>
        <rdfs:comment xml:lang="en">Message Authentication function used to calculate MAC.</rdfs:comment>
        <iotsec:satisfies rdf:resource="&iotsec;Authentication"/>
    </owl:NamedIndividual>
    


    <!-- http://securitytoolbox.appspot.com/stac#f2 -->

    <owl:NamedIndividual rdf:about="&stac;f2">
        <rdf:type rdf:resource="&iotsec;UMTSSecurityAlgorithm"/>
        <rdfs:label xml:lang="en">f2</rdfs:label>
        <rdfs:comment xml:lang="en"></rdfs:comment>
        <dcterms:hasPart rdf:resource="&iotsec;XRES"/>
    </owl:NamedIndividual>
    


    <!-- http://securitytoolbox.appspot.com/stac#f3 -->

    <owl:NamedIndividual rdf:about="&stac;f3">
        <rdf:type rdf:resource="&iotsec;UMTSSecurityAlgorithm"/>
        <rdfs:label xml:lang="en">f3</rdfs:label>
        <rdfs:comment xml:lang="en"></rdfs:comment>
        <dcterms:hasPart rdf:resource="&iotsec;CipherKeyCK"/>
    </owl:NamedIndividual>
    


    <!-- http://securitytoolbox.appspot.com/stac#f4 -->

    <owl:NamedIndividual rdf:about="&stac;f4">
        <rdf:type rdf:resource="&iotsec;UMTSSecurityAlgorithm"/>
        <rdfs:label xml:lang="en">f4</rdfs:label>
        <rdfs:comment xml:lang="en"></rdfs:comment>
        <dcterms:hasPart rdf:resource="&iotsec;IntegrityKeyIK"/>
    </owl:NamedIndividual>
    


    <!-- http://securitytoolbox.appspot.com/stac#f5 -->

    <owl:NamedIndividual rdf:about="&stac;f5">
        <rdf:type rdf:resource="&iotsec;UMTSSecurityAlgorithm"/>
        <rdfs:label xml:lang="en">f5</rdfs:label>
        <rdfs:comment xml:lang="en"></rdfs:comment>
        <dcterms:hasPart rdf:resource="&iotsec;AnonymityKeyAK"/>
    </owl:NamedIndividual>
    


    <!-- http://securitytoolbox.appspot.com/stac#f8 -->

    <owl:NamedIndividual rdf:about="&stac;f8">
        <rdf:type rdf:resource="&iotsec;StreamCipher"/>
        <rdf:type rdf:resource="&iotsec;UMTSSecurityAlgorithm"/>
        <rdfs:label xml:lang="en">f8</rdfs:label>
        <rdfs:comment xml:lang="en"></rdfs:comment>
        <rdfs:comment xml:lang="en">See Paper: Security of mobile internet access with UMTS/HSDP/LTE [Caragata 2009]</rdfs:comment>
        <dcterms:hasPart rdf:resource="&iotsec;CipherKeyCK"/>
        <iotsec:satisfies rdf:resource="&iotsec;Confidentiality"/>
        <dcterms:hasPart rdf:resource="&iotsec;Kasumi"/>
    </owl:NamedIndividual>
    


    <!-- http://securitytoolbox.appspot.com/stac#f9 -->

    <owl:NamedIndividual rdf:about="&stac;f9">
        <rdf:type rdf:resource="&iotsec;UMTSSecurityAlgorithm"/>
        <rdfs:label xml:lang="en">f9</rdfs:label>
        <rdfs:comment xml:lang="en">f9 or UIA (UMTS Integrity Algorithm) is implemented both in the mobile station and the RNC.</rdfs:comment>
        <iotsec:satisfies rdf:resource="&iotsec;Integrity"/>
        <dcterms:hasPart rdf:resource="&iotsec;IntegrityKeyIK"/>
        <dcterms:hasPart rdf:resource="&iotsec;Kasumi"/>
    </owl:NamedIndividual>
    


    <!-- http://semanticweb.org/images/5/53/OntologySecurity.owlAccessControl -->

    <owl:NamedIndividual rdf:about="&securitysw;AccessControl">
        <owl:sameAs rdf:resource="&iotsec;AccessControl"/>
    </owl:NamedIndividual>
    


    <!-- http://semanticweb.org/images/5/53/OntologySecurity.owlAuthentication -->

    <owl:NamedIndividual rdf:about="&securitysw;Authentication"/>
    


    <!-- http://semanticweb.org/images/5/53/OntologySecurity.owlAvailability -->

    <owl:NamedIndividual rdf:about="&securitysw;Availability"/>
    


    <!-- http://semanticweb.org/images/5/53/OntologySecurity.owlConfidentiality -->

    <owl:NamedIndividual rdf:about="&securitysw;Confidentiality"/>
    


    <!-- http://semanticweb.org/images/5/53/OntologySecurity.owlElGammelAlgorithm -->

    <owl:NamedIndividual rdf:about="&securitysw;ElGammelAlgorithm"/>
    


    <!-- http://semanticweb.org/images/5/53/OntologySecurity.owlIntegrity -->

    <owl:NamedIndividual rdf:about="&securitysw;Integrity"/>
    


    <!-- http://semanticweb.org/images/5/53/OntologySecurity.owlMD5 -->

    <owl:NamedIndividual rdf:about="&securitysw;MD5"/>
    


    <!-- http://semanticweb.org/images/5/53/OntologySecurity.owlNonRepudiation -->

    <owl:NamedIndividual rdf:about="&securitysw;NonRepudiation"/>
    


    <!-- http://semanticweb.org/images/5/53/OntologySecurity.owlRIPE-MD -->

    <owl:NamedIndividual rdf:about="&securitysw;RIPE-MD"/>
    


    <!-- http://semanticweb.org/images/5/53/OntologySecurity.owlRSAAlgorithm -->

    <owl:NamedIndividual rdf:about="&securitysw;RSAAlgorithm"/>
    


    <!-- http://semanticweb.org/images/5/53/OntologySecurity.owlSHA1 -->

    <owl:NamedIndividual rdf:about="&securitysw;SHA1"/>
    


    <!-- http://www-usr.inf.ufsm.br/~brunomozza/iotsec/iotsec.owl#AES -->

    <owl:NamedIndividual rdf:about="&iotsec;AES">
        <rdf:type rdf:resource="&iotsec;BlockCipher"/>
        <rdf:type rdf:resource="&iotsec;ManetSecurityMechanism"/>
        <rdfs:label xml:lang="en">Advanced Encryption Standard (AES)</rdfs:label>
        <iotsec:satisfies rdf:resource="&iotsec;Confidentiality"/>
        <owl:sameAs rdf:resource="&iotsec;Rijndael"/>
    </owl:NamedIndividual>
    


    <!-- http://www-usr.inf.ufsm.br/~brunomozza/iotsec/iotsec.owl#AccessControl -->

    <owl:NamedIndividual rdf:about="&iotsec;AccessControl">
        <rdf:type rdf:resource="&iotsec;SecurityProperty"/>
        <rdfs:label xml:lang="en">Access Control</rdfs:label>
        <rdfs:comment xml:lang="en">Access Control is the mechanism that allows owners of resources to define, manage and enforce access conditions applicable to each resource.</rdfs:comment>
        <owl:sameAs rdf:resource="&denker;AccessControl"/>
    </owl:NamedIndividual>
    


    <!-- http://www-usr.inf.ufsm.br/~brunomozza/iotsec/iotsec.owl#Accountability -->

    <owl:NamedIndividual rdf:about="&iotsec;Accountability">
        <rdf:type rdf:resource="&iotsec;SecurityProperty"/>
        <rdfs:label xml:lang="en">Accountability</rdfs:label>
        <owl:sameAs rdf:resource="&herzog;Accountability"/>
    </owl:NamedIndividual>
    


    <!-- http://www-usr.inf.ufsm.br/~brunomozza/iotsec/iotsec.owl#AdversaryInternal -->

    <owl:NamedIndividual rdf:about="&iotsec;AdversaryInternal">
        <rdf:type rdf:resource="&iotsec;ManetVulnerability"/>
        <rdfs:label xml:lang="en">Adversary inside the Network</rdfs:label>
        <rdfs:comment xml:lang="en">The mobile nodes within the MANET can freely join and leave the network. The nodes within network may also behave maliciously. This is hard to detect that the behavior of the node is malicious. Thus this attack is more dangerous than the external attack. These nodes are called compromised nodes [Goyal 2011].</rdfs:comment>
    </owl:NamedIndividual>
    


    <!-- http://www-usr.inf.ufsm.br/~brunomozza/iotsec/iotsec.owl#Anonymity -->

    <owl:NamedIndividual rdf:about="&iotsec;Anonymity"/>
    


    <!-- http://www-usr.inf.ufsm.br/~brunomozza/iotsec/iotsec.owl#ApplicationLayer -->

    <owl:NamedIndividual rdf:about="&iotsec;ApplicationLayer"/>
    


    <!-- http://www-usr.inf.ufsm.br/~brunomozza/iotsec/iotsec.owl#AuthenticationRepeatable -->

    <owl:NamedIndividual rdf:about="&iotsec;AuthenticationRepeatable">
        <rdf:type rdf:resource="&iotsec;BluetoothVulnerability"/>
        <rdfs:label xml:lang="en">Attempts for authentication are repeatable</rdfs:label>
        <rdfs:comment xml:lang="en">A mechanism needs to be included in Bluetooth devices to prevent unlimited authentication requests. The Bluetooth specification requires an exponentially increasing waiting interval between successive authentication attempts. However, it does not require such a waiting interval for authentication challenge requests, so an attacker could collect large numbers of challenge responses (which are encrypted with the secret link key) that could leak information about the secret link key [Padgette 2012].</rdfs:comment>
        <iotsec:affects xml:lang="en">Version before Bluetooth v4.0</iotsec:affects>
    </owl:NamedIndividual>
    


    <!-- http://www-usr.inf.ufsm.br/~brunomozza/iotsec/iotsec.owl#AuthenticationSimple -->

    <owl:NamedIndividual rdf:about="&iotsec;AuthenticationSimple">
        <rdf:type rdf:resource="&iotsec;BluetoothVulnerability"/>
        <rdfs:label xml:lang="en">Device authentication is simple shared-key challenge/response</rdfs:label>
        <rdfs:comment xml:lang="en">One-way-only challenge/response authentication is subject to MITM attacks. Bluetooth provides for mutual authentication, which should be used to provide verification that devices are legitimate [Padgette 2012].</rdfs:comment>
        <iotsec:affects xml:lang="en">Version before Bluetooth v4.0</iotsec:affects>
    </owl:NamedIndividual>
    


    <!-- http://www-usr.inf.ufsm.br/~brunomozza/iotsec/iotsec.owl#Authorization -->

    <owl:NamedIndividual rdf:about="&iotsec;Authorization">
        <rdfs:label xml:lang="en">Authorization</rdfs:label>
        <rdfs:comment xml:lang="en">IoT devices should be able to verify whether certain entities are authorized to access their measured data. At the network layer, only authorized devices should be able to access the IoT network. Unauthorized devices should not be able to route their messages over the IoT devices, because it may deplete their energy [Nguyen, 2015].</rdfs:comment>
    </owl:NamedIndividual>
    


    <!-- http://www-usr.inf.ufsm.br/~brunomozza/iotsec/iotsec.owl#Availability -->

    <owl:NamedIndividual rdf:about="&iotsec;Availability"/>
    


    <!-- http://www-usr.inf.ufsm.br/~brunomozza/iotsec/iotsec.owl#BDADDRAssociatedWithUser -->

    <owl:NamedIndividual rdf:about="&iotsec;BDADDRAssociatedWithUser">
        <rdf:type rdf:resource="&iotsec;BluetoothVulnerability"/>
        <rdfs:label xml:lang="en">Privacy may be compromised if the Bluetooth device address (BD_ADDR) is captured and associated with a particular user.</rdfs:label>
        <rdfs:comment xml:lang="en">Once the BD_ADDR is associated with a particular user, that user’s activities and location could be tracked [Padgette 2012].</rdfs:comment>
        <iotsec:affects xml:lang="en">Version before Bluetooth v4.0</iotsec:affects>
    </owl:NamedIndividual>
    


    <!-- http://www-usr.inf.ufsm.br/~brunomozza/iotsec/iotsec.owl#BandwidthConstraint -->

    <owl:NamedIndividual rdf:about="&iotsec;BandwidthConstraint">
        <rdf:type rdf:resource="&iotsec;ManetVulnerability"/>
        <rdfs:label xml:lang="en">Bandwidth constraint</rdfs:label>
        <rdfs:comment xml:lang="en">Variable low capacity links exists as compared to wireless network which are more susceptible to external noise, interference and signal attenuation effects [Goyal 2011].</rdfs:comment>
    </owl:NamedIndividual>
    


    <!-- http://www-usr.inf.ufsm.br/~brunomozza/iotsec/iotsec.owl#Blowfish -->

    <owl:NamedIndividual rdf:about="&iotsec;Blowfish"/>
    


    <!-- http://www-usr.inf.ufsm.br/~brunomozza/iotsec/iotsec.owl#BluetoothDevicesMode1AreInsecure -->

    <owl:NamedIndividual rdf:about="&iotsec;BluetoothDevicesMode1AreInsecure">
        <rdf:type rdf:resource="&iotsec;BluetoothVulnerability"/>
        <rdfs:label xml:lang="en">Security Mode 1 devices never initiate security mechanisms</rdfs:label>
        <rdfs:comment xml:lang="en">Devices that use Security Mode 1 are inherently insecure. For v2.0 and earlier devices, Security Mode 3 (link level security) is highly recommended [Padgette 2012].</rdfs:comment>
        <iotsec:affects xml:lang="en">Versions before Bluettoh 2.1</iotsec:affects>
    </owl:NamedIndividual>
    


    <!-- http://www-usr.inf.ufsm.br/~brunomozza/iotsec/iotsec.owl#BrokenAuthenticationSession -->

    <owl:NamedIndividual rdf:about="&iotsec;BrokenAuthenticationSession">
        <rdf:type rdf:resource="&iotsec;WebVulnerability"/>
        <rdfs:label xml:lang="en">Broken authentication and session management</rdfs:label>
        <rdfs:comment xml:lang="en">Application functions related to authentication and session management are often not implemented correctly, allowing attackers to compromise passwords, keys, or session tokens, or to exploit other implementation flaws to assume other users’ identities [OWASP Top Ten 2013].</rdfs:comment>
    </owl:NamedIndividual>
    


    <!-- http://www-usr.inf.ufsm.br/~brunomozza/iotsec/iotsec.owl#CAST -->

    <owl:NamedIndividual rdf:about="&iotsec;CAST"/>
    


    <!-- http://www-usr.inf.ufsm.br/~brunomozza/iotsec/iotsec.owl#CSRF -->

    <owl:NamedIndividual rdf:about="&iotsec;CSRF">
        <rdf:type rdf:resource="&iotsec;WebVulnerability"/>
        <rdfs:label xml:lang="en">Cross-Site Request Forgery (CSRF)</rdfs:label>
        <rdfs:comment xml:lang="en">A CSRF attack forces a logged-on victim’s browser to send a forged HTTP request, including the victim’s session cookie and any other automatically included authentication information, to a vulnerable web application. This allows the attacker to force the victim’s browser to generate requests the vulnerable application thinks are legitimate requests from the victim [OWASP Top Ten 2013].</rdfs:comment>
    </owl:NamedIndividual>
    


    <!-- http://www-usr.inf.ufsm.br/~brunomozza/iotsec/iotsec.owl#ChangeUserBankChangePC -->

    <owl:NamedIndividual rdf:about="&iotsec;ChangeUserBankChangePC">
        <rdf:type rdf:resource="&iotsec;RfidVulnerability"/>
        <rdfs:label xml:lang="en">Change of user bank causes change of PC</rdfs:label>
        <rdfs:comment xml:lang="en">User memory bank is initialized to all zero. Once the contents of 03-07h in the bank are changed to non-zero, the PC value of 15h in the EPC bank will be changed to 1. The change of the PC value will lead to the change of the CRC value at the same time. Some systems use PC+EPC+CRC to match the EPC information, for example, Tracer of Impinj. The change of PC and CRC will make tag illegal and bad effect on supply chain [Liu 2014].</rdfs:comment>
    </owl:NamedIndividual>
    


    <!-- http://www-usr.inf.ufsm.br/~brunomozza/iotsec/iotsec.owl#ComponentsKnownVulnerabilities -->

    <owl:NamedIndividual rdf:about="&iotsec;ComponentsKnownVulnerabilities">
        <rdf:type rdf:resource="&iotsec;WebVulnerability"/>
        <rdfs:label xml:lang="en">Using Components with Known Vulnerabilities</rdfs:label>
        <rdfs:comment xml:lang="en">Components, such as libraries, frameworks, and other software modules, almost always run with full privileges. If a vulnerable component is exploited, such an attack can facilitate serious data loss or server takeover. Applications using components with known vulnerabilities may undermine application defenses and enable a range of possible attacks and impacts [OWASP Top Ten 2013].</rdfs:comment>
    </owl:NamedIndividual>
    


    <!-- http://www-usr.inf.ufsm.br/~brunomozza/iotsec/iotsec.owl#Confidentiality -->

    <owl:NamedIndividual rdf:about="&iotsec;Confidentiality">
        <rdfs:label xml:lang="en">Confidentiality</rdfs:label>
        <rdfs:comment xml:lang="en">Exchanged messages in the IoT may need to be protected. An attacker should not gain knowledge about the messages exchanged between a sensor node and any other Internet entity [Nguyen, 2015].</rdfs:comment>
    </owl:NamedIndividual>
    


    <!-- http://www-usr.inf.ufsm.br/~brunomozza/iotsec/iotsec.owl#ConnectivityDevicesMode4WithOthers -->

    <owl:NamedIndividual rdf:about="&iotsec;ConnectivityDevicesMode4WithOthers">
        <rdf:type rdf:resource="&iotsec;BluetoothVulnerability"/>
        <rdfs:label xml:lang="en">Security Mode 4 devices (i.e., v2.1 or later) are allowed to fall back to any other security mode when connecting with devices that do not support Security Mode 4 (i.e., v2.0 and earlier).</rdfs:label>
        <rdfs:comment xml:lang="en">The worst-case scenario would be a device falling back to Security Mode 1, which provides no security. NIST strongly recommends that a Security Mode 4 device fall back to Security Mode 3 in this scenario.</rdfs:comment>
        <iotsec:affects xml:lang="en">Versions Bluetooth v2.1 and v3.0</iotsec:affects>
    </owl:NamedIndividual>
    


    <!-- http://www-usr.inf.ufsm.br/~brunomozza/iotsec/iotsec.owl#Correction -->

    <owl:NamedIndividual rdf:about="&iotsec;Correction">
        <rdf:type rdf:resource="&iotsec;TypeofDefense"/>
    </owl:NamedIndividual>
    


    <!-- http://www-usr.inf.ufsm.br/~brunomozza/iotsec/iotsec.owl#DES -->

    <owl:NamedIndividual rdf:about="&iotsec;DES"/>
    


    <!-- http://www-usr.inf.ufsm.br/~brunomozza/iotsec/iotsec.owl#Deliberate -->

    <owl:NamedIndividual rdf:about="&iotsec;Deliberate"/>
    


    <!-- http://www-usr.inf.ufsm.br/~brunomozza/iotsec/iotsec.owl#Detection -->

    <owl:NamedIndividual rdf:about="&iotsec;Detection">
        <rdf:type rdf:resource="&iotsec;TypeofDefense"/>
    </owl:NamedIndividual>
    


    <!-- http://www-usr.inf.ufsm.br/~brunomozza/iotsec/iotsec.owl#DiscoveredDevicesPronetoAttack -->

    <owl:NamedIndividual rdf:about="&iotsec;DiscoveredDevicesPronetoAttack">
        <rdf:type rdf:resource="&iotsec;BluetoothVulnerability"/>
        <rdfs:label xml:lang="en">Discoverable and/or connectable devices are prone to attack</rdfs:label>
        <iotsec:affects xml:lang="en">All versions</iotsec:affects>
        <rdfs:comment xml:lang="en">Any device that must go into discoverable or connectable mode to pair or connect should only do so for a minimal amount of time. A device should not be in discoverable or connectable mode all the time [Padgette 2012].</rdfs:comment>
    </owl:NamedIndividual>
    


    <!-- http://www-usr.inf.ufsm.br/~brunomozza/iotsec/iotsec.owl#DistributedManagement -->

    <owl:NamedIndividual rdf:about="&iotsec;DistributedManagement">
        <rdf:type rdf:resource="&iotsec;ManetVulnerability"/>
        <rdfs:label xml:lang="en">Distributed management</rdfs:label>
        <rdfs:comment xml:lang="en">MANET doesn’t have a centralized monitor server. The absence of management makes the detection of attacks difficult because it is not east to monitor the traffic in a highly dynamic and large scale ad-hoc network. Lack of centralized management will impede trust management for nodes [Goyal 2011].</rdfs:comment>
    </owl:NamedIndividual>
    


    <!-- http://www-usr.inf.ufsm.br/~brunomozza/iotsec/iotsec.owl#DoSFloodingHLRAuC -->

    <owl:NamedIndividual rdf:about="&iotsec;DoSFloodingHLRAuC">
        <rdf:type rdf:resource="&iotsec;UMTSVulnerability"/>
        <rdfs:label xml:lang="en">DoS by Flooding the HLR/AuC</rdfs:label>
        <rdfs:comment xml:lang="en">This is a much dangerous attack. It is a mobile operator specific attack. Using this attack, services of a particular mobile operator can be blocked. The attack may be launched in two phases:
	Phase I: In this phase the attacker builds a database of IMSIs corresponding to the victim operator. The attacker can easily obtain IMSIs. The attacker can identify the operator from IMSI as digits 4 and 5 (or 4, 5 and 6) represent the operator, within the IMSI structure.
	Phase II: In this phase the attacker quickly generates rrcConnectionRequests corresponding to each IMSI using an automatic procedure. For each request, (except already connected one) VLR/SGSN sends the IMSIs to the HLR/AuC. HLR/AuC checks the validity of IMSIs. Since attacker has obtained all valid IMSIs in phase I, therefore, all the IMSIs pass this validity test. Now HLR computes 5 AVs corresponding to each IMSI. This is a cumbersome process of calculating RAND, MAC, XRES, CK, IK, AK for each IMSI. The AVs corresponding to each IMSI are then sent to VLR/SGSN. For each IMSI, VLR/SGSN selects one AV and sends the RAND and AUTN for authentication. It is the stage where the attacker will not be authenticated, as it cannot calculate RES without knowledge of secret key of the USIM. But this is not the desire of the attacker, actually he has already done the job. His goal is to exhaust the computing resources of HLR/AuC by flooding more and more valid rrcConnectionRequests and making it to compute AVs. This may also cause bandwidth exhaustion between VLR/SGSN and HLR/AuC. This exhaustion of resources will result in DoS to new users who are attempting to connect [Khan 2008].</rdfs:comment>
    </owl:NamedIndividual>
    


    <!-- http://www-usr.inf.ufsm.br/~brunomozza/iotsec/iotsec.owl#DoSVulnerability -->

    <owl:NamedIndividual rdf:about="&iotsec;DoSVulnerability">
        <rdf:type rdf:resource="&iotsec;GSMVulnerability"/>
        <rdfs:label xml:lang="en">Vulnerability to the DoS attack</rdfs:label>
        <rdfs:comment xml:lang="en">A single attacker is capable of disabling an entire GSM cell via a Denial of Service (DoS) attack. The attacker can send the CHANNEL REQUEST message to the BSC for several times but he/she does not complete the protocol and requests another signaling channel. Since the number of signaling channels is limited, this leads to a DoS attack. It is feasible since the call setup protocol performs the resource allocations without adequate authentication. This attack is economical since it does not have any charge for the attacker. It can also be used for many practical situations such as terrorist attacks [Toorani 2008].</rdfs:comment>
    </owl:NamedIndividual>
    


    <!-- http://www-usr.inf.ufsm.br/~brunomozza/iotsec/iotsec.owl#DoSrrcConnectionRejectMessage -->

    <owl:NamedIndividual rdf:about="&iotsec;DoSrrcConnectionRejectMessage">
        <rdf:type rdf:resource="&iotsec;UMTSVulnerability"/>
        <rdfs:label xml:lang="en">DoS using rrcConnectionReject Message</rdfs:label>
        <rdfs:comment xml:lang="en">This is a user specific attack. Again in the first phase the attacker obtains IMSI of the victim. Now attacker waits for rrcConnectionRequest by this user. Initial UE identity is the unique identifier of this message. Initial UE identity may be Temporary Mobile Subscriber Identity (TMSI), Packet Temporary Mobile Subscriber Identity (P-TMSI), IMSI or International Mobile Equipment Identity (IMEI). Usually the first rrcConnectionRequest message contains IMSI of the user. The attacker will respond with rrcConnectionReject message. We know that rrcConnectionReject message is not integrity protected. The only way to assess its genuineness is the comparison of the value of the &quot;Initial UE identity&quot; in the received rrcConnectionReject message with the value of the variable “INITIAL_UE_IDENTITY” already available with UE. If the values are different, the UE shall ignore the rest of the message. If the values are identical, the UE shall terminate the connection. Hence an intruder knowing IMSI of the victim can easily generate a genuine rrcConnectionReject message and cause DoS to the user [Khan 2008].</rdfs:comment>
    </owl:NamedIndividual>
    


    <!-- http://www-usr.inf.ufsm.br/~brunomozza/iotsec/iotsec.owl#DynamicTopology -->

    <owl:NamedIndividual rdf:about="&iotsec;DynamicTopology">
        <rdf:type rdf:resource="&iotsec;ManetVulnerability"/>
        <rdfs:label xml:lang="en">Dynamic topology</rdfs:label>
        <rdfs:comment xml:lang="en">Dynamic topology and changeable nodes membership may disturb the trust relationship among nodes. The trust may also be disturbed if some nodes are detected as compromised. This dynamic behavior could be better protected with distributed and adaptive security mechanisms [Goyal 2011].

	Mobile nodes are autonomous units that are capable of roaming independently. This means that tracking down a particular mobile node in a large scale ad hoc network cannot be done easily [Djenouri 2005].</rdfs:comment>
    </owl:NamedIndividual>
    


    <!-- http://www-usr.inf.ufsm.br/~brunomozza/iotsec/iotsec.owl#E0AlgorithmBREDREncryptionIsWeak -->

    <owl:NamedIndividual rdf:about="&iotsec;E0AlgorithmBREDREncryptionIsWeak">
        <rdf:type rdf:resource="&iotsec;BluetoothVulnerability"/>
        <rdfs:label xml:lang="en">The E0 stream cipher algorithm used for Bluetooth BR/EDR encryption is relatively weak</rdfs:label>
        <rdfs:comment xml:lang="en">FIPS-approved encryption can be achieved by layering application-level FIPS-approved encryption over the Bluetooth BR/EDR encryption. Note that Bluetooth LE uses AES-CCM.</rdfs:comment>
        <iotsec:affects xml:lang="en">Version before Bluetooth v4.0</iotsec:affects>
    </owl:NamedIndividual>
    


    <!-- http://www-usr.inf.ufsm.br/~brunomozza/iotsec/iotsec.owl#ECC -->

    <owl:NamedIndividual rdf:about="&iotsec;ECC"/>
    


    <!-- http://www-usr.inf.ufsm.br/~brunomozza/iotsec/iotsec.owl#ElGamal -->

    <owl:NamedIndividual rdf:about="&iotsec;ElGamal"/>
    


    <!-- http://www-usr.inf.ufsm.br/~brunomozza/iotsec/iotsec.owl#EncryptionLengthKeyIsNegotiable -->

    <owl:NamedIndividual rdf:about="&iotsec;EncryptionLengthKeyIsNegotiable">
        <rdf:type rdf:resource="&iotsec;BluetoothVulnerability"/>
        <rdfs:label xml:lang="en">Encryption key length is negotiable</rdfs:label>
        <rdfs:comment xml:lang="en">Choose PIN codes that are sufficiently random, long and private. Avoid static and weak PINs, such as all zeroes. PIN codes should be random so that malicious users cannot easily guess them. Longer PIN codes are more resistant to brute force attacks. For Bluetooth devices, an eight-character alphanumeric PIN should be used, if possible. The use of a fixed PIN is not acceptable [Xu 2013].

	The v3.0 and earlier specifications allow devices to negotiate encryption keys as small as one byte. Bluetooth LE requires a minimum key size of seven bytes. NIST strongly recommends using the full 128-bit key strength for both BR/EDR (E0) and LE (AES- CCM) [Padgette 2012].</rdfs:comment>
    </owl:NamedIndividual>
    


    <!-- http://www-usr.inf.ufsm.br/~brunomozza/iotsec/iotsec.owl#EncryptionMasterKeyShared -->

    <owl:NamedIndividual rdf:about="&iotsec;EncryptionMasterKeyShared">
        <rdf:type rdf:resource="&iotsec;BluetoothVulnerability"/>
        <rdfs:label xml:lang="en">The master key used for broadcast encryption is shared among all piconet devices</rdfs:label>
        <rdfs:comment xml:lang="en">Secret keys shared amongst more than two parties facilitate impersonation attacks [Padgette 2012].</rdfs:comment>
        <iotsec:affects xml:lang="en">Version before Bluetooth v4.0</iotsec:affects>
    </owl:NamedIndividual>
    


    <!-- http://www-usr.inf.ufsm.br/~brunomozza/iotsec/iotsec.owl#EndtoEndSecurityIsNotPerformed -->

    <owl:NamedIndividual rdf:about="&iotsec;EndtoEndSecurityIsNotPerformed">
        <rdf:type rdf:resource="&iotsec;BluetoothVulnerability"/>
        <rdfs:label xml:lang="en">End-to-End security is not performed</rdfs:label>
        <rdfs:comment xml:lang="en">Invoke link encryption for all Bluetooth connections [Xu 2013].
	Link encryption should be used to secure all data transmissions during a Bluetooth connection; otherwise, transmitted data are vulnerable to eavesdropping [Xu 2013].</rdfs:comment>
    </owl:NamedIndividual>
    


    <!-- http://www-usr.inf.ufsm.br/~brunomozza/iotsec/iotsec.owl#FlawsA3A8Algorithms -->

    <owl:NamedIndividual rdf:about="&iotsec;FlawsA3A8Algorithms">
        <rdf:type rdf:resource="&iotsec;GSMVulnerability"/>
        <rdfs:label xml:lang="en">Flaws in implementation of A3/A8 algorithms</rdfs:label>
        <rdfs:comment xml:lang="en">Although the GSM architecture allows operator to choose any algorithm for A3 and A8, many operators used COMP128 (or COMP128-1) that was secretly developed by the GSM association. The structure of COMP128 was finally discovered by reverse engineering and some revealed documentations, and many security flaws were subsequently discovered. In addition to the fact that COMP128 makes revealing Ki possible especially when specific challenges are introduced, it deliberately sets ten rightmost bits of Kc equal to zero that makes the deployed cryptographic algorithms 1024 times weaker and more vulnerable, due to the decreased keyspace. Some GSM network operators tried another new algorithm for the A3/A8, called COMP128-2. COMP128-2 was also secretly designed and inherited the problem of decreased keyspace. Despite of such important problem, no other problems are reported so far. However, we can prospect for new discovered vulnerabilities in the future as it is secretly designed. An improved version of COMP128-2, called COM128-3, is also proposed that generates 64 bits of session key and resolves the problem of decreased keyspace [Toorani 2008].</rdfs:comment>
    </owl:NamedIndividual>
    


    <!-- http://www-usr.inf.ufsm.br/~brunomozza/iotsec/iotsec.owl#FlawsCryptographicAlgorithms -->

    <owl:NamedIndividual rdf:about="&iotsec;FlawsCryptographicAlgorithms">
        <rdf:type rdf:resource="&iotsec;GSMVulnerability"/>
        <rdfs:label xml:lang="en">Flaws in cryptographic algorithms</rdfs:label>
        <rdfs:comment xml:lang="en">Both A5/1 and A5/2 algorithms were developed in secret. The output of A5/1 is the XOR of three LFSRs. An efficient attack to A5/1 that can be used for a real-time cryptanalysis on a PC includes two kinds of attacks [Biryukov 2001]: The former that requires the first two minutes of eavesdropped encrypted conversation is capable of extracting the ciphering key in about one second, while the latter just needs two seconds of encrypted conversation to extract the ciphering key in several minutes. A5/2 is the deliberately weakened variant of A5/1. An efficient attack to A5/2 requires less than one second of encrypted conversation to extract the ciphering key in less than one second on a PC [Barkan 2003].
	Source [Toorani 2008].</rdfs:comment>
    </owl:NamedIndividual>
    


    <!-- http://www-usr.inf.ufsm.br/~brunomozza/iotsec/iotsec.owl#IDEA -->

    <owl:NamedIndividual rdf:about="&iotsec;IDEA"/>
    


    <!-- http://www-usr.inf.ufsm.br/~brunomozza/iotsec/iotsec.owl#IllegalReader -->

    <owl:NamedIndividual rdf:about="&iotsec;IllegalReader">
        <rdf:type rdf:resource="&iotsec;RfidVulnerability"/>
        <rdfs:label xml:lang="en">Illegal Reader</rdfs:label>
        <rdfs:comment xml:lang="en">The information of tags can be obtained as long as the reader meets the frequency and distance of reading and writing. Therefore, the tag cannot identify an illegal reader when the reader read the tag, which is the premise of causing other security vulnerabilities [Liu 2014].</rdfs:comment>
    </owl:NamedIndividual>
    


    <!-- http://www-usr.inf.ufsm.br/~brunomozza/iotsec/iotsec.owl#IncreasedRedundancyCodingPreference -->

    <owl:NamedIndividual rdf:about="&iotsec;IncreasedRedundancyCodingPreference">
        <rdf:type rdf:resource="&iotsec;GSMVulnerability"/>
        <rdfs:label xml:lang="en">Increased redundancy due to the coding preference</rdfs:label>
        <rdfs:comment xml:lang="en">The Forward Error Correcting (FEC) is performed prior to the ciphering so there is a redundancy that increases the security vulnerabilities of deployed cryptographic algorithms [Toorani 2008].</rdfs:comment>
    </owl:NamedIndividual>
    


    <!-- http://www-usr.inf.ufsm.br/~brunomozza/iotsec/iotsec.owl#Injection -->

    <owl:NamedIndividual rdf:about="&iotsec;Injection">
        <rdf:type rdf:resource="&iotsec;WebVulnerability"/>
    </owl:NamedIndividual>
    


    <!-- http://www-usr.inf.ufsm.br/~brunomozza/iotsec/iotsec.owl#InsecureCryptography -->

    <owl:NamedIndividual rdf:about="&iotsec;InsecureCryptography">
        <rdf:type rdf:resource="&iotsec;CloudVulnerability"/>
        <rdfs:label xml:lang="en">Insecure or obsolete cryptography</rdfs:label>
        <rdfs:comment xml:lang="en">Cryptoanalysis advances can render any cryptographic mechanism or algorithm insecure as novel methods of breaking them are discovered. It’s even more common to find crucial flaws in cryptographic algorithm implementations, which can turn strong encryption into weak encryption (or sometimes no encryption at all). Because broad uptake of cloud computing is unthinkable without the use of cryptography to protect data confidentiality and integrity in the cloud, insecure or obsolete cryptography vulnerabilities are highly relevant for cloud computing [Grobauer 2011].</rdfs:comment>
    </owl:NamedIndividual>
    


    <!-- http://www-usr.inf.ufsm.br/~brunomozza/iotsec/iotsec.owl#InsecureDirectObjectRef -->

    <owl:NamedIndividual rdf:about="&iotsec;InsecureDirectObjectRef">
        <rdf:type rdf:resource="&iotsec;WebVulnerability"/>
        <rdfs:label xml:lang="en">Insecure Direct Object References</rdfs:label>
        <rdfs:comment xml:lang="en">A direct object reference occurs when a developer exposes a reference to an internal implementation object, such as a file, directory, or database key. Without an access control check or other protection, attackers can manipulate these references to access unauthorized data [OWASP Top Ten 2013].</rdfs:comment>
    </owl:NamedIndividual>
    


    <!-- http://www-usr.inf.ufsm.br/~brunomozza/iotsec/iotsec.owl#Integrity -->

    <owl:NamedIndividual rdf:about="&iotsec;Integrity">
        <rdfs:label xml:lang="en">Integrity</rdfs:label>
        <rdfs:comment xml:lang="en">The alteration of messages should be detected by the receiver [Nguyen, 2015].</rdfs:comment>
    </owl:NamedIndividual>
    


    <!-- http://www-usr.inf.ufsm.br/~brunomozza/iotsec/iotsec.owl#IntegrityProtection -->

    <owl:NamedIndividual rdf:about="&iotsec;IntegrityProtection">
        <rdf:type rdf:resource="&iotsec;GSMVulnerability"/>
        <rdfs:label xml:lang="en">Absence of integrity protection</rdfs:label>
        <rdfs:comment xml:lang="en">Although the GSM security architecture considers authentication and confidentiality, there is no provision for any integrity protection of information. Therefore, the recipient cannot verify that a certain message was not tampered with.</rdfs:comment>
    </owl:NamedIndividual>
    


    <!-- http://www-usr.inf.ufsm.br/~brunomozza/iotsec/iotsec.owl#IntegrityProtectionUserData -->

    <owl:NamedIndividual rdf:about="&iotsec;IntegrityProtectionUserData">
        <rdf:type rdf:resource="&iotsec;UMTSVulnerability"/>
        <rdfs:label xml:lang="en">Integrity protection of user data</rdfs:label>
        <rdfs:comment xml:lang="en">Cryptographic integrity protection in UMTS is implemented in only a limited part of the system. Only signaling data is protected and the protection is limited to transmission between the SRNC and UE. User data is not integrity protected. Presently, it is assumed that if the data is successfully decrypted then it has not been changed in the way. The above assumption might be valid for speech and written prose. For user data with high uncertainty of outcome, e.g. figures in a bank transaction, the low-grade integrity protection implicitly offered by encryption/ decryption is not satisfactory [Khan 2008].</rdfs:comment>
    </owl:NamedIndividual>
    


    <!-- http://www-usr.inf.ufsm.br/~brunomozza/iotsec/iotsec.owl#KeyStoringImproperly -->

    <owl:NamedIndividual rdf:about="&iotsec;KeyStoringImproperly">
        <rdf:type rdf:resource="&iotsec;BluetoothVulnerability"/>
        <rdfs:label xml:lang="en">Link keys can be stored improperly</rdfs:label>
        <iotsec:affects xml:lang="en">All versions</iotsec:affects>
        <rdfs:comment xml:lang="en">Link keys can be read or modified by an attacker if they are not securely stored and protected via access controls [Padgette 2012].</rdfs:comment>
    </owl:NamedIndividual>
    


    <!-- http://www-usr.inf.ufsm.br/~brunomozza/iotsec/iotsec.owl#LEPairingNoEavesdroppingProtection -->

    <owl:NamedIndividual rdf:about="&iotsec;LEPairingNoEavesdroppingProtection">
        <rdf:type rdf:resource="&iotsec;BluetoothVulnerability"/>
        <rdfs:label xml:lang="en">Low-Energy Pairing provides no eavesdropping protection</rdfs:label>
        <rdfs:comment xml:lang="en">For v2.1 and later devices using SSP, avoid using the ”Just Work-s” association model. The device must verify that an authenticated link key was generated during pairing [Xu 2013].
	The Just Works association model does not provide MITM protection. Devices that only support Just Works should not be procured if similarly qualified devices that support one of the other association models are available [Xu 2013].
	If successful, eavesdroppers can capture secret keys (i.e., LTK, CSRK, IRK) distributed during LE pairing. Further, MITM attackers can capture and manipulate data transmitted between trusted devices. LE devices should be paired in a secure environment to minimize the risk of eavesdropping and MITM attacks. Just Works pairing should not be used [Padgette 2012].</rdfs:comment>
        <iotsec:affects xml:lang="en">Versions Bluetooth v4.0</iotsec:affects>
    </owl:NamedIndividual>
    


    <!-- http://www-usr.inf.ufsm.br/~brunomozza/iotsec/iotsec.owl#LESecurityMode1Level1NoRequireSecurityMechanisms -->

    <owl:NamedIndividual rdf:about="&iotsec;LESecurityMode1Level1NoRequireSecurityMechanisms">
        <rdf:type rdf:resource="&iotsec;BluetoothVulnerability"/>
        <rdfs:label xml:lang="en">Low-Energy Security Mode 1 Level 1 does not require any security mechanisms</rdfs:label>
        <rdfs:comment xml:lang="en">LE devices and services should use Security Mode 1 Level 3 whenever possible. LE Security Mode 1 Level 3 provides the highest security available for LE devices [Xu 2013].
	Other LE security modes allow unauthenticated pairing and/or no encryption [Xu 2013].
	Similar to BR/EDR Security Mode 1, this is inherently insecure. LE Security Mode 1 Level 3 (authenticated pairing and encryption) is highly recommended instead [Padgette 2012].</rdfs:comment>
    </owl:NamedIndividual>
    


    <!-- http://www-usr.inf.ufsm.br/~brunomozza/iotsec/iotsec.owl#LackingRandomnessOfPIN -->

    <owl:NamedIndividual rdf:about="&iotsec;LackingRandomnessOfPIN">
        <rdf:type rdf:resource="&iotsec;BluetoothVulnerability"/>
        <rdfs:label xml:lang="en">PIN management and randomness is lacking</rdfs:label>
        <rdfs:comment xml:lang="en">Establishing use of adequate PINs in an enterprise setting with many users may be difficult. Scalability problems frequently yield security problems. The best alternative is for one of the devices being paired to generate the PIN using its random number generator [Padgette 2012].</rdfs:comment>
        <iotsec:affects xml:lang="en">Versions Before Bluetooth v2.1</iotsec:affects>
    </owl:NamedIndividual>
    


    <!-- http://www-usr.inf.ufsm.br/~brunomozza/iotsec/iotsec.owl#LimitedPower -->

    <owl:NamedIndividual rdf:about="&iotsec;LimitedPower">
        <rdf:type rdf:resource="&iotsec;ManetVulnerability"/>
        <rdfs:label xml:lang="en">Limited power supply</rdfs:label>
        <rdfs:comment xml:lang="en">The nodes in mobile ad-hoc network need to consider restricted power supply, which will cause several problems. A node in mobile ad-hoc network may behave in a selfish manner when it is finding that there is only limited power supply [Goyal 2011].

	Ad hoc enabled mobile nodes are small and lightweight, therefore, they are often supplied with limited power resources, small batteries, to ensure portability. The security solution should take this restraint into account. Furthermore, this limitation causes a vulnerability since a node powering-off can cause its break-down. Thereby, attackers may targets some nodes batteries to disconnect them, even to make network partition [Djenouri 2005].</rdfs:comment>
    </owl:NamedIndividual>
    


    <!-- http://www-usr.inf.ufsm.br/~brunomozza/iotsec/iotsec.owl#LinkLayer -->

    <owl:NamedIndividual rdf:about="&iotsec;LinkLayer"/>
    


    <!-- http://www-usr.inf.ufsm.br/~brunomozza/iotsec/iotsec.owl#MD5 -->

    <owl:NamedIndividual rdf:about="&iotsec;MD5"/>
    


    <!-- http://www-usr.inf.ufsm.br/~brunomozza/iotsec/iotsec.owl#ManetCooperativeness -->

    <owl:NamedIndividual rdf:about="&iotsec;ManetCooperativeness">
        <rdf:type rdf:resource="&iotsec;ManetVulnerability"/>
        <rdfs:label xml:lang="en">Manet cooperativeness</rdfs:label>
        <rdfs:comment xml:lang="en">Routing algorithm for MANETs usually assumes that nodes are cooperative and non-malicious. As a result a malicious attacker can easily become an important routing agent and disrupt network operation by disobeying the protocol specifications [Goyal 2011].</rdfs:comment>
    </owl:NamedIndividual>
    


    <!-- http://www-usr.inf.ufsm.br/~brunomozza/iotsec/iotsec.owl#ManetScalability -->

    <owl:NamedIndividual rdf:about="&iotsec;ManetScalability">
        <rdf:type rdf:resource="&iotsec;ManetVulnerability"/>
        <rdfs:label xml:lang="en">Manet scalability</rdfs:label>
        <rdfs:comment xml:lang="en">Due to mobility of nodes, scale of ad-hoc network changing all the time. So scalability is a major issue concerning security. Security mechanism should be capable of handling a large network as well as small ones [Goyal 2011].</rdfs:comment>
    </owl:NamedIndividual>
    


    <!-- http://www-usr.inf.ufsm.br/~brunomozza/iotsec/iotsec.owl#MeshArchitecture -->

    <owl:NamedIndividual rdf:about="&iotsec;MeshArchitecture"/>
    


    <!-- http://www-usr.inf.ufsm.br/~brunomozza/iotsec/iotsec.owl#MissingFunctionLevelAccessControl -->

    <owl:NamedIndividual rdf:about="&iotsec;MissingFunctionLevelAccessControl">
        <rdf:type rdf:resource="&iotsec;WebVulnerability"/>
        <rdfs:label xml:lang="en">Missing Function Level Access Control</rdfs:label>
        <rdfs:comment xml:lang="en">Most web applications verify function level access rights before making that functionality visible in the UI. However, applications need to perform the same access control checks on the server when each function is accessed. If requests are not verified, attackers will be able to forge requests in order to access functionality without proper authorization [OWASP Top Ten 2013].</rdfs:comment>
    </owl:NamedIndividual>
    


    <!-- http://www-usr.inf.ufsm.br/~brunomozza/iotsec/iotsec.owl#MultitagCollision -->

    <owl:NamedIndividual rdf:about="&iotsec;MultitagCollision">
        <rdf:type rdf:resource="&iotsec;RfidVulnerability"/>
        <rdfs:label xml:lang="en">Multi-tag collision</rdfs:label>
        <rdfs:comment xml:lang="en">When a reader sends command to a group of tags in its working area, more than one tag answer the command to make the responses mutual interference. As a result, the reader cannot correctly identify any of the tags, and then the reading speed and efficiency are reduced. With the number of tags increasing, the probability of multi-tag collision increases [Liu 2014].</rdfs:comment>
    </owl:NamedIndividual>
    


    <!-- http://www-usr.inf.ufsm.br/~brunomozza/iotsec/iotsec.owl#NetUSB -->

    <owl:NamedIndividual rdf:about="&iotsec;NetUSB">
        <rdf:type rdf:resource="&iotsec;WifiTechnology"/>
        <rdfs:label xml:lang="en">NetUSB
</rdfs:label>
        <rdfs:comment xml:lang="en">NetUSB is a proprietary technology developed by the Taiwanese company KCodes that provides connections to the server with simulate devices that are plugged into the embedded system locally.</rdfs:comment>
    </owl:NamedIndividual>
    


    <!-- http://www-usr.inf.ufsm.br/~brunomozza/iotsec/iotsec.owl#NetworkLayer -->

    <owl:NamedIndividual rdf:about="&iotsec;NetworkLayer"/>
    


    <!-- http://www-usr.inf.ufsm.br/~brunomozza/iotsec/iotsec.owl#NoBoundary -->

    <owl:NamedIndividual rdf:about="&iotsec;NoBoundary">
        <rdf:type rdf:resource="&iotsec;ManetVulnerability"/>
        <rdfs:label xml:lang="en">No predefined Boundary</rdfs:label>
        <rdfs:comment xml:lang="en">In mobile ad-hoc networks we cannot precisely define a physical boundary of the network. The nodes work in a nomadic environment where they are allowed to join and leave the wireless network. As soon as an adversary comes in the radio range of a node it will be able to communicate with that node. The attacks include Eavesdropping impersonation; tempering, replay and Denial of Service (DoS) attack [Goyal 2011].</rdfs:comment>
    </owl:NamedIndividual>
    


    <!-- http://www-usr.inf.ufsm.br/~brunomozza/iotsec/iotsec.owl#NoEndtoEndSecurity -->

    <owl:NamedIndividual rdf:about="&iotsec;NoEndtoEndSecurity">
        <rdf:type rdf:resource="&iotsec;BluetoothVulnerability"/>
        <rdfs:label xml:lang="en">End-to-end security is not performed</rdfs:label>
        <iotsec:affects xml:lang="en">All versions</iotsec:affects>
        <rdfs:comment xml:lang="en">Only individual links are encrypted and authenticated. Data is decrypted at intermediate points. End-to-end security on top of the Bluetooth stack can be provided by use of additional security controls [Padgette 2012].</rdfs:comment>
    </owl:NamedIndividual>
    


    <!-- http://www-usr.inf.ufsm.br/~brunomozza/iotsec/iotsec.owl#NoUserAuthentication -->

    <owl:NamedIndividual rdf:about="&iotsec;NoUserAuthentication">
        <rdf:type rdf:resource="&iotsec;BluetoothVulnerability"/>
        <rdfs:label xml:lang="en">No user authentication exists</rdfs:label>
        <iotsec:affects xml:lang="en">All versions</iotsec:affects>
        <rdfs:comment xml:lang="en">Only device authentication is provided by the specification. Application-level security, including user authentication, can be added via overlay by the application developer [Padgette 2012].</rdfs:comment>
    </owl:NamedIndividual>
    


    <!-- http://www-usr.inf.ufsm.br/~brunomozza/iotsec/iotsec.owl#NonRepudiation -->

    <owl:NamedIndividual rdf:about="&iotsec;NonRepudiation"/>
    


    <!-- http://www-usr.inf.ufsm.br/~brunomozza/iotsec/iotsec.owl#OvertheAirCracking -->

    <owl:NamedIndividual rdf:about="&iotsec;OvertheAirCracking">
        <rdf:type rdf:resource="&iotsec;GSMVulnerability"/>
        <rdfs:label xml:lang="en">Over-the-air cracking</rdfs:label>
        <rdfs:comment xml:lang="en">It is feasible to misuse the vulnerability of COMP128 for extracting the Ki of the target user without any physical access to the SIM. This can be accomplished by sending several challenges over the air to the SIM and analyzing the responses. However, this approach may take several hours. The attacker can also extract IMSI using an approach that will be explained later. After finding Ki and IMSI of the target subscriber, the attacker can clone the SIM and make and receive calls and other services such as SMS in the name of the victim subscriber. However, the attacker will encounter with a slight problem. The GSM network allows only one SIM to access to the network at any given time so if the attacker and the victim subscriber try to access from different locations, the network will realize existence of duplicated cards and disables the affected account [Toorani 2008].
	</rdfs:comment>
    </owl:NamedIndividual>
    


    <!-- http://www-usr.inf.ufsm.br/~brunomozza/iotsec/iotsec.owl#PINsShort -->

    <owl:NamedIndividual rdf:about="&iotsec;PINsShort">
        <rdf:type rdf:resource="&iotsec;BluetoothVulnerability"/>
        <rdfs:label xml:lang="en">PINs can be too short</rdfs:label>
        <iotsec:affects xml:lang="en">Version before Bluetooth v2.1</iotsec:affects>
        <rdfs:comment xml:lang="en">Weak PINs, which are used to protect the generation of link keys during pairing, can be easily guessed. People have a tendency to select short PINs [Padgette 2012].</rdfs:comment>
    </owl:NamedIndividual>
    


    <!-- http://www-usr.inf.ufsm.br/~brunomozza/iotsec/iotsec.owl#PRNGaNoKnown -->

    <owl:NamedIndividual rdf:about="&iotsec;PRNGaNoKnown">
        <rdf:type rdf:resource="&iotsec;BluetoothVulnerability"/>
        <rdfs:label xml:lang="en">Strengths of the pseudo-random number generators (PRNG) are not known</rdfs:label>
        <iotsec:affects xml:lang="en">All versions</iotsec:affects>
        <rdfs:comment xml:lang="en">The Random Number Generator (RNG) may produce static or periodic numbers that may reduce the effectiveness of the security mechanisms. Bluetooth implementations should use strong PRNGs based on NIST standards [Padgette 2012].</rdfs:comment>
    </owl:NamedIndividual>
    


    <!-- http://www-usr.inf.ufsm.br/~brunomozza/iotsec/iotsec.owl#PairingJustWorksModel -->

    <owl:NamedIndividual rdf:about="&iotsec;PairingJustWorksModel">
        <rdf:type rdf:resource="&iotsec;BluetoothVulnerability"/>
        <rdfs:label xml:lang="en">Just Works association model does not provide MITM protection during pairing, which results in an unauthenticated link key</rdfs:label>
        <rdfs:comment xml:lang="en">For highest security, devices should require MITM protection during SSP and refuse to accept unauthenticated link keys generated using Just Works pairing [Padgette 2012].</rdfs:comment>
        <iotsec:affects xml:lang="en">Versions Bluetooth v2.1 and v3.0</iotsec:affects>
    </owl:NamedIndividual>
    


    <!-- http://www-usr.inf.ufsm.br/~brunomozza/iotsec/iotsec.owl#PasswordCracked -->

    <owl:NamedIndividual rdf:about="&iotsec;PasswordCracked">
        <rdf:type rdf:resource="&iotsec;RfidVulnerability"/>
        <rdfs:label xml:lang="en">Password is Cracked</rdfs:label>
        <rdfs:comment xml:lang="en">For people’s living habits, careless attitude and other reasons, password is set very simple. Though the 32 bits password is relative long, it also may be cracked. Once cracked, the information of memory bank can be tampered easily by attacker. If the kill password is cracked, attacker can use kill password to kill the tag and cause it useless [Liu 2014].</rdfs:comment>
    </owl:NamedIndividual>
    


    <!-- http://www-usr.inf.ufsm.br/~brunomozza/iotsec/iotsec.owl#PermissionPublic -->

    <owl:NamedIndividual rdf:about="&iotsec;PermissionPublic">
        <rdf:type rdf:resource="&iotsec;RfidVulnerability"/>
        <rdfs:label xml:lang="en">Reading Permission in Public</rdfs:label>
        <rdfs:comment xml:lang="en">Read permission of tag is not set for access control. Any reader can read the information of tags, which exposes information privacy and leads to information leakage. EPC contains important commercial information. To the whole supply chains in the EPC network, the information leakage is dangerous. Utilizing the leaked information, malicious users can clone the tags and put them mixed with legitimate tags [Liu 2014].</rdfs:comment>
    </owl:NamedIndividual>
    


    <!-- http://www-usr.inf.ufsm.br/~brunomozza/iotsec/iotsec.owl#PhysicalLayer -->

    <owl:NamedIndividual rdf:about="&iotsec;PhysicalLayer"/>
    


    <!-- http://www-usr.inf.ufsm.br/~brunomozza/iotsec/iotsec.owl#PoorPhysicalSecurity -->

    <owl:NamedIndividual rdf:about="&iotsec;PoorPhysicalSecurity">
        <rdf:type rdf:resource="&iotsec;RfidVulnerability"/>
        <rdfs:label xml:lang="en">Poor physical security</rdfs:label>
        <rdfs:comment xml:lang="en">An RFID vandal who is just interested in annoying people or disrupting operation may easily destroy RFID tags with poor physical protection by applying pressure or tension loads, by chemical exposure or even by clipping any visible antennas off. But even if RFID tags escape from the malicious intentions of a vandal they are still susceptible of possible destruction caused by extreme environmental conditions such as too high or too low temperatures or even abrasion caused by rough handling [Liu 2014].</rdfs:comment>
    </owl:NamedIndividual>
    


    <!-- http://www-usr.inf.ufsm.br/~brunomozza/iotsec/iotsec.owl#PresentationLayer -->

    <owl:NamedIndividual rdf:about="&iotsec;PresentationLayer"/>
    


    <!-- http://www-usr.inf.ufsm.br/~brunomozza/iotsec/iotsec.owl#Prevention -->

    <owl:NamedIndividual rdf:about="&iotsec;Prevention">
        <rdf:type rdf:resource="&iotsec;TypeofDefense"/>
    </owl:NamedIndividual>
    


    <!-- http://www-usr.inf.ufsm.br/~brunomozza/iotsec/iotsec.owl#RC4 -->

    <owl:NamedIndividual rdf:about="&iotsec;RC4"/>
    


    <!-- http://www-usr.inf.ufsm.br/~brunomozza/iotsec/iotsec.owl#RIPE-MD -->

    <owl:NamedIndividual rdf:about="&iotsec;RIPE-MD"/>
    


    <!-- http://www-usr.inf.ufsm.br/~brunomozza/iotsec/iotsec.owl#RSA -->

    <owl:NamedIndividual rdf:about="&iotsec;RSA"/>
    


    <!-- http://www-usr.inf.ufsm.br/~brunomozza/iotsec/iotsec.owl#RSN -->

    <owl:NamedIndividual rdf:about="&iotsec;RSN"/>
    


    <!-- http://www-usr.inf.ufsm.br/~brunomozza/iotsec/iotsec.owl#Recovery -->

    <owl:NamedIndividual rdf:about="&iotsec;Recovery">
        <rdf:type rdf:resource="&iotsec;TypeofDefense"/>
    </owl:NamedIndividual>
    


    <!-- http://www-usr.inf.ufsm.br/~brunomozza/iotsec/iotsec.owl#RepetitionEncryptionKeystream -->

    <owl:NamedIndividual rdf:about="&iotsec;RepetitionEncryptionKeystream">
        <rdf:type rdf:resource="&iotsec;BluetoothVulnerability"/>
        <rdfs:label xml:lang="en">The encryption keystream repeats after 23.3 hours of use.</rdfs:label>
        <rdfs:comment xml:lang="en">The encryption keystream is dependent on the link key, EN_RAND, Master BD_ADDR, and Clock.Only the Master’s clock will change during a particular encrypted connection. If a connection lasts more than 23.3 hours, the clock value will begin to repeat, hence generating an identical keystream to that used earlier in the connection. Repeating a keystream is a serious cryptographic vulnerability that would allow an attacker to determine the original plain text [Padgette 2012].</rdfs:comment>
        <iotsec:affects xml:lang="en">Versions before Bluetooth v2.1</iotsec:affects>
    </owl:NamedIndividual>
    


    <!-- http://www-usr.inf.ufsm.br/~brunomozza/iotsec/iotsec.owl#ReplayVulnerability -->

    <owl:NamedIndividual rdf:about="&iotsec;ReplayVulnerability">
        <rdf:type rdf:resource="&iotsec;GSMVulnerability"/>
        <rdfs:label xml:lang="en">Vulnerability to replay attacks</rdfs:label>
        <rdfs:comment xml:lang="en">The attacker can misuse the previously exchanged messages between the subscriber and network in order to perform the replay attacks [Toorani 2008].</rdfs:comment>
    </owl:NamedIndividual>
    


    <!-- http://www-usr.inf.ufsm.br/~brunomozza/iotsec/iotsec.owl#ResourceAvailability -->

    <owl:NamedIndividual rdf:about="&iotsec;ResourceAvailability">
        <rdf:type rdf:resource="&iotsec;ManetVulnerability"/>
        <rdfs:label xml:lang="en">Resource availability</rdfs:label>
        <rdfs:comment xml:lang="en">Resource availability is a major issue in MANET. Providing secure communication in such changing environment as well as protection against specific threats and attacks, leads to development of various security schemes and architectures. Collaborative ad-hoc environments also allow implementation of self-organized security mechanism [Goyal 2011].</rdfs:comment>
    </owl:NamedIndividual>
    


    <!-- http://www-usr.inf.ufsm.br/~brunomozza/iotsec/iotsec.owl#Response -->

    <owl:NamedIndividual rdf:about="&iotsec;Response">
        <rdf:type rdf:resource="&iotsec;TypeofDefense"/>
    </owl:NamedIndividual>
    


    <!-- http://www-usr.inf.ufsm.br/~brunomozza/iotsec/iotsec.owl#RevealSubscriberIdentity -->

    <owl:NamedIndividual rdf:about="&iotsec;RevealSubscriberIdentity">
        <rdf:type rdf:resource="&iotsec;UMTSVulnerability"/>
        <rdfs:label xml:lang="en">Reveal of Subscriber’s Identity</rdfs:label>
        <rdfs:comment xml:lang="en">UMTS offers little protection against identity catching. Although IMSI is replaced by TMSIs after the initial connection request, IMSI is sent clear during the first rrcConnectionRequest and also on the occasions like VLR database crash, VLR’s inability to identify the TMSI. Hence the user identity/location confidentiality and user traceability are clearly violated [Khan 2008].</rdfs:comment>
    </owl:NamedIndividual>
    


    <!-- http://www-usr.inf.ufsm.br/~brunomozza/iotsec/iotsec.owl#Rijndael -->

    <owl:NamedIndividual rdf:about="&iotsec;Rijndael"/>
    


    <!-- http://www-usr.inf.ufsm.br/~brunomozza/iotsec/iotsec.owl#SHA -->

    <owl:NamedIndividual rdf:about="&iotsec;SHA"/>
    


    <!-- http://www-usr.inf.ufsm.br/~brunomozza/iotsec/iotsec.owl#SIMCardCloning -->

    <owl:NamedIndividual rdf:about="&iotsec;SIMCardCloning">
        <rdf:type rdf:resource="&iotsec;GSMVulnerability"/>
        <rdfs:comment xml:lang="en">Another important challenge is to derive the root key Ki from the subscriber&apos;s SIM. In April 1998, the Smartcard Developer Association (SDA) and the ISAAC research group could find an important vulnerability in the COMP128 algorithm that helped them to extract Ki in eight hours by sending many challenges to the SIM. Subsequently, some other schemes were proposed that were based on the chosen challenges and were capable of extracting Ki in fewer times. Ultimately, a side-channel attack, called partitioning attack, was proposed by the IBM researchers that makes attacker capable of extracting Ki if he could access the subscriber&apos;s SIM just for one minute [Rao 2002]. The attacker can then clone the SIM and use it for his fraudulent purposes. The COMP128 algorithm needs large lookup tables that would leak some important information via the side channels when it is implemented on a small SIM [Toorani 2008].</rdfs:comment>
    </owl:NamedIndividual>
    


    <!-- http://www-usr.inf.ufsm.br/~brunomozza/iotsec/iotsec.owl#SSL -->

    <owl:NamedIndividual rdf:about="&iotsec;SSL"/>
    


    <!-- http://www-usr.inf.ufsm.br/~brunomozza/iotsec/iotsec.owl#SSPECDHkeypairsStaticOrWeak -->

    <owl:NamedIndividual rdf:about="&iotsec;SSPECDHkeypairsStaticOrWeak">
        <rdf:type rdf:resource="&iotsec;BluetoothVulnerability"/>
        <rdfs:label xml:lang="en">SSP ECDH keypairs may be static orotherwise weakly generated</rdfs:label>
        <iotsec:affects xml:lang="en">Versions Bluetooth v2.1 and v3.0</iotsec:affects>
        <rdfs:comment xml:lang="en">Weak ECDH keypairs minimize SSP eavesdropping protection,which may allow attackers to determine secret link keys. All devices should have unique, strongly-generated ECDH keypairs that change regularly [Padgette 2012]. </rdfs:comment>
    </owl:NamedIndividual>
    


    <!-- http://www-usr.inf.ufsm.br/~brunomozza/iotsec/iotsec.owl#SecurityMisconfiguration -->

    <owl:NamedIndividual rdf:about="&iotsec;SecurityMisconfiguration">
        <rdf:type rdf:resource="&iotsec;WebVulnerability"/>
        <rdfs:label xml:lang="en">Security misconfiguration</rdfs:label>
        <rdfs:comment xml:lang="en">Good security requires having a secure configuration defined and deployed for the application, frameworks, application server, web server, database server, and platform. Secure settings should be defined, implemented, and maintained, as defaults are often insecure. Additionally, software should be kept up to date [OWASP Top Ten 2013].</rdfs:comment>
    </owl:NamedIndividual>
    


    <!-- http://www-usr.inf.ufsm.br/~brunomozza/iotsec/iotsec.owl#SecurityServicesAreLimited -->

    <owl:NamedIndividual rdf:about="&iotsec;SecurityServicesAreLimited">
        <rdf:type rdf:resource="&iotsec;BluetoothVulnerability"/>
        <rdfs:label xml:lang="en">Security services are limited</rdfs:label>
        <rdfs:comment xml:lang="en">Many Bluetooth stacks are designed to support multiple profiles and associated services. The Bluetooth stack on a device should be locked down to ensure only approved profiles and services are available for use [Xu 2013]. Service and profile lockdown of device Bluetooth stacks should be performed [Xu 2013].</rdfs:comment>
    </owl:NamedIndividual>
    


    <!-- http://www-usr.inf.ufsm.br/~brunomozza/iotsec/iotsec.owl#SecurityServicesLimited -->

    <owl:NamedIndividual rdf:about="&iotsec;SecurityServicesLimited">
        <rdf:type rdf:resource="&iotsec;BluetoothVulnerability"/>
        <rdfs:label xml:lang="en">Security services are limited</rdfs:label>
        <iotsec:affects xml:lang="en">All versions</iotsec:affects>
        <rdfs:comment xml:lang="en">Audit, non-repudiation, and other services are not part of the standard. If needed, these services can be incorporated in an overlay fashion by the application developer [Padgette 2012].</rdfs:comment>
    </owl:NamedIndividual>
    


    <!-- http://www-usr.inf.ufsm.br/~brunomozza/iotsec/iotsec.owl#SentitiveDataExposure -->

    <owl:NamedIndividual rdf:about="&iotsec;SentitiveDataExposure">
        <rdf:type rdf:resource="&iotsec;WebVulnerability"/>
        <rdfs:label xml:lang="en">Sensitive data exposure</rdfs:label>
        <rdfs:comment xml:lang="en">Many web applications do not properly protect sensitive data, such as credit cards, tax IDs, and authentication credentials. Attackers may steal or modify such weakly protected data to conduct credit card fraud, identity theft, or other crimes. Sensitive data deserves extra protection such as encryption at rest or in transit, as well as special precautions when exchanged with the browser [OWASP Top Ten 2013].</rdfs:comment>
    </owl:NamedIndividual>
    


    <!-- http://www-usr.inf.ufsm.br/~brunomozza/iotsec/iotsec.owl#SessionLayer -->

    <owl:NamedIndividual rdf:about="&iotsec;SessionLayer"/>
    


    <!-- http://www-usr.inf.ufsm.br/~brunomozza/iotsec/iotsec.owl#SessionRidingHijacking -->

    <owl:NamedIndividual rdf:about="&iotsec;SessionRidingHijacking">
        <rdf:type rdf:resource="&iotsec;CloudVulnerability"/>
        <rdfs:label xml:lang="en">Session riding and hijacking</rdfs:label>
        <rdfs:comment xml:lang="en">Web application technologies must overcome the problem that, by design, the HTTP protocol is a stateless protocol, whereas Web applications require some notion of session state. Many techniques implement session handling and - as any security professional knowledgeable in Web application security will testify - many session handling implementations are vulnerable to session riding and session hijacking. Whether session riding/hijacking vulnerabilities are intrinsic to Web application technologies or are “only” prevalent in many current implementations is arguable; in any case, such vulnerabilities are certainly relevant for cloud computing [Grobauer 2011].</rdfs:comment>
    </owl:NamedIndividual>
    


    <!-- http://www-usr.inf.ufsm.br/~brunomozza/iotsec/iotsec.owl#ShortRangeProtection -->

    <owl:NamedIndividual rdf:about="&iotsec;ShortRangeProtection">
        <rdf:type rdf:resource="&iotsec;GSMVulnerability"/>
        <rdfs:label xml:lang="en">Short range of protection</rdfs:label>
        <rdfs:comment xml:lang="en">The encryption is only accomplished over the airway path between MS and BTS. There is not any protection over other parts of network and the information is clearly sent over the fixed parts. This is a major exposure for the GSM, especially when the communication between BTS and BSC is performed over the wireless links that have potential vulnerabilities for interception. In some countries, the encryption facility of the air interface is not activated at all. There are also security problems on the GSM backbone. The deployed Signaling System no.7 (SS7) has also several security vulnerabilities. The messages in the current SS7 system is so that they can be modifies or even fabricated into the global SS7 system in an uncontrolled manner [Lorenz 2001]. SS7 incorporates very limited authentication procedures since it was originally designed for the closed telecommunication communities. The interconnection with Internet can also have its potential vulnerabilities. Additional vulnerabilities will be arisen when SS7 systems are interconnected using the Internet. Remote management of the GSM backbone elements that can be conducted by connecting them to the IP networks can also introduce additional vulnerabilities. If the HLR and AuC are physically separated, it can be a new point of vulnerability since the authentication triplets may be obtained from AuC by masquerading as another system entity, e.g. a HLR. Unauthorized accesses to HLR, AuC, and MSC will also cause several problems [Toorani 2008].</rdfs:comment>
    </owl:NamedIndividual>
    


    <!-- http://www-usr.inf.ufsm.br/~brunomozza/iotsec/iotsec.owl#Sinkhole -->

    <owl:NamedIndividual rdf:about="&iotsec;Sinkhole"/>
    


    <!-- http://www-usr.inf.ufsm.br/~brunomozza/iotsec/iotsec.owl#Skipjack -->

    <owl:NamedIndividual rdf:about="&iotsec;Skipjack"/>
    


    <!-- http://www-usr.inf.ufsm.br/~brunomozza/iotsec/iotsec.owl#StaticSSPpasskeys -->

    <owl:NamedIndividual rdf:about="&iotsec;StaticSSPpasskeys">
        <rdf:type rdf:resource="&iotsec;BluetoothVulnerability"/>
        <rdfs:label xml:lang="en">Static SSP passkeys facilitate MITM attacks</rdfs:label>
        <rdfs:comment xml:lang="en">Passkeys provide MITM protection during SSP. Devices should use random, unique passkeys for each pairing attempt [Padgette 2012].</rdfs:comment>
        <iotsec:affects xml:lang="en">Versions Bluetooth v2.1 and v3.0</iotsec:affects>
    </owl:NamedIndividual>
    


    <!-- http://www-usr.inf.ufsm.br/~brunomozza/iotsec/iotsec.owl#TransportLayer -->

    <owl:NamedIndividual rdf:about="&iotsec;TransportLayer"/>
    


    <!-- http://www-usr.inf.ufsm.br/~brunomozza/iotsec/iotsec.owl#TripleDES -->

    <owl:NamedIndividual rdf:about="&iotsec;TripleDES">
        <rdfs:label xml:lang="en">TripleDES</rdfs:label>
        <iotsec:satisfies rdf:resource="&iotsec;Confidentiality"/>
    </owl:NamedIndividual>
    


    <!-- http://www-usr.inf.ufsm.br/~brunomozza/iotsec/iotsec.owl#Trust -->

    <owl:NamedIndividual rdf:about="&iotsec;Trust"/>
    


    <!-- http://www-usr.inf.ufsm.br/~brunomozza/iotsec/iotsec.owl#Twofish -->

    <owl:NamedIndividual rdf:about="&iotsec;Twofish"/>
    


    <!-- http://www-usr.inf.ufsm.br/~brunomozza/iotsec/iotsec.owl#UnauthenticatedMessages -->

    <owl:NamedIndividual rdf:about="&iotsec;UnauthenticatedMessages">
        <rdf:type rdf:resource="&iotsec;WimaxVulnerability"/>
        <rdfs:label xml:lang="en">Unauthenticated messages</rdfs:label>
        <rdfs:comment xml:lang="en">Most of the management messages defined in IEEE 802.16e are integrity protected. Which is done by a hash based message authentication code (HMAC) or alternatively by a cipher based message authentication code (CMAC). But some messages are not covered by any authentication mechanism. This introduces some vulnerability. A couple of management messages are sent over the broadcast management connection. Since in WiMAX security architecture, there is no common key which can be used as the authentication of broadcasted management messages, so the authentication of these messages is difficult. Furthermore, a common key would not completely protect the integrity of the message as M.S sharing the key can be generated by unauthenticated B.S [Kowsar 2010].</rdfs:comment>
    </owl:NamedIndividual>
    


    <!-- http://www-usr.inf.ufsm.br/~brunomozza/iotsec/iotsec.owl#UnencryptedCommunication -->

    <owl:NamedIndividual rdf:about="&iotsec;UnencryptedCommunication">
        <rdf:type rdf:resource="&iotsec;WimaxVulnerability"/>
        <rdfs:label xml:lang="en">Unencrypted management communication</rdfs:label>
        <rdfs:comment xml:lang="en">Mobile WiMAX management messages are still sent in the clear. When a mobile station performs initial network entry it negotiates communication parameters and settings with the base station. Here a lot of information is exchanged such as security negotiation parameters, configuration settings, power settings, mobility parameters, vendor information, mobile stations capabilities. Currently the complete management message exchange in the network entry process is unencrypted and the above mentioned information can be accessed just by listening on the channel [Kowsar 2010].</rdfs:comment>
    </owl:NamedIndividual>
    


    <!-- http://www-usr.inf.ufsm.br/~brunomozza/iotsec/iotsec.owl#UnencryptedWritingPermission -->

    <owl:NamedIndividual rdf:about="&iotsec;UnencryptedWritingPermission">
        <rdf:type rdf:resource="&iotsec;RfidVulnerability"/>
        <rdfs:label xml:lang="en">Unencrypted Writing Permission</rdfs:label>
        <rdfs:comment xml:lang="en">Writing Permission is unencrypted when a tag is produced. Encryption is completely depends on the user&apos;s own decision. If the writing permission is unencrypted, malicious users can tamper the tag easily. Moreover, attackers can also set their own password for each memory bank to make the tag controlled only by them [Liu 2014].</rdfs:comment>
    </owl:NamedIndividual>
    


    <!-- http://www-usr.inf.ufsm.br/~brunomozza/iotsec/iotsec.owl#UnilateralAuthentication -->

    <owl:NamedIndividual rdf:about="&iotsec;UnilateralAuthentication">
        <rdf:type rdf:resource="&iotsec;GSMVulnerability"/>
        <rdfs:label xml:lang="en">Unilateral authentication</rdfs:label>
        <rdfs:comment xml:lang="en">This is the network that authenticates users. The user does not authenticate network so the attacker can use a false BTS with the same mobile network code as the subscriber&apos;s legitimate network to impersonate himself and perform a man-in-the-middle attack. The attacker can then perform several scenarios to modify or fabricate the exchanged data. At the designing phase of the GSM protocols, this kind of attack seemed impractical due to costly required equipments. Currently, this kind of attack is completely applicable due to the decreased costs [Toorani 2008].</rdfs:comment>
    </owl:NamedIndividual>
    


    <!-- http://www-usr.inf.ufsm.br/~brunomozza/iotsec/iotsec.owl#UnitKeysAreStaticAndReused -->

    <owl:NamedIndividual rdf:about="&iotsec;UnitKeysAreStaticAndReused">
        <rdf:type rdf:resource="&iotsec;BluetoothVulnerability"/>
        <rdfs:label xml:lang="en">Link keys based on unit keys are static and reused for every pairing.</rdfs:label>
        <rdfs:comment xml:lang="en">A device that uses unit keys will use the same link key for every device with which 
	it pairs. This is a serious cryptographic key management vulnerability [Padgette 2012].

	Once a device’s unit key is divulged (i.e., upon its first pairing), any other device that has the key can spoof that device or any other device with which it has paired. Further, it can eavesdrop on that device’s connections whether they are encrypted or not [Padgette 2012]. isThreatensBy Spoofing and Eavesdropping.</rdfs:comment>
        <iotsec:affects xml:lang="en">Versions before Bluetooth 1.2</iotsec:affects>
    </owl:NamedIndividual>
    


    <!-- http://www-usr.inf.ufsm.br/~brunomozza/iotsec/iotsec.owl#UnvalidatedRedirectsForwards -->

    <owl:NamedIndividual rdf:about="&iotsec;UnvalidatedRedirectsForwards">
        <rdf:type rdf:resource="&iotsec;WebVulnerability"/>
        <rdfs:label xml:lang="en">Unvalidated Redirects and Forwards</rdfs:label>
        <rdfs:comment xml:lang="en">Web applications frequently redirect and forward users to other pages and websites, and use untrusted data to determine the destination pages. Without proper validation, attackers can redirect victims to phishing or malware sites, or use forwards to access unauthorized pages [OWASP Top Ten 2013].</rdfs:comment>
    </owl:NamedIndividual>
    


    <!-- http://www-usr.inf.ufsm.br/~brunomozza/iotsec/iotsec.owl#UserAnonymity -->

    <owl:NamedIndividual rdf:about="&iotsec;UserAnonymity">
        <rdf:type rdf:resource="&iotsec;GSMVulnerability"/>
        <rdfs:label xml:lang="en">Leaking the user anonymity</rdfs:label>
        <rdfs:comment xml:lang="en">Whenever a subscriber enters a location area for the first time or when the mapping table between the subscriber&apos;s TMSI and IMSI is lost, the network requests the subscriber to clearly declare the IMSI. This can be misused to fail the user&apos;s anonymity and can be accomplished by sending an IDENTITY REQUEST command from a false BTS to the MS of the target user to find the corresponding IMSI [Toorani 2008].</rdfs:comment>
    </owl:NamedIndividual>
    


    <!-- http://www-usr.inf.ufsm.br/~brunomozza/iotsec/iotsec.owl#UserSpecificDoS -->

    <owl:NamedIndividual rdf:about="&iotsec;UserSpecificDoS">
        <rdf:type rdf:resource="&iotsec;UMTSVulnerability"/>
        <rdfs:label xml:lang="en">User Specific DoS by Modifying Initial Security Capabilities of ME or Authentication Parameters</rdfs:label>
        <rdfs:comment xml:lang="en">This attack works in two phases. Initially, the attacker obtains IMSI of the victim. In the second phase, the attacker waits for this particular user (IMSI) to make a connection request. When an rrcConnectionRequest is made by this user, the attacker modifies the message which contains initial security capabilities of the ME. This message is not integrity protected, therefore, an intruder can modify the ME security capabilities and this change will remain undetected until the security mode command reaches the ME. Modification of any of the authentication parameters including AUTN, RAND, or RES (message 4 or 5 of Fig 1) may also result in DoS. These messages are neither encrypted nor integrity protected. Any change in the way will result in non- authentication of network and/or user. In both the cases the network will not be able to distinguish between illegitimate user and DoS attack [Khan 2008].</rdfs:comment>
    </owl:NamedIndividual>
    


    <!-- http://www-usr.inf.ufsm.br/~brunomozza/iotsec/iotsec.owl#UserVisibility -->

    <owl:NamedIndividual rdf:about="&iotsec;UserVisibility">
        <rdf:type rdf:resource="&iotsec;GSMVulnerability"/>
        <rdfs:label xml:lang="en">Lack of user visibility</rdfs:label>
        <rdfs:comment xml:lang="en">The ciphering is controlled by the BTS. The user is not alerted when the ciphering mode is deactivated. A false BTS can also deactivate the ciphering mode and force MS to send data in an unencrypted manner [Toorani 2008].</rdfs:comment>
    </owl:NamedIndividual>
    


    <!-- http://www-usr.inf.ufsm.br/~brunomozza/iotsec/iotsec.owl#VirtualMachineEscape -->

    <owl:NamedIndividual rdf:about="&iotsec;VirtualMachineEscape">
        <rdf:type rdf:resource="&iotsec;CloudVulnerability"/>
        <rdfs:label xml:lang="en">Virtual machine escape</rdfs:label>
        <rdfs:comment xml:lang="en">The possibility that an attacker might successfully escape from a virtualized environment lies in virtualization’s very nature. Hence, we must consider this vulnerability as intrinsic to virtualization and highly relevant to cloud computing [Grobauer 2011].</rdfs:comment>
    </owl:NamedIndividual>
    


    <!-- http://www-usr.inf.ufsm.br/~brunomozza/iotsec/iotsec.owl#XSSVuln -->

    <owl:NamedIndividual rdf:about="&iotsec;XSSVuln">
        <rdf:type rdf:resource="&iotsec;WebVulnerability"/>
        <rdfs:label xml:lang="en">Cross-Site Scripting (XSS)</rdfs:label>
        <rdfs:label xml:lang="en">XSS flaws occur whenever an application takes untrusted data and sends it to a web browser without proper validation or escaping. XSS allows attackers to execute scripts in the victim’s browser which can hijack user sessions, deface web sites, or redirect the user to malicious sites [OWASP Top Ten 2013].</rdfs:label>
    </owl:NamedIndividual>
    


    <!-- http://www.daml.org/services/owl-s/security/security.owl#AccessControl -->

    <owl:NamedIndividual rdf:about="&denker;AccessControl"/>
    


    <!-- http://www.daml.org/services/owl-s/security/security.owl#Anonymity -->

    <owl:NamedIndividual rdf:about="&denker;Anonymity"/>
    


    <!-- http://www.daml.org/services/owl-s/security/security.owl#Authentication -->

    <owl:NamedIndividual rdf:about="&denker;Authentication"/>
    


    <!-- http://www.daml.org/services/owl-s/security/security.owl#Authorization -->

    <owl:NamedIndividual rdf:about="&denker;Authorization"/>
    


    <!-- http://www.daml.org/services/owl-s/security/security.owl#Confidentiality -->

    <owl:NamedIndividual rdf:about="&denker;Confidentiality"/>
    


    <!-- http://www.daml.org/services/owl-s/security/security.owl#DataIntegrity -->

    <owl:NamedIndividual rdf:about="&denker;DataIntegrity"/>
    


    <!-- http://www.ida.liu.se/~iislab/projects/secont/Security.owlAccountability -->

    <owl:NamedIndividual rdf:about="&herzog;Accountability"/>
    


    <!-- http://www.ida.liu.se/~iislab/projects/secont/Security.owlAnonymity -->

    <owl:NamedIndividual rdf:about="&herzog;Anonymity"/>
    


    <!-- http://www.ida.liu.se/~iislab/projects/secont/Security.owlAuthentication -->

    <owl:NamedIndividual rdf:about="&herzog;Authentication"/>
    


    <!-- http://www.ida.liu.se/~iislab/projects/secont/Security.owlAuthorisation -->

    <owl:NamedIndividual rdf:about="&herzog;Authorisation"/>
    


    <!-- http://www.ida.liu.se/~iislab/projects/secont/Security.owlAvailability -->

    <owl:NamedIndividual rdf:about="&herzog;Availability"/>
    


    <!-- http://www.ida.liu.se/~iislab/projects/secont/Security.owlConfidentiality -->

    <owl:NamedIndividual rdf:about="&herzog;Confidentiality"/>
    


    <!-- http://www.ida.liu.se/~iislab/projects/secont/Security.owlIntegrity -->

    <owl:NamedIndividual rdf:about="&herzog;Integrity"/>
    


    <!-- http://www.ida.liu.se/~iislab/projects/secont/Security.owlNon-Repudiation -->

    <owl:NamedIndividual rdf:about="&herzog;Non-Repudiation"/>
</rdf:RDF>
